<?xml version='1.0' encoding='UTF-8'?>
<!DOCTYPE rdf:RDF [
    <!ENTITY dul 'http://www.ontologydesignpatterns.org/ont/dul/DUL.owl#'>
    <!ENTITY owl 'http://www.w3.org/2002/07/owl#'>
    <!ENTITY rdf 'http://www.w3.org/1999/02/22-rdf-syntax-ns#'>
    <!ENTITY rdfs 'http://www.w3.org/2000/01/rdf-schema#'>
    <!ENTITY soma 'http://www.ease-crc.org/ont/SOMA.owl#'>
    <!ENTITY xsd 'http://www.w3.org/2001/XMLSchema#'>
]>

<rdf:RDF
    xmlns:dul="&dul;"
    xmlns:owl="&owl;"
    xmlns:rdf="&rdf;"
    xmlns:rdfs="&rdfs;"
    xmlns:soma="&soma;"
    xmlns:xsd="&xsd;"
>
<owl:Class rdf:about="&soma;Reaching">
  <rdfs:comment>A task in which an Agent moves one or more of its arms towards a location or object.</rdfs:comment>
  <rdfs:isDefinedBy rdf:resource="http://www.ease-crc.org/ont/SOMA-ACT.owl"/>
  <rdfs:subClassOf rdf:resource="&soma;EndEffectorPositioning"/>
  <owl:disjointWith rdf:resource="&soma;Retracting"/>
</owl:Class>

<owl:ObjectProperty rdf:about="&soma;hasPreference">
  <rdfs:label xml:lang="en">Relates an agent to its preference quality.</rdfs:label>
  <rdfs:label xml:lang="en">has preference</rdfs:label>
  <rdfs:domain rdf:resource="&dul;Agent"/>
  <rdfs:isDefinedBy rdf:resource="http://www.ease-crc.org/ont/SOMA-AGENT.owl"/>
  <rdfs:range rdf:resource="&soma;Preference"/>
  <rdfs:subPropertyOf rdf:resource="&dul;hasQuality"/>
  <owl:inverseOf rdf:resource="&soma;isPreferenceOf"/>
</owl:ObjectProperty>

<owl:ObjectProperty rdf:about="&soma;isSupportedBy"
    rdfs:label="is supported by">
  <rdfs:comment>A relation between an object (the supporter) and another object (the supportee) where the supporter cancels the effect of gravity on the supportee.</rdfs:comment>
  <rdfs:comment>Relates a supportee to one of its supporters.</rdfs:comment>
  <rdfs:isDefinedBy rdf:resource="http://www.ease-crc.org/ont/SOMA-OBJ.owl"/>
  <rdfs:isDefinedBy rdf:resource="http://www.ease-crc.org/ont/SOMA-PROC.owl"/>
  <rdfs:subPropertyOf rdf:resource="&soma;interactsWith"/>
  <rdfs:subPropertyOf rdf:resource="&dul;hasCommonBoundary"/>
  <rdfs:domain rdf:resource="&dul;Entity"/>
  <rdfs:range rdf:resource="&dul;Entity"/>
  <owl:inverseOf rdf:resource="&soma;supports"/>
</owl:ObjectProperty>

<rdf:Property rdf:about="&soma;material">
  <rdfs:domain rdf:resource="&soma;Object"/>
  <rdfs:range rdf:resource="&xsd;string"/>
</rdf:Property>

<owl:ObjectProperty rdf:about="&soma;contains">
  <rdfs:comment>A schematic relation asserting containment, understood in a very broad sense, by one Entity of another. The relation is defined with domain and range of maximum generality, as it is possible to construe containment to apply between Events, between Objects, between Qualities and so on. Care should be taken when using it that the construal of containment makes sense and is useful. If a clearer relation expresses the connection between two Entities, use that relation instead. For example, rather than saying an Event contains an Object, it is probably better to say the Event has that Object as a participant. More specific versions of this relation exist, e.g. containsEvent, so it is likely that there will be few situations where it should be used itself. However, by acting as a superproperty to several relations, it captures a core similarity between these and enables taxonomy-based similarity metrics.</rdfs:comment>
  <rdfs:domain rdf:resource="&dul;Entity"/>
  <rdfs:isDefinedBy rdf:resource="http://www.ease-crc.org/ont/SOMA.owl"/>
  <rdfs:range rdf:resource="&dul;Entity"/>
  <rdfs:subPropertyOf rdf:resource="&dul;overlaps"/>
  <owl:inverseOf rdf:resource="&soma;isContainedIn"/>
</owl:ObjectProperty>

<owl:Class rdf:about="&soma;Foolishness"
    rdfs:comment="A description of foolish behavior.">
  <rdfs:isDefinedBy rdf:resource="http://www.ease-crc.org/ont/SOMA.owl"/>
  <rdfs:subClassOf rdf:resource="&soma;Amateurish"/>
</owl:Class>

<owl:Class rdf:about="&soma;Closing">
  <owl:disjointWith rdf:resource="&soma;Delivering"/>
  <owl:disjointWith rdf:resource="&soma;Fetching"/>
  <owl:disjointWith rdf:resource="&soma;Lifting"/>
  <owl:disjointWith rdf:resource="&soma;Opening"/>
  <owl:disjointWith rdf:resource="&soma;Pulling"/>
  <owl:disjointWith rdf:resource="&soma;Pushing"/>
  <owl:disjointWith rdf:resource="&soma;Squeezing"/>
  <rdfs:comment>A task in which an Agent manipulates a container so as to block access to its interior.</rdfs:comment>
  <rdfs:isDefinedBy rdf:resource="http://www.ease-crc.org/ont/SOMA-ACT.owl"/>
  <rdfs:subClassOf rdf:resource="&soma;Actuating"/>
</owl:Class>

<owl:Class rdf:about="&soma;ExecutableFormat">
  <rdfs:subClassOf>
    <owl:Restriction>
      <owl:allValuesFrom rdf:resource="&soma;Executable_Code"/>
      <owl:onProperty rdf:resource="&soma;givesMeaningTo"/>
    </owl:Restriction>
  </rdfs:subClassOf>
  <rdfs:subClassOf rdf:resource="&soma;File_format"/>
  <rdfs:comment xml:lang="en">An Executable Format is a File Format that allows computers to directly execute the content. Examples are MZ (DOS) or COFF.</rdfs:comment>
  <rdfs:isDefinedBy rdf:resource="http://www.ease-crc.org/ont/SOMA-IO.owl"/>
  <rdfs:label xml:lang="en">Executable Format</rdfs:label>
</owl:Class>

<owl:Class rdf:about="&dul;Organism"/>

<owl:Class rdf:about="&soma;HeadTurning">
  <rdfs:comment>A process type classifying a motion of an Agent's head such that the direction this head faces changes relative to the facing direction of the Agent's body as a whole.</rdfs:comment>
  <rdfs:isDefinedBy rdf:resource="http://www.ease-crc.org/ont/SOMA-PROC.owl"/>
  <rdfs:subClassOf rdf:resource="&soma;HeadMovement"/>
</owl:Class>

<owl:Class rdf:about="&soma;FloatingJoint"
    rdfs:comment="A joint that allows motion for all 6 degrees of freedom."
    rdfs:label="Floating joint">
  <rdfs:isDefinedBy rdf:resource="http://www.ease-crc.org/ont/SOMA-OBJ.owl"/>
  <rdfs:subClassOf rdf:resource="&soma;MovableJoint"/>
</owl:Class>

<owl:Class rdf:about="&soma;Intrinsic">
  <rdfs:comment>A physical quality that is independent of context.</rdfs:comment>
  <rdfs:comment>intrinsic</rdfs:comment>
  <rdfs:isDefinedBy rdf:resource="http://www.ease-crc.org/ont/SOMA-OBJ.owl"/>
  <rdfs:subClassOf rdf:resource="&soma;PhysicalQuality"/>
</owl:Class>

<owl:Class rdf:about="&soma;Affordance">
  <rdfs:subClassOf>
    <owl:Restriction>
      <owl:allValuesFrom rdf:resource="&soma;Disposition"/>
      <owl:onProperty rdf:resource="&dul;describes"/>
    </owl:Restriction>
  </rdfs:subClassOf>
  <rdfs:subClassOf>
    <owl:Restriction>
      <owl:onClass rdf:resource="&dul;Role"/>
      <owl:onProperty rdf:resource="&soma;definesBearer"/>
      <owl:qualifiedCardinality rdf:datatype="&xsd;nonNegativeInteger">1</owl:qualifiedCardinality>
    </owl:Restriction>
  </rdfs:subClassOf>
  <rdfs:subClassOf>
    <owl:Restriction>
      <owl:onClass rdf:resource="&dul;Role"/>
      <owl:onProperty rdf:resource="&soma;definesTrigger"/>
      <owl:qualifiedCardinality rdf:datatype="&xsd;nonNegativeInteger">1</owl:qualifiedCardinality>
    </owl:Restriction>
  </rdfs:subClassOf>
  <rdfs:subClassOf>
    <owl:Restriction>
      <owl:onClass rdf:resource="&dul;Task"/>
      <owl:onProperty rdf:resource="&dul;definesTask"/>
      <owl:qualifiedCardinality rdf:datatype="&xsd;nonNegativeInteger">1</owl:qualifiedCardinality>
    </owl:Restriction>
  </rdfs:subClassOf>
  <rdfs:subClassOf rdf:resource="&dul;Relation"/>
  <rdfs:comment>A relation between an object (the bearer) and others (the triggers) that describes the disposition of the bearer to be involved in an action execution that also involves some trigger object.</rdfs:comment>
  <rdfs:isDefinedBy rdf:resource="http://www.ease-crc.org/ont/SOMA-OBJ.owl"/>
</owl:Class>

<owl:Class rdf:about="&soma;Joint">
  <rdfs:subClassOf>
    <owl:Restriction>
      <owl:onClass rdf:resource="&dul;PhysicalObject"/>
      <owl:onProperty rdf:resource="&soma;hasChildLink"/>
      <owl:qualifiedCardinality rdf:datatype="&xsd;nonNegativeInteger">1</owl:qualifiedCardinality>
    </owl:Restriction>
  </rdfs:subClassOf>
  <rdfs:subClassOf>
    <owl:Restriction>
      <owl:onClass rdf:resource="&dul;PhysicalObject"/>
      <owl:onProperty rdf:resource="&soma;hasParentLink"/>
      <owl:qualifiedCardinality rdf:datatype="&xsd;nonNegativeInteger">1</owl:qualifiedCardinality>
    </owl:Restriction>
  </rdfs:subClassOf>
  <rdfs:subClassOf>
    <owl:Restriction>
      <owl:maxQualifiedCardinality rdf:datatype="&xsd;nonNegativeInteger">1</owl:maxQualifiedCardinality>
      <owl:onClass rdf:resource="&soma;JointState"/>
      <owl:onProperty rdf:resource="&soma;hasJointState"/>
    </owl:Restriction>
  </rdfs:subClassOf>
  <rdfs:subClassOf rdf:resource="&dul;PhysicalBody"/>
  <rdfs:comment>An object that is used to articulate links in a kinematic structure.</rdfs:comment>
  <rdfs:isDefinedBy rdf:resource="http://www.ease-crc.org/ont/SOMA-OBJ.owl"/>
  <owl:equivalentClass>
    <owl:Class>
      <owl:unionOf rdf:parseType="Collection">
        <rdf:Description rdf:about="&soma;FixedJoint"/>
        <rdf:Description rdf:about="&soma;MovableJoint"/>
      </owl:unionOf>
    </owl:Class>
  </owl:equivalentClass>
</owl:Class>

<owl:Class rdf:about="&soma;Origin">
  <rdfs:comment>A role classifying the location where an event or object originated.</rdfs:comment>
  <rdfs:isDefinedBy rdf:resource="http://www.ease-crc.org/ont/SOMA-OBJ.owl"/>
  <rdfs:subClassOf rdf:resource="&soma;Location"/>
</owl:Class>

<owl:ObjectProperty rdf:about="&soma;isProcessDefinedIn"
    rdfs:label="is process defined in">
  <rdfs:comment>A relation between a process type and a description that defines it.</rdfs:comment>
  <rdfs:domain rdf:resource="&soma;ProcessType"/>
  <rdfs:isDefinedBy rdf:resource="http://www.ease-crc.org/ont/SOMA-PROC.owl"/>
  <rdfs:range rdf:resource="&dul;Description"/>
  <rdfs:subPropertyOf rdf:resource="&dul;isDefinedIn"/>
</owl:ObjectProperty>

<owl:ObjectProperty rdf:about="&dul;isSettingFor"/>

<owl:Class rdf:about="&dul;PhysicalAttribute"/>

<owl:Class rdf:about="&soma;CrackingTheory">
  <rdfs:subClassOf>
    <owl:Restriction>
      <owl:onProperty rdf:resource="&dul;defines"/>
      <owl:someValuesFrom rdf:resource="&soma;Instrument"/>
    </owl:Restriction>
  </rdfs:subClassOf>
  <rdfs:subClassOf>
    <owl:Restriction>
      <owl:onProperty rdf:resource="&dul;defines"/>
      <owl:someValuesFrom rdf:resource="&soma;Patient"/>
    </owl:Restriction>
  </rdfs:subClassOf>
  <rdfs:subClassOf rdf:resource="&soma;ExecutableSchematicTheory"/>
  <rdfs:comment>A schematic theory of how an agent can inflict damage to the surface of an object.</rdfs:comment>
  <rdfs:isDefinedBy rdf:resource="http://www.ease-crc.org/ont/SOMA-SAY.owl"/>
  <rdfs:label xml:lang="en">Cracking theory</rdfs:label>
</owl:Class>

<owl:Class rdf:about="&soma;Answer"
    rdfs:label="Answer">
  <rdfs:comment>A role that is played by an Information Realization answering some query.</rdfs:comment>
  <rdfs:isDefinedBy rdf:resource="http://www.ease-crc.org/ont/SOMA-ACT.owl"/>
  <rdfs:subClassOf rdf:resource="&soma;Message"/>
</owl:Class>

<owl:Class rdf:about="&soma;Avoiding">
  <rdfs:comment>A task in which an Agent moves so as to not enter or pass through a location.</rdfs:comment>
  <rdfs:isDefinedBy rdf:resource="http://www.ease-crc.org/ont/SOMA-ACT.owl"/>
  <rdfs:subClassOf rdf:resource="&soma;Navigating"/>
</owl:Class>

<owl:Class rdf:about="&soma;MixingTheory">
  <rdfs:subClassOf>
    <owl:Restriction>
      <owl:onProperty rdf:resource="&dul;defines"/>
      <owl:someValuesFrom rdf:resource="&soma;Instrument"/>
    </owl:Restriction>
  </rdfs:subClassOf>
  <rdfs:subClassOf>
    <owl:Restriction>
      <owl:onProperty rdf:resource="&dul;defines"/>
      <owl:someValuesFrom rdf:resource="&soma;Patient"/>
    </owl:Restriction>
  </rdfs:subClassOf>
  <rdfs:subClassOf rdf:resource="&soma;ExecutableSchematicTheory"/>
  <rdfs:comment>A schematic theory about how an agent can mix a fluid or particulate object.</rdfs:comment>
  <rdfs:isDefinedBy rdf:resource="http://www.ease-crc.org/ont/SOMA-SAY.owl"/>
  <rdfs:label xml:lang="en">Mixing theory</rdfs:label>
</owl:Class>

<owl:DatatypeProperty rdf:about="&soma;hasEventEnd"
    rdfs:label="has event end">
  <rdfs:comment>A relation recording when an Event ended. In this case, we think of the Event as something unfolding over some span of time.</rdfs:comment>
  <rdfs:domain rdf:resource="&dul;Event"/>
  <rdfs:isDefinedBy rdf:resource="http://www.ease-crc.org/ont/SOMA.owl"/>
  <rdfs:range rdf:resource="&xsd;double"/>
  <rdfs:subPropertyOf rdf:resource="&soma;hasEventTime"/>
</owl:DatatypeProperty>

<owl:Class rdf:about="&soma;IncompatibleSoftware">
  <rdfs:comment>A description of a situation where two software systems are incompatible with each other.</rdfs:comment>
  <rdfs:isDefinedBy rdf:resource="http://www.ease-crc.org/ont/SOMA-IO.owl"/>
  <rdfs:label xml:lang="en">Incompatible software</rdfs:label>
  <rdfs:subClassOf rdf:resource="&soma;SoftwareDiagnosis"/>
</owl:Class>

<owl:ObjectProperty rdf:about="&soma;isMassAttributeOf"
    rdfs:comment="A relation between physical objects and their mass."
    rdfs:label="is mass attribute of">
  <rdfs:domain rdf:resource="&soma;MassAttribute"/>
  <rdfs:isDefinedBy rdf:resource="http://www.ease-crc.org/ont/SOMA-OBJ.owl"/>
  <rdfs:range rdf:resource="&dul;PhysicalObject"/>
  <rdfs:subPropertyOf rdf:resource="&dul;isRegionFor"/>
</owl:ObjectProperty>

<owl:Class rdf:about="&soma;Selecting">
  <rdfs:comment xml:lang="en">A Task where an Agent decides between two or more options.</rdfs:comment>
  <rdfs:isDefinedBy rdf:resource="http://www.ease-crc.org/ont/SOMA-AGENT.owl"/>
  <rdfs:label xml:lang="en">Selecting</rdfs:label>
  <rdfs:subClassOf rdf:resource="&soma;Deciding"/>
</owl:Class>

<owl:ObjectProperty rdf:about="&soma;isDepositOf"
    rdfs:label="is deposit of">
  <rdfs:comment>A spatial relation holding between an object (the deposit), and objects that are located ontop of it.</rdfs:comment>
  <rdfs:domain rdf:resource="&dul;PhysicalObject"/>
  <rdfs:isDefinedBy rdf:resource="http://www.ease-crc.org/ont/SOMA-OBJ.owl"/>
  <rdfs:range rdf:resource="&dul;PhysicalObject"/>
  <rdfs:subPropertyOf rdf:resource="&dul;isLocationOf"/>
  <owl:inverseOf rdf:resource="&soma;isOntopOf"/>
</owl:ObjectProperty>

<owl:Class rdf:about="&soma;File_format">
  <rdfs:comment xml:lang="en">A File Format is a standard way that information is encoded for storage in a computer file. It specifies how bits are used to encode information in a digital storage medium.

From Wikipedia: https://en.wikipedia.org/wiki/File_format</rdfs:comment>
  <rdfs:isDefinedBy rdf:resource="http://www.ease-crc.org/ont/SOMA-IO.owl"/>
  <rdfs:label xml:lang="en">File Format</rdfs:label>
  <rdfs:subClassOf rdf:resource="&soma;Computer_Language"/>
</owl:Class>

<owl:ObjectProperty rdf:about="&dul;isReferenceOf"/>

<owl:Class rdf:about="&soma;Connectivity">
  <rdfs:subClassOf>
    <owl:Restriction>
      <owl:allValuesFrom rdf:resource="&soma;ConnectedObject"/>
      <owl:onProperty rdf:resource="&soma;affordsTrigger"/>
    </owl:Restriction>
  </rdfs:subClassOf>
  <rdfs:subClassOf>
    <owl:Restriction>
      <owl:allValuesFrom rdf:resource="&soma;ConnectedObject"/>
      <owl:onProperty rdf:resource="&soma;affordsBearer"/>
    </owl:Restriction>
  </rdfs:subClassOf>
  <rdfs:subClassOf rdf:resource="&soma;Disposition"/>
  <rdfs:comment>The disposition of an object (the connected object) to establish a connection with others.</rdfs:comment>
  <rdfs:isDefinedBy rdf:resource="http://www.ease-crc.org/ont/SOMA-OBJ.owl"/>
</owl:Class>

<soma:ExecutionStateRegion rdf:about="&soma;ExecutionState_Failed"
    rdfs:comment="The execution state of a failed activity.">
  <rdf:type rdf:resource="&owl;NamedIndividual"/>
  <rdfs:isDefinedBy rdf:resource="http://www.ease-crc.org/ont/SOMA-ACT.owl"/>
</soma:ExecutionStateRegion>

<owl:Class rdf:about="&soma;Sender">
  <rdfs:subClassOf>
    <owl:Restriction>
      <owl:onProperty rdf:resource="&dul;hasTask"/>
      <owl:someValuesFrom rdf:resource="&soma;CommunicationTask"/>
    </owl:Restriction>
  </rdfs:subClassOf>
  <rdfs:subClassOf rdf:resource="&soma;PerformerRole"/>
  <rdfs:comment xml:lang="en">The Role played by an Agent in a Communication Task that emits some Information Realization with the purpose of percipience by some Receiver.</rdfs:comment>
  <rdfs:isDefinedBy rdf:resource="http://www.ease-crc.org/ont/SOMA-ACT.owl"/>
  <rdfs:label xml:lang="en">Sender</rdfs:label>
</owl:Class>

<owl:AsymmetricProperty rdf:about="&soma;hasTerminalScene"
    rdfs:label="has terminal scene">
  <rdf:type rdf:resource="&owl;IrreflexiveProperty"/>
  <rdf:type rdf:resource="&owl;ObjectProperty"/>
  <rdfs:comment>A relation between StateTransitions and Scenes, which identifies the scene the transition is expected to end at.</rdfs:comment>
  <rdfs:domain rdf:resource="&soma;StateTransition"/>
  <rdfs:isDefinedBy rdf:resource="http://www.ease-crc.org/ont/SOMA.owl"/>
  <rdfs:range rdf:resource="&soma;Scene"/>
  <rdfs:subPropertyOf rdf:resource="&soma;hasTerminalState"/>
  <owl:inverseOf rdf:resource="&soma;isTerminalSceneOf"/>
</owl:AsymmetricProperty>

<owl:Class rdf:about="&soma;MovingTo"
    rdfs:comment="A task in which an Agent moves towards a location.">
  <rdfs:isDefinedBy rdf:resource="http://www.ease-crc.org/ont/SOMA-ACT.owl"/>
  <rdfs:subClassOf rdf:resource="&soma;Navigating"/>
</owl:Class>

<owl:ObjectProperty rdf:about="&soma;hasPhase"
    rdfs:label="has phase">
  <rdfs:comment>A relation used to describe the structure of an Action or Process in terms of phases, i.e. subprocesses and states that occur during its unfolding.</rdfs:comment>
  <rdfs:domain>
    <owl:Class>
      <owl:unionOf rdf:parseType="Collection">
        <rdf:Description rdf:about="&dul;Action"/>
        <rdf:Description rdf:about="&dul;Process"/>
      </owl:unionOf>
    </owl:Class>
  </rdfs:domain>
  <rdfs:isDefinedBy rdf:resource="http://www.ease-crc.org/ont/SOMA.owl"/>
  <rdfs:range>
    <owl:Class>
      <owl:unionOf rdf:parseType="Collection">
        <rdf:Description rdf:about="&soma;State"/>
        <rdf:Description rdf:about="&dul;Process"/>
      </owl:unionOf>
    </owl:Class>
  </rdfs:range>
  <rdfs:subPropertyOf rdf:resource="&dul;hasConstituent"/>
</owl:ObjectProperty>

<owl:DatatypeProperty rdf:about="&soma;hasShapeParameter"
    rdfs:label="has shape parameter">
  <rdfs:comment>Associates a SpaceRegion to some parameter value describing its shape. This is a fairly generic property, and to capture the semantics of the information associated to the SpaceRegion, its more specific subproperties should be used.</rdfs:comment>
  <rdfs:domain rdf:resource="&soma;ShapeRegion"/>
  <rdfs:isDefinedBy rdf:resource="http://www.ease-crc.org/ont/SOMA-OBJ.owl"/>
  <rdfs:range>
    <rdfs:Datatype>
      <owl:unionOf rdf:parseType="Collection">
        <rdf:Description rdf:about="&soma;array_double"/>
        <rdf:Description rdf:about="&xsd;double"/>
        <rdf:Description rdf:about="&xsd;float"/>
        <rdf:Description rdf:about="&xsd;string"/>
      </owl:unionOf>
    </rdfs:Datatype>
  </rdfs:range>
  <rdfs:subPropertyOf rdf:resource="&dul;hasRegionDataValue"/>
</owl:DatatypeProperty>

<owl:Class rdf:about="&soma;Patient">
  <rdfs:isDefinedBy rdf:resource="http://www.ease-crc.org/ont/SOMA-OBJ.owl"/>
  <rdfs:isDefinedBy rdf:resource="http://www.ease-crc.org/ont/SOMA-PROC.owl"/>
  <rdfs:isDefinedBy rdf:resource="http://www.ease-crc.org/ont/SOMA-SAY.owl"/>
  <rdfs:comment>A role classifying an object that undergoes/is the primary object affected by the event.</rdfs:comment>
  <rdfs:subClassOf rdf:resource="&soma;EventAdjacentRole"/>
</owl:Class>

<owl:Class rdf:about="&soma;Opening">
  <owl:disjointWith rdf:resource="&soma;Pulling"/>
  <owl:disjointWith rdf:resource="&soma;Pushing"/>
  <owl:disjointWith rdf:resource="&soma;Squeezing"/>
  <rdfs:comment>A task in which an Agent manipulates a container so as to expose its interior.</rdfs:comment>
  <rdfs:isDefinedBy rdf:resource="http://www.ease-crc.org/ont/SOMA-ACT.owl"/>
  <rdfs:subClassOf rdf:resource="&soma;Actuating"/>
</owl:Class>

<owl:Class rdf:about="&dul;Relation">
  <rdfs:isDefinedBy rdf:resource="http://www.ease-crc.org/ont/SOMA-WF.owl"/>
</owl:Class>

<owl:Class rdf:about="&soma;CognitiveAgent">
  <rdfs:comment xml:lang="en">An agent that is capable to act on its own, in contrast to sub-cognitive Agents, that need to have their intentionality bestowed upon some other agent.</rdfs:comment>
  <rdfs:isDefinedBy rdf:resource="http://www.ease-crc.org/ont/SOMA-IO.owl"/>
  <rdfs:label xml:lang="en">cognitive agent</rdfs:label>
  <rdfs:subClassOf rdf:resource="&dul;Agent"/>
  <owl:disjointWith rdf:resource="&soma;SubCognitiveAgent"/>
</owl:Class>

<owl:ObjectProperty rdf:about="&soma;isSourceFor"
    rdfs:label="is source for">
  <rdf:type rdf:resource="&owl;TransitiveProperty"/>
  <rdfs:comment>The (transitive) relation between an information object and another which was derived from the former.</rdfs:comment>
  <rdfs:domain rdf:resource="&dul;InformationObject"/>
  <rdfs:isDefinedBy rdf:resource="http://www.ease-crc.org/ont/SOMA.owl"/>
  <rdfs:range rdf:resource="&dul;InformationObject"/>
  <rdfs:subPropertyOf rdf:resource="&dul;associatedWith"/>
</owl:ObjectProperty>

<owl:Class rdf:about="&soma;Shaping">
  <rdfs:subClassOf>
    <owl:Restriction>
      <owl:allValuesFrom>
        <owl:Restriction>
          <owl:allValuesFrom rdf:resource="&soma;Shape"/>
          <owl:onProperty rdf:resource="&dul;classifies"/>
        </owl:Restriction>
      </owl:allValuesFrom>
      <owl:onProperty rdf:resource="&soma;affordsSetpoint"/>
    </owl:Restriction>
  </rdfs:subClassOf>
  <rdfs:subClassOf>
    <owl:Restriction>
      <owl:allValuesFrom rdf:resource="&soma;ShapedObject"/>
      <owl:onProperty rdf:resource="&soma;affordsTrigger"/>
    </owl:Restriction>
  </rdfs:subClassOf>
  <rdfs:subClassOf rdf:resource="&soma;Variability"/>
  <rdfs:comment>The disposition of an object (the tool) to change the shape of others.</rdfs:comment>
  <rdfs:isDefinedBy rdf:resource="http://www.ease-crc.org/ont/SOMA-OBJ.owl"/>
</owl:Class>

<owl:ObjectProperty rdf:about="&soma;isConceptIncludedIn"
    rdfs:label="is concept included in">
  <rdfs:comment>A relation recording that a Concept participates in a Situation in some way.</rdfs:comment>
  <rdfs:domain rdf:resource="&dul;Concept"/>
  <rdfs:isDefinedBy rdf:resource="http://www.ease-crc.org/ont/SOMA.owl"/>
  <rdfs:range rdf:resource="&dul;Situation"/>
  <rdfs:subPropertyOf rdf:resource="&dul;isObjectIncludedIn"/>
</owl:ObjectProperty>

<owl:Class rdf:about="&dul;Action">
  <rdfs:comment>The EASE view: an Action is an Event in which an Agent executes some Task, typically defined by a Workflow, towards the achievement of some Goal.</rdfs:comment>
  <rdfs:subClassOf>
    <owl:Restriction>
      <owl:allValuesFrom rdf:resource="&dul;Task"/>
      <owl:onProperty rdf:resource="&dul;executesTask"/>
    </owl:Restriction>
  </rdfs:subClassOf>
</owl:Class>

<owl:Class rdf:about="&soma;LimbMotion"
    rdfs:comment="An Agent moves its limbs in some way."
    rdfs:label="Limb motion">
  <rdfs:subClassOf>
    <owl:Restriction>
      <owl:onProperty rdf:resource="&soma;isProcessTypeOf"/>
      <owl:someValuesFrom>
        <owl:Class>
          <owl:intersectionOf rdf:parseType="Collection">
            <rdf:Description rdf:about="&soma;MovedObject"/>
            <owl:Restriction>
              <owl:allValuesFrom rdf:resource="&soma;Limb"/>
              <owl:onProperty rdf:resource="&dul;classifies"/>
            </owl:Restriction>
          </owl:intersectionOf>
        </owl:Class>
      </owl:someValuesFrom>
    </owl:Restriction>
  </rdfs:subClassOf>
  <rdfs:subClassOf rdf:resource="&soma;DirectedMotion"/>
  <owl:disjointWith rdf:resource="&soma;Locomotion"/>
  <owl:disjointWith rdf:resource="&soma;PrehensileMotion"/>
  <rdfs:isDefinedBy rdf:resource="http://www.ease-crc.org/ont/SOMA-PROC.owl"/>
</owl:Class>

<owl:ObjectProperty rdf:about="&soma;isAskedBy"
    rdfs:comment="A relation from a Query to the Agent who asks it."
    rdfs:label="is asked by">
  <rdfs:domain rdf:resource="&soma;QueryingTask"/>
  <rdfs:isDefinedBy rdf:resource="http://www.ease-crc.org/ont/SOMA-ACT.owl"/>
  <rdfs:range rdf:resource="&dul;Agent"/>
  <rdfs:subPropertyOf rdf:resource="&dul;involvesAgent"/>
</owl:ObjectProperty>

<owl:ObjectProperty rdf:about="&dul;isAbout"/>

<owl:DatatypeProperty rdf:about="&dul;hasRegionDataValue">
  <rdfs:isDefinedBy rdf:resource="http://www.ease-crc.org/ont/SOMA.owl"/>
</owl:DatatypeProperty>

<owl:Class rdf:about="&soma;DesignedFurniture"
    rdfs:label="Designed furniture">
  <rdfs:comment>An object used to make a room or building suitable for living or working.</rdfs:comment>
  <rdfs:isDefinedBy rdf:resource="http://www.ease-crc.org/ont/SOMA-OBJ.owl"/>
  <rdfs:subClassOf rdf:resource="&dul;DesignedArtifact"/>
</owl:Class>

<owl:Class rdf:about="&soma;FixedJoint"
    rdfs:comment="A joint that cannot move, designed to fixiate links."
    rdfs:label="Fixed joint">
  <rdfs:subClassOf>
    <owl:Restriction>
      <owl:onClass rdf:resource="&dul;Entity"/>
      <owl:onProperty rdf:resource="&soma;hasJointState"/>
      <owl:qualifiedCardinality rdf:datatype="&xsd;nonNegativeInteger">0</owl:qualifiedCardinality>
    </owl:Restriction>
  </rdfs:subClassOf>
  <rdfs:subClassOf rdf:resource="&soma;Joint"/>
  <rdfs:isDefinedBy rdf:resource="http://www.ease-crc.org/ont/SOMA-OBJ.owl"/>
  <owl:disjointWith rdf:resource="&soma;MovableJoint"/>
</owl:Class>

<owl:Axiom>
  <rdfs:comment xml:lang="en">The file content.</rdfs:comment>
  <owl:annotatedProperty rdf:resource="&rdfs;subClassOf"/>
  <owl:annotatedSource rdf:resource="&soma;Digital_File"/>
  <owl:annotatedTarget>
    <owl:Restriction rdf:nodeID="bn0">
      <owl:onProperty rdf:resource="&dul;realizes"/>
      <owl:someValuesFrom rdf:resource="&soma;Structured_Text"/>
    </owl:Restriction>
  </owl:annotatedTarget>
</owl:Axiom>

<owl:Class rdf:about="&soma;RoomSurface"
    rdfs:comment="The surface of a room.">
  <rdfs:isDefinedBy rdf:resource="http://www.ease-crc.org/ont/SOMA-OBJ.owl"/>
  <rdfs:label xml:lang="en">Room surface</rdfs:label>
  <rdfs:subClassOf rdf:resource="&soma;Surface"/>
</owl:Class>

<owl:ObjectProperty rdf:about="&dul;definesTask">
  <rdfs:subPropertyOf rdf:resource="&soma;definesEventType"/>
</owl:ObjectProperty>

<owl:Class rdf:about="&dul;Quality"/>

<owl:Class rdf:about="&soma;ClausalObject"
    rdfs:comment="A clause is a phrase containing a subject and a predicate."
    rdfs:label="Clausal object">
  <rdfs:isDefinedBy rdf:resource="http://www.ease-crc.org/ont/SOMA-SAY.owl"/>
  <rdfs:subClassOf rdf:resource="&soma;Phrase"/>
</owl:Class>

<owl:DatatypeProperty rdf:about="&soma;hasShapeScale"
    rdfs:label="has shape scale">
  <rdfs:comment>The scale of a shape, given as a vector of three real numbers to adjust x, y, z components of vertex vectors. In cases where a shape needs to be flipped compared to the shape described by a mesh, one of the scale components will be negative. 

It is often the case that shapes need to be altered from their description in a shape file, and a typical example of this is scaling a mesh. 

In robotics, it is not uncommon to encounter shapes that are flipped compared to the shape in a mesh file. This is because robots often have bilateral symmetry, thus it makes sense to reuse the same meshes for corresponding links of the left and right arms.</rdfs:comment>
  <rdfs:domain rdf:resource="&soma;ShapeRegion"/>
  <rdfs:isDefinedBy rdf:resource="http://www.ease-crc.org/ont/SOMA-OBJ.owl"/>
  <rdfs:range rdf:resource="&soma;array_double"/>
  <rdfs:subPropertyOf rdf:resource="&soma;hasShapeParameter"/>
</owl:DatatypeProperty>

<owl:AsymmetricProperty rdf:about="&soma;hasInitialScene"
    rdfs:label="has initial scene">
  <rdf:type rdf:resource="&owl;IrreflexiveProperty"/>
  <rdf:type rdf:resource="&owl;ObjectProperty"/>
  <rdfs:comment>A relation between StateTransitions and Scenes, which identifies the scene the transition starts from.</rdfs:comment>
  <rdfs:domain rdf:resource="&soma;StateTransition"/>
  <rdfs:isDefinedBy rdf:resource="http://www.ease-crc.org/ont/SOMA.owl"/>
  <rdfs:range rdf:resource="&soma;Scene"/>
  <rdfs:subPropertyOf rdf:resource="&soma;hasInitialState"/>
  <owl:inverseOf rdf:resource="&soma;isInitialSceneOf"/>
</owl:AsymmetricProperty>

<owl:AsymmetricProperty rdf:about="&soma;isCoveredByObject">
  <rdf:type rdf:resource="&owl;IrreflexiveProperty"/>
  <rdf:type rdf:resource="&owl;ObjectProperty"/>
  <rdfs:comment>A relation from an object (the coveree) which is itself, or has its interior, prevented from being accessed from outside by a coverer.</rdfs:comment>
  <rdfs:domain rdf:resource="&dul;PhysicalObject"/>
  <rdfs:isDefinedBy rdf:resource="http://www.ease-crc.org/ont/SOMA-SAY.owl"/>
  <rdfs:range rdf:resource="&dul;PhysicalObject"/>
  <rdfs:subPropertyOf rdf:resource="&soma;interactsWith"/>
</owl:AsymmetricProperty>

<owl:Class rdf:about="&soma;Message">
  <rdfs:subClassOf>
    <owl:Restriction>
      <owl:onProperty rdf:resource="&dul;hasTask"/>
      <owl:someValuesFrom rdf:resource="&soma;CommunicationTask"/>
    </owl:Restriction>
  </rdfs:subClassOf>
  <rdfs:subClassOf>
    <owl:Restriction>
      <owl:allValuesFrom rdf:resource="&dul;InformationRealization"/>
      <owl:onProperty rdf:resource="&dul;classifies"/>
    </owl:Restriction>
  </rdfs:subClassOf>
  <rdfs:subClassOf rdf:resource="&soma;Item"/>
  <rdfs:comment xml:lang="en">A message is a discrete unit of communication intended by the source for consumption by some recipient or group of recipients (Source: https://en.wikipedia.org/wiki/Message).

Note that the Role Message classifies the Information Realization, not the content.</rdfs:comment>
  <rdfs:isDefinedBy rdf:resource="http://www.ease-crc.org/ont/SOMA-ACT.owl"/>
  <rdfs:label xml:lang="en">Message</rdfs:label>
</owl:Class>

<owl:DatatypeProperty rdf:about="&dul;hasDataValue">
  <rdfs:isDefinedBy rdf:resource="http://www.ease-crc.org/ont/SOMA.owl"/>
</owl:DatatypeProperty>

<owl:Class rdf:about="&dul;Workflow">
  <rdfs:isDefinedBy rdf:resource="http://www.ease-crc.org/ont/SOMA-WF.owl"/>
</owl:Class>

<owl:Class rdf:about="&soma;Labeling">
  <rdfs:label>A task in which an agent annotates some objects with names, e.g., labeling the feeling of a tip-of-the-tongue event as such.</rdfs:label>
  <rdfs:label>Labeling</rdfs:label>
  <rdfs:isDefinedBy rdf:resource="http://www.ease-crc.org/ont/SOMA-ACT.owl"/>
  <rdfs:subClassOf rdf:resource="&soma;Interpreting"/>
</owl:Class>

<owl:Class rdf:about="&soma;InterfaceSpecification">
  <rdfs:comment xml:lang="en">The Specification of an Interface between software, computer hardware, peripheral devices, humans and combinations of these.

Source: https://en.wikipedia.org/wiki/Interface_(computing)</rdfs:comment>
  <rdfs:isDefinedBy rdf:resource="http://www.ease-crc.org/ont/SOMA-IO.owl"/>
  <rdfs:label xml:lang="en">Interface Specification</rdfs:label>
  <rdfs:subClassOf rdf:resource="&dul;Design"/>
</owl:Class>

<owl:ObjectProperty rdf:about="&soma;definesParticipant">
  <rdfs:comment>A Description definesParticipant a Concept to classify participants in Events associated to that Description.

The prototypical example is a Task, which is a concept to classify Actions (a form of Event). A Task may define several Roles, with which to classify participants in the event of that Task's execution.</rdfs:comment>
  <rdfs:domain rdf:resource="&dul;Description"/>
  <rdfs:isDefinedBy rdf:resource="http://www.ease-crc.org/ont/SOMA-WF.owl"/>
  <rdfs:range rdf:resource="&dul;Concept"/>
  <rdfs:subPropertyOf rdf:resource="&dul;defines"/>
</owl:ObjectProperty>

<owl:Class rdf:about="&soma;Standing">
  <rdfs:comment>A motion by which an Agent arranges its body in an upright configuration. Typically, it makes sense to speak of standing for bodies where some limbs are dedicated to moving the whole body while some limbs are used for manipulation of other objects.</rdfs:comment>
  <rdfs:isDefinedBy rdf:resource="http://www.ease-crc.org/ont/SOMA-PROC.owl"/>
  <rdfs:subClassOf rdf:resource="&soma;PosturalMoving"/>
</owl:Class>

<owl:ObjectProperty rdf:about="&dul;includesEvent"/>

<owl:Class rdf:about="&soma;ProcessFlow"
    rdfs:comment="A description that structures a Process."
    rdfs:label="Process flow">
  <rdfs:subClassOf>
    <owl:Restriction>
      <owl:onProperty rdf:resource="&soma;definesProcess"/>
      <owl:someValuesFrom rdf:resource="&soma;ProcessType"/>
    </owl:Restriction>
  </rdfs:subClassOf>
  <rdfs:subClassOf rdf:resource="&dul;Description"/>
  <rdfs:isDefinedBy rdf:resource="http://www.ease-crc.org/ont/SOMA-PROC.owl"/>
</owl:Class>

<owl:ObjectProperty rdf:about="&soma;definesInput">
  <rdfs:comment>The defined participant is an "input": 

- some object existing at the beginning of a Task's execution, and that will be acted on during the execution of the task;
- some region/value which informs the way in which the Task will be executed.</rdfs:comment>
  <rdfs:domain rdf:resource="&dul;Description"/>
  <rdfs:isDefinedBy rdf:resource="http://www.ease-crc.org/ont/SOMA-WF.owl"/>
  <rdfs:range>
    <owl:Class>
      <owl:unionOf rdf:parseType="Collection">
        <rdf:Description rdf:about="&dul;Parameter"/>
        <rdf:Description rdf:about="&dul;Role"/>
      </owl:unionOf>
    </owl:Class>
  </rdfs:range>
  <rdfs:subPropertyOf rdf:resource="&soma;definesParticipant"/>
</owl:ObjectProperty>

<owl:ObjectProperty rdf:about="&dul;isDescribedBy">
  <rdfs:isDefinedBy rdf:resource="http://www.ease-crc.org/ont/SOMA-OBJ.owl"/>
  <rdfs:isDefinedBy rdf:resource="http://www.ease-crc.org/ont/SOMA-STATE.owl"/>
</owl:ObjectProperty>

<owl:ObjectProperty rdf:about="&soma;hasParentLink"
    rdfs:label="has parent link">
  <rdfs:comment>Relates a joint to the link it connects which is closer to the root of the kinematic chain.</rdfs:comment>
  <rdfs:domain rdf:resource="&soma;Joint"/>
  <rdfs:isDefinedBy rdf:resource="http://www.ease-crc.org/ont/SOMA-OBJ.owl"/>
  <rdfs:range rdf:resource="&dul;PhysicalObject"/>
  <rdfs:subPropertyOf rdf:resource="&dul;hasConstituent"/>
  <owl:inverseOf rdf:resource="&soma;isParentLinkOf"/>
</owl:ObjectProperty>

<owl:Class rdf:about="&dul;Agent">
  <rdfs:comment xml:lang="en">Generally, agents are goal-directed entities that are able to monitor their environment to select and perform efficient means-ends actions that are available in a given situation to achieve an intended goal. Agency, therefore, implies the ability to perceive and to change the environment of the agent. Crucially, it also entails intentionality to represent the goal-state in the future, equifinal variability to be able to achieve the intended goal-state with different actions in different contexts, and rationality of actions in relation to their goal to produce the most efficient action available (Source: https://en.wikipedia.org/wiki/Agency_(psychology)).

While we follow this definition, we do so loosely: We do not require the intentionality to be sourced by the agent. E.g., a running computer program (see Software instance) can be seen as an actor and therefore participate in Actions, e.g. some Communication Action, while its intentionality has been bestowed upon it from the agents who started the program or gave an input (e.g., via a mouse click) to achieve some goal.</rdfs:comment>
  <rdfs:isDefinedBy rdf:resource="http://www.ease-crc.org/ont/SOMA-STATE.owl"/>
</owl:Class>

<owl:ObjectProperty rdf:about="&dul;isEventIncludedIn"/>

<owl:ObjectProperty rdf:about="&soma;isExecutorDefinedIn">
  <rdfs:isDefinedBy rdf:resource="http://www.ease-crc.org/ont/SOMA-OBJ.owl"/>
</owl:ObjectProperty>

<owl:Class rdf:about="&soma;Remembering">
  <rdfs:comment xml:lang="en">A Mental task in which the Agent recalls a record of a previous state of affairs in the world.

The Agent must have witnessed and memorized this state of affairs in order to record it. Remembering commits itself to accuracy: the Agent attempts to reconstruct as accurate a record as it can. Note, this does not mean the Agent will communicate the recollection accurately.

The difference to Memory retrieval is that for this Task, we are concerned with knowledge about a previous world state. Memory Retrieval is more general in the sense that it also includes the retrieval of learned facts and rules.</rdfs:comment>
  <rdfs:isDefinedBy rdf:resource="http://www.ease-crc.org/ont/SOMA-ACT.owl"/>
  <rdfs:subClassOf>
    <owl:Class>
      <owl:intersectionOf rdf:parseType="Collection">
        <rdf:Description rdf:about="&soma;InformationRetrieval"/>
        <rdf:Description rdf:about="&soma;Retrospecting"/>
      </owl:intersectionOf>
    </owl:Class>
  </rdfs:subClassOf>
</owl:Class>

<owl:ObjectProperty rdf:about="&soma;affordsSetpoint"
    rdfs:label="affords setpoint">
  <rdfs:comment>Relates a disposition to the setpoint parameter defined by the affordance describing the disposition.</rdfs:comment>
  <rdfs:domain rdf:resource="&soma;Disposition"/>
  <rdfs:isDefinedBy rdf:resource="http://www.ease-crc.org/ont/SOMA-OBJ.owl"/>
  <rdfs:range rdf:resource="&soma;Setpoint"/>
  <rdfs:subPropertyOf rdf:resource="&soma;affordsConcept"/>
  <owl:inverseOf rdf:resource="&soma;isSetpointAffordedBy"/>
  <owl:propertyChainAxiom rdf:parseType="Collection">
    <rdf:Description rdf:about="&dul;isDescribedBy"/>
    <rdf:Description rdf:about="&soma;definesSetpoint"/>
  </owl:propertyChainAxiom>
</owl:ObjectProperty>

<owl:Class rdf:about="&soma;FailedAttempt"
    rdfs:comment="A description of a failed attempt to achieve some goal.">
  <rdfs:isDefinedBy rdf:resource="http://www.ease-crc.org/ont/SOMA.owl"/>
  <rdfs:label xml:lang="en">Failed attempt</rdfs:label>
  <rdfs:subClassOf rdf:resource="&soma;Unsuccessfulness"/>
</owl:Class>

<owl:Class rdf:about="&soma;Accident">
  <rdfs:comment>An Event for which causes are unknown and/or considered irrelevant. This is true also for "final causes" (that is, intentions) of Agents participating in the Accident: it is not the intentions of these Agents to bring about the Accident.

Note a distinction between this definition and some informal, everyday uses of "accident" which require a causal structure and responsibility to be ascertained. An accident, in the informal sense, may require an explanation as to who made a mistake in bringing about the event; a "traffic accident", where we want to know who's responsible, is an example of this.

Such an event does NOT fall under the definition of Accident here. An example of Accident would be a fair coin landing Heads: the causal chain for why this exact face landed is not important, all that matters is the brute fact that the coin landed Heads.</rdfs:comment>
  <rdfs:comment>also think about "mistakes": (Mihai:) yes, but consider whether those might qualify as Situations. Likewise for Accidents, actually.</rdfs:comment>
  <rdfs:isDefinedBy rdf:resource="http://www.ease-crc.org/ont/SOMA.owl"/>
  <rdfs:subClassOf rdf:resource="&dul;Event"/>
  <owl:disjointWith rdf:resource="&dul;Action"/>
</owl:Class>

<owl:Class rdf:about="&dul;Diagnosis"/>

<owl:Class rdf:about="&soma;ExistingObjectRole">
  <rdfs:subClassOf>
    <owl:Restriction>
      <owl:allValuesFrom rdf:resource="&dul;PhysicalObject"/>
      <owl:onProperty rdf:resource="&dul;classifies"/>
    </owl:Restriction>
  </rdfs:subClassOf>
  <rdfs:subClassOf rdf:resource="&soma;RelationAdjacentRole"/>
  <rdfs:comment>A role that requires of its filler simply to exist, unlike other roles that may demand e.g. agentive or instrumental participation in some executable schema or plan (AgentRole and Instrument respectively).

The intention behind such a simple role is to have a way to represent, in a schematic formalism used to describe some scene, that an object is present. In particular, the schema used to convey this information is the ESTSchemaTheory, which has ExistingObjectRole as its sole defined role.</rdfs:comment>
  <rdfs:isDefinedBy rdf:resource="http://www.ease-crc.org/ont/SOMA-OBJ.owl"/>
  <rdfs:label xml:lang="en">Existing object role</rdfs:label>
</owl:Class>

<owl:Class rdf:about="&dul;PhysicalBody"/>

<owl:Class rdf:about="&soma;EnclosedObject">
  <rdfs:comment>An object included within the spatial boundaries of another object.</rdfs:comment>
  <rdfs:isDefinedBy rdf:resource="http://www.ease-crc.org/ont/SOMA-OBJ.owl"/>
  <rdfs:label xml:lang="en">Enclosed object</rdfs:label>
  <rdfs:subClassOf rdf:resource="&soma;IncludedObject"/>
</owl:Class>

<owl:ObjectProperty rdf:about="&soma;containsObject"
    rdfs:label="contains object">
  <rdfs:subPropertyOf rdf:resource="&soma;contains"/>
  <rdfs:subPropertyOf rdf:resource="&dul;isLocationOf"/>
  <rdf:type rdf:resource="&owl;TransitiveProperty"/>
  <rdfs:comment>A spatial relation holding between a container, and objects it contains.</rdfs:comment>
  <rdfs:domain rdf:resource="&dul;PhysicalObject"/>
  <rdfs:isDefinedBy rdf:resource="http://www.ease-crc.org/ont/SOMA-OBJ.owl"/>
  <rdfs:range rdf:resource="&dul;PhysicalObject"/>
  <owl:inverseOf rdf:resource="&soma;isInsideOf"/>
</owl:ObjectProperty>

<owl:Class rdf:about="&dul;Situation">
  <rdfs:isDefinedBy rdf:resource="http://www.ease-crc.org/ont/SOMA-PROC.owl"/>
  <rdfs:subClassOf>
    <owl:Class>
      <owl:complementOf>
        <owl:Class>
          <owl:intersectionOf rdf:parseType="Collection">

            <owl:Restriction>
              <owl:onProperty rdf:resource="http://www.ease-crc.org/ont/SOMA.owl/manifestsIn"/>
              <owl:someValuesFrom rdf:resource="&dul;Event"/>
            </owl:Restriction>

            <owl:Restriction>
              <owl:onProperty rdf:resource="http://www.ease-crc.org/ont/SOMA.owl/prevents"/>
              <owl:someValuesFrom>
                <owl:Restriction>
                  <owl:onProperty rdf:resource="http://www.ease-crc.org/ont/SOMA.owl/manifestsIn"/>
                  <owl:someValuesFrom rdf:resource="&dul;Event"/>
                </owl:Restriction>
              </owl:someValuesFrom>
            </owl:Restriction>
          </owl:intersectionOf>
        </owl:Class>
      </owl:complementOf>
    </owl:Class>
  </rdfs:subClassOf>
</owl:Class>

<owl:ObjectProperty rdf:about="&soma;involvesArtifact"
    rdfs:comment="Artifact participation."
    rdfs:label="involves artifact">
  <rdfs:domain rdf:resource="&dul;Event"/>
  <rdfs:isDefinedBy rdf:resource="http://www.ease-crc.org/ont/SOMA.owl"/>
  <rdfs:range rdf:resource="&dul;PhysicalArtifact"/>
  <rdfs:subPropertyOf rdf:resource="&dul;hasParticipant"/>
  <owl:inverseOf rdf:resource="&soma;isArtifactInvolvedIn"/>
</owl:ObjectProperty>

<owl:ObjectProperty rdf:about="&soma;isJointLimitOf"
    rdfs:comment="Relates a joint to its physical limits."
    rdfs:label="is joint limit of">
  <rdfs:domain rdf:resource="&soma;JointLimit"/>
  <rdfs:isDefinedBy rdf:resource="http://www.ease-crc.org/ont/SOMA-OBJ.owl"/>
  <rdfs:range rdf:resource="&soma;Joint"/>
  <rdfs:subPropertyOf rdf:resource="&dul;isRegionFor"/>
</owl:ObjectProperty>

<owl:Class rdf:about="&soma;Turning">
  <rdfs:comment>A motion by which an agent changes which way their body faces.</rdfs:comment>
  <rdfs:isDefinedBy rdf:resource="http://www.ease-crc.org/ont/SOMA-PROC.owl"/>
  <rdfs:subClassOf rdf:resource="&soma;PosturalMoving"/>
</owl:Class>

<owl:Class rdf:about="&dul;Object"/>

<owl:ObjectProperty rdf:about="&soma;hasShapeRegion"
    rdfs:label="has shape region">
  <rdfs:comment>A relation between physical objects and their shape attribute.</rdfs:comment>
  <rdfs:domain>
    <owl:Class>
      <owl:unionOf rdf:parseType="Collection">
        <rdf:Description rdf:about="&soma;Shape"/>
        <rdf:Description rdf:about="&dul;PhysicalObject"/>
      </owl:unionOf>
    </owl:Class>
  </rdfs:domain>
  <rdfs:isDefinedBy rdf:resource="http://www.ease-crc.org/ont/SOMA-OBJ.owl"/>
  <rdfs:range rdf:resource="&soma;ShapeRegion"/>
  <rdfs:subPropertyOf rdf:resource="&dul;hasRegion"/>
  <owl:inverseOf rdf:resource="&soma;isShapeRegionOf"/>
</owl:ObjectProperty>

<owl:DatatypeProperty rdf:about="&soma;hasJointVelocityLimit"
    rdfs:label="has joint velocity limit">
  <rdfs:comment>The maximum velocity of a joint given in m/s (prismatic joints) or rad/s (hinged joints).</rdfs:comment>
  <rdfs:domain rdf:resource="&soma;JointLimit"/>
  <rdfs:isDefinedBy rdf:resource="http://www.ease-crc.org/ont/SOMA-OBJ.owl"/>
  <rdfs:range rdf:resource="&xsd;double"/>
  <rdfs:subPropertyOf rdf:resource="&soma;hasJointParameter"/>
</owl:DatatypeProperty>

<owl:Class rdf:about="&soma;PuttingDown">
  <rdfs:comment>A task in which an Agent puts down an object they have kinematic control over, e.g. a grasped object.</rdfs:comment>
  <rdfs:isDefinedBy rdf:resource="http://www.ease-crc.org/ont/SOMA-ACT.owl"/>
  <rdfs:subClassOf rdf:resource="&soma;Manipulating"/>
</owl:Class>

<owl:ObjectProperty rdf:about="&soma;hasSuccessor">
  <rdfs:comment>Indicates that a Task is the successor in a Succedence Relation: that is, it is the Task to execute last.</rdfs:comment>
  <rdfs:domain rdf:resource="&soma;Succedence"/>
  <rdfs:isDefinedBy rdf:resource="http://www.ease-crc.org/ont/SOMA-WF.owl"/>
  <rdfs:label xml:lang="en">has successor</rdfs:label>
  <rdfs:range rdf:resource="&dul;Workflow"/>
  <rdfs:subPropertyOf rdf:resource="&dul;hasPart"/>
</owl:ObjectProperty>

<owl:Class rdf:about="&dul;Concept">
  <rdfs:isDefinedBy rdf:resource="http://www.ease-crc.org/ont/SOMA-WF.owl"/>
</owl:Class>

<owl:Class rdf:about="&soma;GetTaskParameter">
  <rdfs:comment>A task in which an Agent computes some parameter relevant for another task.</rdfs:comment>
  <rdfs:isDefinedBy rdf:resource="http://www.ease-crc.org/ont/SOMA-ACT.owl"/>
  <rdfs:label xml:lang="en">Get task parameter</rdfs:label>
  <rdfs:subClassOf rdf:resource="&soma;Planning"/>
</owl:Class>

<owl:Class rdf:about="&soma;SocialQuality"
    rdfs:label="Social quality">
  <rdfs:comment>Any aspect of an entity that specifies social characteristics.</rdfs:comment>
  <rdfs:isDefinedBy rdf:resource="http://www.ease-crc.org/ont/SOMA-OBJ.owl"/>
  <rdfs:subClassOf rdf:resource="&dul;Quality"/>
</owl:Class>

<owl:ObjectProperty rdf:about="&soma;hasGoal">
  <rdfs:comment>A relation from an Entity to a Goal it pursues. Agents can pursue Goals, and Tasks are also construed as pursuing Goals.</rdfs:comment>
  <rdfs:domain rdf:resource="&dul;Entity"/>
  <rdfs:isDefinedBy rdf:resource="http://www.ease-crc.org/ont/SOMA.owl"/>
  <rdfs:label xml:lang="en">has goal</rdfs:label>
  <rdfs:range rdf:resource="&dul;Goal"/>
  <rdfs:subPropertyOf rdf:resource="&dul;isDescribedBy"/>
</owl:ObjectProperty>

<owl:Class rdf:about="&soma;ConditionalSuccedence">
  <rdfs:comment>A relation that holds between two OGPTasks that belong to the same OGPWorkflow, and which means that, if a condition is met, the successor task invocation is to be executed after the predecessor task invocation completes.

The condition is a conjunction of CounterfactualBindings. These bindings may be RoleRoleBindings (meaning, test whether the fillers for these Roles/Parameters are the same) or RoleFillerBindings (meaning, test whether the filler of the Role unifies with the candidate Entity).

An empty conjunction of CounterfactualBindings is assumed to be True.</rdfs:comment>
  <rdfs:comment>Note: in RobotWorkflows, Tasks typically may have several possible successors, to be selected based on condition-testing.</rdfs:comment>
  <rdfs:subClassOf>
    <owl:Restriction>
      <owl:allValuesFrom rdf:resource="&soma;CounterfactualBinding"/>
      <owl:onProperty rdf:resource="&soma;hasBinding"/>
    </owl:Restriction>
  </rdfs:subClassOf>
  <rdfs:subClassOf rdf:resource="&soma;Succedence"/>
  <rdfs:isDefinedBy rdf:resource="http://www.ease-crc.org/ont/SOMA-WF.owl"/>
  <rdfs:label xml:lang="en">Conditional succedence</rdfs:label>
</owl:Class>

<owl:Class rdf:about="&soma;Database">
  <rdfs:comment xml:lang="en">A Database is a Software that organizes a collection of data stored and and allows for access, usually via some query engine.

Source: https://en.wikipedia.org/wiki/Database</rdfs:comment>
  <rdfs:isDefinedBy rdf:resource="http://www.ease-crc.org/ont/SOMA-IO.owl"/>
  <rdfs:subClassOf rdf:resource="&soma;SoftwareRole"/>
</owl:Class>

<owl:ObjectProperty rdf:about="&dul;isRoleOf"/>

<owl:Class rdf:about="&soma;ImageSchemaTheory">
  <rdfs:comment>A theory that describes an image-schematic relationship between some entities.

Image schemas are considered as fundamental, pre-conceptual, building blocks of cognition. They were introduced to characterize how human beings are believed to organize and make sense of experience.

For SOMA, whereas the focus of executable schematic theories is to describe how an agent might act, image schematic theories focus on descriptions of how objects behave in the absence of, or after, an active intervention from an agent.</rdfs:comment>
  <rdfs:isDefinedBy rdf:resource="http://www.ease-crc.org/ont/SOMA-SAY.owl"/>
  <rdfs:label xml:lang="en">Image schema theory</rdfs:label>
  <rdfs:subClassOf rdf:resource="&soma;SchematicTheory"/>
</owl:Class>

<owl:ObjectProperty rdf:about="&soma;isDefinedInAffordance"
    rdfs:comment="A relation between a Concept and an Affordance."
    rdfs:label="is defined in affordance">
  <rdfs:domain rdf:resource="&dul;Concept"/>
  <rdfs:isDefinedBy rdf:resource="http://www.ease-crc.org/ont/SOMA-OBJ.owl"/>
  <rdfs:range rdf:resource="&soma;Affordance"/>
  <rdfs:subPropertyOf rdf:resource="&dul;isDefinedIn"/>
</owl:ObjectProperty>

<owl:ObjectProperty rdf:about="&dul;directlyFollows"/>

<owl:ObjectProperty rdf:about="&dul;isLocationOf"/>

<owl:AsymmetricProperty rdf:about="&soma;meets"
    soma:symbol="m">
  <rdf:type rdf:resource="&owl;IrreflexiveProperty"/>
  <rdf:type rdf:resource="&owl;ObjectProperty"/>
  <rdfs:comment>A relation between entities, expressing a 'sequence' schema where one of the entities exactly ends where the other entity starts.</rdfs:comment>
  <rdfs:domain rdf:resource="&dul;Entity"/>
  <rdfs:isDefinedBy rdf:resource="http://www.ease-crc.org/ont/SOMA.owl"/>
  <rdfs:range rdf:resource="&dul;Entity"/>
  <rdfs:subPropertyOf rdf:resource="&dul;directlyPrecedes"/>
  <owl:inverseOf rdf:resource="&soma;metBy"/>
</owl:AsymmetricProperty>

<owl:Class rdf:about="&soma;IntermediateGrasp"
    rdfs:label="Intermediate grasp">
  <owl:disjointWith rdf:resource="&soma;PowerGrasp"/>
  <owl:disjointWith rdf:resource="&soma;PrecisionGrasp"/>
  <rdfs:comment>A kind of grasp that acquires kinematic control over the gripped object, but without attempting to achieve either strong holding force nor precision of subsequent movement of the gripped object.</rdfs:comment>
  <rdfs:isDefinedBy rdf:resource="http://www.ease-crc.org/ont/SOMA-PROC.owl"/>
  <rdfs:subClassOf rdf:resource="&soma;GraspingMotion"/>
</owl:Class>

<owl:ObjectProperty rdf:about="&soma;isStateTypeOf"
    rdfs:label="is state type of">
  <rdfs:comment>A relation between roles and state types, e.g. 'the chair is the supporter of the person sitting on it'.</rdfs:comment>
  <rdfs:domain rdf:resource="&soma;StateType"/>
  <rdfs:isDefinedBy rdf:resource="http://www.ease-crc.org/ont/SOMA-STATE.owl"/>
  <rdfs:range rdf:resource="&dul;Role"/>
  <rdfs:subPropertyOf rdf:resource="&dul;isRelatedToConcept"/>
</owl:ObjectProperty>

<owl:Class rdf:about="&soma;Fetching">
  <owl:disjointWith rdf:resource="&soma;Lifting"/>
  <owl:disjointWith rdf:resource="&soma;Opening"/>
  <owl:disjointWith rdf:resource="&soma;Pulling"/>
  <owl:disjointWith rdf:resource="&soma;Pushing"/>
  <owl:disjointWith rdf:resource="&soma;Squeezing"/>
  <rdfs:comment>A task in which an Agent retrieves an object from a particular location, which puts the object under the Agent's control, who can now e.g. transport the object somewhere else; this task may include repositioning the Agent to better reach the object. Note that while in normal linguistic use fetch can mean transport, we use it here to refer only to (a part of) the first stage of transport.</rdfs:comment>
  <rdfs:isDefinedBy rdf:resource="http://www.ease-crc.org/ont/SOMA-ACT.owl"/>
  <rdfs:subClassOf rdf:resource="&soma;PhysicalAcquiring"/>
</owl:Class>

<owl:Class rdf:about="&soma;DepositedObject"
    rdfs:comment="An object placed ontop of another one.">
  <rdfs:isDefinedBy rdf:resource="http://www.ease-crc.org/ont/SOMA-OBJ.owl"/>
  <rdfs:label xml:lang="en">Deposited object</rdfs:label>
  <rdfs:subClassOf rdf:resource="&soma;Patient"/>
</owl:Class>

<owl:Class rdf:about="&soma;PouredObject"
    rdfs:label="Poured object">
  <rdfs:comment>An object being poured into or onto some other object. A role of some fluid or substance that is the patient of pouring task.</rdfs:comment>
  <rdfs:isDefinedBy rdf:resource="http://www.ease-crc.org/ont/SOMA-OBJ.owl"/>
  <rdfs:subClassOf rdf:resource="&soma;Patient"/>
</owl:Class>

<owl:Class rdf:about="&soma;ClientRole">
  <rdfs:subClassOf>
    <owl:Restriction>
      <owl:onProperty rdf:resource="&dul;isDefinedIn"/>
      <owl:someValuesFrom rdf:resource="&soma;Client-Server_Specification"/>
    </owl:Restriction>
  </rdfs:subClassOf>
  <rdfs:subClassOf rdf:resource="&soma;InterfaceComponentRole"/>
  <rdfs:comment xml:lang="en">The Client-server model is a distributed application structure that partitions tasks or workloads between the providers of a resource or service, called servers, and service requesters, called clients Often clients and servers communicate over a computer network on separate hardware, but both client and server may reside in the same system. A server host runs one or more server programs, which share their resources with clients. A client usually does not share any of its resources, but it requests content or service from a server. Clients, therefore, initiate communication sessions with servers, which await incoming requests. Examples of computer applications that use the client-server model are email, network printing, and the World Wide Web.

Source: https://en.wikipedia.org/wiki/Client%E2%80%93server_model</rdfs:comment>
  <rdfs:isDefinedBy rdf:resource="http://www.ease-crc.org/ont/SOMA-IO.owl"/>
  <rdfs:label xml:lang="en">Client role</rdfs:label>
</owl:Class>

<owl:Class rdf:about="&soma;Sluggishness"
    rdfs:comment="A description of sluggish behavior.">
  <rdfs:isDefinedBy rdf:resource="http://www.ease-crc.org/ont/SOMA.owl"/>
  <rdfs:subClassOf rdf:resource="&soma;Amateurish"/>
</owl:Class>

<owl:Class rdf:about="&soma;SpatioTemporalRole">
  <rdfs:comment>Roles that classify entities which locate an event or object in space and time.</rdfs:comment>
  <rdfs:isDefinedBy rdf:resource="http://www.ease-crc.org/ont/SOMA-OBJ.owl"/>
  <rdfs:label xml:lang="en">Spatio-temporal role</rdfs:label>
  <rdfs:subClassOf rdf:resource="&soma;EventAdjacentRole"/>
</owl:Class>

<owl:Class rdf:about="&soma;PhysicalQuality"
    rdfs:label="Physical quality">
  <rdfs:subClassOf>
    <owl:Restriction>
      <owl:onClass rdf:resource="&dul;PhysicalObject"/>
      <owl:onProperty rdf:resource="&dul;isQualityOf"/>
      <owl:qualifiedCardinality rdf:datatype="&xsd;nonNegativeInteger">1</owl:qualifiedCardinality>
    </owl:Restriction>
  </rdfs:subClassOf>
  <rdfs:subClassOf rdf:resource="&dul;Quality"/>
  <rdfs:comment>Any aspect of an entity that is dependent on its physical manifestation.</rdfs:comment>
  <rdfs:isDefinedBy rdf:resource="http://www.ease-crc.org/ont/SOMA-OBJ.owl"/>
</owl:Class>

<owl:Class rdf:about="&soma;ModifyingPhysicalObject">
  <rdfs:comment>Superconcept for tasks that involve affecting some state that an object is in (e.g. where it is located), without creating or destroying the object.</rdfs:comment>
  <rdfs:isDefinedBy rdf:resource="http://www.ease-crc.org/ont/SOMA-ACT.owl"/>
  <rdfs:label xml:lang="en">Modifying physical object</rdfs:label>
  <rdfs:subClassOf rdf:resource="&soma;PhysicalTask"/>
</owl:Class>

<owl:ObjectProperty rdf:about="&soma;isAnsweredBy"
    rdfs:comment="A relation from a Query to an Agent who answers it."
    rdfs:label="is answered by">
  <rdfs:domain rdf:resource="&dul;Event"/>
  <rdfs:isDefinedBy rdf:resource="http://www.ease-crc.org/ont/SOMA-SAY.owl"/>
  <rdfs:range rdf:resource="&dul;Agent"/>
  <rdfs:subPropertyOf rdf:resource="&dul;involvesAgent"/>
</owl:ObjectProperty>

<owl:Class rdf:about="&soma;Collision">
  <rdfs:comment>A contact event of objects bumping into each other such that their movement is affected.</rdfs:comment>
  <rdfs:isDefinedBy rdf:resource="http://www.ease-crc.org/ont/SOMA-PROC.owl"/>
  <rdfs:subClassOf rdf:resource="&soma;ProcessType"/>
</owl:Class>

<owl:Class rdf:about="&soma;PhysicalAction"
    rdfs:label="Physical action">
  <rdfs:comment>An action performed by an agent by using its body in some way to interact with the physical world, e.g., through manipulation of objects, or by changing the posture.</rdfs:comment>
  <rdfs:isDefinedBy rdf:resource="http://www.ease-crc.org/ont/SOMA-ACT.owl"/>
  <rdfs:subClassOf rdf:resource="&dul;Action"/>
</owl:Class>

<owl:Class rdf:about="&soma;RemovedObject"
    rdfs:comment="An object that is removed from another."
    rdfs:label="Removed object">
  <rdfs:isDefinedBy rdf:resource="http://www.ease-crc.org/ont/SOMA-OBJ.owl"/>
  <rdfs:subClassOf rdf:resource="&soma;ExcludedObject"/>
</owl:Class>

<owl:Class rdf:about="&soma;RecipientRole">
  <rdfs:comment>A role which classifies an agent who receives an object modified or created by an action.</rdfs:comment>
  <rdfs:isDefinedBy rdf:resource="http://www.ease-crc.org/ont/SOMA-OBJ.owl"/>
  <rdfs:label xml:lang="en">Recipent role</rdfs:label>
  <rdfs:subClassOf rdf:resource="&soma;BeneficiaryRole"/>
</owl:Class>

<owl:Class rdf:about="&soma;SoftwareInstance">
  <rdfs:subClassOf>
    <owl:Class>
      <owl:intersectionOf rdf:parseType="Collection">
        <rdf:Description rdf:about="&dul;SocialAgent"/>
        <owl:Restriction>
          <owl:onProperty rdf:resource="&dul;actsFor"/>
          <owl:someValuesFrom rdf:resource="&dul;Agent"/>
        </owl:Restriction>
      </owl:intersectionOf>
    </owl:Class>
  </rdfs:subClassOf>
  <rdfs:subClassOf>
    <owl:Restriction>
      <owl:onProperty rdf:resource="&soma;isDesignedBy"/>
      <owl:someValuesFrom rdf:resource="&soma;Software"/>
    </owl:Restriction>
  </rdfs:subClassOf>
  <rdfs:comment xml:lang="en">A Software instance is an entity to represent the agent that emerges from and while executing software: Some object, that can perform actions and communicate via some interfaces.
In this view, we see the of an Agent required intentionality its intentionality as bestowed upon the Software instance from the agents who started the program or gave an input (e.g., via a mouse click) to achieve some goal.

Another apporach might be to not model this entity at all and only see Execution of Software as a Process (see, e.g., https://en.wikipedia.org/wiki/Execution_(computing)). However, this would complicate modeling communication between running Software processes.</rdfs:comment>
  <rdfs:isDefinedBy rdf:resource="http://www.ease-crc.org/ont/SOMA-IO.owl"/>
  <rdfs:label xml:lang="en">Software instance</rdfs:label>
</owl:Class>

<owl:Class rdf:about="&soma;HingeJoint"
    rdfs:comment="A joint that rotates along an axis."
    rdfs:label="Hinge joint">
  <rdfs:isDefinedBy rdf:resource="http://www.ease-crc.org/ont/SOMA-OBJ.owl"/>
  <rdfs:subClassOf rdf:resource="&soma;MovableJoint"/>
</owl:Class>

<owl:DatatypeProperty rdf:about="&soma;hasWidth"
    rdfs:comment="The width of a shape."
    rdfs:label="has width">
  <rdfs:domain rdf:resource="&soma;ShapeRegion"/>
  <rdfs:isDefinedBy rdf:resource="http://www.ease-crc.org/ont/SOMA-OBJ.owl"/>
  <rdfs:range rdf:resource="&xsd;float"/>
  <rdfs:subPropertyOf rdf:resource="&soma;hasShapeParameter"/>
</owl:DatatypeProperty>

<owl:DatatypeProperty rdf:about="&soma;hasFrictionValue"
    rdfs:label="has friction value">
  <rdfs:comment>The coefficient of friction denotes the ratio of friction force between touching objects. The coefficient is dimensionless.</rdfs:comment>
  <rdfs:domain rdf:resource="&soma;FrictionAttribute"/>
  <rdfs:isDefinedBy rdf:resource="http://www.ease-crc.org/ont/SOMA-OBJ.owl"/>
  <rdfs:range rdf:resource="&xsd;double"/>
  <rdfs:subPropertyOf rdf:resource="&dul;hasRegionDataValue"/>
</owl:DatatypeProperty>

<owl:Class rdf:about="&soma;SupportedObject"
    rdfs:comment="An object that is supported by some supporter.">
  <rdfs:isDefinedBy rdf:resource="http://www.ease-crc.org/ont/SOMA-OBJ.owl"/>
  <rdfs:label xml:lang="en">Supported object</rdfs:label>
  <rdfs:subClassOf rdf:resource="&soma;ConnectedObject"/>
</owl:Class>

<owl:ObjectProperty rdf:about="&dul;hasComponent">
  <rdfs:isDefinedBy rdf:resource="http://www.ease-crc.org/ont/SOMA.owl"/>
</owl:ObjectProperty>

<owl:Class rdf:about="&soma;BehavioralDiagnosis"
    rdfs:comment="A diagnosis of how a system interacts with its world."
    rdfs:label="Behavioral diagnosis">
  <rdfs:subClassOf>
    <owl:Restriction>
      <owl:onProperty rdf:resource="&dul;hasConstituent"/>
      <owl:someValuesFrom rdf:resource="&dul;Goal"/>
    </owl:Restriction>
  </rdfs:subClassOf>
  <rdfs:subClassOf rdf:resource="&dul;Diagnosis"/>
  <rdfs:isDefinedBy rdf:resource="http://www.ease-crc.org/ont/SOMA.owl"/>
</owl:Class>

<owl:Axiom>
  <rdfs:comment>A SituationTransition that manifests in some Event also includes an Action. (NOTE (MP): Typically, the Event manifesting it would be that included Action actually so perhaps we can just require that manifestations of SituationTransitions be Actions?)</rdfs:comment>
  <owl:annotatedProperty rdf:resource="&rdfs;subClassOf"/>
  <owl:annotatedSource>
    <owl:Class>
      <rdfs:subClassOf>
        <owl:Restriction rdf:nodeID="bn1">
          <owl:onProperty rdf:resource="&dul;includesEvent"/>
          <owl:someValuesFrom rdf:resource="&dul;Action"/>
        </owl:Restriction>
      </rdfs:subClassOf>
      <owl:intersectionOf rdf:parseType="Collection">
        <rdf:Description rdf:about="&soma;SituationTransition"/>
        <owl:Restriction>
          <owl:onProperty rdf:resource="http://www.ease-crc.org/ont/SOMA.owl/manifestsIn"/>
          <owl:someValuesFrom rdf:resource="&dul;Event"/>
        </owl:Restriction>
      </owl:intersectionOf>
    </owl:Class>
  </owl:annotatedSource>
  <owl:annotatedTarget rdf:nodeID="bn1"/>
</owl:Axiom>

<owl:Class rdf:about="&soma;Option">
  <rdfs:comment xml:lang="en">The Role of objects that are used, e.g., in Selecting Tasks.</rdfs:comment>
  <rdfs:isDefinedBy rdf:resource="http://www.ease-crc.org/ont/SOMA-AGENT.owl"/>
  <rdfs:label xml:lang="en">Option</rdfs:label>
  <rdfs:subClassOf rdf:resource="&soma;ResourceRole"/>
</owl:Class>

<owl:Class rdf:about="&soma;RoleFillerBinding"
    rdfs:comment="A binding that connects a role to a particular filler.">
  <rdfs:isDefinedBy rdf:resource="http://www.ease-crc.org/ont/SOMA-WF.owl"/>
  <rdfs:label xml:lang="en">Role filler binding</rdfs:label>
  <rdfs:subClassOf rdf:resource="&soma;Binding"/>
  <owl:disjointWith rdf:resource="&soma;RoleRoleBinding"/>
</owl:Class>

<owl:ObjectProperty rdf:about="&soma;isPhysicallyContainedIn"
    rdfs:label="is physically contained in">
  <rdfs:comment>A spatial relation holding between an object (the container), and objects it contains.</rdfs:comment>
  <rdfs:domain rdf:resource="&dul;Entity"/>
  <rdfs:isDefinedBy rdf:resource="http://www.ease-crc.org/ont/SOMA-OBJ.owl"/>
  <rdfs:range rdf:resource="&dul;Entity"/>
  <rdfs:subPropertyOf rdf:resource="&dul;isLocationOf"/>
</owl:ObjectProperty>

<owl:Class rdf:about="&soma;Walking">
  <rdfs:comment>An agent, under its own power, moves over some solid surface.</rdfs:comment>
  <rdfs:isDefinedBy rdf:resource="http://www.ease-crc.org/ont/SOMA-PROC.owl"/>
  <rdfs:subClassOf rdf:resource="&soma;Locomotion"/>
</owl:Class>

<owl:Class rdf:about="http://www.ease-crc.org/ont/SOMA.owl#6DPose">
  <rdfs:subClassOf>
    <owl:Restriction>
      <owl:onDataRange rdf:resource="&xsd;string"/>
      <owl:onProperty rdf:resource="&soma;hasPositionData"/>
      <owl:qualifiedCardinality rdf:datatype="&xsd;nonNegativeInteger">1</owl:qualifiedCardinality>
    </owl:Restriction>
  </rdfs:subClassOf>
  <rdfs:subClassOf rdf:resource="&dul;SpaceRegion"/>
  <rdfs:comment>A point in three dimensional space, given as translation in a reference coordinate system, and an orientation of a coordinate system centered at that point relative to the reference coordinate system.</rdfs:comment>
  <rdfs:isDefinedBy rdf:resource="http://www.ease-crc.org/ont/SOMA-OBJ.owl"/>
  <rdfs:label xml:lang="en">6D pose</rdfs:label>
</owl:Class>

<owl:Class rdf:about="&soma;ExperiencerRole">
  <rdfs:comment>A role used in frame semantics to classify agents performing perception actions, or being the subjects affected by some biological process.</rdfs:comment>
  <rdfs:isDefinedBy rdf:resource="http://www.ease-crc.org/ont/SOMA-OBJ.owl"/>
  <rdfs:label xml:lang="en">Experiencer role</rdfs:label>
  <rdfs:subClassOf rdf:resource="&soma;PerformerRole"/>
</owl:Class>

<owl:ObjectProperty rdf:about="&soma;involvesPlace"
    rdfs:label="involves place">
  <rdfs:comment>A relation recording that an Event makes some use of a PhysicalPlace. Typically this place is where the Event is located.</rdfs:comment>
  <rdfs:domain rdf:resource="&dul;Event"/>
  <rdfs:isDefinedBy rdf:resource="http://www.ease-crc.org/ont/SOMA.owl"/>
  <rdfs:range rdf:resource="&dul;PhysicalPlace"/>
  <rdfs:subPropertyOf rdf:resource="&dul;hasParticipant"/>
  <owl:inverseOf rdf:resource="&soma;isPlaceInvolvedIn"/>
</owl:ObjectProperty>

<owl:Class rdf:about="&soma;GraspTransfer">
  <rdfs:comment>A task in which an Agent switches which of its end effectors holds an object.</rdfs:comment>
  <rdfs:isDefinedBy rdf:resource="http://www.ease-crc.org/ont/SOMA-ACT.owl"/>
  <rdfs:label xml:lang="en">Grasp transfer</rdfs:label>
  <rdfs:subClassOf rdf:resource="&soma;Grasping"/>
</owl:Class>

<owl:Class rdf:about="&soma;MentalAction"
    rdfs:label="Mental action">
  <rdfs:subClassOf>
    <owl:Restriction>
      <owl:allValuesFrom>
        <owl:Class>
          <owl:unionOf rdf:parseType="Collection">
            <rdf:Description rdf:about="&dul;Agent"/>
            <rdf:Description rdf:about="&dul;SocialObject"/>
          </owl:unionOf>
        </owl:Class>
      </owl:allValuesFrom>
      <owl:onProperty rdf:resource="&dul;hasParticipant"/>
    </owl:Restriction>
  </rdfs:subClassOf>
  <rdfs:subClassOf rdf:resource="&dul;Action"/>
  <rdfs:comment>An Event construed as the Agent participant affecting Entities that are representations of actual or potential Entities or Events in the physical world in which the Agent is embodied. These representations are maintained by the Agent participant in the 'Mental action' event.

One could argue Mental actions are all Physical actions, because anything the Agent may use to maintain such representations will be physical things, However, we make this distinction because for Mental actions it is less important to consider the physical support of the representation and how it changes, and more important to track how the information content of the representation changes.</rdfs:comment>
  <rdfs:isDefinedBy rdf:resource="http://www.ease-crc.org/ont/SOMA-ACT.owl"/>
</owl:Class>

<owl:Class rdf:about="&dul;PhysicalAgent">
  <rdfs:isDefinedBy rdf:resource="http://www.ease-crc.org/ont/SOMA-PROC.owl"/>
</owl:Class>

<owl:ObjectProperty rdf:about="&soma;isOccurringIn"
    rdfs:label="is occurring in">
  <rdfs:comment>A relation between an event and an event type, e.g. 'taking the cup from the table' is an occurence of the motion 'approaching'.</rdfs:comment>
  <rdfs:domain rdf:resource="&dul;EventType"/>
  <rdfs:isDefinedBy rdf:resource="http://www.ease-crc.org/ont/SOMA.owl"/>
  <rdfs:range rdf:resource="&dul;Event"/>
  <rdfs:subPropertyOf rdf:resource="&dul;classifies"/>
</owl:ObjectProperty>

<owl:Class rdf:about="&soma;Finger"
    rdfs:comment="A limb used for grasping objects.">
  <rdfs:subClassOf>
    <owl:Restriction>
      <owl:onProperty rdf:resource="&dul;isPartOf"/>
      <owl:someValuesFrom rdf:resource="&soma;Hand"/>
    </owl:Restriction>
  </rdfs:subClassOf>
  <rdfs:subClassOf rdf:resource="&soma;Limb"/>
  <rdfs:isDefinedBy rdf:resource="http://www.ease-crc.org/ont/SOMA-OBJ.owl"/>
</owl:Class>

<owl:ObjectProperty rdf:about="&soma;isDispositionOf"
    rdfs:comment="Associates a disposition quality to the object holding it."
    rdfs:label="is disposition of">
  <rdfs:domain rdf:resource="&soma;Disposition"/>
  <rdfs:isDefinedBy rdf:resource="http://www.ease-crc.org/ont/SOMA-OBJ.owl"/>
  <rdfs:range rdf:resource="&dul;Object"/>
  <rdfs:subPropertyOf rdf:resource="&dul;isQualityOf"/>
</owl:ObjectProperty>

<owl:Class rdf:about="&soma;PhysicsProcess"
    rdfs:label="Physical process">
  <rdfs:subClassOf>
    <owl:Restriction>
      <owl:onProperty rdf:resource="&dul;hasParticipant"/>
      <owl:someValuesFrom rdf:resource="&dul;PhysicalObject"/>
    </owl:Restriction>
  </rdfs:subClassOf>
  <rdfs:subClassOf rdf:resource="&dul;Process"/>
  <rdfs:comment>A process involving physical objects and phenomena which does not change the chemical constituency of the affected objects.</rdfs:comment>
  <rdfs:isDefinedBy rdf:resource="http://www.ease-crc.org/ont/SOMA-PROC.owl"/>
</owl:Class>

<owl:Class rdf:about="&soma;CommandingTask">
  <rdfs:subClassOf>
    <owl:Restriction>
      <owl:allValuesFrom>
        <owl:Restriction>
          <owl:onProperty rdf:resource="&dul;hasParticipant"/>
          <owl:someValuesFrom rdf:resource="&soma;ImperativeClause"/>
        </owl:Restriction>
      </owl:allValuesFrom>
      <owl:onProperty rdf:resource="&dul;classifies"/>
    </owl:Restriction>
  </rdfs:subClassOf>
  <rdfs:subClassOf rdf:resource="&soma;IllocutionaryTask"/>
  <rdfs:comment xml:lang="en">An Illocutionary act where the Sender emits some Message with the intent to cause the Receiver to perform some action.</rdfs:comment>
  <rdfs:isDefinedBy rdf:resource="http://www.ease-crc.org/ont/SOMA-ACT.owl"/>
  <rdfs:label xml:lang="en">Commanding task</rdfs:label>
</owl:Class>

<owl:Class rdf:about="&soma;Singleton"
    rdfs:comment="A 'Set' that contains exactly one member.">
  <rdfs:isDefinedBy rdf:resource="http://www.ease-crc.org/ont/SOMA-AGENT.owl"/>
  <owl:equivalentClass>
    <owl:Class>
      <owl:intersectionOf rdf:parseType="Collection">
        <rdf:Description rdf:about="&dul;Set"/>
        <owl:Restriction>
          <owl:onClass rdf:resource="&dul;Entity"/>
          <owl:onProperty rdf:resource="&soma;encapsulates"/>
          <owl:qualifiedCardinality rdf:datatype="&xsd;nonNegativeInteger">1</owl:qualifiedCardinality>
        </owl:Restriction>
      </owl:intersectionOf>
    </owl:Class>
  </owl:equivalentClass>
</owl:Class>

<owl:Class rdf:about="&soma;Pushing">
  <rdfs:comment>A task in which an Agent moves an object in a direction loosely from the the contact point between agent and object towards object's center of mass. todo: define subclass 'PushingOver'? Would we expect two distinct contacts with the same surface then?</rdfs:comment>
  <rdfs:isDefinedBy rdf:resource="http://www.ease-crc.org/ont/SOMA-ACT.owl"/>
  <rdfs:subClassOf rdf:resource="&soma;Actuating"/>
  <owl:disjointWith rdf:resource="&soma;Squeezing"/>
</owl:Class>

<owl:ObjectProperty rdf:about="&soma;interactsWith"
    rdfs:comment="A relation between objects that interact with each other."
    rdfs:label="interacts with">
  <rdfs:isDefinedBy rdf:resource="http://www.ease-crc.org/ont/SOMA-PROC.owl"/>
  <rdfs:isDefinedBy rdf:resource="http://www.ease-crc.org/ont/SOMA-SAY.owl"/>
  <rdf:type rdf:resource="&owl;SymmetricProperty"/>
  <rdfs:domain rdf:resource="&dul;PhysicalObject"/>
  <rdfs:range rdf:resource="&dul;PhysicalObject"/>
  <rdfs:subPropertyOf rdf:resource="&dul;associatedWith"/>
</owl:ObjectProperty>

<soma:ExecutionStateRegion rdf:about="&soma;ExecutionState_Succeeded"
    rdfs:comment="The execution state of a succeeded activity.">
  <rdf:type rdf:resource="&owl;NamedIndividual"/>
  <rdfs:isDefinedBy rdf:resource="http://www.ease-crc.org/ont/SOMA-ACT.owl"/>
</soma:ExecutionStateRegion>

<owl:Class rdf:about="&soma;PrecisionGrasp"
    rdfs:label="Precision grasp">
  <rdfs:comment>An Agent grasps an object, and focuses on obtaining precise kinematic control over it. This is useful for then following precise movements, e.g. when writing.</rdfs:comment>
  <rdfs:isDefinedBy rdf:resource="http://www.ease-crc.org/ont/SOMA-PROC.owl"/>
  <rdfs:subClassOf rdf:resource="&soma;GraspingMotion"/>
</owl:Class>

<owl:Class rdf:about="&soma;Capability">
  <rdfs:comment>Capability</rdfs:comment>
  <rdfs:comment>The disposition of an agent to bring about certain effects, and to achieve certain goals.</rdfs:comment>
  <rdfs:comment>The tendency of an object (the bearer) to be able to perform certain tasks together with others (the triggers) and in which the Bearer is the executor of the associated Task and will therefore usually be an Agent.</rdfs:comment>
  <rdfs:isDefinedBy rdf:resource="http://www.ease-crc.org/ont/SOMA-ACT.owl"/>
  <rdfs:isDefinedBy rdf:resource="http://www.ease-crc.org/ont/SOMA-OBJ.owl"/>
  <rdfs:subClassOf>
    <owl:Restriction>
      <owl:onClass>
        <owl:Class>
          <owl:intersectionOf rdf:parseType="Collection">
            <rdf:Description rdf:about="&soma;Affordance"/>
            <owl:Restriction>
              <owl:onClass rdf:resource="&dul;Role"/>
              <owl:onProperty rdf:resource="&soma;definesBearer"/>
              <owl:qualifiedCardinality rdf:datatype="&xsd;nonNegativeInteger">1</owl:qualifiedCardinality>
            </owl:Restriction>

            <owl:Restriction>
              <owl:onClass rdf:resource="&dul;Role"/>
              <owl:onProperty rdf:resource="&soma;definesTrigger"/>
              <owl:qualifiedCardinality rdf:datatype="&xsd;nonNegativeInteger">1</owl:qualifiedCardinality>
            </owl:Restriction>

            <owl:Restriction>
              <owl:onClass rdf:resource="&dul;Task"/>
              <owl:onProperty rdf:resource="&dul;definesTask"/>
              <owl:qualifiedCardinality rdf:datatype="&xsd;nonNegativeInteger">1</owl:qualifiedCardinality>
            </owl:Restriction>
          </owl:intersectionOf>
        </owl:Class>
      </owl:onClass>
      <owl:onProperty rdf:resource="&dul;isDescribedBy"/>
      <owl:qualifiedCardinality rdf:datatype="&xsd;nonNegativeInteger">1</owl:qualifiedCardinality>
    </owl:Restriction>
  </rdfs:subClassOf>
  <rdfs:subClassOf rdf:resource="&soma;Disposition"/>
</owl:Class>

<owl:ObjectProperty rdf:about="&soma;isOutputRoleOf"
    rdfs:comment="A relation between an output roles and its Task.">
  <rdfs:domain rdf:resource="&dul;Role"/>
  <rdfs:isDefinedBy rdf:resource="http://www.ease-crc.org/ont/SOMA.owl"/>
  <rdfs:label xml:lang="en">is output role of</rdfs:label>
  <rdfs:range rdf:resource="&dul;Task"/>
  <rdfs:subPropertyOf rdf:resource="&dul;hasTask"/>
  <owl:inverseOf rdf:resource="&soma;isTaskOfOutputRole"/>
</owl:ObjectProperty>

<owl:ObjectProperty rdf:about="&soma;causes">
  <soma:UsageGuideline xml:lang="en">Simple relationship between two actions to express that the object (the reaction) would not have occured if it were not for the subject (the cause), e.g., a Communication Action classified as an Querying Task causes another Communication Task classified as an Answering Task and the latter would not have occured without the former. An example without Agents involved is some domino stone that would not have toppled without the first one toppling.

When Agents are involved, the relation might be seen as an abstraction of the execution of some plan that arises from changing the agents goal that is due to perceiving the cause. However, currently it is unclear how to model such a pattern and therefore not included in SOMA.

This relation is seen as transitive.</soma:UsageGuideline>
  <rdf:type rdf:resource="&owl;TransitiveProperty"/>
  <rdfs:isDefinedBy rdf:resource="http://www.ease-crc.org/ont/SOMA-ACT.owl"/>
  <rdfs:label xml:lang="en">causes</rdfs:label>
  <rdfs:subPropertyOf rdf:resource="&soma;affects"/>
  <owl:inverseOf rdf:resource="&soma;isReactionTo"/>
</owl:ObjectProperty>

<owl:Class rdf:about="&soma;Transient">
  <rdfs:subClassOf>
    <owl:Restriction>
      <owl:onProperty rdf:resource="&soma;transitionsFrom"/>
      <owl:someValuesFrom rdf:resource="&dul;Object"/>
    </owl:Restriction>
  </rdfs:subClassOf>
  <rdfs:subClassOf rdf:resource="&dul;Object"/>
  <rdfs:comment>Objects may undergo changes during Processes; however, while the change Process is in operation, one cannot strictly say either the input of the Process still exists, nor that the result exists yet.

A prototypical example is making a pancake on a heater. When PancakeMix is put on the hot plate, it ceases to be PancakeMix-- already, the chemical structure of the substance gets altered-- however it is only after sufficient heating that this object becomes a Pancake.

Transients are the objects undergoing such change processes; they are no longer the initial objects fed into the process, nor are they the objects produced as results.

Instead, a Transient transitionsFrom some initial Object that was fed into a change Process. Typically, a Transient may transitionTo some resulting Object (though not always, some processes simply destroy objects).

It is also possible that a Transient transitionsBack to the initial object. An example is the catalyst in a chemical reaction; another example is a loaf of bread after a slice has been cut off.</rdfs:comment>
  <rdfs:isDefinedBy rdf:resource="http://www.ease-crc.org/ont/SOMA-OBJ.owl"/>
</owl:Class>

<owl:Class rdf:about="&soma;Flipping">
  <rdfs:subClassOf>
    <owl:Restriction>
      <owl:onProperty rdf:resource="&soma;isTaskAffordedBy"/>
      <owl:someValuesFrom rdf:resource="&soma;Shifting"/>
    </owl:Restriction>
  </rdfs:subClassOf>
  <rdfs:subClassOf rdf:resource="&soma;Actuating"/>
  <rdfs:comment>The task in which the agent turns an object over by using a tool or by manipulating</rdfs:comment>
  <rdfs:isDefinedBy rdf:resource="http://www.ease-crc.org/ont/SOMA-ACT.owl"/>
</owl:Class>

<soma:ExecutionStateRegion rdf:about="&soma;ExecutionState_Active"
    rdfs:comment="The execution state of an ongoing activity.">
  <rdf:type rdf:resource="&owl;NamedIndividual"/>
  <rdfs:isDefinedBy rdf:resource="http://www.ease-crc.org/ont/SOMA-ACT.owl"/>
</soma:ExecutionStateRegion>

<owl:Axiom>
  <rdfs:comment>If something is a terminal situation then it must be a manifested situation (regardless of whether it was expected or not).</rdfs:comment>
  <owl:annotatedProperty rdf:resource="&rdfs;range"/>
  <owl:annotatedSource rdf:resource="&soma;hasTerminalSituation"/>
  <owl:annotatedTarget>
    <owl:Class rdf:nodeID="bn2">
      <owl:complementOf rdf:resource="http://www.ease-crc.org/ont/SOMA.owl/NonmanifestedSituation"/>
    </owl:Class>
  </owl:annotatedTarget>
</owl:Axiom>

<owl:Class rdf:about="&soma;KnowledgeRepresentationLanguage">
  <rdfs:comment xml:lang="en">A Knowledge Representation Language is a Language with fixed semantics and syntax to describe some knowledge. Examples are JSON and the different OWL Profiles.</rdfs:comment>
  <rdfs:isDefinedBy rdf:resource="http://www.ease-crc.org/ont/SOMA-IO.owl"/>
  <rdfs:label xml:lang="en">Knowledge Representation Language</rdfs:label>
  <rdfs:subClassOf rdf:resource="&soma;Computer_Language"/>
</owl:Class>

<owl:ObjectProperty rdf:about="&soma;encapsulates">
  <rdfs:comment xml:lang="en">The relation between an Ordered element' and an 'Entity' it contains.</rdfs:comment>
  <rdfs:domain rdf:resource="&soma;OrderedElement"/>
  <rdfs:isDefinedBy rdf:resource="http://www.ease-crc.org/ont/SOMA-AGENT.owl"/>
  <rdfs:label xml:lang="en">encapsulates</rdfs:label>
  <rdfs:range rdf:resource="&dul;Entity"/>
  <rdfs:subPropertyOf rdf:resource="&dul;associatedWith"/>
</owl:ObjectProperty>

<owl:Class rdf:about="&soma;CommunicationReport">
  <rdfs:comment>A task in which an Agent endeavors to describe truthfully some state of affairs.</rdfs:comment>
  <rdfs:isDefinedBy rdf:resource="http://www.ease-crc.org/ont/SOMA-ACT.owl"/>
  <rdfs:label xml:lang="en">Communication report</rdfs:label>
  <rdfs:subClassOf rdf:resource="&soma;CommunicationTask"/>
</owl:Class>

<owl:Class rdf:about="&soma;Progression">
  <rdfs:comment>A situation that sattisies a description of how a process evolves over time.</rdfs:comment>
  <rdfs:isDefinedBy rdf:resource="http://www.ease-crc.org/ont/SOMA-PROC.owl"/>
  <rdfs:subClassOf rdf:resource="&dul;Situation"/>
  <owl:equivalentClass>
    <owl:Restriction>
      <owl:onProperty rdf:resource="&dul;satisfies"/>
      <owl:someValuesFrom rdf:resource="&soma;ProcessFlow"/>
    </owl:Restriction>
  </owl:equivalentClass>
</owl:Class>

<owl:Class rdf:about="&dul;FormalEntity"/>

<owl:Class rdf:about="&soma;ColorRegion"
    rdfs:comment="Encodes the color of an object."
    rdfs:label="Color region">
  <rdfs:subClassOf>
    <owl:Restriction>
      <owl:allValuesFrom rdf:resource="&soma;Color"/>
      <owl:onProperty rdf:resource="&dul;isRegionFor"/>
    </owl:Restriction>
  </rdfs:subClassOf>
  <rdfs:subClassOf rdf:resource="&dul;PhysicalAttribute"/>
  <rdfs:isDefinedBy rdf:resource="http://www.ease-crc.org/ont/SOMA-OBJ.owl"/>
</owl:Class>

<owl:Class rdf:about="&soma;Client-Server_Specification">
  <rdfs:subClassOf>
    <owl:Class>
      <owl:intersectionOf rdf:parseType="Collection">

        <owl:Restriction>
          <owl:onProperty rdf:resource="&dul;definesRole"/>
          <owl:someValuesFrom rdf:resource="&soma;ClientRole"/>
        </owl:Restriction>

        <owl:Restriction>
          <owl:onProperty rdf:resource="&dul;definesRole"/>
          <owl:someValuesFrom rdf:resource="&soma;ServerRole"/>
        </owl:Restriction>
      </owl:intersectionOf>
    </owl:Class>
  </rdfs:subClassOf>
  <rdfs:subClassOf rdf:resource="&soma;InterfaceSpecification"/>
  <rdfs:comment xml:lang="en">An API Secification that describes the well known Client-Server pattern:

The Client-server model is a distributed application structure that partitions tasks or workloads between the providers of a resource or service, called servers, and service requesters, called clients Often clients and servers communicate over a computer network on separate hardware, but both client and server may reside in the same system. A server host runs one or more server programs, which share their resources with clients. A client usually does not share any of its resources, but it requests content or service from a server. Clients, therefore, initiate communication sessions with servers, which await incoming requests. Examples of computer applications that use the client-server model are email, network printing, and the World Wide Web.

Source: https://en.wikipedia.org/wiki/Client%E2%80%93server_model</rdfs:comment>
  <rdfs:isDefinedBy rdf:resource="http://www.ease-crc.org/ont/SOMA-IO.owl"/>
  <rdfs:label xml:lang="en">Client-Server Specification</rdfs:label>
</owl:Class>

<owl:Class rdf:about="&soma;PowerGrasp"
    rdfs:label="Power grasp">
  <rdfs:comment>An Agent grasps an object, and focuses on obtaining a strong grasping force upon it, resulting in a grasp able to resist significant outside disturbances. This is useful when using tools with which to later exert force on other things, e.g. when hammering nails.</rdfs:comment>
  <rdfs:isDefinedBy rdf:resource="http://www.ease-crc.org/ont/SOMA-PROC.owl"/>
  <rdfs:subClassOf rdf:resource="&soma;GraspingMotion"/>
  <owl:disjointWith rdf:resource="&soma;PrecisionGrasp"/>
</owl:Class>

<owl:Class rdf:about="&soma;ResourceRole">
  <rdfs:comment>A role classifying objects that are useful or even necessary to sustain the unfolding of an event.

Resources are usually not agentive; a different set of roles classifies the agentive participants in actions. Likewise, typically resources do not play causative or goal roles for the event.

Resources are often consumed by their participation in an event, but this need not always be the case. An instrument and capital are examples of resources that are reusable.</rdfs:comment>
  <rdfs:isDefinedBy rdf:resource="http://www.ease-crc.org/ont/SOMA-OBJ.owl"/>
  <rdfs:label xml:lang="en">Resource role</rdfs:label>
  <rdfs:subClassOf rdf:resource="&soma;EventAdjacentRole"/>
</owl:Class>

<owl:Class rdf:about="&soma;Slicing">
  <rdfs:comment>A particular kind of cutting where the goal is to produce slices from some solid object.</rdfs:comment>
  <rdfs:isDefinedBy rdf:resource="http://www.ease-crc.org/ont/SOMA-ACT.owl"/>
  <rdfs:subClassOf rdf:resource="&soma;Cutting"/>
</owl:Class>

<owl:ObjectProperty rdf:about="&soma;isParameterDefinedIn"
    rdfs:comment="A relation between a description and a parameter."
    rdfs:label="is parameter defined in">
  <rdfs:domain rdf:resource="&dul;Parameter"/>
  <rdfs:isDefinedBy rdf:resource="http://www.ease-crc.org/ont/SOMA-OBJ.owl"/>
  <rdfs:range rdf:resource="&dul;Description"/>
  <rdfs:subPropertyOf rdf:resource="&dul;isDefinedIn"/>
</owl:ObjectProperty>

<owl:ObjectProperty rdf:about="&soma;startedBy"
    soma:symbol="si">
  <rdf:type rdf:resource="&owl;TransitiveProperty"/>
  <rdfs:comment>`A starts B` means that A starts exactly where B starts, and that A strictly ends before B. As in "I start my day with a coffee".</rdfs:comment>
  <rdfs:domain rdf:resource="&dul;Event"/>
  <rdfs:isDefinedBy rdf:resource="http://www.ease-crc.org/ont/SOMA.owl"/>
  <rdfs:label xml:lang="en">started by</rdfs:label>
  <rdfs:range rdf:resource="&dul;Event"/>
  <rdfs:subPropertyOf rdf:resource="&soma;coOccurs"/>
  <owl:inverseOf rdf:resource="&soma;starts"/>
</owl:ObjectProperty>

<owl:Class rdf:about="&soma;Triplestore">
  <rdfs:comment xml:lang="en">A Triplestore or RDF store is a purpose-built database for the storage and retrieval of triples through semantic queries.</rdfs:comment>
  <rdfs:isDefinedBy rdf:resource="http://www.ease-crc.org/ont/SOMA-IO.owl"/>
  <rdfs:label xml:lang="en">Triplestore</rdfs:label>
  <rdfs:subClassOf rdf:resource="&soma;GraphDatabase"/>
</owl:Class>

<owl:Class rdf:about="&soma;Status">
  <rdfs:comment>A role that can be played by some parameter which indicates the state of affairs of some entity, e.g. a flag describing the outcome of an action in terms of success or failure, or an indicator of whether a device is turned on or off.</rdfs:comment>
  <rdfs:isDefinedBy rdf:resource="http://www.ease-crc.org/ont/SOMA.owl"/>
  <rdfs:subClassOf rdf:resource="&dul;Parameter"/>
</owl:Class>

<owl:Class rdf:about="&soma;Knowledge">
  <rdfs:isDefinedBy rdf:resource="http://www.ease-crc.org/ont/SOMA-ACT.owl"/>
  <rdfs:subClassOf rdf:resource="&soma;Item"/>
</owl:Class>

<owl:Class rdf:about="&soma;Clumsiness"
    rdfs:comment="A description of clumsy behavior.">
  <rdfs:isDefinedBy rdf:resource="http://www.ease-crc.org/ont/SOMA.owl"/>
  <rdfs:subClassOf rdf:resource="&soma;Amateurish"/>
</owl:Class>

<owl:ObjectProperty rdf:about="&soma;isShapeOf"
    rdfs:comment="Relates a shape quality to the object the shape belongs to."
    rdfs:label="is shape of">
  <rdfs:domain rdf:resource="&soma;Shape"/>
  <rdfs:isDefinedBy rdf:resource="http://www.ease-crc.org/ont/SOMA-OBJ.owl"/>
  <rdfs:range rdf:resource="&dul;PhysicalObject"/>
  <rdfs:subPropertyOf rdf:resource="&dul;isQualityOf"/>
</owl:ObjectProperty>

<owl:Class rdf:about="&soma;InterrogativeClause"
    rdfs:label="Interrogative clause">
  <rdfs:comment>A clause which makes a request, typically information, of some agent.

Note that in a semantic sense such clauses always request information, but in a pragmatic sense they can be used to convey commands or requests for action, such as e.g. "can you close the door?" The question is not just a request for information about ability, but a request to perform a task.</rdfs:comment>
  <rdfs:isDefinedBy rdf:resource="http://www.ease-crc.org/ont/SOMA-SAY.owl"/>
  <rdfs:subClassOf rdf:resource="&soma;ClausalObject"/>
</owl:Class>

<owl:ObjectProperty rdf:about="&soma;transitionsFrom">
  <rdfs:comment>A property which relates a Transient to an Object it changes from. This is useful to model objects which, through participation in a process, transform themselves so that an ontological reclassification is necessary. An example of this is dough undergoing the Maillard reaction through baking.</rdfs:comment>
  <rdfs:domain rdf:resource="&soma;Transient"/>
  <rdfs:isDefinedBy rdf:resource="http://www.ease-crc.org/ont/SOMA-OBJ.owl"/>
  <rdfs:label xml:lang="en">transitions from</rdfs:label>
  <rdfs:range rdf:resource="&dul;Object"/>
  <rdfs:subPropertyOf rdf:resource="&dul;hasCommonBoundary"/>
</owl:ObjectProperty>

<owl:ObjectProperty rdf:about="&soma;simultaneous"
    soma:symbol="=">
  <rdf:type rdf:resource="&owl;SymmetricProperty"/>
  <rdf:type rdf:resource="&owl;TransitiveProperty"/>
  <rdfs:comment>`A simultaneous B` means that A strictly starts and ends at the same time instant as B, i.e. their temporal extend is equal.</rdfs:comment>
  <rdfs:domain rdf:resource="&dul;Event"/>
  <rdfs:isDefinedBy rdf:resource="http://www.ease-crc.org/ont/SOMA.owl"/>
  <rdfs:range rdf:resource="&dul;Event"/>
  <rdfs:subPropertyOf rdf:resource="&soma;coOccurs"/>
</owl:ObjectProperty>

<owl:AsymmetricProperty rdf:about="&soma;coversObject">
  <rdf:type rdf:resource="&owl;IrreflexiveProperty"/>
  <rdf:type rdf:resource="&owl;ObjectProperty"/>
  <rdfs:comment>A relationship from an object (the coverer) that blocks access to another or its interior (the coveree).</rdfs:comment>
  <rdfs:domain rdf:resource="&dul;PhysicalObject"/>
  <rdfs:isDefinedBy rdf:resource="http://www.ease-crc.org/ont/SOMA-SAY.owl"/>
  <rdfs:range rdf:resource="&dul;PhysicalObject"/>
  <rdfs:subPropertyOf rdf:resource="&soma;interactsWith"/>
  <owl:inverseOf rdf:resource="&soma;isCoveredByObject"/>
</owl:AsymmetricProperty>

<owl:Class rdf:about="&soma;MetaCognitionTopic">
  <rdfs:comment>A topic for a description that an Agent might make of its own cognitive processes and actions.</rdfs:comment>
  <rdfs:isDefinedBy rdf:resource="http://www.ease-crc.org/ont/SOMA-ACT.owl"/>
  <rdfs:subClassOf rdf:resource="&soma;ThinkAloudTopic"/>
</owl:Class>

<owl:Class rdf:about="&soma;QueryAnsweringTask"
    rdfs:label="Query answering task">
  <rdfs:comment xml:lang="en">An Answering task that is the reaction to some Query answering task.

In a lot of cases, such a task is also an Assertion task, e.g., in the following discourse:

"How will the weather be tomorrow?"
"It is going to rain in the morning."

However, sometimes this might be not the case, e.g., with counterquestions.</rdfs:comment>
  <rdfs:isDefinedBy rdf:resource="http://www.ease-crc.org/ont/SOMA-ACT.owl"/>
  <owl:equivalentClass>
    <owl:Class>
      <owl:intersectionOf rdf:parseType="Collection">
        <rdf:Description rdf:about="&soma;AnsweringTask"/>
        <owl:Restriction>
          <owl:allValuesFrom>
            <owl:Restriction>
              <owl:allValuesFrom>
                <owl:Restriction>
                  <owl:onProperty rdf:resource="&dul;isClassifiedBy"/>
                  <owl:someValuesFrom rdf:resource="&soma;QueryingTask"/>
                </owl:Restriction>
              </owl:allValuesFrom>
              <owl:onProperty rdf:resource="&soma;isReactionTo"/>
            </owl:Restriction>
          </owl:allValuesFrom>
          <owl:onProperty rdf:resource="&dul;classifies"/>
        </owl:Restriction>
      </owl:intersectionOf>
    </owl:Class>
  </owl:equivalentClass>
</owl:Class>

<owl:Class rdf:about="&soma;SituationTransition">
  <rdfs:comment>A transition between two situations, usually brought about by the Action of some Agent.</rdfs:comment>
  <rdfs:isDefinedBy rdf:resource="http://www.ease-crc.org/ont/SOMA-ACT.owl"/>
  <rdfs:label xml:lang="en">Situation transition</rdfs:label>
  <rdfs:subClassOf rdf:resource="&dul;Transition"/>
</owl:Class>

<owl:Class rdf:about="&soma;Creation"
    rdfs:label="Creation">
  <rdfs:subClassOf>
    <owl:Restriction>
      <owl:onProperty rdf:resource="&soma;isProcessTypeOf"/>
      <owl:someValuesFrom rdf:resource="&soma;CreatedObject"/>
    </owl:Restriction>
  </rdfs:subClassOf>
  <rdfs:subClassOf rdf:resource="&soma;ProcessType"/>
  <rdfs:comment>A process by which an Entity is created in the physical world.

Note, most of the physical Entities we will be considering here are in fact arrangements of many other, smaller physical Entities. Therefore another way to look at this is, a 'Physical creation' is the process by which a set of physical Entities is arranged in a certain way, and the arrangement is then itself considered a physical Entity.</rdfs:comment>
  <rdfs:isDefinedBy rdf:resource="http://www.ease-crc.org/ont/SOMA-PROC.owl"/>
</owl:Class>

<owl:ObjectProperty rdf:about="&soma;hasInputParameter"
    rdfs:label="has input parameter">
  <rdfs:comment>A relation between a Task and one of its input parameters.</rdfs:comment>
  <rdfs:comment>A relation from an EventType (typically, a Task) and a parameter describing some state of affairs before the event classified by the EventType takes place, and which contributes towards that event happening.</rdfs:comment>
  <rdfs:domain rdf:resource="&dul;EventType"/>
  <rdfs:isDefinedBy rdf:resource="http://www.ease-crc.org/ont/SOMA.owl"/>
  <rdfs:range rdf:resource="&dul;Parameter"/>
  <rdfs:subPropertyOf rdf:resource="&dul;hasParameter"/>
  <owl:inverseOf rdf:resource="&soma;isInputParameterFor"/>
</owl:ObjectProperty>

<owl:Class rdf:about="&soma;ParkingArms">
  <rdfs:comment>A task by which an Agent arranges its arms in such a way so as to minimize opportunities for collision while moving through the environment.</rdfs:comment>
  <rdfs:isDefinedBy rdf:resource="http://www.ease-crc.org/ont/SOMA-ACT.owl"/>
  <rdfs:label xml:lang="en">Parking arms</rdfs:label>
  <rdfs:subClassOf rdf:resource="&soma;AssumingArmPose"/>
</owl:Class>

<owl:Class rdf:about="&soma;Linkage">
  <rdfs:subClassOf>
    <owl:Restriction>
      <owl:allValuesFrom rdf:resource="&soma;LinkedObject"/>
      <owl:onProperty rdf:resource="&soma;affordsBearer"/>
    </owl:Restriction>
  </rdfs:subClassOf>
  <rdfs:subClassOf>
    <owl:Restriction>
      <owl:allValuesFrom rdf:resource="&soma;LinkedObject"/>
      <owl:onProperty rdf:resource="&soma;affordsTrigger"/>
    </owl:Restriction>
  </rdfs:subClassOf>
  <rdfs:subClassOf rdf:resource="&soma;Connectivity"/>
  <rdfs:comment>The disposition of an object (the linked object) to establish a connection with others by being linked together.</rdfs:comment>
  <rdfs:isDefinedBy rdf:resource="http://www.ease-crc.org/ont/SOMA-OBJ.owl"/>
</owl:Class>

<owl:DatatypeProperty rdf:about="&soma;hasFilePath"
    rdfs:label="has file path">
  <rdfs:comment>Associates an entity to some file containing data about it. For example, can be used to describe physical objects via a mesh file.</rdfs:comment>
  <rdfs:domain rdf:resource="&dul;Entity"/>
  <rdfs:isDefinedBy rdf:resource="http://www.ease-crc.org/ont/SOMA-OBJ.owl"/>
  <rdfs:range rdf:resource="&xsd;string"/>
  <rdfs:subPropertyOf rdf:resource="&dul;hasDataValue"/>
</owl:DatatypeProperty>

<owl:Class rdf:about="&soma;PrehensileEffector"
    rdfs:label="Prehensile effector">
  <rdfs:isDefinedBy rdf:resource="http://www.ease-crc.org/ont/SOMA-OBJ.owl"/>
  <rdfs:isDefinedBy rdf:resource="http://www.ease-crc.org/ont/SOMA-PROC.owl"/>
  <rdfs:comment>An effector used to grasp objects, such as a hand of a human, or the long prehensile tail of a monkey.</rdfs:comment>
  <rdfs:subClassOf rdf:resource="&soma;PhysicalEffector"/>
</owl:Class>

<owl:Class rdf:about="&soma;Executable_Code">
  <rdfs:comment xml:lang="en">Executable Code is Code that when compiled / interpreted, has some clear entrance point and can be executed. Note the difference to an Executable File, which is the file that contains such (compiled) code.</rdfs:comment>
  <rdfs:isDefinedBy rdf:resource="http://www.ease-crc.org/ont/SOMA-IO.owl"/>
  <rdfs:label xml:lang="en">Executable Code</rdfs:label>
  <rdfs:subClassOf rdf:resource="&soma;Computer_Program"/>
  <owl:equivalentClass>
    <owl:Class>
      <owl:intersectionOf rdf:parseType="Collection">
        <rdf:Description rdf:about="&soma;Computer_Program"/>
        <owl:Restriction>
          <owl:onProperty rdf:resource="&soma;isGivenMeaningBy"/>
          <owl:someValuesFrom rdf:resource="&soma;ExecutableFormat"/>
        </owl:Restriction>
      </owl:intersectionOf>
    </owl:Class>
  </owl:equivalentClass>
</owl:Class>

<owl:Class rdf:about="&soma;Manipulating">
  <rdfs:subClassOf>
    <owl:Restriction>
      <owl:allValuesFrom rdf:resource="&soma;PhysicalAction"/>
      <owl:onProperty rdf:resource="&dul;classifies"/>
    </owl:Restriction>
  </rdfs:subClassOf>
  <rdfs:subClassOf rdf:resource="&soma;PhysicalTask"/>
  <rdfs:comment>Tasks where the goal is to move the prehensile effectors, ie. hands, of an agent so as to achieve some spatial or functional relation with some manipulated object. 

Spatial relations refer to positioning the hands in certain ways relative to the manipulated object, for example nearing or distancing them, or aligning them with some relevant axis.

Functional relations here refer to interactions between the hands and manipulated object which constrain the possible behavior of the object. Examples of functional relations in manipulation are support and kinematic control.

Note that manipulation tasks are usually performed with the intention of moving an object in some way, so there is a large conceptual overlap between Manipulating and Actuating.

However these concepts are nonetheless distinguished in what they "profile", ie. what they focus on as particularly important.

Actuating profiles the movement of the object itself.

Manipulating profiles the movement of the hands and the functional relations, such as kinematic control, they establish with the manipulated object.

Note: we employ Manipulating here in its literal, original sense, of using hands for some purpose, and not in the metaphorical sense of exerting psychological pressure on someone.</rdfs:comment>
  <rdfs:isDefinedBy rdf:resource="http://www.ease-crc.org/ont/SOMA-ACT.owl"/>
</owl:Class>

<owl:Class rdf:about="&soma;Extrinsic">
  <rdfs:comment>A physical quality that depends on relationships to other objects, such as the color of an object which depends on light conditions in the environment.</rdfs:comment>
  <rdfs:isDefinedBy rdf:resource="http://www.ease-crc.org/ont/SOMA-OBJ.owl"/>
  <rdfs:subClassOf rdf:resource="&soma;PhysicalQuality"/>
  <owl:disjointWith rdf:resource="&soma;Intrinsic"/>
</owl:Class>

<owl:Ontology rdf:about="http://www.ease-crc.org/ont/SOMA.owl"
    owl:versionInfo="2.1.0">
  <owl:imports rdf:resource="http://www.ease-crc.org/ont/DUL.owl"/>
</owl:Ontology>

<owl:ObjectProperty rdf:about="&dul;follows"/>

<owl:Class rdf:about="&soma;HeadMovement">
  <rdfs:comment>The Agent moves a part of their body carrying high-bandwidth sensors such as cameras. The movement of other body parts is not significant.</rdfs:comment>
  <rdfs:comment>todo: (Mihai:) This seems too specific, given the "Directed"/"Undirected motion" categories.</rdfs:comment>
  <rdfs:isDefinedBy rdf:resource="http://www.ease-crc.org/ont/SOMA-PROC.owl"/>
  <rdfs:subClassOf rdf:resource="&soma;BodyMovement"/>
</owl:Class>

<owl:Class rdf:about="&soma;PlacingTheory">
  <rdfs:subClassOf>
    <owl:Restriction>
      <owl:onProperty rdf:resource="&dul;defines"/>
      <owl:someValuesFrom rdf:resource="&soma;Destination"/>
    </owl:Restriction>
  </rdfs:subClassOf>
  <rdfs:subClassOf>
    <owl:Restriction>
      <owl:onProperty rdf:resource="&dul;defines"/>
      <owl:someValuesFrom rdf:resource="&soma;Patient"/>
    </owl:Restriction>
  </rdfs:subClassOf>
  <rdfs:subClassOf rdf:resource="&soma;ExecutableSchematicTheory"/>
  <rdfs:comment>A schematic theory of how an agent can place a patient at a particular goal location.</rdfs:comment>
  <rdfs:isDefinedBy rdf:resource="http://www.ease-crc.org/ont/SOMA-SAY.owl"/>
  <rdfs:label xml:lang="en">Placing theory</rdfs:label>
</owl:Class>

<owl:ObjectProperty rdf:about="&soma;isNetForceOf"
    rdfs:label="is net force of">
  <rdfs:comment>A relation between a physical object and the total force acting on it.</rdfs:comment>
  <rdfs:domain rdf:resource="&soma;NetForce"/>
  <rdfs:isDefinedBy rdf:resource="http://www.ease-crc.org/ont/SOMA-OBJ.owl"/>
  <rdfs:range rdf:resource="&dul;PhysicalObject"/>
  <rdfs:subPropertyOf rdf:resource="&dul;isRegionFor"/>
</owl:ObjectProperty>

<owl:Class rdf:about="&soma;Threshold">
  <rdfs:comment>A role played by a parameter which indicates some value that, when crossed, triggers some condition.</rdfs:comment>
  <rdfs:isDefinedBy rdf:resource="http://www.ease-crc.org/ont/SOMA.owl"/>
  <rdfs:subClassOf rdf:resource="&dul;Parameter"/>
</owl:Class>

<owl:Class rdf:about="&soma;RecordedEpisode"
    rdfs:comment="An episode which has been recorded.">
  <rdfs:subClassOf>
    <owl:Restriction>
      <owl:onProperty rdf:resource="&soma;includesRecord"/>
      <owl:someValuesFrom rdf:resource="&dul;InformationObject"/>
    </owl:Restriction>
  </rdfs:subClassOf>
  <rdfs:subClassOf rdf:resource="&soma;Episode"/>
  <rdfs:isDefinedBy rdf:resource="http://www.ease-crc.org/ont/SOMA.owl"/>
</owl:Class>

<owl:Class rdf:about="&soma;Deformation">
  <rdfs:subClassOf>
    <owl:Restriction>
      <owl:onClass rdf:resource="&soma;ShapedObject"/>
      <owl:onProperty rdf:resource="&soma;isProcessTypeOf"/>
      <owl:qualifiedCardinality rdf:datatype="&xsd;nonNegativeInteger">1</owl:qualifiedCardinality>
    </owl:Restriction>
  </rdfs:subClassOf>
  <rdfs:subClassOf rdf:resource="&soma;Alteration"/>
  <rdfs:comment>A process by which a physical Entity changes its shape under the influence of some factors outside of the Entity.

Note, changes of shape may be self-caused; for example, a gas will naturally disperse. This however would be a different type of process (Dispersion).

A soft slab of clay deforming under its own weight on Earth would still count as deformation: it is the gravity of the Earth (so, a factor outside the slab of clay) which makes the slab change shape.</rdfs:comment>
  <rdfs:isDefinedBy rdf:resource="http://www.ease-crc.org/ont/SOMA-PROC.owl"/>
  <owl:disjointWith rdf:resource="&soma;FluidFlow"/>
</owl:Class>

<owl:Class rdf:about="&soma;CircularCylinder"
    rdfs:comment="A cylinder figure with circular cross section."
    rdfs:label="Circular cylinder">
  <rdfs:subClassOf>
    <owl:Restriction>
      <owl:onDataRange rdf:resource="&xsd;float"/>
      <owl:onProperty rdf:resource="&soma;hasRadius"/>
      <owl:qualifiedCardinality rdf:datatype="&xsd;nonNegativeInteger">1</owl:qualifiedCardinality>
    </owl:Restriction>
  </rdfs:subClassOf>
  <rdfs:subClassOf rdf:resource="&soma;CylinderShape"/>
  <rdfs:isDefinedBy rdf:resource="http://www.ease-crc.org/ont/SOMA-OBJ.owl"/>
</owl:Class>

<owl:Class rdf:about="&soma;GreenColor"
    rdfs:comment="A color region with dominant green color."
    rdfs:label="Green color">
  <rdfs:isDefinedBy rdf:resource="http://www.ease-crc.org/ont/SOMA-OBJ.owl"/>
  <rdfs:subClassOf rdf:resource="&soma;ColorRegion"/>
</owl:Class>

<owl:Class rdf:about="&soma;UndirectedMotion"
    rdfs:label="Undirected motion">
  <rdfs:comment>A Motion of a physical Entity for which a destination or path are unknown and/or considered irrelevant; the important aspect about this Motion is simply that it occurs, rather than where it is headed or how it proceeds towards it.</rdfs:comment>
  <rdfs:isDefinedBy rdf:resource="http://www.ease-crc.org/ont/SOMA-PROC.owl"/>
  <rdfs:subClassOf rdf:resource="&soma;Motion"/>
</owl:Class>

<owl:Class rdf:about="&dul;DesignedArtifact"/>

<owl:Class rdf:about="&soma;PathRole"
    rdfs:comment="A role that classifies the path of a motion.">
  <rdfs:isDefinedBy rdf:resource="http://www.ease-crc.org/ont/SOMA-OBJ.owl"/>
  <rdfs:label xml:lang="en">Path role</rdfs:label>
  <rdfs:subClassOf rdf:resource="&soma;SpatioTemporalRole"/>
</owl:Class>

<owl:Class rdf:about="&soma;Alteration">
  <rdfs:comment>A process by which an aspect of some object changes such as ice cream melting in the sun.</rdfs:comment>
  <rdfs:isDefinedBy rdf:resource="http://www.ease-crc.org/ont/SOMA-PROC.owl"/>
  <rdfs:subClassOf rdf:resource="&soma;ProcessType"/>
</owl:Class>

<owl:Class rdf:about="&soma;Boiling">
  <rdfs:comment>In each instance of this collection some liquid matter is raised to its boilingPoint and is thereby changed from being in the Liquid-StateOfMatter to being in the Gaseous-StateOfMatter.</rdfs:comment>
  <rdfs:isDefinedBy rdf:resource="http://www.ease-crc.org/ont/SOMA-PROC.owl"/>
  <rdfs:subClassOf rdf:resource="&soma;Vaporizing"/>
</owl:Class>

<owl:ObjectProperty rdf:about="&soma;isPerformerDefinedIn">
  <rdfs:comment xml:lang="en">Relates an affordance which is a relation between a bearer and a trigger, to the role of the performer when the affordance is manifested.</rdfs:comment>
  <rdfs:domain rdf:resource="&dul;Role"/>
  <rdfs:isDefinedBy rdf:resource="http://www.ease-crc.org/ont/SOMA-OBJ.owl"/>
  <rdfs:label xml:lang="en">is performer defined in</rdfs:label>
  <rdfs:range rdf:resource="&dul;Description"/>
  <rdfs:subPropertyOf rdf:resource="&dul;isRoleDefinedIn"/>
</owl:ObjectProperty>

<owl:ObjectProperty rdf:about="&dul;realizes"/>

<owl:Class rdf:about="&soma;FunctionalControl">
  <rdfs:subClassOf>
    <owl:Restriction>
      <owl:onProperty rdf:resource="&soma;isStateTypeOf"/>
      <owl:someValuesFrom rdf:resource="&soma;Item"/>
    </owl:Restriction>
  </rdfs:subClassOf>
  <rdfs:subClassOf>
    <owl:Restriction>
      <owl:onProperty rdf:resource="&soma;isStateTypeOf"/>
      <owl:someValuesFrom rdf:resource="&soma;Restrictor"/>
    </owl:Restriction>
  </rdfs:subClassOf>
  <rdfs:subClassOf rdf:resource="&soma;StateType"/>
  <rdfs:comment>Classifies States in which an object restricts the movement of another, at least partially. Usually neither object is construed to be an agent.

Note that this State focuses on how the interaction of, usually non-agentive, objects restricts their motion. This is in contrast to Blockage/Accessibility states where the placement of some objects influences the access to some of them by a third, usually agentive party.</rdfs:comment>
  <rdfs:isDefinedBy rdf:resource="http://www.ease-crc.org/ont/SOMA-STATE.owl"/>
  <rdfs:label xml:lang="en">Functional state</rdfs:label>
</owl:Class>

<owl:ObjectProperty rdf:about="&soma;hasNextStep"
    rdfs:label="has next step">
  <rdfs:comment>An ordering relation between tasks in a workflow, saying that a task is followed by another.</rdfs:comment>
  <rdfs:domain rdf:resource="&dul;Task"/>
  <rdfs:isDefinedBy rdf:resource="http://www.ease-crc.org/ont/SOMA-WF.owl"/>
  <rdfs:range rdf:resource="&dul;Task"/>
  <rdfs:subPropertyOf rdf:resource="&dul;directlyPrecedes"/>
  <owl:inverseOf rdf:resource="&soma;hasPreviousStep"/>
</owl:ObjectProperty>

<owl:ObjectProperty rdf:about="&soma;includesConcept"
    rdfs:label="includes concept">
  <rdfs:comment>A relation recording that a Situation has a Concept as participant in some sort of role.</rdfs:comment>
  <rdfs:domain rdf:resource="&dul;Situation"/>
  <rdfs:isDefinedBy rdf:resource="http://www.ease-crc.org/ont/SOMA.owl"/>
  <rdfs:range rdf:resource="&dul;Concept"/>
  <rdfs:subPropertyOf rdf:resource="&dul;includesObject"/>
  <owl:inverseOf rdf:resource="&soma;isConceptIncludedIn"/>
</owl:ObjectProperty>

<owl:Class rdf:about="&soma;CheckingObjectPresence">
  <rdfs:comment>A task by which an Agent uses its sensors to check for the presence of a specific object and to obtain some other information about it, e.g. pose.</rdfs:comment>
  <rdfs:isDefinedBy rdf:resource="http://www.ease-crc.org/ont/SOMA-ACT.owl"/>
  <rdfs:label xml:lang="en">Checking object presence</rdfs:label>
  <rdfs:subClassOf rdf:resource="&soma;Perceiving"/>
</owl:Class>

<owl:ObjectProperty rdf:about="&soma;isSetpointDefinedIn"
    rdfs:comment="Defines the dedicated goal region of a description."
    rdfs:label="is setpoint defined in">
  <rdfs:domain rdf:resource="&soma;Setpoint"/>
  <rdfs:isDefinedBy rdf:resource="http://www.ease-crc.org/ont/SOMA-OBJ.owl"/>
  <rdfs:range rdf:resource="&dul;Description"/>
  <rdfs:subPropertyOf rdf:resource="&soma;isParameterDefinedIn"/>
</owl:ObjectProperty>

<owl:ObjectProperty rdf:about="&soma;isTaskOfInputRole"
    rdfs:comment="A relation between a Task and one of its input roles.">
  <rdfs:domain rdf:resource="&dul;Task"/>
  <rdfs:isDefinedBy rdf:resource="http://www.ease-crc.org/ont/SOMA.owl"/>
  <rdfs:label xml:lang="en">is task of input role</rdfs:label>
  <rdfs:range rdf:resource="&dul;Role"/>
  <rdfs:subPropertyOf rdf:resource="&dul;isTaskOf"/>
</owl:ObjectProperty>

<owl:Axiom>
  <rdfs:comment>If a transition has an initial situation then it also has a manifestation.</rdfs:comment>
  <owl:annotatedProperty rdf:resource="&rdfs;subClassOf"/>
  <owl:annotatedSource>
    <owl:Restriction>
      <rdfs:subClassOf>
        <owl:Restriction rdf:nodeID="bn3">
          <owl:onProperty rdf:resource="http://www.ease-crc.org/ont/SOMA.owl/manifestsIn"/>
          <owl:someValuesFrom rdf:resource="&dul;Event"/>
        </owl:Restriction>
      </rdfs:subClassOf>
      <owl:onProperty rdf:resource="&soma;hasInitialSituation"/>
      <owl:someValuesFrom rdf:resource="&dul;Situation"/>
    </owl:Restriction>
  </owl:annotatedSource>
  <owl:annotatedTarget rdf:nodeID="bn3"/>
</owl:Axiom>

<owl:DatatypeProperty rdf:about="&soma;isReificationOf"
    rdfs:label="is reification of">
  <rdfs:comment>An auxiliary property that is used to generate object individuals, called reifications, from any other Entity, e.g. from relations, classes, data types. These reifications can then be used in DL axioms as any other named individual.</rdfs:comment>
  <rdfs:domain rdf:resource="&dul;Description"/>
  <rdfs:isDefinedBy rdf:resource="http://www.ease-crc.org/ont/SOMA.owl"/>
  <rdfs:range rdf:resource="&xsd;anyURI"/>
  <rdfs:subPropertyOf rdf:resource="&dul;hasDataValue"/>
</owl:DatatypeProperty>

<owl:Class rdf:about="&soma;Reification"
    rdfs:comment="A description that *describes* a formal entity.">
  <rdfs:subClassOf>
    <owl:Restriction>
      <owl:onDataRange rdf:resource="&xsd;anyURI"/>
      <owl:onProperty rdf:resource="&soma;isReificationOf"/>
      <owl:qualifiedCardinality rdf:datatype="&xsd;nonNegativeInteger">1</owl:qualifiedCardinality>
    </owl:Restriction>
  </rdfs:subClassOf>
  <rdfs:subClassOf rdf:resource="&dul;Description"/>
  <rdfs:isDefinedBy rdf:resource="http://www.ease-crc.org/ont/SOMA.owl"/>
</owl:Class>

<owl:ObjectProperty rdf:about="&dul;precedes"/>

<owl:Class rdf:about="&soma;Introspecting">
  <rdfs:comment xml:lang="en">A mentalk task in which an Agent gathers and processes information about its own mental tasks via, e.g., Meta Reasoning.</rdfs:comment>
  <rdfs:isDefinedBy rdf:resource="http://www.ease-crc.org/ont/SOMA-ACT.owl"/>
  <rdfs:label xml:lang="en">Introspecting</rdfs:label>
  <rdfs:subClassOf rdf:resource="&soma;InformationAcquisition"/>
</owl:Class>

<owl:ObjectProperty rdf:about="&dul;hasPart">
  <rdfs:isDefinedBy rdf:resource="http://www.ease-crc.org/ont/SOMA-PROC.owl"/>
  <rdfs:isDefinedBy rdf:resource="http://www.ease-crc.org/ont/SOMA-STATE.owl"/>
  <rdfs:isDefinedBy rdf:resource="http://www.ease-crc.org/ont/SOMA-WF.owl"/>
  <rdfs:isDefinedBy rdf:resource="http://www.ease-crc.org/ont/SOMA.owl"/>
</owl:ObjectProperty>

<owl:Class rdf:about="&soma;BeneficiaryRole">
  <rdfs:comment>A role classifying an agent for whose benefit an action is performed.</rdfs:comment>
  <rdfs:isDefinedBy rdf:resource="http://www.ease-crc.org/ont/SOMA-OBJ.owl"/>
  <rdfs:label xml:lang="en">Beneficiary role</rdfs:label>
  <rdfs:subClassOf rdf:resource="&soma;GoalRole"/>
</owl:Class>

<owl:Class rdf:about="&dul;SocialObjectAttribute"/>

<owl:Class rdf:about="&soma;MetaCognitionPlanningTopic"
    rdfs:label="Meta cognition planning topic">
  <rdfs:comment>A topic used while an Agent describes the planning it does for its own cognitive processes and actions.</rdfs:comment>
  <rdfs:isDefinedBy rdf:resource="http://www.ease-crc.org/ont/SOMA-ACT.owl"/>
  <rdfs:subClassOf rdf:resource="&soma;MetaCognitionTopic"/>
</owl:Class>

<owl:ObjectProperty rdf:about="&dul;hasConstituent">
  <rdfs:isDefinedBy rdf:resource="http://www.ease-crc.org/ont/SOMA.owl"/>
</owl:ObjectProperty>

<owl:Class rdf:about="&soma;MetaCognitionEvaluationTopic"
    rdfs:label="Meta cognition evaluation topic">
  <rdfs:comment>A topic used while an Agent describes its own cognitive processes and acions to evaluate them according to some metric.</rdfs:comment>
  <rdfs:isDefinedBy rdf:resource="http://www.ease-crc.org/ont/SOMA-ACT.owl"/>
  <rdfs:subClassOf rdf:resource="&soma;MetaCognitionTopic"/>
</owl:Class>

<owl:Class rdf:about="&soma;ShapeRegion"
    rdfs:label="Shape region">
  <rdfs:subClassOf>
    <owl:Restriction>
      <owl:maxQualifiedCardinality rdf:datatype="&xsd;nonNegativeInteger">1</owl:maxQualifiedCardinality>
      <owl:onClass rdf:resource="http://www.ease-crc.org/ont/SOMA.owl#6DPose"/>
      <owl:onProperty rdf:resource="&soma;hasSpaceRegion"/>
    </owl:Restriction>
  </rdfs:subClassOf>
  <rdfs:subClassOf rdf:resource="&dul;Region"/>
  <rdfs:comment>Encodes the shape of an object.

Note that sometimes the shape as actually used for some purpose may be displaced. This is the case, e.g., for robot links which use a mesh file to describe their shape, but the reference pose of the link uses the mesh translated/rotated in the link's local coordinate frame.</rdfs:comment>
  <rdfs:isDefinedBy rdf:resource="http://www.ease-crc.org/ont/SOMA-OBJ.owl"/>
</owl:Class>

<owl:ObjectProperty rdf:about="&dul;describes">
  <rdfs:isDefinedBy rdf:resource="http://www.ease-crc.org/ont/SOMA-STATE.owl"/>
  <rdfs:isDefinedBy rdf:resource="http://www.ease-crc.org/ont/SOMA-WF.owl"/>
</owl:ObjectProperty>

<owl:Class rdf:about="&soma;UnavailableSoftware">
  <rdfs:comment>A description of a situation where some software dependency is not available.</rdfs:comment>
  <rdfs:isDefinedBy rdf:resource="http://www.ease-crc.org/ont/SOMA-IO.owl"/>
  <rdfs:label xml:lang="en">Unavailable software</rdfs:label>
  <rdfs:subClassOf rdf:resource="&soma;SoftwareDiagnosis"/>
</owl:Class>

<owl:ObjectProperty rdf:about="http://www.ease-crc.org/ont/SOMA.owl/hasRequiredInitialSituation">
  <rdfs:subPropertyOf rdf:resource="&soma;hasInitialSituation"/>
  <rdfs:subPropertyOf rdf:resource="&dul;hasPrecondition"/>
  <rdfs:comment>A relationship between a Situation x and another Situation y that precedes it, such that without y manifesting, it would be impossible for x to manifest.</rdfs:comment>
  <rdfs:domain rdf:resource="&soma;SituationTransition"/>
  <rdfs:isDefinedBy rdf:resource="http://www.ease-crc.org/ont/SOMA-ACT.owl"/>
  <rdfs:label xml:lang="en">has required initial situation</rdfs:label>
  <rdfs:range rdf:resource="&dul;Situation"/>
</owl:ObjectProperty>

<owl:Class rdf:about="&soma;TechnicalDiagnosis"
    rdfs:comment="A functional diagnosis of a technical system."
    rdfs:label="Technical diagnosis">
  <rdfs:subClassOf>
    <owl:Restriction>
      <owl:onProperty rdf:resource="&dul;hasConstituent"/>
      <owl:someValuesFrom rdf:resource="&dul;DesignedArtifact"/>
    </owl:Restriction>
  </rdfs:subClassOf>
  <rdfs:subClassOf rdf:resource="&soma;FunctionalDiagnosis"/>
  <rdfs:isDefinedBy rdf:resource="http://www.ease-crc.org/ont/SOMA.owl"/>
</owl:Class>

<rdf:Description rdf:about="&dul;realizesSelfInformation">
  <rdfs:label xml:lang="en">realizes self information</rdfs:label>
</rdf:Description>

<owl:AsymmetricProperty rdf:about="&soma;overlappedOn"
    soma:symbol="o"
    rdfs:label="overlapped on">
  <rdf:type rdf:resource="&owl;IrreflexiveProperty"/>
  <rdf:type rdf:resource="&owl;ObjectProperty"/>
  <rdfs:comment>A schematic relation between any entities that also implies ordering, e.g. "she has worked into the night".</rdfs:comment>
  <rdfs:domain rdf:resource="&dul;Entity"/>
  <rdfs:isDefinedBy rdf:resource="http://www.ease-crc.org/ont/SOMA.owl"/>
  <rdfs:range rdf:resource="&dul;Entity"/>
  <rdfs:subPropertyOf rdf:resource="&dul;overlaps"/>
</owl:AsymmetricProperty>

<owl:ObjectProperty rdf:about="&soma;hasJointState"
    rdfs:comment="Relates a joint to its state."
    rdfs:label="has joint state">
  <rdfs:domain rdf:resource="&soma;Joint"/>
  <rdfs:isDefinedBy rdf:resource="http://www.ease-crc.org/ont/SOMA-OBJ.owl"/>
  <rdfs:range rdf:resource="&soma;JointState"/>
  <rdfs:subPropertyOf rdf:resource="&dul;hasRegion"/>
  <owl:inverseOf rdf:resource="&soma;isJointStateOf"/>
</owl:ObjectProperty>

<rdfs:Datatype rdf:about="&soma;array_float">
  <rdfs:isDefinedBy rdf:resource="http://www.ease-crc.org/ont/SOMA.owl"/>
  <owl:equivalentClass rdf:resource="&xsd;string"/>
</rdfs:Datatype>

<owl:Class rdf:about="&soma;AttentionShift">
  <rdfs:comment xml:lang="en">A mental task in which the executing Agent shifts his attention from some Information to another.</rdfs:comment>
  <rdfs:isDefinedBy rdf:resource="http://www.ease-crc.org/ont/SOMA-ACT.owl"/>
  <rdfs:label xml:lang="en">Attention shifting</rdfs:label>
  <rdfs:subClassOf rdf:resource="&soma;MentalTask"/>
</owl:Class>

<owl:Class rdf:about="&soma;HardwareDiagnosis"
    rdfs:comment="A diagnosis of the hardware of a system."
    rdfs:label="Hardware diagnosis">
  <rdfs:isDefinedBy rdf:resource="http://www.ease-crc.org/ont/SOMA.owl"/>
  <rdfs:subClassOf rdf:resource="&soma;TechnicalDiagnosis"/>
</owl:Class>

<owl:Class rdf:about="&soma;SoftwareLibrary">
  <rdfs:isDefinedBy rdf:resource="http://www.ease-crc.org/ont/SOMA-IO.owl"/>
  <rdfs:label xml:lang="en">Software Library</rdfs:label>
  <rdfs:subClassOf rdf:resource="&soma;Software"/>
</owl:Class>

<owl:Class rdf:about="&soma;TaskInvocation">
  <rdfs:subClassOf>
    <owl:Restriction>
      <owl:allValuesFrom rdf:resource="&soma;FactualBinding"/>
      <owl:onProperty rdf:resource="&soma;hasBinding"/>
    </owl:Restriction>
  </rdfs:subClassOf>
  <rdfs:subClassOf>
    <owl:Restriction>
      <owl:onClass rdf:resource="&dul;Task"/>
      <owl:onProperty rdf:resource="&dul;definesTask"/>
      <owl:qualifiedCardinality rdf:datatype="&xsd;nonNegativeInteger">1</owl:qualifiedCardinality>
    </owl:Restriction>
  </rdfs:subClassOf>
  <rdfs:subClassOf rdf:resource="&dul;Workflow"/>
  <rdfs:comment>An elementary workflow consisting in the invocation of one single task. It is used as a descriptive context inside of which factual bindings are valid between the task's arguments and other entities (such as the "local variables" of a larger workflow).</rdfs:comment>
  <rdfs:isDefinedBy rdf:resource="http://www.ease-crc.org/ont/SOMA-WF.owl"/>
  <rdfs:label xml:lang="en">Task invocation</rdfs:label>
</owl:Class>

<owl:Class rdf:about="&soma;Size">
  <rdfs:comment>The magnitude or dimension of a thing which can be measured as length, width, height, diameter, perimeter, area, volume.</rdfs:comment>
  <rdfs:isDefinedBy rdf:resource="http://www.ease-crc.org/ont/SOMA-OBJ.owl"/>
  <rdfs:subClassOf rdf:resource="&soma;Intrinsic"/>
</owl:Class>

<owl:Class rdf:about="&soma;Tempering">
  <rdfs:subClassOf>
    <owl:Restriction>
      <owl:allValuesFrom>
        <owl:Restriction>
          <owl:allValuesFrom rdf:resource="&soma;Temperature"/>
          <owl:onProperty rdf:resource="&dul;classifies"/>
        </owl:Restriction>
      </owl:allValuesFrom>
      <owl:onProperty rdf:resource="&soma;affordsSetpoint"/>
    </owl:Restriction>
  </rdfs:subClassOf>
  <rdfs:subClassOf rdf:resource="&soma;Variability"/>
  <rdfs:comment>The disposition of an object (the tool) to change the temperature of others.</rdfs:comment>
  <rdfs:isDefinedBy rdf:resource="http://www.ease-crc.org/ont/SOMA-OBJ.owl"/>
</owl:Class>

<owl:ObjectProperty rdf:about="&soma;isPreferenceOf">
  <rdfs:comment xml:lang="en">Relates a preference quality to the agent the preference belongs to.</rdfs:comment>
  <rdfs:domain rdf:resource="&soma;Preference"/>
  <rdfs:isDefinedBy rdf:resource="http://www.ease-crc.org/ont/SOMA-AGENT.owl"/>
  <rdfs:label xml:lang="en">is preference of</rdfs:label>
  <rdfs:range rdf:resource="&dul;Agent"/>
  <rdfs:subPropertyOf rdf:resource="&dul;isQualityOf"/>
</owl:ObjectProperty>

<owl:ObjectProperty rdf:about="&soma;hasChildLink"
    rdfs:label="has child link">
  <rdfs:comment>Relates a joint to the link it connects which is closer to the end of the kinematic chain.</rdfs:comment>
  <rdfs:domain rdf:resource="&soma;Joint"/>
  <rdfs:isDefinedBy rdf:resource="http://www.ease-crc.org/ont/SOMA-OBJ.owl"/>
  <rdfs:range rdf:resource="&dul;PhysicalObject"/>
  <rdfs:subPropertyOf rdf:resource="&dul;hasConstituent"/>
  <owl:inverseOf rdf:resource="&soma;isChildLinkOf"/>
</owl:ObjectProperty>

<owl:Class rdf:about="&soma;Holding">
  <rdfs:comment>A task by which an Agent keeps an object over which it has kinematic control, typically via grasping, at some specified pose.</rdfs:comment>
  <rdfs:isDefinedBy rdf:resource="http://www.ease-crc.org/ont/SOMA-ACT.owl"/>
  <rdfs:subClassOf rdf:resource="&soma;Manipulating"/>
</owl:Class>

<owl:ObjectProperty rdf:about="&dul;isPartOf">
  <rdfs:isDefinedBy rdf:resource="http://www.ease-crc.org/ont/SOMA-PROC.owl"/>
</owl:ObjectProperty>

<owl:ObjectProperty rdf:about="&soma;affects"
    rdfs:label="affects">
  <rdfs:comment>Simple relationship between two actions to express that a variation in the course or outcome of the subject (the affector) would have resulted in a variation in the object (the affectee), e.g., a planning task that sets parameters such as goal position affects the subsequently executed pick-and-place task that uses that parameter.</rdfs:comment>
  <rdfs:isDefinedBy rdf:resource="http://www.ease-crc.org/ont/SOMA-ACT.owl"/>
  <rdfs:subPropertyOf rdf:resource="&dul;precedes"/>
  <owl:inverseOf rdf:resource="&soma;isAffectedBy"/>
</owl:ObjectProperty>

<owl:Class rdf:about="&dul;Configuration"/>

<owl:Class rdf:about="&soma;Unsuccessfulness">
  <rdfs:comment>A description of a situation with a goal that was not or not fully achieved by some system.</rdfs:comment>
  <rdfs:isDefinedBy rdf:resource="http://www.ease-crc.org/ont/SOMA.owl"/>
  <rdfs:subClassOf rdf:resource="&soma;SuccessDiagnosis"/>
</owl:Class>

<owl:ObjectProperty rdf:about="&soma;hasNetForce"
    rdfs:label="has net force">
  <rdfs:comment>A relation between a physical object and the total force acting on it.</rdfs:comment>
  <rdfs:domain rdf:resource="&dul;PhysicalObject"/>
  <rdfs:isDefinedBy rdf:resource="http://www.ease-crc.org/ont/SOMA-OBJ.owl"/>
  <rdfs:range rdf:resource="&soma;NetForce"/>
  <rdfs:subPropertyOf rdf:resource="&dul;hasRegion"/>
  <owl:inverseOf rdf:resource="&soma;isNetForceOf"/>
</owl:ObjectProperty>

<owl:Class rdf:about="&soma;Serving">
  <rdfs:subClassOf>
    <owl:Restriction>
      <owl:allValuesFrom>
        <owl:Class>
          <owl:intersectionOf rdf:parseType="Collection">
            <rdf:Description rdf:about="&dul;Action"/>
            <owl:Class>
              <owl:unionOf rdf:parseType="Collection">

                <owl:Restriction>
                  <owl:onProperty rdf:resource="&dul;hasParticipant"/>
                  <owl:someValuesFrom rdf:resource="&dul;PhysicalAgent"/>
                </owl:Restriction>

                <owl:Restriction>
                  <owl:onProperty rdf:resource="&dul;hasParticipant"/>
                  <owl:someValuesFrom rdf:resource="&dul;PhysicalObject"/>
                </owl:Restriction>
              </owl:unionOf>
            </owl:Class>
          </owl:intersectionOf>
        </owl:Class>
      </owl:allValuesFrom>
      <owl:onProperty rdf:resource="&dul;classifies"/>
    </owl:Restriction>
  </rdfs:subClassOf>
  <rdfs:subClassOf rdf:resource="&soma;Delivering"/>
  <rdfs:comment>The task in which the agent delivers an object to a physical agent</rdfs:comment>
  <rdfs:isDefinedBy rdf:resource="http://www.ease-crc.org/ont/SOMA-ACT.owl"/>
</owl:Class>

<owl:Class rdf:about="&soma;Arm"
    rdfs:comment="A limb used to reach for objects.">
  <rdfs:isDefinedBy rdf:resource="http://www.ease-crc.org/ont/SOMA-OBJ.owl"/>
  <rdfs:subClassOf rdf:resource="&soma;Limb"/>
</owl:Class>

<owl:Class rdf:about="&soma;Catching">
  <rdfs:comment>A task by which an Agent stops a moving object and gains kinematic control over it, usually by grasping.</rdfs:comment>
  <rdfs:isDefinedBy rdf:resource="http://www.ease-crc.org/ont/SOMA-ACT.owl"/>
  <rdfs:subClassOf rdf:resource="&soma;Actuating"/>
  <owl:disjointWith rdf:resource="&soma;PickingUp"/>
</owl:Class>

<owl:Class rdf:about="&soma;Delivering">
  <rdfs:subClassOf>
    <owl:Restriction>
      <owl:onProperty rdf:resource="&soma;isTaskAffordedBy"/>
      <owl:someValuesFrom rdf:resource="&soma;Shifting"/>
    </owl:Restriction>
  </rdfs:subClassOf>
  <rdfs:subClassOf rdf:resource="&soma;Actuating"/>
  <owl:disjointWith rdf:resource="&soma;Fetching"/>
  <owl:disjointWith rdf:resource="&soma;Lifting"/>
  <owl:disjointWith rdf:resource="&soma;Opening"/>
  <owl:disjointWith rdf:resource="&soma;Pulling"/>
  <owl:disjointWith rdf:resource="&soma;Pushing"/>
  <owl:disjointWith rdf:resource="&soma;Squeezing"/>
  <rdfs:comment>A task in which an Agent brings an item that the Agent already carries to a specified target.</rdfs:comment>
  <rdfs:isDefinedBy rdf:resource="http://www.ease-crc.org/ont/SOMA-ACT.owl"/>
</owl:Class>

<owl:ObjectProperty rdf:about="&soma;hasStateType"
    rdfs:label="has state type">
  <rdfs:comment>A relation between roles and state types, e.g. 'the chair is the supporter of the person sitting on it'.</rdfs:comment>
  <rdfs:domain rdf:resource="&dul;Role"/>
  <rdfs:isDefinedBy rdf:resource="http://www.ease-crc.org/ont/SOMA-STATE.owl"/>
  <rdfs:range rdf:resource="&soma;StateType"/>
  <rdfs:subPropertyOf rdf:resource="&dul;isRelatedToConcept"/>
  <owl:inverseOf rdf:resource="&soma;isStateTypeOf"/>
</owl:ObjectProperty>

<owl:ObjectProperty rdf:about="&soma;hasPhysicalComponent"
    rdfs:label="has physical component">
  <rdfs:isDefinedBy rdf:resource="http://www.ease-crc.org/ont/SOMA-OBJ.owl"/>
  <rdfs:isDefinedBy rdf:resource="http://www.ease-crc.org/ont/SOMA.owl"/>
  <rdfs:comment>A relation used to describe the structure of a PhysicalObject in terms of physical components, i.e. what other PhysicalObjects are components of it.</rdfs:comment>
  <rdfs:domain rdf:resource="&dul;PhysicalObject"/>
  <rdfs:range rdf:resource="&dul;PhysicalObject"/>
  <rdfs:subPropertyOf rdf:resource="&dul;hasComponent"/>
</owl:ObjectProperty>

<owl:Class rdf:about="&soma;Premise"
    rdfs:label="Premises">
  <rdfs:comment>The role of an object that is used to infer some conclusion via some inference rules.</rdfs:comment>
  <rdfs:isDefinedBy rdf:resource="http://www.ease-crc.org/ont/SOMA-ACT.owl"/>
  <rdfs:subClassOf rdf:resource="&soma;Knowledge"/>
</owl:Class>

<owl:Class rdf:about="&soma;Releasing">
  <rdfs:comment>A task in which an agent relinquishes its kinematic control over an object, typically by releasing it from its grasp.</rdfs:comment>
  <rdfs:isDefinedBy rdf:resource="http://www.ease-crc.org/ont/SOMA-ACT.owl"/>
  <rdfs:subClassOf rdf:resource="&soma;Manipulating"/>
</owl:Class>

<soma:Reification rdf:about="&soma;RDFType">
  <soma:isReificationOf rdf:datatype="&xsd;anyURI">http://www.w3.org/2001/XMLSchema#type</soma:isReificationOf>
  <rdf:type rdf:resource="&owl;NamedIndividual"/>
  <rdfs:isDefinedBy rdf:resource="http://www.ease-crc.org/ont/SOMA.owl"/>
</soma:Reification>

<owl:ObjectProperty rdf:about="&soma;hasStep"
    rdfs:comment="A relation between a Workflow and a Task it contains."
    rdfs:label="has step">
  <rdfs:domain rdf:resource="&dul;Workflow"/>
  <rdfs:isDefinedBy rdf:resource="http://www.ease-crc.org/ont/SOMA-WF.owl"/>
  <rdfs:range rdf:resource="&dul;Task"/>
  <rdfs:subPropertyOf rdf:resource="&dul;definesTask"/>
  <owl:inverseOf rdf:resource="&soma;isStepOf"/>
</owl:ObjectProperty>

<owl:Class rdf:about="&soma;Surface"
    rdfs:comment="The outside part or uppermost layer of something.">
  <rdfs:isDefinedBy rdf:resource="http://www.ease-crc.org/ont/SOMA-OBJ.owl"/>
  <rdfs:subClassOf rdf:resource="&dul;PhysicalPlace"/>
</owl:Class>

<owl:Class rdf:about="&soma;FunctionalSpatialSchemaTheory">
  <rdfs:subClassOf>
    <owl:Restriction>
      <owl:onProperty rdf:resource="&dul;defines"/>
      <owl:someValuesFrom rdf:resource="&soma;LocatumRole"/>
    </owl:Restriction>
  </rdfs:subClassOf>
  <rdfs:subClassOf>
    <owl:Restriction>
      <owl:onProperty rdf:resource="&dul;defines"/>
      <owl:someValuesFrom rdf:resource="&soma;RelatumRole"/>
    </owl:Restriction>
  </rdfs:subClassOf>
  <rdfs:subClassOf rdf:resource="&soma;ImageSchemaTheory"/>
  <rdfs:comment>The superclass for theories describing functional spatial relations.

Adopted from GUM-4-space (Bateman et al. 2010).</rdfs:comment>
  <rdfs:isDefinedBy rdf:resource="http://www.ease-crc.org/ont/SOMA-SAY.owl"/>
  <rdfs:label xml:lang="en">Functional spatial schema theory</rdfs:label>
</owl:Class>

<owl:Class rdf:about="&soma;VideoData">
  <rdfs:comment>An information object containing data for audio-visual modalities.</rdfs:comment>
  <rdfs:isDefinedBy rdf:resource="http://www.ease-crc.org/ont/SOMA-NEEM.owl"/>
  <rdfs:label xml:lang="en">Video data</rdfs:label>
  <rdfs:subClassOf rdf:resource="&dul;InformationObject"/>
</owl:Class>

<owl:Class rdf:about="&dul;TimeInterval"/>

<owl:Class rdf:about="&soma;Masterful"
    rdfs:comment="A description of masterful behavior.">
  <rdfs:isDefinedBy rdf:resource="http://www.ease-crc.org/ont/SOMA.owl"/>
  <rdfs:subClassOf rdf:resource="&soma;DexterityDiagnosis"/>
</owl:Class>

<owl:Class rdf:about="&soma;HasQualityRegion">
  <rdfs:comment>The relation between an individual quality and a region.</rdfs:comment>
  <rdfs:comment>todo(DB): added for NEEMs (quale change), but not sure yet about it...</rdfs:comment>
  <rdfs:subClassOf>
    <owl:Restriction>
      <owl:onClass rdf:resource="&dul;Quality"/>
      <owl:onProperty rdf:resource="&dul;hasQuality"/>
      <owl:qualifiedCardinality rdf:datatype="&xsd;nonNegativeInteger">1</owl:qualifiedCardinality>
    </owl:Restriction>
  </rdfs:subClassOf>
  <rdfs:subClassOf>
    <owl:Restriction>
      <owl:onClass rdf:resource="&dul;Region"/>
      <owl:onProperty rdf:resource="&dul;hasRegion"/>
      <owl:qualifiedCardinality rdf:datatype="&xsd;nonNegativeInteger">1</owl:qualifiedCardinality>
    </owl:Restriction>
  </rdfs:subClassOf>
  <rdfs:subClassOf rdf:resource="&dul;Relation"/>
  <rdfs:isDefinedBy rdf:resource="http://www.ease-crc.org/ont/SOMA-OBJ.owl"/>
  <rdfs:label xml:lang="en">Has quality region</rdfs:label>
</owl:Class>

<owl:Class rdf:about="&soma;Cover">
  <rdfs:comment>An object used to cover up others, such as a lid used as a cover for a pot.</rdfs:comment>
  <rdfs:isDefinedBy rdf:resource="http://www.ease-crc.org/ont/SOMA-OBJ.owl"/>
  <rdfs:subClassOf rdf:resource="&soma;Barrier"/>
</owl:Class>

<owl:Class rdf:about="&soma;DeviceStateRange"
    rdfs:comment="This class defines the values that a device state can take.">
  <rdfs:isDefinedBy rdf:resource="http://www.ease-crc.org/ont/SOMA-OBJ.owl"/>
  <rdfs:label xml:lang="en">Device state range</rdfs:label>
  <rdfs:subClassOf rdf:resource="&dul;Region"/>
  <owl:equivalentClass>
    <owl:Class>
      <owl:unionOf rdf:parseType="Collection">
        <rdf:Description rdf:about="&soma;DeviceTurnedOff"/>
        <rdf:Description rdf:about="&soma;DeviceTurnedOn"/>
      </owl:unionOf>
    </owl:Class>
  </owl:equivalentClass>
</owl:Class>

<owl:ObjectProperty rdf:about="&soma;isRootLinkOf"
    rdfs:label="is root link of">
  <rdfs:comment>Relates an object to kinematic components at the root of the kinematic chain.</rdfs:comment>
  <rdfs:domain rdf:resource="&dul;PhysicalObject"/>
  <rdfs:isDefinedBy rdf:resource="http://www.ease-crc.org/ont/SOMA-OBJ.owl"/>
  <rdfs:range rdf:resource="&dul;PhysicalObject"/>
  <rdfs:subPropertyOf rdf:resource="&soma;isLinkOf"/>
</owl:ObjectProperty>

<owl:Class rdf:about="&soma;HumanActivityRecording">
  <rdfs:comment>An episode in which one or more human beings perform an activity and are recorded doing so.</rdfs:comment>
  <rdfs:isDefinedBy rdf:resource="http://www.ease-crc.org/ont/SOMA.owl"/>
  <rdfs:subClassOf rdf:resource="&soma;RecordedEpisode"/>
</owl:Class>

<owl:Class rdf:about="&soma;Cuttability">
  <rdfs:subClassOf>
    <owl:Restriction>
      <owl:allValuesFrom rdf:resource="&soma;CutObject"/>
      <owl:onProperty rdf:resource="&soma;affordsBearer"/>
    </owl:Restriction>
  </rdfs:subClassOf>
  <rdfs:subClassOf>
    <owl:Restriction>
      <owl:allValuesFrom rdf:resource="&soma;Cutter"/>
      <owl:onProperty rdf:resource="&soma;affordsTrigger"/>
    </owl:Restriction>
  </rdfs:subClassOf>
  <rdfs:subClassOf rdf:resource="&soma;Disposition"/>
  <rdfs:comment>The disposition of an object (the barrier) which makes it able to be cut down (into pieces) usually by some other object with role as a Cutter. Such as a cucumber has cuttability disposition which can be cut by a knife.</rdfs:comment>
  <rdfs:isDefinedBy rdf:resource="http://www.ease-crc.org/ont/SOMA-OBJ.owl"/>
</owl:Class>

<owl:ObjectProperty rdf:about="&soma;affordsConcept"
    rdfs:label="affords concept">
  <rdfs:comment>A relation between a disposition and a concept defined in the affordance that describes the disposition.</rdfs:comment>
  <rdfs:domain rdf:resource="&soma;Disposition"/>
  <rdfs:isDefinedBy rdf:resource="http://www.ease-crc.org/ont/SOMA-OBJ.owl"/>
  <rdfs:range rdf:resource="&dul;Concept"/>
  <rdfs:subPropertyOf rdf:resource="&dul;associatedWith"/>
  <owl:inverseOf rdf:resource="&soma;isConceptAffordedBy"/>
  <owl:propertyChainAxiom rdf:parseType="Collection">
    <rdf:Description rdf:about="&dul;isDescribedBy"/>
    <rdf:Description rdf:about="&soma;affordanceDefines"/>
  </owl:propertyChainAxiom>
</owl:ObjectProperty>

<owl:Class rdf:about="&soma;PerformerRole">
  <rdfs:subClassOf>
    <owl:Restriction>
      <owl:allValuesFrom rdf:resource="&dul;Agent"/>
      <owl:onProperty rdf:resource="&dul;classifies"/>
    </owl:Restriction>
  </rdfs:subClassOf>
  <rdfs:subClassOf rdf:resource="&soma;CausativeRole"/>
  <rdfs:comment>A role classifying an Agent responsible for performing an Action.

The entity playing an PerformerRole is endowed with sentience and the capacity to deliberately choose actions in pursuit of goals. This distinguishes Agents from other causes that could bring an event about.</rdfs:comment>
  <rdfs:isDefinedBy rdf:resource="http://www.ease-crc.org/ont/SOMA-OBJ.owl"/>
  <rdfs:label xml:lang="en">Performer role</rdfs:label>
</owl:Class>

<owl:ObjectProperty rdf:about="&dul;isRoleDefinedIn"/>

<owl:ObjectProperty rdf:about="&soma;isOccurrenceOf"
    rdfs:label="is occurence of">
  <rdfs:comment>A relation between an event and an event type, e.g. 'taking the cup from the table' is an occurence of the motion 'approaching'.</rdfs:comment>
  <rdfs:domain rdf:resource="&dul;Event"/>
  <rdfs:isDefinedBy rdf:resource="http://www.ease-crc.org/ont/SOMA.owl"/>
  <rdfs:range rdf:resource="&dul;EventType"/>
  <rdfs:subPropertyOf rdf:resource="&dul;isClassifiedBy"/>
  <owl:inverseOf rdf:resource="&soma;isOccurringIn"/>
</owl:ObjectProperty>

<owl:Class rdf:about="&soma;Discourse">
  <rdfs:comment xml:lang="en">A mental task, in which two or more agents discuss some topic via multiple Illocutionary acts, which are part of this task.</rdfs:comment>
  <rdfs:isDefinedBy rdf:resource="http://www.ease-crc.org/ont/SOMA-ACT.owl"/>
  <rdfs:label xml:lang="en">Discourse</rdfs:label>
  <rdfs:subClassOf rdf:resource="&soma;CommunicationTask"/>
</owl:Class>

<soma:ExecutionStateRegion rdf:about="&soma;ExecutionState_Paused"
    rdfs:comment="The execution state of a paused activity.">
  <rdf:type rdf:resource="&owl;NamedIndividual"/>
  <rdfs:isDefinedBy rdf:resource="http://www.ease-crc.org/ont/SOMA-ACT.owl"/>
</soma:ExecutionStateRegion>

<owl:ObjectProperty rdf:about="&soma;isTerminalStateOf"
    rdfs:label="is terminal state of">
  <rdfs:comment>A relation recording that a Situation was where a Transition ended.</rdfs:comment>
  <rdfs:domain rdf:resource="&dul;Situation"/>
  <rdfs:isDefinedBy rdf:resource="http://www.ease-crc.org/ont/SOMA.owl"/>
  <rdfs:range rdf:resource="&dul;Transition"/>
  <rdfs:subPropertyOf rdf:resource="&soma;isSituationIncludedIn"/>
</owl:ObjectProperty>

<owl:ObjectProperty rdf:about="&dul;hasParameter"/>

<owl:Class rdf:about="&soma;ExecutionStateRegion"
    rdfs:label="Execution state region">
  <rdfs:comment>A region containing labels that describe different states in the evolution/completion of a task execution.</rdfs:comment>
  <rdfs:isDefinedBy rdf:resource="http://www.ease-crc.org/ont/SOMA-ACT.owl"/>
  <rdfs:subClassOf rdf:resource="&dul;Region"/>
  <owl:equivalentClass>
    <owl:Class>
      <owl:oneOf rdf:parseType="Collection">
        <rdf:Description rdf:about="&soma;ExecutionState_Active"/>
        <rdf:Description rdf:about="&soma;ExecutionState_Cancelled"/>
        <rdf:Description rdf:about="&soma;ExecutionState_Failed"/>
        <rdf:Description rdf:about="&soma;ExecutionState_Paused"/>
        <rdf:Description rdf:about="&soma;ExecutionState_Pending"/>
        <rdf:Description rdf:about="&soma;ExecutionState_Succeeded"/>
      </owl:oneOf>
    </owl:Class>
  </owl:equivalentClass>
</owl:Class>

<owl:Class rdf:about="&soma;InformationRetrieval">
  <rdfs:subClassOf>
    <owl:Restriction>
      <owl:onProperty rdf:resource="&soma;isTaskOfOutputRole"/>
      <owl:someValuesFrom rdf:resource="&soma;Knowledge"/>
    </owl:Restriction>
  </rdfs:subClassOf>
  <rdfs:subClassOf rdf:resource="&soma;InformationAcquisition"/>
  <rdfs:comment xml:lang="en">A mental task in which an Agent recalls some knowledge that has been memorized previously.

Examples include a human remembering some information or a computer retrieving knowledge from a database.

The difference to Remembering is that for this Task, we are concerned with knowledge about a previous world state. Memory Retrieval is more general in the sense that it also includes the retrieval of learned facts and rules.</rdfs:comment>
  <rdfs:isDefinedBy rdf:resource="http://www.ease-crc.org/ont/SOMA-ACT.owl"/>
  <rdfs:label xml:lang="en">Information retrieval</rdfs:label>
</owl:Class>

<owl:ObjectProperty rdf:about="&soma;hasFrictionAttribute"
    rdfs:label="has friction attribute">
  <rdfs:comment>A relation between physical objects and their friction attribute.</rdfs:comment>
  <rdfs:domain rdf:resource="&dul;PhysicalObject"/>
  <rdfs:isDefinedBy rdf:resource="http://www.ease-crc.org/ont/SOMA-OBJ.owl"/>
  <rdfs:range rdf:resource="&soma;FrictionAttribute"/>
  <rdfs:subPropertyOf rdf:resource="&dul;hasRegion"/>
</owl:ObjectProperty>

<owl:Axiom>
  <rdfs:comment>If something is an initial situation of some transition, then it must manifest.</rdfs:comment>
  <owl:annotatedProperty rdf:resource="&rdfs;range"/>
  <owl:annotatedSource rdf:resource="&soma;hasInitialSituation"/>
  <owl:annotatedTarget>
    <owl:Class rdf:nodeID="bn4">
      <owl:complementOf rdf:resource="http://www.ease-crc.org/ont/SOMA.owl/NonmanifestedSituation"/>
    </owl:Class>
  </owl:annotatedTarget>
</owl:Axiom>

<owl:Class rdf:about="&soma;ThinkAloudActionTopic"
    rdfs:comment="A topic used when an Agent states what they are doing."
    rdfs:label="Think aloud action topic">
  <rdfs:isDefinedBy rdf:resource="http://www.ease-crc.org/ont/SOMA-ACT.owl"/>
  <rdfs:subClassOf rdf:resource="&soma;ThinkAloudTopic"/>
</owl:Class>

<owl:ObjectProperty rdf:about="&soma;isReactionTo"
    rdfs:label="is reaction to">
  <rdf:type rdf:resource="&owl;TransitiveProperty"/>
  <rdfs:comment xml:lang="en">Simple relationship between two actions to express that the subject (the reaction) would not have occured if it were not for the object (the cause), e.g., a Communication Action classified as an Answering Task is a reaction to another Communication Task classified as a Query Task and would not have occured without the other. An example without Agents involved would be some domino stone would not have toppled without the first one toppling.

When Agents are involved, the relation might be seen as an abstraction of the execution of some plan that arises from changing the agents goal that is due to perceiving the cause. However, currently it is unclear how to model such a pattern and therefore not included in SOMA.

This relation is seen as transitive.</rdfs:comment>
  <rdfs:domain rdf:resource="&dul;Event"/>
  <rdfs:isDefinedBy rdf:resource="http://www.ease-crc.org/ont/SOMA-ACT.owl"/>
  <rdfs:range rdf:resource="&dul;Event"/>
  <rdfs:subPropertyOf rdf:resource="&soma;isAffectedBy"/>
</owl:ObjectProperty>

<owl:Class rdf:about="&soma;RelationAdjacentRole">
  <rdfs:comment>A role classifying an object participating in some relation, e.g. a participant in a spatial relation or a linguistic fragment in a rhetorical relation to another.</rdfs:comment>
  <rdfs:isDefinedBy rdf:resource="http://www.ease-crc.org/ont/SOMA-OBJ.owl"/>
  <rdfs:label xml:lang="en">Relation adjacent role</rdfs:label>
  <rdfs:subClassOf rdf:resource="&dul;Role"/>
</owl:Class>

<owl:ObjectProperty rdf:about="&soma;definesBearer"
    rdfs:label="defines bearer">
  <rdfs:comment>Relates an affordance which is a relation between a bearer and a trigger, to the role of the bearer when the affordance is manifested.</rdfs:comment>
  <rdfs:domain rdf:resource="&soma;Affordance"/>
  <rdfs:isDefinedBy rdf:resource="http://www.ease-crc.org/ont/SOMA-OBJ.owl"/>
  <rdfs:range rdf:resource="&dul;Role"/>
  <rdfs:subPropertyOf rdf:resource="&dul;definesRole"/>
  <owl:inverseOf rdf:resource="&soma;isBearerDefinedIn"/>
</owl:ObjectProperty>

<owl:Class rdf:about="&soma;PluginRole">
  <rdfs:subClassOf>
    <owl:Restriction>
      <owl:onProperty rdf:resource="&dul;isDefinedIn"/>
      <owl:someValuesFrom rdf:resource="&soma;PluginSpecification"/>
    </owl:Restriction>
  </rdfs:subClassOf>
  <rdfs:subClassOf rdf:resource="&soma;InterfaceComponentRole"/>
  <rdfs:comment xml:lang="en">In the Plug-in-Host pattern, a Host application provides services which the Plug-in can use, including a way for Plug-ins to register themselves with the Host application and a protocol for the exchange of data withPplug-ins. Plug-ins depend on the services provided by the host application and do not usually work by themselves. Conversely, the host application operates independently of the plug-ins, making it possible for end-users to add and update plug-ins dynamically without needing to make changes to the host application.

Source: https://en.wikipedia.org/wiki/Plug-in_(computing)</rdfs:comment>
  <rdfs:isDefinedBy rdf:resource="http://www.ease-crc.org/ont/SOMA-IO.owl"/>
  <rdfs:label xml:lang="en">Plugin role</rdfs:label>
</owl:Class>

<owl:ObjectProperty rdf:about="&soma;hasBinding">
  <rdfs:comment>Asserts that in a context described by Description, a Binding relation holds.</rdfs:comment>
  <rdfs:domain rdf:resource="&dul;Description"/>
  <rdfs:isDefinedBy rdf:resource="http://www.ease-crc.org/ont/SOMA-WF.owl"/>
  <rdfs:label xml:lang="en">has binding</rdfs:label>
  <rdfs:range rdf:resource="&soma;Binding"/>
  <rdfs:subPropertyOf rdf:resource="&dul;hasPart"/>
</owl:ObjectProperty>

<rdf:Property rdf:about="&soma;position">
  <rdfs:domain rdf:resource="&soma;Location"/>
  <rdfs:range rdf:resource="&xsd;string"/>
</rdf:Property>

<owl:Class rdf:about="&soma;Prediction"
    rdfs:label="Predicting">
  <rdfs:comment>A Mental task in which the Agent endeavours to construct a representation of a future state of the world. Prediction commits itself to some degree of accuracy: the Agent believes that eventually something similar to the predicted state will come to pass.</rdfs:comment>
  <rdfs:isDefinedBy rdf:resource="http://www.ease-crc.org/ont/SOMA-ACT.owl"/>
  <rdfs:subClassOf rdf:resource="&soma;Prospecting"/>
</owl:Class>

<owl:ObjectProperty rdf:about="&soma;before"
    soma:symbol="&lt;">
  <rdf:type rdf:resource="&owl;TransitiveProperty"/>
  <rdfs:comment>A relation between entities, expressing a 'sequence' schema where one of the entities strictly ends before the other one.</rdfs:comment>
  <rdfs:domain rdf:resource="&dul;Entity"/>
  <rdfs:isDefinedBy rdf:resource="http://www.ease-crc.org/ont/SOMA.owl"/>
  <rdfs:range rdf:resource="&dul;Entity"/>
  <rdfs:subPropertyOf rdf:resource="&dul;precedes"/>
</owl:ObjectProperty>

<owl:Class rdf:about="&soma;AnsweringTask">
  <owl:equivalentClass>
    <owl:Class>
      <owl:intersectionOf rdf:parseType="Collection">
        <rdf:Description rdf:about="&soma;IllocutionaryTask"/>
        <owl:Restriction>
          <owl:allValuesFrom>
            <owl:Restriction>
              <owl:allValuesFrom>
                <owl:Restriction>
                  <owl:onProperty rdf:resource="&dul;isClassifiedBy"/>
                  <owl:someValuesFrom rdf:resource="&soma;CommandingTask"/>
                </owl:Restriction>
              </owl:allValuesFrom>
              <owl:onProperty rdf:resource="&soma;isReactionTo"/>
            </owl:Restriction>
          </owl:allValuesFrom>
          <owl:onProperty rdf:resource="&dul;classifies"/>
        </owl:Restriction>
      </owl:intersectionOf>
    </owl:Class>
  </owl:equivalentClass>
  <owl:equivalentClass>
    <owl:Restriction>
      <owl:onProperty rdf:resource="&dul;isTaskOf"/>
      <owl:someValuesFrom rdf:resource="&soma;Answer"/>
    </owl:Restriction>
  </owl:equivalentClass>
  <rdfs:comment xml:lang="en">An Illocutionary act where the Sender emits some Message to the Receiver as a reaction to some previous Communication task where the Roles where switched, i.e., the Sender (Receiver) of the Answering task has been the Sender (Sender) for the cause.</rdfs:comment>
  <rdfs:isDefinedBy rdf:resource="http://www.ease-crc.org/ont/SOMA-ACT.owl"/>
  <rdfs:label xml:lang="en">Answering task</rdfs:label>
</owl:Class>

<owl:DatatypeProperty rdf:about="&soma;hasHeight"
    rdfs:comment="The height of a shape."
    rdfs:label="has height">
  <rdfs:domain rdf:resource="&soma;ShapeRegion"/>
  <rdfs:isDefinedBy rdf:resource="http://www.ease-crc.org/ont/SOMA-OBJ.owl"/>
  <rdfs:range rdf:resource="&xsd;float"/>
  <rdfs:subPropertyOf rdf:resource="&soma;hasShapeParameter"/>
</owl:DatatypeProperty>

<owl:Class rdf:about="&soma;AssertionTask">
  <rdfs:subClassOf>
    <owl:Restriction>
      <owl:allValuesFrom>
        <owl:Restriction>
          <owl:onProperty rdf:resource="&dul;hasParticipant"/>
          <owl:someValuesFrom rdf:resource="&soma;DeclarativeClause"/>
        </owl:Restriction>
      </owl:allValuesFrom>
      <owl:onProperty rdf:resource="&dul;classifies"/>
    </owl:Restriction>
  </rdfs:subClassOf>
  <rdfs:subClassOf rdf:resource="&soma;IllocutionaryTask"/>
  <rdfs:comment xml:lang="en">An Illocutionary Act where the Sender emits some Message with the intent to change what the Receiver believes to be true in some context. Often, assertions are of facts about the real world, but this need not be the case. Assertions can communicate what someone believes, or refer to a world that is entirely fictional. In all these cases however, assertions are intended to update the listener's model (of the real world, or of the speaker's beliefs, or of the fictional world etc.).</rdfs:comment>
  <rdfs:isDefinedBy rdf:resource="http://www.ease-crc.org/ont/SOMA-ACT.owl"/>
  <rdfs:label xml:lang="en">Assertion task</rdfs:label>
</owl:Class>

<owl:ObjectProperty rdf:about="&dul;isExpressedBy">
  <rdfs:subPropertyOf rdf:resource="&dul;isReferenceOf"/>
</owl:ObjectProperty>

<owl:Class rdf:about="&soma;Location">
  <rdfs:comment>A role classifying a location of interest, often specified as a spatial relation between several objects, themselves usually classified by spatial relation roles.</rdfs:comment>
  <rdfs:isDefinedBy rdf:resource="http://www.ease-crc.org/ont/SOMA-OBJ.owl"/>
  <rdfs:subClassOf rdf:resource="&soma;SpatioTemporalRole"/>
</owl:Class>

<soma:Location rdf:about="location1">
  <soma:location rdf:datatype="&xsd;string">table</soma:location>
  <soma:position rdf:datatype="&xsd;string">on</soma:position>
</soma:Location>

<owl:DatatypeProperty rdf:about="&soma;hasColorValue"
    rdfs:label="has color value">
  <rdfs:comment>Associates a ColorRegion to numerical data describing the color.</rdfs:comment>
  <rdfs:domain rdf:resource="&soma;ColorRegion"/>
  <rdfs:isDefinedBy rdf:resource="http://www.ease-crc.org/ont/SOMA-OBJ.owl"/>
  <rdfs:subPropertyOf rdf:resource="&dul;hasRegionDataValue"/>
</owl:DatatypeProperty>

<owl:ObjectProperty rdf:about="&soma;terminates">
  <rdfs:comment xml:lang="en">The association between an Event that terminates another Event, e.g., the Action of picking an apple from a bowl of fruits terminates the State of containment between the apple and the bowl.</rdfs:comment>
  <rdfs:domain rdf:resource="&dul;Event"/>
  <rdfs:isDefinedBy rdf:resource="http://www.ease-crc.org/ont/SOMA-ACT.owl"/>
  <rdfs:label xml:lang="en">terminates</rdfs:label>
  <rdfs:range rdf:resource="&dul;Event"/>
  <rdfs:subPropertyOf rdf:resource="&dul;associatedWith"/>
  <owl:propertyChainAxiom rdf:parseType="Collection">
    <rdf:Description rdf:about="&soma;causesTransition"/>
    <rdf:Description rdf:about="&soma;hasInitialSituation"/>
    <rdf:Description rdf:about="&dul;includesEvent"/>
  </owl:propertyChainAxiom>
</owl:ObjectProperty>

<owl:Class rdf:about="&soma;MentalTask">
  <rdfs:subClassOf>
    <owl:Restriction>
      <owl:allValuesFrom rdf:resource="&soma;MentalAction"/>
      <owl:onProperty rdf:resource="&dul;classifies"/>
    </owl:Restriction>
  </rdfs:subClassOf>
  <rdfs:subClassOf rdf:resource="&dul;Task"/>
  <rdfs:comment>A Task classifying some MentalAction, that is, an Action through which an Agent manipulates representations stored in its own cognition.</rdfs:comment>
  <rdfs:isDefinedBy rdf:resource="http://www.ease-crc.org/ont/SOMA-ACT.owl"/>
  <rdfs:label xml:lang="en">Mental task</rdfs:label>
</owl:Class>

<owl:Class rdf:about="&soma;ArchiveFile"
    rdfs:label="Archive File">
  <rdfs:comment xml:lang="en">An archive file is a computer file that is composed of one or more files along with metadata.

Source: https://en.wikipedia.org/wiki/Archive_file</rdfs:comment>
  <rdfs:isDefinedBy rdf:resource="http://www.ease-crc.org/ont/SOMA-IO.owl"/>
  <rdfs:subClassOf rdf:resource="&soma;Digital_File"/>
  <owl:equivalentClass>
    <owl:Class>
      <owl:intersectionOf rdf:parseType="Collection">
        <rdf:Description rdf:about="&soma;Digital_File"/>
        <owl:Restriction>
          <owl:onProperty rdf:resource="&dul;realizes"/>
          <owl:someValuesFrom rdf:resource="&soma;ArchiveText"/>
        </owl:Restriction>
      </owl:intersectionOf>
    </owl:Class>
  </owl:equivalentClass>
</owl:Class>

<owl:Class rdf:about="&soma;Container"
    rdfs:comment="A role classifying an object used to contain others.">
  <rdfs:isDefinedBy rdf:resource="http://www.ease-crc.org/ont/SOMA-OBJ.owl"/>
  <rdfs:isDefinedBy rdf:resource="http://www.ease-crc.org/ont/SOMA-STATE.owl"/>
  <rdfs:subClassOf rdf:resource="&soma;Restrictor"/>
</owl:Class>

<owl:Class rdf:about="&soma;CylinderShape"
    rdfs:label="Cylinder shape">
  <rdfs:subClassOf>
    <owl:Restriction>
      <owl:onProperty rdf:resource="&soma;hasRadius"/>
      <owl:someValuesFrom rdf:resource="&xsd;float"/>
    </owl:Restriction>
  </rdfs:subClassOf>
  <rdfs:subClassOf>
    <owl:Restriction>
      <owl:onDataRange rdf:resource="&xsd;float"/>
      <owl:onProperty rdf:resource="&soma;hasLength"/>
      <owl:qualifiedCardinality rdf:datatype="&xsd;nonNegativeInteger">1</owl:qualifiedCardinality>
    </owl:Restriction>
  </rdfs:subClassOf>
  <rdfs:subClassOf rdf:resource="&soma;ShapeRegion"/>
  <rdfs:comment>A solid geometrical figure with straight parallel sides and a circular or oval cross section.</rdfs:comment>
  <rdfs:isDefinedBy rdf:resource="http://www.ease-crc.org/ont/SOMA-OBJ.owl"/>
</owl:Class>

<owl:ObjectProperty rdf:about="&soma;definesSetpoint"
    rdfs:comment="Defines the dedicated goal region of a description."
    rdfs:label="defines setpoint">
  <rdfs:domain rdf:resource="&dul;Description"/>
  <rdfs:isDefinedBy rdf:resource="http://www.ease-crc.org/ont/SOMA-OBJ.owl"/>
  <rdfs:range rdf:resource="&soma;Setpoint"/>
  <rdfs:subPropertyOf rdf:resource="&soma;definesParameter"/>
  <owl:inverseOf rdf:resource="&soma;isSetpointDefinedIn"/>
</owl:ObjectProperty>

<owl:Class rdf:about="&soma;AestheticDesign"
    rdfs:label="Aesthetic Design">
  <rdfs:comment>A design that describes an aesthetic quality of an object.

Aesthetics is the philosophical study of beauty and taste. The term stems from the Greek word 'aisthetikos', meaning 'of sense perception', and is related to the study of sensory values. From design point of view, aesthetics refers to the visual attractiveness of an object. Visual aesthetics have these key elements: Color, Shape, Pattern, Line, Texture, Visual weight, Balance, Scale, Proximity and Movement.</rdfs:comment>
  <rdfs:isDefinedBy rdf:resource="http://www.ease-crc.org/ont/SOMA-OBJ.owl"/>
  <rdfs:subClassOf rdf:resource="&dul;Design"/>
</owl:Class>

<owl:Class rdf:about="&soma;Algorithm">
  <rdfs:comment xml:lang="en">An Algorithm is a finite sequence of well-defined instructions, typically used to solve a class of specific problems or to perform a computation.

From Wikipedia: https://en.wikipedia.org/wiki/Algorithm</rdfs:comment>
  <rdfs:isDefinedBy rdf:resource="http://www.ease-crc.org/ont/SOMA-IO.owl"/>
  <rdfs:label xml:lang="en">Algorithm</rdfs:label>
  <rdfs:subClassOf rdf:resource="&dul;Plan"/>
</owl:Class>

<owl:Class rdf:about="&soma;Retrospecting">
  <rdfs:comment>A Mental task in which an Agent endeavors to construct a representation of a past state of affairs of the world it is embodied in.</rdfs:comment>
  <rdfs:comment>Done by analogy with Prospecting. Currently mono-subcategory, but perhaps we might find more.

As an example, a kind of Abductive reasoning would fit here: reconstruction, in which the agent attempts to create a representation of a past state of affairs which the agent has not actually observed, based on traces and clues surviving to the present.</rdfs:comment>
  <rdfs:isDefinedBy rdf:resource="http://www.ease-crc.org/ont/SOMA-ACT.owl"/>
  <rdfs:subClassOf rdf:resource="&soma;InformationAcquisition"/>
</owl:Class>

<owl:Class rdf:about="&soma;ResultRole">
  <rdfs:comment>A role classifying the object that is the outcome of a creation or modification action or process.</rdfs:comment>
  <rdfs:isDefinedBy rdf:resource="http://www.ease-crc.org/ont/SOMA-OBJ.owl"/>
  <rdfs:label xml:lang="en">Result role</rdfs:label>
  <rdfs:subClassOf rdf:resource="&soma;GoalRole"/>
</owl:Class>

<owl:ObjectProperty rdf:about="&soma;hasBindingRole">
  <rdfs:comment>Indicates that a Role/Parameter is going to be associated to some filler, or other Role/Parameter, by a Binding. The Binding is only valid in some descriptive context such as a Narrative or Workflow.</rdfs:comment>
  <rdfs:domain rdf:resource="&soma;Binding"/>
  <rdfs:isDefinedBy rdf:resource="http://www.ease-crc.org/ont/SOMA-WF.owl"/>
  <rdfs:label xml:lang="en">has binding role</rdfs:label>
  <rdfs:range>
    <owl:Class>
      <owl:unionOf rdf:parseType="Collection">
        <rdf:Description rdf:about="&dul;Parameter"/>
        <rdf:Description rdf:about="&dul;Role"/>
      </owl:unionOf>
    </owl:Class>
  </rdfs:range>
  <rdfs:subPropertyOf rdf:resource="&dul;hasPart"/>
</owl:ObjectProperty>

<owl:Class rdf:about="&soma;RoleRoleBinding"
    rdfs:comment="A binding that asserts that two roles have the same filler.">
  <rdfs:subClassOf>
    <owl:Restriction>
      <owl:allValuesFrom>
        <owl:Class>
          <owl:unionOf rdf:parseType="Collection">
            <rdf:Description rdf:about="&dul;Parameter"/>
            <rdf:Description rdf:about="&dul;Role"/>
          </owl:unionOf>
        </owl:Class>
      </owl:allValuesFrom>
      <owl:onProperty rdf:resource="&soma;hasBindingFiller"/>
    </owl:Restriction>
  </rdfs:subClassOf>
  <rdfs:subClassOf rdf:resource="&soma;Binding"/>
  <rdfs:isDefinedBy rdf:resource="http://www.ease-crc.org/ont/SOMA-WF.owl"/>
  <rdfs:label xml:lang="en">Role role binding</rdfs:label>
</owl:Class>

<owl:Class rdf:about="&soma;Coverage">
  <rdfs:subClassOf>
    <owl:Restriction>
      <owl:allValuesFrom rdf:resource="&soma;Cover"/>
      <owl:onProperty rdf:resource="&soma;affordsBearer"/>
    </owl:Restriction>
  </rdfs:subClassOf>
  <rdfs:subClassOf>
    <owl:Restriction>
      <owl:allValuesFrom rdf:resource="&soma;CoveredObject"/>
      <owl:onProperty rdf:resource="&soma;affordsTrigger"/>
    </owl:Restriction>
  </rdfs:subClassOf>
  <rdfs:subClassOf rdf:resource="&soma;Blockage"/>
  <rdfs:comment>The disposition of an object (the cover) to hide or to protect objects by covering them. An example is a door that covers items in a container to e.g. prevent dust getting inside of the container.</rdfs:comment>
  <rdfs:isDefinedBy rdf:resource="http://www.ease-crc.org/ont/SOMA-OBJ.owl"/>
</owl:Class>

<owl:Class rdf:about="&soma;Blockage">
  <rdfs:subClassOf>
    <owl:Restriction>
      <owl:allValuesFrom rdf:resource="&soma;Barrier"/>
      <owl:onProperty rdf:resource="&soma;affordsBearer"/>
    </owl:Restriction>
  </rdfs:subClassOf>
  <rdfs:subClassOf>
    <owl:Restriction>
      <owl:allValuesFrom rdf:resource="&soma;BlockedObject"/>
      <owl:onProperty rdf:resource="&soma;affordsTrigger"/>
    </owl:Restriction>
  </rdfs:subClassOf>
  <rdfs:subClassOf rdf:resource="&soma;Disposition"/>
  <rdfs:comment>The disposition of an object (the barrier) to prevent others from accessing, leaving, or seeing a restricted space, or group.</rdfs:comment>
  <rdfs:isDefinedBy rdf:resource="http://www.ease-crc.org/ont/SOMA-OBJ.owl"/>
</owl:Class>

<owl:Class rdf:about="&soma;Language">
  <rdfs:subClassOf>
    <owl:Restriction>
      <owl:allValuesFrom rdf:resource="&soma;Text"/>
      <owl:onProperty rdf:resource="&soma;givesMeaningTo"/>
    </owl:Restriction>
  </rdfs:subClassOf>
  <rdfs:subClassOf rdf:resource="&soma;System"/>
  <rdfs:comment xml:lang="en">A Language is a structured System for communication.

From Wikipedia: https://en.wikipedia.org/wiki/Language</rdfs:comment>
  <rdfs:isDefinedBy rdf:resource="http://www.ease-crc.org/ont/SOMA-IO.owl"/>
  <rdfs:label xml:lang="en">Language</rdfs:label>
</owl:Class>

<owl:Class rdf:about="&soma;TemperatureRegion"
    rdfs:comment="Encodes the temperature of an object.">
  <rdfs:isDefinedBy rdf:resource="http://www.ease-crc.org/ont/SOMA-OBJ.owl"/>
  <rdfs:label xml:lang="en">Temperature region</rdfs:label>
  <rdfs:subClassOf rdf:resource="&dul;Region"/>
</owl:Class>

<owl:ObjectProperty rdf:about="&soma;movesObject">
  <rdfs:comment>A relation from an agent to an object that the agent causes to move.</rdfs:comment>
  <rdfs:domain rdf:resource="&dul;Agent"/>
  <rdfs:isDefinedBy rdf:resource="http://www.ease-crc.org/ont/SOMA-SAY.owl"/>
  <rdfs:range rdf:resource="&dul;PhysicalObject"/>
  <rdfs:subPropertyOf rdf:resource="&soma;interactsWith"/>
</owl:ObjectProperty>

<owl:Class rdf:about="&soma;RevoluteJoint"
    rdfs:label="Revolute joint">
  <rdfs:subClassOf>
    <owl:Restriction>
      <owl:onClass rdf:resource="&soma;JointLimit"/>
      <owl:onProperty rdf:resource="&soma;hasJointLimit"/>
      <owl:qualifiedCardinality rdf:datatype="&xsd;nonNegativeInteger">1</owl:qualifiedCardinality>
    </owl:Restriction>
  </rdfs:subClassOf>
  <rdfs:subClassOf rdf:resource="&soma;HingeJoint"/>
  <rdfs:comment>A hinge joint that rotates along an axis and has a limited range specified by the upper and lower limits.</rdfs:comment>
  <rdfs:isDefinedBy rdf:resource="http://www.ease-crc.org/ont/SOMA-OBJ.owl"/>
</owl:Class>

<owl:ObjectProperty rdf:about="&soma;isLinkedTo"
    rdfs:label="is linked to">
  <rdf:type rdf:resource="&owl;SymmetricProperty"/>
  <rdfs:comment>A spatial relation holding between objects that are linked with each other such that they resist spatial separation.</rdfs:comment>
  <rdfs:domain rdf:resource="&dul;PhysicalObject"/>
  <rdfs:isDefinedBy rdf:resource="http://www.ease-crc.org/ont/SOMA-OBJ.owl"/>
  <rdfs:range rdf:resource="&dul;PhysicalObject"/>
  <rdfs:subPropertyOf rdf:resource="&dul;hasLocation"/>
</owl:ObjectProperty>

<owl:Class rdf:about="&soma;FluidFlow"
    rdfs:label="Fluid flow">
  <rdfs:subClassOf>
    <owl:Restriction>
      <owl:onProperty rdf:resource="&soma;isProcessTypeOf"/>
      <owl:someValuesFrom rdf:resource="&soma;MovedObject"/>
    </owl:Restriction>
  </rdfs:subClassOf>
  <rdfs:subClassOf rdf:resource="&soma;Motion"/>
  <rdfs:comment>A process by which a fluid moves or is moved from a location to another, but such that it maintains its constitution. A fluid is an Entity made of many smaller Entities, loosely bound to each other.

An issue to highlight here is the maintenance of constitution. Fluids-- gases in particular-- are prone to disperse. Such a process is not flow however, because the loose bounds between the constituents become even looser, to the point of the original Entity becoming entirely discombobulated. </rdfs:comment>
  <rdfs:isDefinedBy rdf:resource="http://www.ease-crc.org/ont/SOMA-PROC.owl"/>
</owl:Class>

<owl:Class rdf:about="&soma;CreatedObject"
    rdfs:comment="An object that is created.">
  <rdfs:isDefinedBy rdf:resource="http://www.ease-crc.org/ont/SOMA-OBJ.owl"/>
  <rdfs:isDefinedBy rdf:resource="http://www.ease-crc.org/ont/SOMA-PROC.owl"/>
  <rdfs:label xml:lang="en">Created object</rdfs:label>
  <rdfs:subClassOf rdf:resource="&soma;Patient"/>
</owl:Class>

<owl:ObjectProperty rdf:about="&dul;isRegionFor"/>

<owl:ObjectProperty rdf:about="&dul;isTaskOf"/>

<owl:Class rdf:about="&soma;System">
  <rdfs:comment xml:lang="en">A system is a group of interacting or interrelated elements that act according to a set of rules to form a unified whole.

From Wikipedia: https://en.wikipedia.org/wiki/System</rdfs:comment>
  <rdfs:isDefinedBy rdf:resource="http://www.ease-crc.org/ont/SOMA-IO.owl"/>
  <rdfs:label xml:lang="en">System</rdfs:label>
  <rdfs:subClassOf rdf:resource="&dul;SocialObject"/>
</owl:Class>

<owl:Class rdf:about="&soma;PickingUp">
  <rdfs:comment>A task in which the Agent uses one or more of its grippers to grasp a usually stationary object.</rdfs:comment>
  <rdfs:isDefinedBy rdf:resource="http://www.ease-crc.org/ont/SOMA-ACT.owl"/>
  <rdfs:subClassOf rdf:resource="&soma;Manipulating"/>
</owl:Class>

<owl:ObjectProperty rdf:about="&dul;defines">
  <rdfs:isDefinedBy rdf:resource="http://www.ease-crc.org/ont/SOMA-PROC.owl"/>
  <rdfs:isDefinedBy rdf:resource="http://www.ease-crc.org/ont/SOMA-WF.owl"/>
</owl:ObjectProperty>

<owl:Class rdf:about="&soma;Digital_File">
  <rdfs:label xml:lang="en">Computer File</rdfs:label>
  <rdfs:label xml:lang="en">Digital File</rdfs:label>
  <rdfs:subClassOf rdf:nodeID="bn0"/>
  <rdfs:subClassOf>
    <owl:Restriction rdf:nodeID="bn5">
      <owl:onProperty rdf:resource="&soma;hasNameString"/>
      <owl:someValuesFrom rdf:resource="&xsd;string"/>
    </owl:Restriction>
  </rdfs:subClassOf>
  <rdfs:subClassOf rdf:resource="&dul;InformationRealization"/>
  <rdfs:comment xml:lang="en">Any file that exists as a digital resource (but not its content), e.g., a text file actually laying on some hard drive, but not the contained text.</rdfs:comment>
  <rdfs:isDefinedBy rdf:resource="http://www.ease-crc.org/ont/SOMA-IO.owl"/>
</owl:Class>

<owl:Class rdf:about="&dul;Region"/>

<owl:Class rdf:about="&soma;DirectedMotion"
    rdfs:label="Directed motion">
  <rdfs:comment>A Motion that is considered to be toward a location or along a path. It is not important that the final location or path be the intention of some Agent, but it is considered that the important feature of this Motion is that it has a path and/or destination.</rdfs:comment>
  <rdfs:isDefinedBy rdf:resource="http://www.ease-crc.org/ont/SOMA-PROC.owl"/>
  <rdfs:subClassOf rdf:resource="&soma;Motion"/>
  <owl:disjointWith rdf:resource="&soma;UndirectedMotion"/>
</owl:Class>

<owl:Class rdf:about="&soma;PhysicalState"
    rdfs:label="Physical state">
  <rdfs:subClassOf>
    <owl:Restriction>
      <owl:onProperty rdf:resource="&dul;hasParticipant"/>
      <owl:someValuesFrom rdf:resource="&dul;PhysicalObject"/>
    </owl:Restriction>
  </rdfs:subClassOf>
  <rdfs:subClassOf rdf:resource="&soma;State"/>
  <rdfs:comment>A State describing how Entities in the physical world relate to each other.</rdfs:comment>
  <rdfs:isDefinedBy rdf:resource="http://www.ease-crc.org/ont/SOMA-STATE.owl"/>
</owl:Class>

<owl:Class rdf:about="&soma;CommunicationTask">
  <rdfs:subClassOf>
    <owl:Class>
      <owl:intersectionOf rdf:parseType="Collection">

        <owl:Restriction>
          <owl:onProperty rdf:resource="&dul;isTaskOf"/>
          <owl:someValuesFrom rdf:resource="&soma;Channel"/>
        </owl:Restriction>

        <owl:Restriction>
          <owl:onProperty rdf:resource="&dul;isTaskOf"/>
          <owl:someValuesFrom rdf:resource="&soma;Message"/>
        </owl:Restriction>

        <owl:Restriction>
          <owl:onProperty rdf:resource="&dul;isTaskOf"/>
          <owl:someValuesFrom rdf:resource="&soma;Receiver"/>
        </owl:Restriction>

        <owl:Restriction>
          <owl:onProperty rdf:resource="&dul;isTaskOf"/>
          <owl:someValuesFrom rdf:resource="&soma;Sender"/>
        </owl:Restriction>
      </owl:intersectionOf>
    </owl:Class>
  </rdfs:subClassOf>
  <rdfs:subClassOf>
    <owl:Restriction>
      <owl:allValuesFrom>
        <owl:Restriction>
          <owl:allValuesFrom>
            <owl:Class>
              <owl:unionOf rdf:parseType="Collection">
                <rdf:Description rdf:about="&dul;Agent"/>
                <rdf:Description rdf:about="&dul;SocialObject"/>
              </owl:unionOf>
            </owl:Class>
          </owl:allValuesFrom>
          <owl:onProperty rdf:resource="&dul;hasParticipant"/>
        </owl:Restriction>
      </owl:allValuesFrom>
      <owl:onProperty rdf:resource="&dul;classifies"/>
    </owl:Restriction>
  </rdfs:subClassOf>
  <rdfs:subClassOf rdf:resource="&dul;Task"/>
  <rdfs:comment>A Task in which two or more Agents exchange information. A CommunicationTask classifies only Events that have only Agents and Social objects as participants.

Of course, the means of exchange is Physical, however this concept is to classify events for which we are not interested in the physical substrate, but rather who communicated and what the information content was.</rdfs:comment>
  <rdfs:isDefinedBy rdf:resource="http://www.ease-crc.org/ont/SOMA-ACT.owl"/>
  <rdfs:label xml:lang="en">Communication task</rdfs:label>
</owl:Class>

<owl:Class rdf:about="&dul;SpaceRegion"/>

<owl:ObjectProperty rdf:about="&soma;isLocalizationOf"
    rdfs:label="is localization of">
  <rdfs:comment>Relates a localization quality to the object the localization belongs to.</rdfs:comment>
  <rdfs:domain rdf:resource="&soma;Localization"/>
  <rdfs:isDefinedBy rdf:resource="http://www.ease-crc.org/ont/SOMA-OBJ.owl"/>
  <rdfs:range rdf:resource="&dul;PhysicalObject"/>
  <rdfs:subPropertyOf rdf:resource="&dul;isQualityOf"/>
</owl:ObjectProperty>

<owl:Class rdf:about="&soma;Containment">
  <rdfs:comment>Classifies States in which an object is placed inside another.</rdfs:comment>
  <rdfs:comment>The disposition of an object (the container) to contain others.</rdfs:comment>
  <rdfs:isDefinedBy rdf:resource="http://www.ease-crc.org/ont/SOMA-OBJ.owl"/>
  <rdfs:isDefinedBy rdf:resource="http://www.ease-crc.org/ont/SOMA-STATE.owl"/>
  <rdfs:subClassOf>
    <owl:Restriction>
      <owl:allValuesFrom rdf:resource="&soma;Container"/>
      <owl:onProperty rdf:resource="&soma;affordsBearer"/>
    </owl:Restriction>
  </rdfs:subClassOf>
  <rdfs:subClassOf>
    <owl:Restriction>
      <owl:allValuesFrom rdf:resource="&soma;IncludedObject"/>
      <owl:onProperty rdf:resource="&soma;affordsTrigger"/>
    </owl:Restriction>
  </rdfs:subClassOf>
  <rdfs:subClassOf>
    <owl:Restriction>
      <owl:allValuesFrom>
        <owl:Restriction>
          <owl:onProperty rdf:resource="&dul;hasQuality"/>
          <owl:someValuesFrom rdf:resource="&soma;Capacity"/>
        </owl:Restriction>
      </owl:allValuesFrom>
      <owl:onProperty rdf:resource="&soma;isDispositionOf"/>
    </owl:Restriction>
  </rdfs:subClassOf>
  <rdfs:subClassOf rdf:resource="&soma;Disposition"/>
</owl:Class>

<owl:DatatypeProperty rdf:about="&soma;hasJointVelocity"
    rdfs:label="has joint velocity">
  <rdfs:comment>The velocity of a joint given in m/s (prismatic joints) or rad/s (hinged joints).</rdfs:comment>
  <rdfs:domain rdf:resource="&soma;JointState"/>
  <rdfs:isDefinedBy rdf:resource="http://www.ease-crc.org/ont/SOMA-OBJ.owl"/>
  <rdfs:range rdf:resource="&xsd;double"/>
  <rdfs:subPropertyOf rdf:resource="&soma;hasJointParameter"/>
</owl:DatatypeProperty>

<owl:Class rdf:about="&soma;ThinkAloudObstructionTopic"
    rdfs:label="Think aloud obstruction topic">
  <rdfs:comment>A topic used when an Agent describes some state of affairs that prevents them from performing an action.</rdfs:comment>
  <rdfs:isDefinedBy rdf:resource="http://www.ease-crc.org/ont/SOMA-ACT.owl"/>
  <rdfs:subClassOf rdf:resource="&soma;ThinkAloudTopic"/>
</owl:Class>

<owl:Class rdf:about="&soma;Grasping">
  <rdfs:comment>A task in which an Agent uses its end effectors to grasp an object, thus gaining kinematic control over it.</rdfs:comment>
  <rdfs:isDefinedBy rdf:resource="http://www.ease-crc.org/ont/SOMA-ACT.owl"/>
  <rdfs:subClassOf rdf:resource="&soma;Manipulating"/>
  <owl:disjointWith rdf:resource="&soma;Releasing"/>
</owl:Class>

<owl:ObjectProperty rdf:about="http://www.ease-crc.org/ont/SOMA.owl/preventedBy"
    rdfs:label="prevented by">
  <rdfs:comment>A relationship indicating a Situation is prevented by another from manifesting.</rdfs:comment>
  <rdfs:domain rdf:resource="&dul;Situation"/>
  <rdfs:isDefinedBy rdf:resource="http://www.ease-crc.org/ont/SOMA-ACT.owl"/>
  <rdfs:range rdf:resource="&dul;Situation"/>
  <rdfs:subPropertyOf rdf:resource="&dul;hasSetting"/>
  <owl:inverseOf rdf:resource="http://www.ease-crc.org/ont/SOMA.owl/prevents"/>
</owl:ObjectProperty>

<owl:ObjectProperty rdf:about="&soma;orders">
  <rdfs:comment xml:lang="en">The relation between an 'Order' and the sorted 'Order item' (sorted via the relations 'precedes' and 'follows' between the 'Order item's)</rdfs:comment>
  <rdfs:domain rdf:resource="&soma;Order"/>
  <rdfs:isDefinedBy rdf:resource="http://www.ease-crc.org/ont/SOMA-AGENT.owl"/>
  <rdfs:label xml:lang="en">orders</rdfs:label>
  <rdfs:range rdf:resource="&soma;OrderedElement"/>
  <rdfs:subPropertyOf rdf:resource="&dul;associatedWith"/>
</owl:ObjectProperty>

<owl:Class rdf:about="&soma;DesignedTool"
    rdfs:label="Designed tool">
  <rdfs:isDefinedBy rdf:resource="http://www.ease-crc.org/ont/SOMA-IO.owl"/>
  <rdfs:isDefinedBy rdf:resource="http://www.ease-crc.org/ont/SOMA-OBJ.owl"/>
  <rdfs:comment>An item designed to enable some action, in which it will play an instrumental role.</rdfs:comment>
  <rdfs:subClassOf rdf:resource="&dul;DesignedArtifact"/>
</owl:Class>

<owl:Class rdf:about="&soma;InsertedObject"
    rdfs:comment="An object inserted into another object.">
  <rdfs:isDefinedBy rdf:resource="http://www.ease-crc.org/ont/SOMA-OBJ.owl"/>
  <rdfs:label xml:lang="en">Inserted object</rdfs:label>
  <rdfs:subClassOf rdf:resource="&soma;EnclosedObject"/>
</owl:Class>

<owl:Class rdf:about="&soma;Insertion">
  <rdfs:subClassOf>
    <owl:Restriction>
      <owl:allValuesFrom rdf:resource="&soma;InsertedObject"/>
      <owl:onProperty rdf:resource="&soma;affordsTrigger"/>
    </owl:Restriction>
  </rdfs:subClassOf>
  <rdfs:subClassOf rdf:resource="&soma;Enclosing"/>
  <rdfs:comment>The disposition of an object (the container) to contain other objects that can be inserted into the container through a portal.</rdfs:comment>
  <rdfs:isDefinedBy rdf:resource="http://www.ease-crc.org/ont/SOMA-OBJ.owl"/>
</owl:Class>

<owl:Class rdf:about="&soma;Sharpness">
  <rdfs:comment>The quality of having a thin edge or point that can cut something or make a hole into something. It is worth to note here that the social aspect of sharpness such as the quality of being clear, intelligent etc is not considered as sharpness according to this definition.</rdfs:comment>
  <rdfs:isDefinedBy rdf:resource="http://www.ease-crc.org/ont/SOMA-OBJ.owl"/>
  <rdfs:subClassOf rdf:resource="&soma;Intrinsic"/>
</owl:Class>

<owl:Class rdf:about="&soma;ForceAttribute"
    rdfs:label="Force attribute">
  <rdfs:subClassOf>
    <owl:Restriction>
      <owl:onDataRange rdf:resource="&soma;array_double"/>
      <owl:onProperty rdf:resource="&soma;hasForceValue"/>
      <owl:qualifiedCardinality rdf:datatype="&xsd;nonNegativeInteger">1</owl:qualifiedCardinality>
    </owl:Restriction>
  </rdfs:subClassOf>
  <rdfs:subClassOf rdf:resource="&dul;PhysicalAttribute"/>
  <rdfs:comment>The value of a force dynamical characteristic. An example is the force exerted on another object when pushing it.</rdfs:comment>
  <rdfs:isDefinedBy rdf:resource="http://www.ease-crc.org/ont/SOMA-OBJ.owl"/>
</owl:Class>

<owl:Class rdf:about="&soma;Material"
    rdfs:comment="The matter from which a thing is made.">
  <rdfs:isDefinedBy rdf:resource="http://www.ease-crc.org/ont/SOMA-OBJ.owl"/>
  <rdfs:subClassOf rdf:resource="&soma;Intrinsic"/>
</owl:Class>

<owl:Class rdf:about="&soma;ChemicalProcess"
    rdfs:label="Chemical process">
  <rdfs:comment>A process by which the chemical constituency of an Entity or set of Entities changes.

In some sense any process that results in entities being created or destroyed might trivially fit here, however this concept is intended specifically for Events where the occuring chemical reactions are of importance.</rdfs:comment>
  <rdfs:isDefinedBy rdf:resource="http://www.ease-crc.org/ont/SOMA-PROC.owl"/>
  <rdfs:subClassOf rdf:resource="&dul;Process"/>
</owl:Class>

<owl:Class rdf:about="&soma;CoveredObject"
    rdfs:comment="An object that is covered.">
  <rdfs:isDefinedBy rdf:resource="http://www.ease-crc.org/ont/SOMA-OBJ.owl"/>
  <rdfs:label xml:lang="en">Covered object</rdfs:label>
  <rdfs:subClassOf rdf:resource="&soma;BlockedObject"/>
</owl:Class>

<owl:ObjectProperty rdf:about="&soma;involvesEffector"
    rdfs:comment="Effector participation."
    rdfs:label="involves effector">
  <rdfs:domain rdf:resource="&dul;Event"/>
  <rdfs:isDefinedBy rdf:resource="http://www.ease-crc.org/ont/SOMA-OBJ.owl"/>
  <rdfs:range rdf:resource="&soma;PhysicalEffector"/>
  <rdfs:subPropertyOf rdf:resource="&dul;hasParticipant"/>
  <owl:inverseOf rdf:resource="&soma;isEffectorInvolvedIn"/>
</owl:ObjectProperty>

<owl:Class rdf:about="&soma;StructuralDesign"
    rdfs:label="Structural Design">
  <rdfs:comment>A design of an object which describes its stability, strength and rigidity, and considers the way in which parts of an object are arranged. 
        </rdfs:comment>
  <rdfs:isDefinedBy rdf:resource="http://www.ease-crc.org/ont/SOMA-OBJ.owl"/>
  <rdfs:subClassOf rdf:resource="&dul;Design"/>
</owl:Class>

<owl:ObjectProperty rdf:about="&soma;hasBindingFiller">
  <rdfs:comment>Indicates that an Entity is described by a Binding, in that it is associated with the Role/Parameter that the Binding binds it to. The Binding is only valid in some descriptive context such as a Workflow or Narrative.

Note, the filler can be a Role/Parameter as well, and there are two distinct interpretations, depending on whether the Binding is a RoleRoleBinding or a RoleFillerBinding. See the comments on Binding for more details.

Only RoleFillerBindings can have general Entities as fillers. RoleRoleBindings can only connect to Roles or Parameters via this property.</rdfs:comment>
  <rdfs:domain rdf:resource="&soma;Binding"/>
  <rdfs:isDefinedBy rdf:resource="http://www.ease-crc.org/ont/SOMA-WF.owl"/>
  <rdfs:label xml:lang="en">has binding filler</rdfs:label>
  <rdfs:range rdf:resource="&dul;Entity"/>
  <rdfs:subPropertyOf rdf:resource="&dul;describes"/>
</owl:ObjectProperty>

<owl:ObjectProperty rdf:about="&soma;supports">
  <rdfs:comment>A relation between an object (the supporter) and another object (the supportee) where the supporter cancels the effect of gravity on the supportee.</rdfs:comment>
  <rdfs:comment>Relates a supportee to one of its supporters.</rdfs:comment>
  <rdfs:isDefinedBy rdf:resource="http://www.ease-crc.org/ont/SOMA-OBJ.owl"/>
  <rdfs:isDefinedBy rdf:resource="http://www.ease-crc.org/ont/SOMA-PROC.owl"/>
  <rdfs:subPropertyOf rdf:resource="&soma;interactsWith"/>
  <rdfs:subPropertyOf rdf:resource="&dul;hasCommonBoundary"/>
  <rdfs:domain rdf:resource="&dul;Entity"/>
  <rdfs:range rdf:resource="&dul;Entity"/>
</owl:ObjectProperty>

<soma:ExecutionStateRegion rdf:about="&soma;ExecutionState_Cancelled"
    rdfs:comment="The execution state of a cancelled activity.">
  <rdf:type rdf:resource="&owl;NamedIndividual"/>
  <rdfs:isDefinedBy rdf:resource="http://www.ease-crc.org/ont/SOMA-ACT.owl"/>
</soma:ExecutionStateRegion>

<owl:Class rdf:about="&soma;CommunicationTopic">
  <rdfs:subClassOf>
    <owl:Restriction>
      <owl:allValuesFrom>
        <owl:Class>
          <owl:intersectionOf rdf:parseType="Collection">
            <rdf:Description rdf:about="&dul;SocialObject"/>
            <owl:Restriction>
              <owl:onProperty rdf:resource="&dul;isParticipantIn"/>
              <owl:someValuesFrom>
                <owl:Restriction>
                  <owl:onProperty rdf:resource="&dul;isClassifiedBy"/>
                  <owl:someValuesFrom rdf:resource="&soma;CommunicationTask"/>
                </owl:Restriction>
              </owl:someValuesFrom>
            </owl:Restriction>
          </owl:intersectionOf>
        </owl:Class>
      </owl:allValuesFrom>
      <owl:onProperty rdf:resource="&dul;classifies"/>
    </owl:Restriction>
  </rdfs:subClassOf>
  <rdfs:subClassOf rdf:resource="&soma;ResourceRole"/>
  <rdfs:comment>A role that appears in communication tasks, and indicates what the communication is about.

CommunicationTopic can only classify a Social object that participates in an Action that is classified as (the execution of) a CommunicationTask.

Note that classifies here is used in the plays-role sense. This isn't to say that the social object, ie the information exchanged in the communication, is an instance of the topic. Rather, the topic role refers to what the information is about.

For example, if the topic of a communication is flowers, this does not mean the words themselves are flowers, merely that, in some sense, they are about flowers.</rdfs:comment>
  <rdfs:isDefinedBy rdf:resource="http://www.ease-crc.org/ont/SOMA-ACT.owl"/>
  <rdfs:label xml:lang="en">Communication topic</rdfs:label>
</owl:Class>

<owl:Class rdf:about="&soma;Successfulness">
  <rdfs:comment>A description of a situation with a goal that was achieved by some system.</rdfs:comment>
  <rdfs:isDefinedBy rdf:resource="http://www.ease-crc.org/ont/SOMA.owl"/>
  <rdfs:subClassOf rdf:resource="&soma;SuccessDiagnosis"/>
  <owl:disjointWith rdf:resource="&soma;Unsuccessfulness"/>
</owl:Class>

<owl:ObjectProperty rdf:about="&dul;isClassifiedBy"/>

<owl:Class rdf:about="&soma;Inability">
  <rdfs:comment>A description of a situation with a goal that some system is unable to achieve.</rdfs:comment>
  <rdfs:isDefinedBy rdf:resource="http://www.ease-crc.org/ont/SOMA.owl"/>
  <rdfs:subClassOf rdf:resource="&soma;Unsuccessfulness"/>
</owl:Class>

<owl:Class rdf:about="&soma;ContainmentState">
  <rdfs:subClassOf>
    <owl:Restriction>
      <owl:onProperty rdf:resource="&soma;isStateTypeOf"/>
      <owl:someValuesFrom>
        <owl:Class>
          <owl:intersectionOf rdf:parseType="Collection">
            <rdf:Description rdf:about="&soma;Container"/>
            <owl:Restriction>
              <owl:allValuesFrom>
                <owl:Restriction>
                  <owl:onProperty rdf:resource="&soma;hasDisposition"/>
                  <owl:someValuesFrom rdf:resource="&soma;Containment"/>
                </owl:Restriction>
              </owl:allValuesFrom>
              <owl:onProperty rdf:resource="&dul;classifies"/>
            </owl:Restriction>
          </owl:intersectionOf>
        </owl:Class>
      </owl:someValuesFrom>
    </owl:Restriction>
  </rdfs:subClassOf>
  <rdfs:subClassOf rdf:resource="&soma;FunctionalControl"/>
  <rdfs:comment>Classifies States in which an object is kept inside another object.</rdfs:comment>
  <rdfs:isDefinedBy rdf:resource="http://www.ease-crc.org/ont/SOMA-STATE.owl"/>
  <rdfs:label xml:lang="en">Containment state</rdfs:label>
</owl:Class>

<owl:ObjectProperty rdf:about="http://www.ease-crc.org/ont/SOMA.owl/prevents"
    rdfs:label="prevents">
  <rdfs:comment>A relationship indicating that a situation does or would prevent another from manifesting. Useful for reasoning about planning (what to do to avoid some bad outcome) and failure recovery (what aspects of the world state prevent continuing the plan?).</rdfs:comment>
  <rdfs:domain rdf:resource="&dul;Situation"/>
  <rdfs:isDefinedBy rdf:resource="http://www.ease-crc.org/ont/SOMA-ACT.owl"/>
  <rdfs:range rdf:resource="&dul;Situation"/>
  <rdfs:subPropertyOf rdf:resource="&dul;isSettingFor"/>
</owl:ObjectProperty>

<owl:Class rdf:about="&soma;Variability">
  <rdfs:subClassOf>
    <owl:Restriction>
      <owl:allValuesFrom rdf:resource="&soma;Tool"/>
      <owl:onProperty rdf:resource="&soma;affordsBearer"/>
    </owl:Restriction>
  </rdfs:subClassOf>
  <rdfs:subClassOf>
    <owl:Restriction>
      <owl:allValuesFrom rdf:resource="&soma;AlteredObject"/>
      <owl:onProperty rdf:resource="&soma;affordsTrigger"/>
    </owl:Restriction>
  </rdfs:subClassOf>
  <rdfs:subClassOf rdf:resource="&soma;Disposition"/>
  <rdfs:comment>The disposition of an object (the tool) to change some aspect of others.</rdfs:comment>
  <rdfs:isDefinedBy rdf:resource="http://www.ease-crc.org/ont/SOMA-OBJ.owl"/>
</owl:Class>

<owl:Class rdf:about="&soma;Hand"
    rdfs:comment="A prehensile effector including palm, fingers, and thumb.">
  <rdfs:isDefinedBy rdf:resource="http://www.ease-crc.org/ont/SOMA-OBJ.owl"/>
  <rdfs:subClassOf rdf:resource="&soma;PrehensileEffector"/>
</owl:Class>

<owl:Class rdf:about="&soma;Navigating">
  <rdfs:comment>A task in which an Agent moves through space so as to arrive at some location, follow some path, or increase its distance from some location or other entity. Often, navigation involves finding paths around obstacles and forbidden areas.</rdfs:comment>
  <rdfs:isDefinedBy rdf:resource="http://www.ease-crc.org/ont/SOMA-ACT.owl"/>
  <rdfs:subClassOf rdf:resource="&soma;PhysicalTask"/>
</owl:Class>

<owl:ObjectProperty rdf:about="&soma;during"
    soma:symbol="d">
  <rdfs:subPropertyOf rdf:resource="&soma;coOccurs"/>
  <rdfs:subPropertyOf rdf:resource="&soma;isContainedIn"/>
  <rdf:type rdf:resource="&owl;TransitiveProperty"/>
  <rdfs:comment>`A during B` means that B strictly starts before, and ends after A, i.e. A is wholly contained in B.</rdfs:comment>
  <rdfs:domain rdf:resource="&dul;Event"/>
  <rdfs:isDefinedBy rdf:resource="http://www.ease-crc.org/ont/SOMA.owl"/>
  <rdfs:range rdf:resource="&dul;Event"/>
</owl:ObjectProperty>

<owl:Class rdf:about="&soma;CanCut">
  <rdfs:subClassOf>
    <owl:Restriction>
      <owl:allValuesFrom rdf:resource="&soma;Cutter"/>
      <owl:onProperty rdf:resource="&soma;affordsBearer"/>
    </owl:Restriction>
  </rdfs:subClassOf>
  <rdfs:subClassOf>
    <owl:Restriction>
      <owl:allValuesFrom rdf:resource="&soma;CutObject"/>
      <owl:onProperty rdf:resource="&soma;affordsTrigger"/>
    </owl:Restriction>
  </rdfs:subClassOf>
  <rdfs:subClassOf rdf:resource="&soma;Variability"/>
  <rdfs:comment>The disposition of an object (the tool) to cut other objects. Such as a knife has cutting ability to cut a cucumber into pieces.</rdfs:comment>
  <rdfs:isDefinedBy rdf:resource="http://www.ease-crc.org/ont/SOMA-OBJ.owl"/>
</owl:Class>

<owl:Class rdf:about="&soma;QueryingTask">
  <rdfs:subClassOf>
    <owl:Restriction>
      <owl:onProperty rdf:resource="&dul;isTaskOf"/>
      <owl:someValuesFrom rdf:resource="&soma;Query"/>
    </owl:Restriction>
  </rdfs:subClassOf>
  <rdfs:subClassOf>
    <owl:Restriction>
      <owl:allValuesFrom>
        <owl:Restriction>
          <owl:onProperty rdf:resource="&dul;hasParticipant"/>
          <owl:someValuesFrom rdf:resource="&soma;InterrogativeClause"/>
        </owl:Restriction>
      </owl:allValuesFrom>
      <owl:onProperty rdf:resource="&dul;classifies"/>
    </owl:Restriction>
  </rdfs:subClassOf>
  <rdfs:subClassOf rdf:resource="&soma;IllocutionaryTask"/>
  <rdfs:comment>An Illocutionary act where the Sender of the Message does so to trigger the Receiver to return some information that is specified within the content of the Message.</rdfs:comment>
  <rdfs:isDefinedBy rdf:resource="http://www.ease-crc.org/ont/SOMA-ACT.owl"/>
  <rdfs:label xml:lang="en">Querying task</rdfs:label>
</owl:Class>

<owl:Class rdf:about="&soma;Motion">
  <rdfs:comment>An EventType that classifies motion Processes.</rdfs:comment>
  <rdfs:comment>Motion type</rdfs:comment>
  <rdfs:isDefinedBy rdf:resource="http://www.ease-crc.org/ont/SOMA-PROC.owl"/>
  <rdfs:subClassOf rdf:resource="&soma;ProcessType"/>
</owl:Class>

<owl:Class rdf:about="&soma;PushingAway">
  <rdfs:comment>A task in which an Agent pushes an object in front of themselves.</rdfs:comment>
  <rdfs:isDefinedBy rdf:resource="http://www.ease-crc.org/ont/SOMA-ACT.owl"/>
  <rdfs:label xml:lang="en">Pushing away</rdfs:label>
  <rdfs:subClassOf rdf:resource="&soma;Pushing"/>
  <owl:disjointWith rdf:resource="&soma;PushingDown"/>
</owl:Class>

<owl:Class rdf:about="&soma;ExecutableSchematicTheory">
  <rdfs:subClassOf>
    <owl:Restriction>
      <owl:onProperty rdf:resource="&dul;defines"/>
      <owl:someValuesFrom rdf:resource="&soma;PerformerRole"/>
    </owl:Restriction>
  </rdfs:subClassOf>
  <rdfs:subClassOf rdf:resource="&soma;SchematicTheory"/>
  <rdfs:comment>Also known as "executing schemas" or "x-schemas", these were defined by Bergen and Chang in their work "Embodied Construction Grammar in Simulation-Based Language Understanding" as:

"Executing schemas, or x-schemas, are dynamic representations motivated in part by motor and perceptual systems (Bailey 1997; Narayanan 1997), on the assumption that the same underlying representations used for executing and perceiving an action are brought to bear in understanding language about that action. The x-schema formalism is an extension of Petri nets (Murata 1989) that can model sequential, concurrent, and
asynchronous events"

SOMA does not restrict the formalism of ExecutableSchematicTheories; i.e. they don't have to be Petri Nets.

They maintain their role however as representations able to drive a simulation, at some level of abstraction, of an embodied action. This level of abstraction may be still fairly underspecified as in the case of the original x-schemas and as such not a plan that an agent could run in an actual physical environment without further information.</rdfs:comment>
  <rdfs:isDefinedBy rdf:resource="http://www.ease-crc.org/ont/SOMA-SAY.owl"/>
  <rdfs:label xml:lang="en">Executable schematic theory</rdfs:label>
</owl:Class>

<owl:ObjectProperty rdf:about="&soma;directlyCauses">
  <rdfs:comment xml:lang="en">Non-transitive version of "causes".</rdfs:comment>
  <rdfs:domain rdf:resource="&dul;Event"/>
  <rdfs:isDefinedBy rdf:resource="http://www.ease-crc.org/ont/SOMA-ACT.owl"/>
  <rdfs:label xml:lang="en">directly causes</rdfs:label>
  <rdfs:range rdf:resource="&dul;Event"/>
  <rdfs:subPropertyOf rdf:resource="&soma;causes"/>
  <owl:inverseOf rdf:resource="&soma;isDirectReactionTo"/>
  <owl:propertyChainAxiom rdf:parseType="Collection">
    <rdf:Description rdf:about="&soma;causesTransition"/>
    <rdf:Description rdf:about="&soma;hasTerminalScene"/>
    <rdf:Description rdf:about="&dul;includesEvent"/>
  </owl:propertyChainAxiom>
</owl:ObjectProperty>

<owl:ObjectProperty rdf:about="&soma;describesQuality"
    rdfs:comment="Relates a description to a quality that it describes."
    rdfs:label="describes quality">
  <rdfs:domain rdf:resource="&dul;Description"/>
  <rdfs:isDefinedBy rdf:resource="http://www.ease-crc.org/ont/SOMA-OBJ.owl"/>
  <rdfs:range rdf:resource="&dul;Quality"/>
  <rdfs:subPropertyOf rdf:resource="&dul;describes"/>
  <owl:inverseOf rdf:resource="&soma;isQualityDescribedBy"/>
</owl:ObjectProperty>

<soma:Object rdf:about="object1">
  <soma:material rdf:datatype="&xsd;string">cardboard</soma:material>
  <soma:texture rdf:datatype="&xsd;string">smooth</soma:texture>
  <soma:type rdf:datatype="&xsd;string">box of Cheez-It crackers</soma:type>
</soma:Object>

<owl:Class rdf:about="&soma;StateTransition">
  <rdfs:isDefinedBy rdf:resource="http://www.ease-crc.org/ont/SOMA-SAY.owl"/>
  <rdfs:isDefinedBy rdf:resource="http://www.ease-crc.org/ont/SOMA.owl"/>
  <rdfs:subClassOf>
    <owl:Restriction>
      <owl:onProperty rdf:resource="&soma;hasInitialScene"/>
      <owl:someValuesFrom rdf:resource="&soma;Scene"/>
    </owl:Restriction>
  </rdfs:subClassOf>
  <rdfs:subClassOf>
    <owl:Restriction>
      <owl:onProperty rdf:resource="&soma;hasTerminalScene"/>
      <owl:someValuesFrom rdf:resource="&soma;Scene"/>
    </owl:Restriction>
  </rdfs:subClassOf>
  <rdfs:subClassOf>
    <owl:Restriction>
      <owl:onProperty rdf:resource="&dul;includesEvent"/>
      <owl:someValuesFrom rdf:resource="&dul;Action"/>
    </owl:Restriction>
  </rdfs:subClassOf>
  <rdfs:subClassOf>
    <owl:Restriction>
      <owl:onProperty rdf:resource="&dul;satisfies"/>
      <owl:someValuesFrom rdf:resource="&soma;ImageSchemaTheory"/>
    </owl:Restriction>
  </rdfs:subClassOf>
  <rdfs:subClassOf rdf:resource="&dul;Transition"/>
  <rdfs:comment>A transition between two states brought about by the Action of some Agent.</rdfs:comment>
  <rdfs:label xml:lang="en">State transition</rdfs:label>
</owl:Class>

<owl:Class rdf:about="&soma;HostRole">
  <rdfs:subClassOf>
    <owl:Restriction>
      <owl:onProperty rdf:resource="&dul;isDefinedIn"/>
      <owl:someValuesFrom rdf:resource="&soma;PluginSpecification"/>
    </owl:Restriction>
  </rdfs:subClassOf>
  <rdfs:subClassOf rdf:resource="&soma;InterfaceComponentRole"/>
  <rdfs:comment xml:lang="en">In the Plug-in-Host pattern, a Host application provides services which the Plug-in can use, including a way for Plug-ins to register themselves with the Host application and a protocol for the exchange of data withPplug-ins. Plug-ins depend on the services provided by the host application and do not usually work by themselves. Conversely, the host application operates independently of the plug-ins, making it possible for end-users to add and update plug-ins dynamically without needing to make changes to the host application.

Source: https://en.wikipedia.org/wiki/Plug-in_(computing)</rdfs:comment>
  <rdfs:isDefinedBy rdf:resource="http://www.ease-crc.org/ont/SOMA-IO.owl"/>
  <rdfs:label xml:lang="en">Host role</rdfs:label>
</owl:Class>

<owl:Class rdf:about="&soma;Fluid">
  <rdfs:isDefinedBy rdf:resource="http://www.ease-crc.org/ont/SOMA-PROC.owl"/>
  <rdfs:isDefinedBy rdf:resource="http://www.ease-crc.org/ont/SOMA.owl"/>
  <rdfs:comment>A substance with a consistency such that it can flow or diffuse.</rdfs:comment>
  <rdfs:subClassOf rdf:resource="&dul;Substance"/>
</owl:Class>

<owl:Class rdf:about="&soma;Lifting"
    rdfs:comment="todo: how to distinguish from e.g. 'pushing from the table'">
  <owl:disjointWith rdf:resource="&soma;Opening"/>
  <owl:disjointWith rdf:resource="&soma;Pulling"/>
  <owl:disjointWith rdf:resource="&soma;Pushing"/>
  <owl:disjointWith rdf:resource="&soma;Squeezing"/>
  <rdfs:isDefinedBy rdf:resource="http://www.ease-crc.org/ont/SOMA-ACT.owl"/>
  <rdfs:subClassOf rdf:resource="&soma;Actuating"/>
</owl:Class>

<owl:Class rdf:about="&dul;Design">
  <rdfs:isDefinedBy rdf:resource="http://www.ease-crc.org/ont/SOMA-OBJ.owl"/>
</owl:Class>

<owl:Class rdf:about="&soma;Storage">
  <rdfs:subClassOf>
    <owl:Restriction>
      <owl:allValuesFrom rdf:resource="&soma;StoredObject"/>
      <owl:onProperty rdf:resource="&soma;affordsTrigger"/>
    </owl:Restriction>
  </rdfs:subClassOf>
  <rdfs:subClassOf rdf:resource="&soma;Enclosing"/>
  <rdfs:comment>The disposition of an object (the container) to store other objects. Storage of an object would facilitate several objectives; such as to store objects in a safe or usual place, to prevent the substances e.g. prevention of milk going bad by storing them in a refrigrator.</rdfs:comment>
  <rdfs:isDefinedBy rdf:resource="http://www.ease-crc.org/ont/SOMA-OBJ.owl"/>
</owl:Class>

<owl:ObjectProperty rdf:about="&soma;isEffectorInvolvedIn"
    rdfs:comment="Effector participation."
    rdfs:label="is effector involved in">
  <rdfs:domain rdf:resource="&soma;PhysicalEffector"/>
  <rdfs:isDefinedBy rdf:resource="http://www.ease-crc.org/ont/SOMA-OBJ.owl"/>
  <rdfs:range rdf:resource="&dul;Event"/>
  <rdfs:subPropertyOf rdf:resource="&dul;isParticipantIn"/>
</owl:ObjectProperty>

<owl:Class rdf:about="&soma;SoftwareDiagnosis"
    rdfs:comment="A diagnosis of the software of a system."
    rdfs:label="Software diagnosis">
  <rdfs:isDefinedBy rdf:resource="http://www.ease-crc.org/ont/SOMA.owl"/>
  <rdfs:subClassOf rdf:resource="&soma;TechnicalDiagnosis"/>
</owl:Class>

<owl:Class rdf:about="&soma;PreferenceRegion">
  <rdfs:subClassOf>
    <owl:Restriction>
      <owl:onProperty rdf:resource="&dul;isRegionFor"/>
      <owl:someValuesFrom rdf:resource="&soma;Preference"/>
    </owl:Restriction>
  </rdfs:subClassOf>
  <rdfs:subClassOf rdf:resource="&dul;SocialObjectAttribute"/>
  <rdfs:comment xml:lang="en">The 'Region' of 'Preference's, containing all possible 'Order's between all possible 'Situation's.</rdfs:comment>
  <rdfs:isDefinedBy rdf:resource="http://www.ease-crc.org/ont/SOMA-AGENT.owl"/>
  <rdfs:label xml:lang="en">Preference region</rdfs:label>
</owl:Class>

<owl:DatatypeProperty rdf:about="&soma;hasIntervalTime"
    rdfs:label="has interval time">
  <rdfs:comment>Superproperty of relations used to connect moments in time to a TimeInterval.</rdfs:comment>
  <rdfs:domain rdf:resource="&dul;TimeInterval"/>
  <rdfs:isDefinedBy rdf:resource="http://www.ease-crc.org/ont/SOMA.owl"/>
  <rdfs:range rdf:resource="&xsd;float"/>
  <rdfs:subPropertyOf rdf:resource="&dul;hasRegionDataValue"/>
</owl:DatatypeProperty>

<owl:ObjectProperty rdf:about="&soma;finishedBy"
    soma:symbol="fi">
  <rdf:type rdf:resource="&owl;TransitiveProperty"/>
  <rdfs:comment>`A finishes B` means that A ends exactly where B ends, and that B strictly starts before A.  As in "I finish my day by taking a shower".</rdfs:comment>
  <rdfs:domain rdf:resource="&dul;Event"/>
  <rdfs:isDefinedBy rdf:resource="http://www.ease-crc.org/ont/SOMA.owl"/>
  <rdfs:label xml:lang="en">finished by</rdfs:label>
  <rdfs:range rdf:resource="&dul;Event"/>
  <rdfs:subPropertyOf rdf:resource="&soma;coOccurs"/>
  <owl:inverseOf rdf:resource="&soma;finishes"/>
</owl:ObjectProperty>

<owl:ObjectProperty rdf:about="&soma;derivedFrom"
    rdfs:label="derived from">
  <rdf:type rdf:resource="&owl;TransitiveProperty"/>
  <rdfs:comment>The (transitive) relation between an information object and another which it has been derived from.</rdfs:comment>
  <rdfs:domain rdf:resource="&dul;InformationObject"/>
  <rdfs:isDefinedBy rdf:resource="http://www.ease-crc.org/ont/SOMA.owl"/>
  <rdfs:range rdf:resource="&dul;InformationObject"/>
  <rdfs:subPropertyOf rdf:resource="&dul;associatedWith"/>
  <owl:inverseOf rdf:resource="&soma;isSourceFor"/>
</owl:ObjectProperty>

<owl:ObjectProperty rdf:about="&soma;givesMeaningTo">
  <rdfs:comment xml:lang="en">The relation between a System and Information Object that is given meaning to by said system, e.g., a Language might give meaning to some word, sentence, text, etc., but without the knowledge of said System (Language), the text will not make sense to a reader.</rdfs:comment>
  <rdfs:domain rdf:resource="&soma;System"/>
  <rdfs:isDefinedBy rdf:resource="http://www.ease-crc.org/ont/SOMA-IO.owl"/>
  <rdfs:label xml:lang="en">gives meaning to</rdfs:label>
  <rdfs:range rdf:resource="&dul;InformationObject"/>
  <rdfs:subPropertyOf rdf:resource="&dul;associatedWith"/>
  <owl:inverseOf rdf:resource="&soma;isGivenMeaningBy"/>
</owl:ObjectProperty>

<owl:DatatypeProperty rdf:about="&soma;hasDepth"
    rdfs:comment="The depth of a shape."
    rdfs:label="has depth">
  <rdfs:domain rdf:resource="&soma;ShapeRegion"/>
  <rdfs:isDefinedBy rdf:resource="http://www.ease-crc.org/ont/SOMA-OBJ.owl"/>
  <rdfs:range rdf:resource="&xsd;float"/>
  <rdfs:subPropertyOf rdf:resource="&soma;hasShapeParameter"/>
</owl:DatatypeProperty>

<soma:StatusFailure rdf:about="&soma;FailWFNoContinuation">
  <rdf:type rdf:resource="&owl;NamedIndividual"/>
  <rdfs:comment>A particular kind of failure: the workflow fails because there is no way to continue it, and the normal exit has not been reached.</rdfs:comment>
  <rdfs:isDefinedBy rdf:resource="http://www.ease-crc.org/ont/SOMA-WF.owl"/>
</soma:StatusFailure>

<owl:ObjectProperty rdf:about="&soma;hasOutputParameter"
    rdfs:label="has output parameter">
  <rdfs:comment>A relation between a Task and one of its output parameters.</rdfs:comment>
  <rdfs:comment>A relation from an EventType (typically a Task) to a Parameter describing an outcome of the event classified by the EventType.</rdfs:comment>
  <rdfs:domain rdf:resource="&dul;EventType"/>
  <rdfs:isDefinedBy rdf:resource="http://www.ease-crc.org/ont/SOMA.owl"/>
  <rdfs:range rdf:resource="&dul;Parameter"/>
  <rdfs:subPropertyOf rdf:resource="&dul;hasParameter"/>
  <owl:inverseOf rdf:resource="&soma;isOutputParameterFor"/>
</owl:ObjectProperty>

<owl:ObjectProperty rdf:about="&soma;isInitialStateOf"
    rdfs:label="is initial state of">
  <rdfs:comment>A relation recording that a Situation was where a Transition began.</rdfs:comment>
  <rdfs:domain rdf:resource="&dul;Situation"/>
  <rdfs:isDefinedBy rdf:resource="http://www.ease-crc.org/ont/SOMA.owl"/>
  <rdfs:range rdf:resource="&dul;Transition"/>
  <rdfs:subPropertyOf rdf:resource="&soma;isSituationIncludedIn"/>
</owl:ObjectProperty>

<owl:ObjectProperty rdf:about="&soma;affordanceDefines"
    rdfs:label="affordance defines">
  <rdfs:comment>A relation between an Affordance and a Concept (often an EventType).</rdfs:comment>
  <rdfs:domain rdf:resource="&soma;Affordance"/>
  <rdfs:isDefinedBy rdf:resource="http://www.ease-crc.org/ont/SOMA-OBJ.owl"/>
  <rdfs:range rdf:resource="&dul;Concept"/>
  <rdfs:subPropertyOf rdf:resource="&dul;defines"/>
  <owl:inverseOf rdf:resource="&soma;isDefinedInAffordance"/>
</owl:ObjectProperty>

<owl:Class rdf:about="&dul;Goal"/>

<owl:Class rdf:about="&soma;Positioning">
  <rdfs:comment>A task in which an Agent places an object at a particular position.</rdfs:comment>
  <rdfs:isDefinedBy rdf:resource="http://www.ease-crc.org/ont/SOMA-ACT.owl"/>
  <rdfs:subClassOf rdf:resource="&soma;Actuating"/>
</owl:Class>

<owl:Class rdf:about="&soma;RedColor"
    rdfs:comment="A color region with dominant red color."
    rdfs:label="Red color">
  <rdfs:isDefinedBy rdf:resource="http://www.ease-crc.org/ont/SOMA-OBJ.owl"/>
  <rdfs:subClassOf rdf:resource="&soma;ColorRegion"/>
</owl:Class>

<owl:Class rdf:about="&soma;ControlTheory">
  <rdfs:comment>A description of functional-spatial configurations where one object controls another object's position in space, e.g. if a pot moves, then the popcorn contained therein moves, as well. Note that the objects do not need to be in direct contact.

Adopted from GUM-4-space (Bateman et al. 2010).</rdfs:comment>
  <rdfs:isDefinedBy rdf:resource="http://www.ease-crc.org/ont/SOMA-SAY.owl"/>
  <rdfs:label xml:lang="en">Control theory</rdfs:label>
  <rdfs:subClassOf rdf:resource="&soma;FunctionalSpatialSchemaTheory"/>
</owl:Class>

<owl:Class rdf:about="&soma;Order">
  <rdfs:subClassOf>
    <owl:Restriction>
      <owl:onProperty rdf:resource="&soma;orders"/>
      <owl:someValuesFrom rdf:resource="&soma;OrderedElement"/>
    </owl:Restriction>
  </rdfs:subClassOf>
  <rdfs:subClassOf rdf:resource="&dul;FormalEntity"/>
  <rdfs:comment xml:lang="en">An 'Order' sorts two or more 'Order item's via the relations 'precedes' and 'follows'.</rdfs:comment>
  <rdfs:isDefinedBy rdf:resource="http://www.ease-crc.org/ont/SOMA-AGENT.owl"/>
  <rdfs:label xml:lang="en">Order</rdfs:label>
</owl:Class>

<owl:ObjectProperty rdf:about="&soma;isDirectSourceFor"
    rdfs:label="is direct source for">
  <rdfs:comment>The (transitive) relation between an information object and another which was derived from the former.</rdfs:comment>
  <rdfs:isDefinedBy rdf:resource="http://www.ease-crc.org/ont/SOMA.owl"/>
  <rdfs:subPropertyOf rdf:resource="&soma;isSourceFor"/>
  <owl:propertyChainAxiom rdf:parseType="Collection">
    <rdf:Description rdf:about="&dul;isRealizedBy"/>
    <rdf:Description rdf:about="&dul;hasRole"/>
    <rdf:Description rdf:about="&soma;isInputRoleOf"/>
    <rdf:Description rdf:about="&soma;isTaskOfCreatedRole"/>
    <rdf:Description rdf:about="&dul;isRoleOf"/>
    <rdf:Description rdf:about="&dul;realizes"/>
  </owl:propertyChainAxiom>
</owl:ObjectProperty>

<owl:Class rdf:about="&dul;SocialAgent"/>

<owl:Class rdf:about="&dul;PhysicalArtifact">
  <rdfs:isDefinedBy rdf:resource="http://www.ease-crc.org/ont/SOMA-PROC.owl"/>
</owl:Class>

<owl:Class rdf:about="&soma;Purification">
  <rdfs:subClassOf>
    <owl:Restriction>
      <owl:allValuesFrom>
        <owl:Restriction>
          <owl:allValuesFrom>
            <owl:Class>
              <owl:intersectionOf rdf:parseType="Collection">
                <rdf:Description rdf:about="&soma;Clean"/>
                <owl:Restriction>
                  <owl:allValuesFrom rdf:resource="&soma;Cleanliness"/>
                  <owl:onProperty rdf:resource="&dul;isRegionFor"/>
                </owl:Restriction>
              </owl:intersectionOf>
            </owl:Class>
          </owl:allValuesFrom>
          <owl:onProperty rdf:resource="&dul;classifies"/>
        </owl:Restriction>
      </owl:allValuesFrom>
      <owl:onProperty rdf:resource="&soma;affordsSetpoint"/>
    </owl:Restriction>
  </rdfs:subClassOf>
  <rdfs:subClassOf>
    <owl:Restriction>
      <owl:allValuesFrom>
        <owl:Restriction>
          <owl:allValuesFrom rdf:resource="&dul;PhysicalObject"/>
          <owl:onProperty rdf:resource="&dul;classifies"/>
        </owl:Restriction>
      </owl:allValuesFrom>
      <owl:onProperty rdf:resource="&soma;affordsTrigger"/>
    </owl:Restriction>
  </rdfs:subClassOf>
  <rdfs:subClassOf rdf:resource="&soma;Variability"/>
  <rdfs:comment>The disposition of an object (the tool) to change the cleanliness of others.</rdfs:comment>
  <rdfs:isDefinedBy rdf:resource="http://www.ease-crc.org/ont/SOMA-OBJ.owl"/>
</owl:Class>

<owl:DatatypeProperty rdf:about="&soma;hasJointEffort"
    rdfs:label="has joint effort">
  <rdfs:comment>The effort applied in a joint given in N (prismatic joint) or N*m (hinged joints).</rdfs:comment>
  <rdfs:domain rdf:resource="&soma;JointState"/>
  <rdfs:isDefinedBy rdf:resource="http://www.ease-crc.org/ont/SOMA-OBJ.owl"/>
  <rdfs:range rdf:resource="&xsd;double"/>
  <rdfs:subPropertyOf rdf:resource="&soma;hasJointParameter"/>
</owl:DatatypeProperty>

<owl:ObjectProperty rdf:about="&soma;isDesignFor">
  <rdfs:comment xml:lang="en">A special relation between a Design and an Object, to indicate that the Design describes a way to construct the Object.</rdfs:comment>
  <rdfs:domain rdf:resource="&dul;Design"/>
  <rdfs:isDefinedBy rdf:resource="http://www.ease-crc.org/ont/SOMA-IO.owl"/>
  <rdfs:label xml:lang="en">is design for</rdfs:label>
  <rdfs:range rdf:resource="&dul;Object"/>
  <rdfs:subPropertyOf rdf:resource="&dul;describes"/>
  <owl:inverseOf rdf:resource="&soma;isDesignedBy"/>
</owl:ObjectProperty>

<owl:Class rdf:about="&soma;Amateurish"
    rdfs:comment="A description of amateurish behavior.">
  <rdfs:isDefinedBy rdf:resource="http://www.ease-crc.org/ont/SOMA.owl"/>
  <rdfs:subClassOf rdf:resource="&soma;DexterityDiagnosis"/>
  <owl:disjointWith rdf:resource="&soma;Masterful"/>
</owl:Class>

<owl:DatatypeProperty rdf:about="&soma;hasJointEffortLimit"
    rdfs:label="has joint effort limit">
  <rdfs:comment>The maximum effort applied in a joint given in N (prismatic joint) or N*m (hinged joints).</rdfs:comment>
  <rdfs:domain rdf:resource="&soma;JointLimit"/>
  <rdfs:isDefinedBy rdf:resource="http://www.ease-crc.org/ont/SOMA-OBJ.owl"/>
  <rdfs:range rdf:resource="&xsd;double"/>
  <rdfs:subPropertyOf rdf:resource="&soma;hasJointParameter"/>
</owl:DatatypeProperty>

<owl:Class rdf:about="&soma;Antagonist">
  <rdfs:comment>A role that classifies entities that are opposed to the tendency of some agonist.</rdfs:comment>
  <rdfs:isDefinedBy rdf:resource="http://www.ease-crc.org/ont/SOMA-PROC.owl"/>
  <rdfs:subClassOf rdf:resource="&soma;Patient"/>
</owl:Class>

<owl:Class rdf:about="&soma;State">
  <rdfs:isDefinedBy rdf:resource="http://www.ease-crc.org/ont/SOMA-SAY.owl"/>
  <rdfs:isDefinedBy rdf:resource="http://www.ease-crc.org/ont/SOMA.owl"/>
  <rdfs:comment>States are stative and homeomeric events.

For stative events, the mereological sum of two instances has the same type as both instances. This is, for example, the state of sitting on a chair, or the process of a pendulum swinging around.

The difference between states and processes is that states are, in addition, homeomeric, and processes are not.  This means that, when considering time slices  of an event, for states, these time slices always have the same type as the state, but for processes this is not the case.</rdfs:comment>
  <rdfs:subClassOf rdf:resource="&dul;Event"/>
</owl:Class>

<owl:Class rdf:about="&soma;ESTSchemaTheory">
  <rdfs:subClassOf>
    <owl:Restriction>
      <owl:onProperty rdf:resource="&dul;defines"/>
      <owl:someValuesFrom rdf:resource="&soma;ExistingObjectRole"/>
    </owl:Restriction>
  </rdfs:subClassOf>
  <rdfs:subClassOf>
    <owl:Restriction>
      <owl:cardinality rdf:datatype="&xsd;nonNegativeInteger">1</owl:cardinality>
      <owl:onProperty rdf:resource="&dul;defines"/>
    </owl:Restriction>
  </rdfs:subClassOf>
  <rdfs:subClassOf rdf:resource="&soma;ImageSchemaTheory"/>
  <rdfs:comment>A schematic theory that describes the existence of an entity.

Developmental psychology posits that "object permanence" (the assumption that physical objects keep existing even when the agent doesn't perceive them, which consequently informs reasoning about where an object should be, even when perception of it is lost) is a cognitive ability that is not, at least in the very young human child, immediately manifest. Rather, it seems learned via interaction, and usually is among an infant's cognitive repertoire by age 2.

In SOMA, we represent this ability of a cognitive agent as an ability to generate and maintain ESTSchemaTheories. Each instance of such a theory refers to one particular physical object, the one that the instance of the ESTSchemaTheory asserts to exist.

Because each instance of an ESTSchemaTheory refers to a single object, ESTSchemaTheories are not associated to any relation between OWL individuals.</rdfs:comment>
  <rdfs:isDefinedBy rdf:resource="http://www.ease-crc.org/ont/SOMA-SAY.owl"/>
  <rdfs:label xml:lang="en">EST schema theory</rdfs:label>
</owl:Class>

<owl:Class rdf:about="&soma;FormalLanguage">
  <rdfs:subClassOf>
    <owl:Restriction>
      <owl:allValuesFrom rdf:resource="&soma;Structured_Text"/>
      <owl:onProperty rdf:resource="&soma;givesMeaningTo"/>
    </owl:Restriction>
  </rdfs:subClassOf>
  <rdfs:subClassOf rdf:resource="&soma;Language"/>
  <rdfs:comment xml:lang="en">A Formal Language consists of words whose letters are taken from an alphabet and are well-formed according to a specific set of rules.

From Wikipedia: https://en.wikipedia.org/wiki/Formal_language</rdfs:comment>
  <rdfs:isDefinedBy rdf:resource="http://www.ease-crc.org/ont/SOMA-IO.owl"/>
  <rdfs:label xml:lang="en">Formal Language</rdfs:label>
</owl:Class>

<owl:Class rdf:about="&soma;JointLimit"
    rdfs:comment="The physical limits of a joint."
    rdfs:label="Joint limit">
  <rdfs:isDefinedBy rdf:resource="http://www.ease-crc.org/ont/SOMA-OBJ.owl"/>
  <rdfs:subClassOf rdf:resource="&dul;PhysicalAttribute"/>
</owl:Class>

<owl:Class rdf:about="&dul;Substance">
  <rdfs:isDefinedBy rdf:resource="http://www.ease-crc.org/ont/SOMA-PROC.owl"/>
</owl:Class>

<owl:Class rdf:about="&soma;CommitedObject">
  <rdfs:comment>An object committed to a bigger whole. After being committed, the object does not exist anymore in its old form.</rdfs:comment>
  <rdfs:isDefinedBy rdf:resource="http://www.ease-crc.org/ont/SOMA-OBJ.owl"/>
  <rdfs:label xml:lang="en">Commited object</rdfs:label>
  <rdfs:subClassOf rdf:resource="&soma;ConnectedObject"/>
</owl:Class>

<owl:ObjectProperty rdf:about="&soma;hasPreviousStep"
    rdfs:label="has previous step">
  <rdfs:comment>An ordering relation between tasks in some workflow, stating that a task is preceded by another.</rdfs:comment>
  <rdfs:domain rdf:resource="&dul;Task"/>
  <rdfs:isDefinedBy rdf:resource="http://www.ease-crc.org/ont/SOMA-WF.owl"/>
  <rdfs:range rdf:resource="&dul;Task"/>
  <rdfs:subPropertyOf rdf:resource="&dul;directlyFollows"/>
</owl:ObjectProperty>

<owl:DatatypeProperty rdf:about="&soma;hasJointPosition"
    rdfs:label="has joint position">
  <rdfs:comment>The position of a joint given in m (prismatic joints) or rad (hinged joints).</rdfs:comment>
  <rdfs:domain rdf:resource="&soma;JointState"/>
  <rdfs:isDefinedBy rdf:resource="http://www.ease-crc.org/ont/SOMA-OBJ.owl"/>
  <rdfs:range rdf:resource="&xsd;double"/>
  <rdfs:subPropertyOf rdf:resource="&soma;hasJointParameter"/>
</owl:DatatypeProperty>

<owl:Class rdf:about="&soma;ThinkAloudPlanTopic"
    rdfs:label="Think aloud plan topic">
  <rdfs:comment>A topic used when an Agent describes what they intend to do. Note, this is not about describing the process through which this plan was constructed; that is covered by the MetaCognitionPlanningTopic.</rdfs:comment>
  <rdfs:isDefinedBy rdf:resource="http://www.ease-crc.org/ont/SOMA-ACT.owl"/>
  <rdfs:subClassOf rdf:resource="&soma;ThinkAloudTopic"/>
</owl:Class>

<owl:Class rdf:about="&soma;SelfReflection">
  <rdfs:label>Self-reflection</rdfs:label>
  <rdfs:label>The task of evaluating the personal cognitive processes.</rdfs:label>
  <rdfs:isDefinedBy rdf:resource="http://www.ease-crc.org/ont/SOMA-ACT.owl"/>
  <rdfs:subClassOf rdf:resource="&soma;MetacognitiveControlling"/>
</owl:Class>

<owl:DatatypeProperty rdf:about="&soma;hasDataFormat">
  <rdfs:comment>A property linking an InformationRealization to a string specifying a format name, e.g. URDF or STL.</rdfs:comment>
  <rdfs:domain rdf:resource="&dul;InformationRealization"/>
  <rdfs:isDefinedBy rdf:resource="http://www.ease-crc.org/ont/SOMA.owl"/>
  <rdfs:range rdf:resource="&xsd;string"/>
  <rdfs:subPropertyOf rdf:resource="&dul;hasDataValue"/>
</owl:DatatypeProperty>

<owl:ObjectProperty rdf:about="http://www.ease-crc.org/ont/SOMA.owl/manifestsIn"
    rdfs:label="manifests in">
  <rdfs:comment>A relationship indicating that a Situation is realized in an Event that actually happened.</rdfs:comment>
  <rdfs:isDefinedBy rdf:resource="http://www.ease-crc.org/ont/SOMA-ACT.owl"/>
  <rdfs:subPropertyOf rdf:resource="&dul;includesEvent"/>
</owl:ObjectProperty>

<owl:Class rdf:about="&soma;Arranging">
  <rdfs:comment>A task in which an Agent places a collection of objects at some set of relative poses to each other.</rdfs:comment>
  <rdfs:isDefinedBy rdf:resource="http://www.ease-crc.org/ont/SOMA-ACT.owl"/>
  <rdfs:subClassOf rdf:resource="&soma;Constructing"/>
</owl:Class>

<owl:Class rdf:about="&soma;KineticFrictionAttribute"
    rdfs:label="Kinetic friction attribute">
  <rdfs:comment>Friction that occurs when two touching objects are moving relative to each other.</rdfs:comment>
  <rdfs:isDefinedBy rdf:resource="http://www.ease-crc.org/ont/SOMA-OBJ.owl"/>
  <rdfs:subClassOf rdf:resource="&soma;FrictionAttribute"/>
</owl:Class>

<owl:Class rdf:about="&soma;ReleasingMotion"
    rdfs:label="Releasing motion">
  <rdfs:comment>A motion by which a prehensile effector relinquishes kinematic control over an object.</rdfs:comment>
  <rdfs:isDefinedBy rdf:resource="http://www.ease-crc.org/ont/SOMA-PROC.owl"/>
  <rdfs:subClassOf rdf:resource="&soma;PrehensileMotion"/>
</owl:Class>

<owl:Class rdf:about="&soma;PhysicalTask">
  <rdfs:subClassOf>
    <owl:Restriction>
      <owl:allValuesFrom>
        <owl:Class>
          <owl:intersectionOf rdf:parseType="Collection">
            <rdf:Description rdf:about="&dul;Action"/>
            <owl:Class>
              <owl:unionOf rdf:parseType="Collection">

                <owl:Restriction>
                  <owl:onProperty rdf:resource="&dul;hasParticipant"/>
                  <owl:someValuesFrom rdf:resource="&dul;PhysicalAgent"/>
                </owl:Restriction>

                <owl:Restriction>
                  <owl:onProperty rdf:resource="&dul;hasParticipant"/>
                  <owl:someValuesFrom rdf:resource="&dul;PhysicalObject"/>
                </owl:Restriction>
              </owl:unionOf>
            </owl:Class>
          </owl:intersectionOf>
        </owl:Class>
      </owl:allValuesFrom>
      <owl:onProperty rdf:resource="&dul;classifies"/>
    </owl:Restriction>
  </rdfs:subClassOf>
  <rdfs:subClassOf rdf:resource="&dul;Task"/>
  <rdfs:comment>A task in which a PhysicalAgent affects some physical object.</rdfs:comment>
  <rdfs:isDefinedBy rdf:resource="http://www.ease-crc.org/ont/SOMA-ACT.owl"/>
  <rdfs:label xml:lang="en">Physical task</rdfs:label>
</owl:Class>

<owl:ObjectProperty rdf:about="&soma;isTriggerAffordedBy"
    rdfs:label="is trigger afforded by">
  <rdfs:comment>Relates a disposition to the trigger role defined by the affordance describing the disposition.</rdfs:comment>
  <rdfs:domain rdf:resource="&dul;Role"/>
  <rdfs:isDefinedBy rdf:resource="http://www.ease-crc.org/ont/SOMA-OBJ.owl"/>
  <rdfs:range rdf:resource="&soma;Disposition"/>
  <rdfs:subPropertyOf rdf:resource="&soma;isConceptAffordedBy"/>
  <owl:propertyChainAxiom rdf:parseType="Collection">
    <rdf:Description rdf:about="&soma;isTriggerDefinedIn"/>
    <rdf:Description rdf:about="&dul;describes"/>
  </owl:propertyChainAxiom>
</owl:ObjectProperty>

<owl:Class rdf:about="&soma;PouringInto"
    rdfs:label="Pouring into">
  <rdfs:comment>The task in which the agent pours the substance into another object.</rdfs:comment>
  <rdfs:isDefinedBy rdf:resource="http://www.ease-crc.org/ont/SOMA-ACT.owl"/>
  <rdfs:subClassOf rdf:resource="&soma;Pouring"/>
</owl:Class>

<owl:Class rdf:about="&soma;Software">
  <rdfs:label xml:lang="en">Software</rdfs:label>
  <rdfs:label xml:lang="en">We see Software as the Design of a DesignedTool: the running instance of said Software. Software as a design also follows the Function-Behaviour-Structure model:

The Function is the purpose or problem solving embodied by the Software Instance, e.g., sorting a list.

The Behaviour are the algoirthms used by the Software Instance, e.g., Bubble Sort.

The Structure is the organization of files, classes, objects and method calls of the program code.</rdfs:label>
  <rdfs:subClassOf>
    <owl:Restriction>
      <owl:onProperty rdf:resource="&dul;describes"/>
      <owl:someValuesFrom rdf:resource="&soma;Software_Configuration"/>
    </owl:Restriction>
  </rdfs:subClassOf>
  <rdfs:subClassOf>
    <owl:Restriction>
      <owl:allValuesFrom>
        <owl:Class>
          <owl:unionOf rdf:parseType="Collection">
            <rdf:Description rdf:about="&soma;SoftwareInstance"/>
            <rdf:Description rdf:about="&soma;Software_Configuration"/>
          </owl:unionOf>
        </owl:Class>
      </owl:allValuesFrom>
      <owl:onProperty rdf:resource="&dul;describes"/>
    </owl:Restriction>
  </rdfs:subClassOf>
  <rdfs:subClassOf rdf:resource="&dul;Design"/>
  <rdfs:isDefinedBy rdf:resource="http://www.ease-crc.org/ont/SOMA-IO.owl"/>
</owl:Class>

<owl:Class rdf:about="&soma;Restrictor">
  <rdfs:isDefinedBy rdf:resource="http://www.ease-crc.org/ont/SOMA-OBJ.owl"/>
  <rdfs:isDefinedBy rdf:resource="http://www.ease-crc.org/ont/SOMA-STATE.owl"/>
  <rdfs:comment>A role classifying an object used to deny access to some other entity.</rdfs:comment>
  <rdfs:subClassOf rdf:resource="&soma;Instrument"/>
</owl:Class>

<owl:ObjectProperty rdf:about="&soma;isAffectedBy"
    rdfs:label="is affected by">
  <rdfs:comment>Simple relationship between two actions to express that a variation in the course or outcome of the object (the affector) would have resulted in a variation in the subject (the affectee), e.g., a planning task that sets parameters such as goal position affects the subsequently executed pick-and-place task that uses that parameter.</rdfs:comment>
  <rdfs:isDefinedBy rdf:resource="http://www.ease-crc.org/ont/SOMA-ACT.owl"/>
  <rdfs:subPropertyOf rdf:resource="&dul;follows"/>
</owl:ObjectProperty>

<owl:Class rdf:about="&soma;Prospecting">
  <rdfs:comment>A Mental task in which an Agent endeavours to construct a representation of a future state of affairs of the world it is embodied in.</rdfs:comment>
  <rdfs:isDefinedBy rdf:resource="http://www.ease-crc.org/ont/SOMA-ACT.owl"/>
  <rdfs:subClassOf rdf:resource="&soma;DerivingInformation"/>
</owl:Class>

<owl:DatatypeProperty rdf:about="&soma;hasPositionData"
    rdfs:comment="Associates a spatial region to a position."
    rdfs:label="has position data">
  <rdfs:domain rdf:resource="&dul;SpaceRegion"/>
  <rdfs:isDefinedBy rdf:resource="http://www.ease-crc.org/ont/SOMA-OBJ.owl"/>
  <rdfs:range rdf:resource="&xsd;string"/>
  <rdfs:subPropertyOf rdf:resource="&soma;hasSpaceParameter"/>
</owl:DatatypeProperty>

<owl:Class rdf:about="&soma;MovableJoint"
    rdfs:label="Movable joint">
  <rdfs:subClassOf>
    <owl:Restriction>
      <owl:onClass rdf:resource="&soma;JointState"/>
      <owl:onProperty rdf:resource="&soma;hasJointState"/>
      <owl:qualifiedCardinality rdf:datatype="&xsd;nonNegativeInteger">1</owl:qualifiedCardinality>
    </owl:Restriction>
  </rdfs:subClassOf>
  <rdfs:subClassOf rdf:resource="&soma;Joint"/>
  <rdfs:comment>A joint where the two connected links can move relative to each other in some dimension.</rdfs:comment>
  <rdfs:isDefinedBy rdf:resource="http://www.ease-crc.org/ont/SOMA-OBJ.owl"/>
</owl:Class>

<owl:Class rdf:about="&soma;PreferenceOrder">
  <rdfs:label>Preference order</rdfs:label>
  <rdfs:label xml:lang="en">The relation between a 'Preference' and the 'Order' that the 'Preference' defines over Descriptions of Situations.</rdfs:label>
  <rdfs:subClassOf>
    <owl:Restriction>
      <owl:onProperty rdf:resource="&soma;orders"/>
      <owl:someValuesFrom rdf:resource="&soma;OrderedElement"/>
    </owl:Restriction>
  </rdfs:subClassOf>
  <rdfs:subClassOf>
    <owl:Restriction>
      <owl:allValuesFrom>
        <owl:Restriction>
          <owl:allValuesFrom rdf:resource="&dul;Description"/>
          <owl:onProperty rdf:resource="&soma;encapsulates"/>
        </owl:Restriction>
      </owl:allValuesFrom>
      <owl:onProperty rdf:resource="&soma;orders"/>
    </owl:Restriction>
  </rdfs:subClassOf>
  <rdfs:subClassOf>
    <owl:Restriction>
      <owl:allValuesFrom rdf:resource="&soma;Preference"/>
      <owl:onProperty rdf:resource="&dul;describes"/>
    </owl:Restriction>
  </rdfs:subClassOf>
  <rdfs:subClassOf rdf:resource="&dul;SocialRelation"/>
  <rdfs:isDefinedBy rdf:resource="http://www.ease-crc.org/ont/SOMA-AGENT.owl"/>
</owl:Class>

<owl:Class rdf:about="&soma;IncludedObject">
  <rdfs:comment>An object that is contained in something. This is meant very general and includes, e.g., elements contained in a set, or things that are spatially contained within the boundaries of some object.</rdfs:comment>
  <rdfs:isDefinedBy rdf:resource="http://www.ease-crc.org/ont/SOMA-OBJ.owl"/>
  <rdfs:label xml:lang="en">Included object</rdfs:label>
  <rdfs:subClassOf rdf:resource="&soma;Patient"/>
</owl:Class>

<owl:Class rdf:about="&soma;CommunicationAction">
  <rdfs:subClassOf>
    <owl:Restriction>
      <owl:onProperty rdf:resource="&dul;hasParticipant"/>
      <owl:someValuesFrom rdf:resource="&soma;LinguisticObject"/>
    </owl:Restriction>
  </rdfs:subClassOf>
  <rdfs:subClassOf rdf:resource="&dul;Action"/>
  <rdfs:comment xml:lang="en">An action in which an Agent uses some actuator for communication purposes.</rdfs:comment>
  <rdfs:isDefinedBy rdf:resource="http://www.ease-crc.org/ont/SOMA-ACT.owl"/>
  <rdfs:label xml:lang="en">Locutionary action</rdfs:label>
</owl:Class>

<owl:ObjectProperty rdf:about="&soma;transitionsBack">
  <rdfs:subPropertyOf rdf:resource="&soma;transitionsFrom"/>
  <rdfs:subPropertyOf rdf:resource="&soma;transitionsTo"/>
  <rdfs:comment>A property which relates a Transient to an Object it both changes from and changes into. This is useful to model objects which, through participation in a process, transform themselves so that an ontological reclassification is necessary, however this transformation is reversible and at the end of the process the objects revert to their previous kind. An example of this is catalysts in chemistry.</rdfs:comment>
  <rdfs:domain rdf:resource="&soma;Transient"/>
  <rdfs:isDefinedBy rdf:resource="http://www.ease-crc.org/ont/SOMA-OBJ.owl"/>
  <rdfs:label xml:lang="en">transitions back</rdfs:label>
  <rdfs:range rdf:resource="&dul;Object"/>
</owl:ObjectProperty>

<owl:Class rdf:about="&soma;BlockedObject"
    rdfs:comment="An object that is blocked from accessing something.">
  <rdfs:isDefinedBy rdf:resource="http://www.ease-crc.org/ont/SOMA-OBJ.owl"/>
  <rdfs:label xml:lang="en">Blocked object</rdfs:label>
  <rdfs:subClassOf rdf:resource="&soma;Patient"/>
</owl:Class>

<owl:Class rdf:about="&soma;Assembling">
  <rdfs:comment>A task in which an Agent connects some objects such that they form a cohesive whole, and which also imposes constraints on the objects' relative motions. Often, the objects that make up an assemblage can also be separated again.</rdfs:comment>
  <rdfs:isDefinedBy rdf:resource="http://www.ease-crc.org/ont/SOMA-ACT.owl"/>
  <rdfs:subClassOf rdf:resource="&soma;Constructing"/>
</owl:Class>

<owl:ObjectProperty rdf:about="&dul;includesObject"/>

<owl:Class rdf:about="&soma;Choice">
  <rdfs:comment xml:lang="en">The output of a, e.g, Selecting Task.</rdfs:comment>
  <rdfs:isDefinedBy rdf:resource="http://www.ease-crc.org/ont/SOMA-AGENT.owl"/>
  <rdfs:label xml:lang="en">Choice</rdfs:label>
  <rdfs:subClassOf rdf:resource="&soma;ResultRole"/>
</owl:Class>

<owl:Class rdf:about="&soma;Configuration">
  <rdfs:subClassOf>
    <owl:Restriction>
      <owl:onProperty rdf:resource="&dul;describes"/>
      <owl:someValuesFrom rdf:resource="&soma;StateType"/>
    </owl:Restriction>
  </rdfs:subClassOf>
  <rdfs:subClassOf rdf:resource="&dul;Description"/>
  <rdfs:comment>A description of a State. This includes e.g. what acceptable regions for participant objects of the State might look like.
A configuration of the world is construed to be stable on its own. Outside disturbances may cause state transitions, and the settling into some other, self-stable configuration.

Several other Description subclasses may function as Configurations. For example, a Goal is a description of a desired State. A Norm describes a State that should be maintained. A Diagnosis describes a State that causes certain symptoms etc.

Note a couple of issues here. First one relates to what "configuration" means; in particular, this doesn't mean a configuration that is unchanging according to any viewpoint. The analogy here is the "macrostate" from thermodynamics: a macrostate with two gases mixed does not mean all gas particles are motionless, but rather that the locations and movements of gas particles are such that any particle is likely to have as many neighbors of one type as the other.

The second issue relates to what is "outside". The state is a configuration of some, but not necessarily all, Entities in the world. Entities not in this configuration are outside of it.</rdfs:comment>
  <rdfs:isDefinedBy rdf:resource="http://www.ease-crc.org/ont/SOMA-STATE.owl"/>
</owl:Class>

<owl:ObjectProperty rdf:about="&soma;hasSoftwareAgent"
    rdfs:label="has software agent">
  <rdfs:comment>A relation from an Event and the SoftwareAgent responsible for making that Event happen.</rdfs:comment>
  <rdfs:domain rdf:resource="&dul;Event"/>
  <rdfs:isDefinedBy rdf:resource="http://www.ease-crc.org/ont/SOMA.owl"/>
  <rdfs:range rdf:resource="&soma;SoftwareInstance"/>
  <rdfs:subPropertyOf rdf:resource="&dul;involvesAgent"/>
</owl:ObjectProperty>

<owl:Class rdf:about="&soma;DeviceTurnedOn"
    rdfs:comment="A value indicating a device is in operation.">
  <rdfs:isDefinedBy rdf:resource="http://www.ease-crc.org/ont/SOMA-OBJ.owl"/>
  <rdfs:label xml:lang="en">Device turned on</rdfs:label>
  <rdfs:subClassOf rdf:resource="&soma;DeviceStateRange"/>
</owl:Class>

<owl:Class rdf:about="&soma;PosturalMoving">
  <rdfs:comment>The Agent changes or takes an overall configuration of its body but is otherwise not significantly affecting other objects nor moving a significant amount from its original location.

Posture changes may take place as part of other actions, for example turning when walking.</rdfs:comment>
  <rdfs:isDefinedBy rdf:resource="http://www.ease-crc.org/ont/SOMA-PROC.owl"/>
  <rdfs:subClassOf rdf:resource="&soma;BodyMovement"/>
</owl:Class>

<owl:Class rdf:about="&soma;Stirring">
  <rdfs:subClassOf>
    <owl:Restriction>
      <owl:onProperty rdf:resource="&soma;isTaskAffordedBy"/>
      <owl:someValuesFrom rdf:resource="&soma;Composing"/>
    </owl:Restriction>
  </rdfs:subClassOf>
  <rdfs:subClassOf rdf:resource="&soma;Mixing"/>
  <rdfs:comment>A task in which an agent dissolves small particles like sugar or salt in fluid</rdfs:comment>
  <rdfs:isDefinedBy rdf:resource="http://www.ease-crc.org/ont/SOMA-ACT.owl"/>
</owl:Class>

<owl:ObjectProperty rdf:about="&dul;isComponentOf"/>

<rdfs:Datatype rdf:about="&soma;array_int">
  <rdfs:isDefinedBy rdf:resource="http://www.ease-crc.org/ont/SOMA.owl"/>
  <owl:equivalentClass rdf:resource="&xsd;string"/>
</rdfs:Datatype>

<owl:ObjectProperty rdf:about="&soma;hasQuale"
    rdfs:label="has quale">
  <rdfs:comment>Relates a quality to its "value", called quale, which is an atomic quality region.</rdfs:comment>
  <rdfs:domain rdf:resource="&dul;Quality"/>
  <rdfs:isDefinedBy rdf:resource="http://www.ease-crc.org/ont/SOMA-OBJ.owl"/>
  <rdfs:range rdf:resource="&dul;Region"/>
  <rdfs:subPropertyOf rdf:resource="&dul;hasRegion"/>
  <owl:inverseOf rdf:resource="&soma;isQualeOf"/>
</owl:ObjectProperty>

<owl:ObjectProperty rdf:about="&soma;answers">
  <rdfs:label>The relation between an answering message and the message it answers.</rdfs:label>
  <rdfs:label>answers</rdfs:label>
  <rdfs:domain rdf:resource="&soma;Answer"/>
  <rdfs:isDefinedBy rdf:resource="http://www.ease-crc.org/ont/SOMA-ACT.owl"/>
  <rdfs:range rdf:resource="&soma;Message"/>
  <rdfs:subPropertyOf rdf:resource="&soma;relatesToAnotherRole"/>
  <owl:inverseOf rdf:resource="&soma;hasAnswer"/>
</owl:ObjectProperty>

<owl:Class rdf:about="&soma;PhysicalAcquiring">
  <rdfs:comment>The goal of this task is to make some object usable for other tasks, by possibly changing its physical state. Usually, it overlaps some task that describes the manner in which an object is obtained.

The prototypical example of PhysicalAcquiring is picking up an object.

Note that buying an object is NOT PhysicalAcquiring. Buying, or ownership transfer in general, also involves an adjustment in social structures describing ownership.</rdfs:comment>
  <rdfs:isDefinedBy rdf:resource="http://www.ease-crc.org/ont/SOMA-ACT.owl"/>
  <rdfs:label xml:lang="en">Physical acquiring</rdfs:label>
  <rdfs:subClassOf rdf:resource="&soma;ModifyingPhysicalObject"/>
</owl:Class>

<owl:ObjectProperty rdf:about="&soma;hasTerminalState"
    rdfs:comment="A relation from a Transition to the Situation it ends in."
    rdfs:label="has terminal state">
  <rdfs:domain rdf:resource="&dul;Transition"/>
  <rdfs:isDefinedBy rdf:resource="http://www.ease-crc.org/ont/SOMA.owl"/>
  <rdfs:range rdf:resource="&dul;Situation"/>
  <rdfs:subPropertyOf rdf:resource="&soma;includesSituation"/>
  <owl:inverseOf rdf:resource="&soma;isTerminalStateOf"/>
</owl:ObjectProperty>

<owl:DatatypeProperty rdf:about="&soma;hasRGBValue"
    rdfs:label="has rgb value">
  <rdfs:comment>Associates a ColorRegion to numerical data describing the color. This data uses the Red-Green-Blue color space.</rdfs:comment>
  <rdfs:domain rdf:resource="&soma;ColorRegion"/>
  <rdfs:isDefinedBy rdf:resource="http://www.ease-crc.org/ont/SOMA-OBJ.owl"/>
  <rdfs:range rdf:resource="&xsd;string"/>
  <rdfs:subPropertyOf rdf:resource="&soma;hasColorValue"/>
</owl:DatatypeProperty>

<owl:ObjectProperty rdf:about="&soma;hasPredecessor">
  <rdfs:comment>Indicates that a Task is the predecessor in a Succedence Relation; that is, this is the task to execute first.</rdfs:comment>
  <rdfs:domain rdf:resource="&soma;Succedence"/>
  <rdfs:isDefinedBy rdf:resource="http://www.ease-crc.org/ont/SOMA-WF.owl"/>
  <rdfs:label xml:lang="en">has predecessor</rdfs:label>
  <rdfs:range rdf:resource="&dul;Workflow"/>
  <rdfs:subPropertyOf rdf:resource="&dul;hasPart"/>
</owl:ObjectProperty>

<owl:Class rdf:about="&soma;PouringOnto"
    rdfs:label="Pouring onto">
  <rdfs:comment>The task in which an agent pours the substance on top of an object</rdfs:comment>
  <rdfs:isDefinedBy rdf:resource="http://www.ease-crc.org/ont/SOMA-ACT.owl"/>
  <rdfs:subClassOf rdf:resource="&soma;Pouring"/>
</owl:Class>

<owl:Class rdf:about="&soma;PhysicalEffector"
    rdfs:label="Physical effector">
  <rdfs:isDefinedBy rdf:resource="http://www.ease-crc.org/ont/SOMA-OBJ.owl"/>
  <rdfs:isDefinedBy rdf:resource="http://www.ease-crc.org/ont/SOMA-PROC.owl"/>
  <rdfs:subClassOf>
    <owl:Restriction>
      <owl:onProperty>
        <rdf:Description>
          <owl:inverseOf rdf:resource="&dul;hasPart"/>
        </rdf:Description>
      </owl:onProperty>
      <owl:someValuesFrom rdf:resource="&dul;PhysicalAgent"/>
    </owl:Restriction>
  </rdfs:subClassOf>
  <rdfs:subClassOf rdf:resource="&soma;FunctionalPart"/>
  <rdfs:comment>A functional part belonging to an Agent and which allows that Agent to act upon its surroundings.</rdfs:comment>
</owl:Class>

<owl:Class rdf:about="&soma;ConnectedObject"
    rdfs:comment="An object that is combined with another object.">
  <rdfs:isDefinedBy rdf:resource="http://www.ease-crc.org/ont/SOMA-OBJ.owl"/>
  <rdfs:isDefinedBy rdf:resource="http://www.ease-crc.org/ont/SOMA-STATE.owl"/>
  <rdfs:label xml:lang="en">Connected object</rdfs:label>
  <rdfs:subClassOf rdf:resource="&soma;Patient"/>
</owl:Class>

<owl:Class rdf:about="&dul;InformationRealization">
  <rdfs:subClassOf>
    <owl:Restriction>
      <owl:onProperty rdf:resource="&soma;hasPersistentIdentifier"/>
      <owl:someValuesFrom rdf:resource="&xsd;string"/>
    </owl:Restriction>
  </rdfs:subClassOf>
  <rdfs:subClassOf>
    <owl:Restriction>
      <owl:onDataRange rdf:resource="&xsd;string"/>
      <owl:onProperty rdf:resource="&soma;hasDataFormat"/>
      <owl:qualifiedCardinality rdf:datatype="&xsd;nonNegativeInteger">1</owl:qualifiedCardinality>
    </owl:Restriction>
  </rdfs:subClassOf>
  <rdfs:comment>In SOMA-compliant systems, the way to use InformationObjects to specify extra data about an individual entity is to employ the 'is about' and 'expresses' properties (or their inverses 'is reference of' and 'is expressed by') and to supply a persistent identifier for a realization of the InformationObject.

As a prototypical example, consider an individual called Action_XYZ, about which we have some data for which the meaning is described by Description_ABC. The data would be an individual InformationObject_DEF, and the following property assertions would hold:

InformationObject_DEF 'is about' Action_XYZ
InformationObject_DEF expresses Description_ABC


Usually, an individual InformationObject would be connected to (at least) an InformationRealization individual. For example, suppose there is such an InformationRealization individual, InformationRealization_123. Then, this individual will have data properties describing its format and persistent identifier

InformationRealization_123 hasPersistentIdentifier 'doi'
InformationRealization_123 hasDataFormat 'urdf'</rdfs:comment>
</owl:Class>

<owl:Class rdf:about="&soma;Impediment">
  <rdfs:subClassOf>
    <owl:Restriction>
      <owl:allValuesFrom rdf:resource="&soma;Obstacle"/>
      <owl:onProperty rdf:resource="&soma;affordsBearer"/>
    </owl:Restriction>
  </rdfs:subClassOf>
  <rdfs:subClassOf>
    <owl:Restriction>
      <owl:allValuesFrom rdf:resource="&soma;RestrictedObject"/>
      <owl:onProperty rdf:resource="&soma;affordsTrigger"/>
    </owl:Restriction>
  </rdfs:subClassOf>
  <rdfs:subClassOf rdf:resource="&soma;Blockage"/>
  <rdfs:comment>The disposition of an object (the obstacle) to prohibit certain ways of entering or leaving a space or group. An example is a doorstopper constraining a door, prohibiting it to enter the area behind it.</rdfs:comment>
  <rdfs:isDefinedBy rdf:resource="http://www.ease-crc.org/ont/SOMA-OBJ.owl"/>
</owl:Class>

<owl:Class rdf:about="&soma;ServerRole">
  <rdfs:subClassOf>
    <owl:Restriction>
      <owl:onProperty rdf:resource="&dul;isDefinedIn"/>
      <owl:someValuesFrom rdf:resource="&soma;Client-Server_Specification"/>
    </owl:Restriction>
  </rdfs:subClassOf>
  <rdfs:subClassOf rdf:resource="&soma;InterfaceComponentRole"/>
  <rdfs:comment xml:lang="en">The Client-server model is a distributed application structure that partitions tasks or workloads between the providers of a resource or service, called servers, and service requesters, called clients Often clients and servers communicate over a computer network on separate hardware, but both client and server may reside in the same system. A server host runs one or more server programs, which share their resources with clients. A client usually does not share any of its resources, but it requests content or service from a server. Clients, therefore, initiate communication sessions with servers, which await incoming requests. Examples of computer applications that use the client-server model are email, network printing, and the World Wide Web.

Source: https://en.wikipedia.org/wiki/Client%E2%80%93server_model</rdfs:comment>
  <rdfs:isDefinedBy rdf:resource="http://www.ease-crc.org/ont/SOMA-IO.owl"/>
  <rdfs:label xml:lang="en">Server role</rdfs:label>
</owl:Class>

<owl:ObjectProperty rdf:about="&soma;hasSuccedence">
  <rdfs:comment>A relation between a Workflow and a Succedence that appears in it.</rdfs:comment>
  <rdfs:domain rdf:resource="&dul;Workflow"/>
  <rdfs:isDefinedBy rdf:resource="http://www.ease-crc.org/ont/SOMA-WF.owl"/>
  <rdfs:label xml:lang="en">has succedence</rdfs:label>
  <rdfs:range rdf:resource="&soma;Succedence"/>
  <rdfs:subPropertyOf rdf:resource="&dul;hasPart"/>
</owl:ObjectProperty>

<owl:Class rdf:about="&soma;Transporting">
  <rdfs:comment>A task by which an Agent carries an item from a source to a destination location.</rdfs:comment>
  <rdfs:isDefinedBy rdf:resource="http://www.ease-crc.org/ont/SOMA-ACT.owl"/>
  <rdfs:subClassOf rdf:resource="&soma;ModifyingPhysicalObject"/>
</owl:Class>

<soma:ExecutionStateRegion rdf:about="&soma;ExecutionState_Pending"
    rdfs:comment="The execution state of a pending activity.">
  <rdf:type rdf:resource="&owl;NamedIndividual"/>
  <rdfs:isDefinedBy rdf:resource="http://www.ease-crc.org/ont/SOMA-ACT.owl"/>
</soma:ExecutionStateRegion>

<owl:Class rdf:about="&dul;SocialObject"/>

<owl:Class rdf:about="&soma;DetectedObject"
    rdfs:comment="An object that is detected.">
  <rdfs:isDefinedBy rdf:resource="http://www.ease-crc.org/ont/SOMA-OBJ.owl"/>
  <rdfs:label xml:lang="en">Detected object</rdfs:label>
  <rdfs:subClassOf rdf:resource="&soma;Patient"/>
</owl:Class>

<owl:ObjectProperty rdf:about="&soma;after"
    soma:symbol="&gt;">
  <rdf:type rdf:resource="&owl;TransitiveProperty"/>
  <rdfs:comment>A relation between entities, expressing a 'sequence' schema where one of the entities strictly ends before the other one.</rdfs:comment>
  <rdfs:domain rdf:resource="&dul;Entity"/>
  <rdfs:isDefinedBy rdf:resource="http://www.ease-crc.org/ont/SOMA.owl"/>
  <rdfs:range rdf:resource="&dul;Entity"/>
  <rdfs:subPropertyOf rdf:resource="&dul;follows"/>
  <owl:inverseOf rdf:resource="&soma;before"/>
</owl:ObjectProperty>

<owl:ObjectProperty rdf:about="&soma;hasSpaceRegion"
    rdfs:comment="Relates an entity to a space region."
    rdfs:label="has space region">
  <rdfs:domain>
    <owl:Class>
      <owl:unionOf rdf:parseType="Collection">
        <rdf:Description rdf:about="&soma;Localization"/>
        <rdf:Description rdf:about="&soma;ShapeRegion"/>
        <rdf:Description rdf:about="&dul;PhysicalObject"/>
      </owl:unionOf>
    </owl:Class>
  </rdfs:domain>
  <rdfs:isDefinedBy rdf:resource="http://www.ease-crc.org/ont/SOMA-OBJ.owl"/>
  <rdfs:range rdf:resource="&dul;SpaceRegion"/>
  <rdfs:subPropertyOf rdf:resource="&dul;hasRegion"/>
  <owl:inverseOf rdf:resource="&soma;isSpaceRegionFor"/>
</owl:ObjectProperty>

<owl:Class rdf:about="&soma;Item">
  <rdfs:isDefinedBy rdf:resource="http://www.ease-crc.org/ont/SOMA-OBJ.owl"/>
  <rdfs:isDefinedBy rdf:resource="http://www.ease-crc.org/ont/SOMA-STATE.owl"/>
  <rdfs:comment>A role played by a non-agentive object operated on by an action.</rdfs:comment>
  <rdfs:subClassOf rdf:resource="&soma;Patient"/>
</owl:Class>

<owl:ObjectProperty rdf:about="&soma;isSpaceRegionFor"
    rdfs:comment="Relates a space region to an entity."
    rdfs:label="is space region for">
  <rdfs:domain rdf:resource="&dul;SpaceRegion"/>
  <rdfs:isDefinedBy rdf:resource="http://www.ease-crc.org/ont/SOMA-OBJ.owl"/>
  <rdfs:range>
    <owl:Class>
      <owl:unionOf rdf:parseType="Collection">
        <rdf:Description rdf:about="&soma;Localization"/>
        <rdf:Description rdf:about="&dul;PhysicalObject"/>
      </owl:unionOf>
    </owl:Class>
  </rdfs:range>
  <rdfs:subPropertyOf rdf:resource="&dul;isRegionFor"/>
</owl:ObjectProperty>

<owl:Class rdf:about="&soma;Shape"
    rdfs:comment="The external form, contours, or outline of an object.">
  <rdfs:subClassOf>
    <owl:Restriction>
      <owl:onProperty rdf:resource="&dul;hasRegion"/>
      <owl:someValuesFrom rdf:resource="&soma;ShapeRegion"/>
    </owl:Restriction>
  </rdfs:subClassOf>
  <rdfs:subClassOf>
    <owl:Restriction>
      <owl:allValuesFrom rdf:resource="&soma;ShapeRegion"/>
      <owl:onProperty rdf:resource="&dul;hasRegion"/>
    </owl:Restriction>
  </rdfs:subClassOf>
  <rdfs:subClassOf rdf:resource="&soma;Intrinsic"/>
  <rdfs:isDefinedBy rdf:resource="http://www.ease-crc.org/ont/SOMA-OBJ.owl"/>
</owl:Class>

<owl:ObjectProperty rdf:about="&soma;isTaskOfCreatedRole"
    rdfs:label="is task of created role">
  <rdfs:comment>A relation between a Task and one of its output roles. The difference to IsTaskOfOutputRole is that the latter is also applicable, e.g., for Deciding between objects, where the selected object is not created, but still an outcome of that task.</rdfs:comment>
  <rdfs:domain rdf:resource="&dul;Task"/>
  <rdfs:isDefinedBy rdf:resource="http://www.ease-crc.org/ont/SOMA-ACT.owl"/>
  <rdfs:range rdf:resource="&dul;Role"/>
  <rdfs:subPropertyOf rdf:resource="&soma;isTaskOfOutputRole"/>
</owl:ObjectProperty>

<owl:Class rdf:about="&soma;SocialState"
    rdfs:label="Social state">
  <rdfs:comment>A State which describes how Agents relate to each other.

One can argue that any Social state is a Physical state, since anything the Agents may use to construct a social relationship is made of physical things. The difference is that the physical support of the social relationships is not important here, what matters instead is the nature and content of the social relations, regardless of how they are physically realized.</rdfs:comment>
  <rdfs:comment>Note here a distinction: the Agents involved must be able to communicate. This is because while it is often assumed that an Agent has or aspires to have similar cognitive capacities to a human, This need not be the case; in particular, not all Agents need to maintain theories of mind about each other and therefore not all Agents need to communicate with each other. It is hard to see what sort of meaning Social concepts might have to such Agents, since Social concepts are all about shared constructions.

Note also that the DUL SocialAgent class is not an appropriate restriction however. SocialAgent is one that exists by agreement of PhysicalAgents. For example, a corporation or a nation are SocialAgents. An Agent with the capability to engage socially is not necessarily a DUL SocialAgent.</rdfs:comment>
  <rdfs:subClassOf>
    <owl:Restriction>
      <owl:onProperty rdf:resource="&dul;hasParticipant"/>
      <owl:someValuesFrom rdf:resource="&dul;Agent"/>
    </owl:Restriction>
  </rdfs:subClassOf>
  <rdfs:subClassOf rdf:resource="&soma;State"/>
  <rdfs:isDefinedBy rdf:resource="http://www.ease-crc.org/ont/SOMA-STATE.owl"/>
</owl:Class>

<owl:Class rdf:about="&soma;Pulling">
  <owl:disjointWith rdf:resource="&soma;Pushing"/>
  <owl:disjointWith rdf:resource="&soma;Squeezing"/>
  <rdfs:comment>A task in which an Agent moves an object in a direction loosely from the object's center of mass towards the contact point between agent and object.</rdfs:comment>
  <rdfs:isDefinedBy rdf:resource="http://www.ease-crc.org/ont/SOMA-ACT.owl"/>
  <rdfs:subClassOf rdf:resource="&soma;Actuating"/>
</owl:Class>

<owl:Class rdf:about="&soma;DependentPlace">
  <rdfs:comment>A feature that is not part of its host, like a hole in a piece of cheese.</rdfs:comment>
  <rdfs:isDefinedBy rdf:resource="http://www.ease-crc.org/ont/SOMA-OBJ.owl"/>
  <rdfs:label xml:lang="en">Dependent place</rdfs:label>
  <rdfs:subClassOf rdf:resource="&soma;Feature"/>
</owl:Class>

<owl:ObjectProperty rdf:about="&soma;hasFeature"
    rdfs:comment="Associates a physical object to one of its features."
    rdfs:label="has feature">
  <rdfs:domain rdf:resource="&dul;PhysicalObject"/>
  <rdfs:isDefinedBy rdf:resource="http://www.ease-crc.org/ont/SOMA-OBJ.owl"/>
  <rdfs:range rdf:resource="&soma;Feature"/>
  <rdfs:subPropertyOf rdf:resource="&dul;hasConstituent"/>
  <owl:inverseOf rdf:resource="&soma;isFeatureOf"/>
</owl:ObjectProperty>

<owl:Class rdf:about="&soma;RestrictedObject"
    rdfs:comment="An object with restrictions to access something.">
  <rdfs:isDefinedBy rdf:resource="http://www.ease-crc.org/ont/SOMA-OBJ.owl"/>
  <rdfs:label xml:lang="en">Restricted object</rdfs:label>
  <rdfs:subClassOf rdf:resource="&soma;BlockedObject"/>
</owl:Class>

<rdfs:Datatype rdf:about="&soma;array_double">
  <rdfs:isDefinedBy rdf:resource="http://www.ease-crc.org/ont/SOMA.owl"/>
  <owl:equivalentClass rdf:resource="&xsd;string"/>
</rdfs:Datatype>

<owl:Class rdf:about="&soma;Ontology_Language">
  <rdfs:subClassOf>
    <owl:Restriction>
      <owl:allValuesFrom rdf:resource="&soma;Ontology"/>
      <owl:onProperty rdf:resource="&soma;givesMeaningTo"/>
    </owl:Restriction>
  </rdfs:subClassOf>
  <rdfs:subClassOf rdf:resource="&soma;KnowledgeRepresentationLanguage"/>
  <rdfs:comment xml:lang="en">An Ontology Language is a Knowledge Representation Language to describe knowledge about properties of a subject area and how they are related, by defining a set of concepts and categories that represent the subject using logic. Examples are the different OWL Profiles.

Source: https://en.wikipedia.org/wiki/Ontology_(information_science)</rdfs:comment>
  <rdfs:isDefinedBy rdf:resource="http://www.ease-crc.org/ont/SOMA-IO.owl"/>
  <rdfs:label xml:lang="en">Ontology Language</rdfs:label>
</owl:Class>

<owl:ObjectProperty rdf:about="&soma;isFirstStepOf"
    rdfs:label="is first step of">
  <rdfs:comment>A relation stating that some task is the first one in a workflow.</rdfs:comment>
  <rdfs:domain rdf:resource="&dul;Task"/>
  <rdfs:isDefinedBy rdf:resource="http://www.ease-crc.org/ont/SOMA-WF.owl"/>
  <rdfs:range rdf:resource="&dul;Workflow"/>
  <rdfs:subPropertyOf rdf:resource="&soma;isStepOf"/>
</owl:ObjectProperty>

<owl:ObjectProperty rdf:about="&soma;isLinkOf"
    rdfs:comment="Relates an object to its kinematic components."
    rdfs:label="is link of">
  <rdfs:domain rdf:resource="&dul;PhysicalObject"/>
  <rdfs:isDefinedBy rdf:resource="http://www.ease-crc.org/ont/SOMA-OBJ.owl"/>
  <rdfs:range rdf:resource="&dul;PhysicalObject"/>
  <rdfs:subPropertyOf rdf:resource="&dul;isComponentOf"/>
</owl:ObjectProperty>

<owl:Class rdf:about="&soma;Vaporizing"
    rdfs:comment="Some material transitions from a liquid to a gaseous phase.">
  <rdfs:subClassOf>
    <owl:Restriction>
      <owl:onProperty rdf:resource="&soma;isProcessTypeOf"/>
      <owl:someValuesFrom>
        <owl:Class>
          <owl:intersectionOf rdf:parseType="Collection">
            <rdf:Description rdf:about="&soma;AlteredObject"/>
            <owl:Restriction>
              <owl:allValuesFrom rdf:resource="&dul;Substance"/>
              <owl:onProperty rdf:resource="&dul;classifies"/>
            </owl:Restriction>
          </owl:intersectionOf>
        </owl:Class>
      </owl:someValuesFrom>
    </owl:Restriction>
  </rdfs:subClassOf>
  <rdfs:subClassOf rdf:resource="&soma;PhaseTransition"/>
  <rdfs:isDefinedBy rdf:resource="http://www.ease-crc.org/ont/SOMA-PROC.owl"/>
  <rdfs:seeAlso>Transitions from a solid to a gaseous phase are usually referred to as Sublimation.</rdfs:seeAlso>
</owl:Class>

<owl:Class rdf:about="&soma;RelevantPart">
  <rdfs:comment>Features that are relevant parts of their host, like a bump or an edge.</rdfs:comment>
  <rdfs:isDefinedBy rdf:resource="http://www.ease-crc.org/ont/SOMA-OBJ.owl"/>
  <rdfs:label xml:lang="en">Relevant part</rdfs:label>
  <rdfs:subClassOf rdf:resource="&soma;Feature"/>
</owl:Class>

<owl:ObjectProperty rdf:about="&dul;isParticipantIn">
  <rdfs:isDefinedBy rdf:resource="http://www.ease-crc.org/ont/SOMA.owl"/>
</owl:ObjectProperty>

<owl:Class rdf:about="&soma;MedicalDiagnosis"
    rdfs:comment="A functional diagnosis of an organism."
    rdfs:label="Medical diagnosis">
  <rdfs:subClassOf>
    <owl:Restriction>
      <owl:onProperty rdf:resource="&dul;hasConstituent"/>
      <owl:someValuesFrom rdf:resource="&dul;Organism"/>
    </owl:Restriction>
  </rdfs:subClassOf>
  <rdfs:subClassOf rdf:resource="&soma;FunctionalDiagnosis"/>
  <rdfs:isDefinedBy rdf:resource="http://www.ease-crc.org/ont/SOMA.owl"/>
  <owl:disjointWith rdf:resource="&soma;TechnicalDiagnosis"/>
</owl:Class>

<owl:ObjectProperty rdf:about="&soma;isTaskAffordedBy"
    rdfs:label="is task afforded by">
  <rdfs:comment>Relates a disposition to the task defined by the affordance describing the disposition.</rdfs:comment>
  <rdfs:domain rdf:resource="&dul;Task"/>
  <rdfs:isDefinedBy rdf:resource="http://www.ease-crc.org/ont/SOMA-OBJ.owl"/>
  <rdfs:range rdf:resource="&soma;Disposition"/>
  <rdfs:subPropertyOf rdf:resource="&soma;isConceptAffordedBy"/>
  <owl:propertyChainAxiom rdf:parseType="Collection">
    <rdf:Description rdf:about="&soma;isTaskDefinedInAffordance"/>
    <rdf:Description rdf:about="&dul;describes"/>
  </owl:propertyChainAxiom>
</owl:ObjectProperty>

<rdfs:Datatype rdf:about="&soma;array_string">
  <rdfs:isDefinedBy rdf:resource="http://www.ease-crc.org/ont/SOMA.owl"/>
  <owl:equivalentClass rdf:resource="&xsd;string"/>
</rdfs:Datatype>

<owl:ObjectProperty rdf:about="&soma;isTriggerDefinedIn"
    rdfs:label="is trigger defined in">
  <rdfs:comment>Relates an affordance which is a relation between a bearer and a trigger, to the role of the trigger when the affordance is manifested.</rdfs:comment>
  <rdfs:domain rdf:resource="&dul;Role"/>
  <rdfs:isDefinedBy rdf:resource="http://www.ease-crc.org/ont/SOMA-OBJ.owl"/>
  <rdfs:range rdf:resource="&soma;Affordance"/>
  <rdfs:subPropertyOf rdf:resource="&dul;isRoleDefinedIn"/>
</owl:ObjectProperty>

<owl:ObjectProperty rdf:about="&soma;isPerformedBy"
    rdfs:comment="A relation from an Action to the Agent who performs it."
    rdfs:label="is performed by">
  <rdfs:domain rdf:resource="&dul;Action"/>
  <rdfs:isDefinedBy rdf:resource="http://www.ease-crc.org/ont/SOMA-ACT.owl"/>
  <rdfs:range rdf:resource="&dul;Agent"/>
  <rdfs:subPropertyOf rdf:resource="&dul;involvesAgent"/>
</owl:ObjectProperty>

<owl:AsymmetricProperty rdf:about="&soma;hasTerminalSituation">
  <rdf:type rdf:resource="&owl;IrreflexiveProperty"/>
  <rdf:type rdf:resource="&owl;ObjectProperty"/>
  <rdfs:range rdf:nodeID="bn2"/>
  <rdfs:range rdf:resource="&dul;Situation"/>
  <rdfs:comment>A relation between SituationTransitions and Situations, which identifies the Situation the transition ends at.</rdfs:comment>
  <rdfs:domain rdf:resource="&soma;SituationTransition"/>
  <rdfs:isDefinedBy rdf:resource="http://www.ease-crc.org/ont/SOMA-ACT.owl"/>
  <rdfs:label xml:lang="en">has terminal situation</rdfs:label>
  <rdfs:subPropertyOf rdf:resource="&soma;hasTerminalState"/>
  <owl:inverseOf rdf:resource="&soma;isTerminalSituationOf"/>
</owl:AsymmetricProperty>

<owl:AnnotationProperty rdf:about="&soma;nickname">
  <rdfs:comment>Similar to rdfs:label, but without GUI or reasoner impact in Protege; avoiding Protege problems is why this is not a label subproperty. Nicknames are used by particular software working with the ontology as a way to give community-specific names to concepts. Communities are identified by the subproperty of nickname.</rdfs:comment>
  <rdfs:isDefinedBy rdf:resource="http://www.ease-crc.org/ont/SOMA.owl"/>
</owl:AnnotationProperty>

<owl:Class rdf:about="&soma;ThinkAloudSceneKnowledgeTopic"
    rdfs:label="Think aloud scene knowledge topic">
  <rdfs:comment>A topic used when an Agent describes what they know about their environment, including knowledge of world states that they do not currently perceive.</rdfs:comment>
  <rdfs:isDefinedBy rdf:resource="http://www.ease-crc.org/ont/SOMA-ACT.owl"/>
  <rdfs:subClassOf rdf:resource="&soma;ThinkAloudKnowledgeTopic"/>
</owl:Class>

<owl:Class rdf:about="&soma;Dirty"
    rdfs:comment="A cleanliness region with values considered as dirty.">
  <rdfs:isDefinedBy rdf:resource="http://www.ease-crc.org/ont/SOMA-OBJ.owl"/>
  <rdfs:subClassOf rdf:resource="&soma;CleanlinessRegion"/>
</owl:Class>

<owl:Class rdf:about="&soma;InductiveReasoning">
  <rdfs:comment>A task in which the Agent endeavors to accumulate confidence in some general statement about the world, by gathering instances in which this general statement appears to apply. Note that perfect confidence can never be guaranteed by induction.

Induction is often described as a move from many "specifics" (swan A is white, swan B is white, swan C is white, ...) to the "general" (all swans are white).</rdfs:comment>
  <rdfs:isDefinedBy rdf:resource="http://www.ease-crc.org/ont/SOMA-ACT.owl"/>
  <rdfs:label xml:lang="en">Inductive resoning</rdfs:label>
  <rdfs:subClassOf rdf:resource="&soma;Reasoning"/>
</owl:Class>

<owl:Class rdf:about="&dul;Collection"/>

<owl:ObjectProperty rdf:about="&dul;isRealizedBy"/>

<owl:Class rdf:about="&soma;Interpreting">
  <rdfs:comment xml:lang="en">A task in which an Agent interpretes some information, e.g., makes sense of some incoming message or its visible surroundings.</rdfs:comment>
  <rdfs:isDefinedBy rdf:resource="http://www.ease-crc.org/ont/SOMA-ACT.owl"/>
  <rdfs:label xml:lang="en">Interpreting</rdfs:label>
  <rdfs:subClassOf rdf:resource="&soma;DerivingInformation"/>
</owl:Class>

<owl:Class rdf:about="&soma;KinoDynamicData">
  <rdfs:subClassOf>
    <owl:Restriction>
      <owl:allValuesFrom rdf:resource="&dul;PhysicalObject"/>
      <owl:onProperty rdf:resource="&dul;isAbout"/>
    </owl:Restriction>
  </rdfs:subClassOf>
  <rdfs:subClassOf rdf:resource="&dul;InformationObject"/>
  <rdfs:comment>An InformationObject containing data about how a physical object is put together such that its parts may move relative to each other, and what the physical characteristics of those parts are.</rdfs:comment>
  <rdfs:isDefinedBy rdf:resource="http://www.ease-crc.org/ont/SOMA-NEEM.owl"/>
  <rdfs:label xml:lang="en">Kino-dynamic data</rdfs:label>
</owl:Class>

<owl:Class rdf:about="&soma;QueryEngine">
  <rdfs:comment xml:lang="en">A Query Engine is a Software that can answer some queries.</rdfs:comment>
  <rdfs:isDefinedBy rdf:resource="http://www.ease-crc.org/ont/SOMA-IO.owl"/>
  <rdfs:label xml:lang="en">Query engine</rdfs:label>
  <rdfs:subClassOf rdf:resource="&soma;SoftwareRole"/>
</owl:Class>

<owl:Class rdf:about="&soma;QueryLanguage">
  <rdfs:comment xml:lang="en">Query languages, are Computer languages used to make queries in databases and information systems (Source: https://en.wikipedia.org/wiki/Query_language).

Note that despite their name, Query languages typically come with syntax and semantic to not only ask for information, but also provide them, e.g., via SQL Update. In that sense, the term "query" from above refers to any formal object of information exchange with a database.</rdfs:comment>
  <rdfs:isDefinedBy rdf:resource="http://www.ease-crc.org/ont/SOMA-IO.owl"/>
  <rdfs:label xml:lang="en">Query language</rdfs:label>
  <rdfs:subClassOf rdf:resource="&soma;Computer_Language"/>
</owl:Class>

<owl:Class rdf:about="&soma;RelationalDatabase">
  <rdfs:comment xml:lang="en">A Relational Database is a Database based on the relational model of data, which organizes data into one or more tables (or "relations") of columns and rows, with a unique key identifying each row.

Source: https://en.wikipedia.org/wiki/Relational_database</rdfs:comment>
  <rdfs:isDefinedBy rdf:resource="http://www.ease-crc.org/ont/SOMA-IO.owl"/>
  <rdfs:label xml:lang="en">Relational database</rdfs:label>
  <rdfs:subClassOf rdf:resource="&soma;Database"/>
</owl:Class>

<owl:DatatypeProperty rdf:about="&soma;hasPriority"
    rdfs:comment="A relation asserting some entity has a particular priority.">
  <rdfs:domain rdf:resource="&dul;Task"/>
  <rdfs:isDefinedBy rdf:resource="http://www.ease-crc.org/ont/SOMA-WF.owl"/>
  <rdfs:subPropertyOf rdf:resource="&dul;hasDataValue"/>
</owl:DatatypeProperty>

<owl:ObjectProperty rdf:about="&soma;definesParameter"
    rdfs:comment="A relation between a description and a parameter."
    rdfs:label="defines parameter">
  <rdfs:domain rdf:resource="&dul;Description"/>
  <rdfs:isDefinedBy rdf:resource="http://www.ease-crc.org/ont/SOMA-OBJ.owl"/>
  <rdfs:range rdf:resource="&dul;Parameter"/>
  <rdfs:subPropertyOf rdf:resource="&dul;defines"/>
  <owl:inverseOf rdf:resource="&soma;isParameterDefinedIn"/>
</owl:ObjectProperty>

<owl:ObjectProperty rdf:about="&dul;isExecutedIn">
  <rdfs:subPropertyOf rdf:resource="&soma;isOccurringIn"/>
</owl:ObjectProperty>

<owl:AsymmetricProperty rdf:about="&soma;hasInitialSituation">
  <rdf:type rdf:resource="&owl;IrreflexiveProperty"/>
  <rdf:type rdf:resource="&owl;ObjectProperty"/>
  <rdfs:range rdf:nodeID="bn4"/>
  <rdfs:range rdf:resource="&dul;Situation"/>
  <rdfs:comment>A relation between SituationTransitions and Situations, which identifies the Situation the transition starts from.</rdfs:comment>
  <rdfs:domain rdf:resource="&soma;SituationTransition"/>
  <rdfs:isDefinedBy rdf:resource="http://www.ease-crc.org/ont/SOMA-ACT.owl"/>
  <rdfs:label xml:lang="en">has initial situation</rdfs:label>
  <rdfs:subPropertyOf rdf:resource="&soma;hasInitialState"/>
  <owl:inverseOf rdf:resource="&soma;isInitialSituationOf"/>
</owl:AsymmetricProperty>

<owl:Class rdf:about="&soma;AssumingPose">
  <rdfs:comment>A task by which an Agent arranges its body, or part of it, according to some configuration.</rdfs:comment>
  <rdfs:isDefinedBy rdf:resource="http://www.ease-crc.org/ont/SOMA-ACT.owl"/>
  <rdfs:label xml:lang="en">Assuming pose</rdfs:label>
  <rdfs:subClassOf rdf:resource="&soma;PhysicalTask"/>
</owl:Class>

<owl:ObjectProperty rdf:about="&dul;satisfies">
  <rdfs:isDefinedBy rdf:resource="http://www.ease-crc.org/ont/SOMA-PROC.owl"/>
</owl:ObjectProperty>

<owl:Class rdf:about="&soma;Disposition">
  <rdfs:comment>The tendency of an object (the bearer) to make certain events happen with others (the triggers).</rdfs:comment>
  <rdfs:comment>extrinsic</rdfs:comment>
  <rdfs:subClassOf>
    <owl:Restriction>
      <owl:onClass rdf:resource="&soma;Affordance"/>
      <owl:onProperty rdf:resource="&dul;isDescribedBy"/>
      <owl:qualifiedCardinality rdf:datatype="&xsd;nonNegativeInteger">1</owl:qualifiedCardinality>
    </owl:Restriction>
  </rdfs:subClassOf>
  <rdfs:subClassOf>
    <owl:Restriction>
      <owl:onClass>
        <owl:Class>
          <owl:intersectionOf rdf:parseType="Collection">
            <rdf:Description rdf:about="&soma;Affordance"/>
            <owl:Restriction>
              <owl:onClass rdf:resource="&dul;Role"/>
              <owl:onProperty rdf:resource="&soma;definesBearer"/>
              <owl:qualifiedCardinality rdf:datatype="&xsd;nonNegativeInteger">1</owl:qualifiedCardinality>
            </owl:Restriction>

            <owl:Restriction>
              <owl:onClass rdf:resource="&dul;EventType"/>
              <owl:onProperty rdf:resource="&soma;definesEventType"/>
              <owl:qualifiedCardinality rdf:datatype="&xsd;nonNegativeInteger">1</owl:qualifiedCardinality>
            </owl:Restriction>

            <owl:Restriction>
              <owl:onClass rdf:resource="&dul;Role"/>
              <owl:onProperty rdf:resource="&soma;definesTrigger"/>
              <owl:qualifiedCardinality rdf:datatype="&xsd;nonNegativeInteger">1</owl:qualifiedCardinality>
            </owl:Restriction>
          </owl:intersectionOf>
        </owl:Class>
      </owl:onClass>
      <owl:onProperty rdf:resource="&dul;isDescribedBy"/>
      <owl:qualifiedCardinality rdf:datatype="&xsd;nonNegativeInteger">1</owl:qualifiedCardinality>
    </owl:Restriction>
  </rdfs:subClassOf>
  <rdfs:subClassOf rdf:resource="&soma;Extrinsic"/>
  <rdfs:isDefinedBy rdf:resource="http://www.ease-crc.org/ont/SOMA-OBJ.owl"/>
</owl:Class>

<owl:DatatypeProperty rdf:about="&soma;hasReferenceFrame"
    rdfs:label="has reference frame">
  <rdfs:comment>Gives the name associated to the local coordinate frame of a SpaceRegion.</rdfs:comment>
  <rdfs:domain rdf:resource="&dul;SpaceRegion"/>
  <rdfs:isDefinedBy rdf:resource="http://www.ease-crc.org/ont/SOMA-OBJ.owl"/>
  <rdfs:range rdf:resource="&xsd;string"/>
  <rdfs:subPropertyOf rdf:resource="&soma;hasSpaceParameter"/>
</owl:DatatypeProperty>

<owl:ObjectProperty rdf:about="&soma;isTaskDefinedInAffordance"
    rdfs:label="is task defined in affordance">
  <rdfs:subPropertyOf rdf:resource="&soma;isDefinedInAffordance"/>
  <rdfs:subPropertyOf rdf:resource="&dul;isTaskDefinedIn"/>
  <rdfs:comment>A relation between a Task and an Affordance, such that the task is defined in terms of using the affordance.</rdfs:comment>
  <rdfs:domain rdf:resource="&dul;Task"/>
  <rdfs:isDefinedBy rdf:resource="http://www.ease-crc.org/ont/SOMA-OBJ.owl"/>
  <rdfs:range rdf:resource="&soma;Affordance"/>
</owl:ObjectProperty>

<owl:ObjectProperty rdf:about="&soma;isOutputParameterFor"
    rdfs:label="is output parameter for">
  <rdfs:comment>A relation between a Task and one of its output parameters.</rdfs:comment>
  <rdfs:comment>A relation from a Parameter to an EventType (typically, a Task). The parameter describes an outcome of the event classified by the EventType.</rdfs:comment>
  <rdfs:domain rdf:resource="&dul;Parameter"/>
  <rdfs:isDefinedBy rdf:resource="http://www.ease-crc.org/ont/SOMA.owl"/>
  <rdfs:range rdf:resource="&dul;EventType"/>
  <rdfs:subPropertyOf rdf:resource="&dul;isParameterFor"/>
</owl:ObjectProperty>

<owl:DatatypeProperty rdf:about="&soma;hasForceValue"
    rdfs:comment="A value that quantifies a force given in Newton."
    rdfs:label="has force value">
  <rdfs:domain rdf:resource="&soma;ForceAttribute"/>
  <rdfs:isDefinedBy rdf:resource="http://www.ease-crc.org/ont/SOMA-OBJ.owl"/>
  <rdfs:range rdf:resource="&soma;array_double"/>
  <rdfs:subPropertyOf rdf:resource="&dul;hasRegionDataValue"/>
</owl:DatatypeProperty>

<owl:Class rdf:about="&soma;Planning">
  <rdfs:subClassOf>
    <owl:Restriction>
      <owl:onProperty rdf:resource="&dul;isTaskOf"/>
      <owl:someValuesFrom>
        <owl:Restriction>
          <owl:onProperty rdf:resource="&dul;classifies"/>
          <owl:someValuesFrom rdf:resource="&dul;Plan"/>
        </owl:Restriction>
      </owl:someValuesFrom>
    </owl:Restriction>
  </rdfs:subClassOf>
  <rdfs:subClassOf rdf:resource="&soma;Deciding"/>
  <rdfs:comment>A Mental task in which the Agent endeavours to create a sequence of actions for itself which, if followed, will bring about a particular state of affairs in the world. This particular state of affairs is known to the agent and is often called the goal state of the planning action. Planning commits itself to feasibility: the Agent attempts to find a sequence of actions that it believes it will actually be able to perform.</rdfs:comment>
  <rdfs:isDefinedBy rdf:resource="http://www.ease-crc.org/ont/SOMA-ACT.owl"/>
</owl:Class>

<owl:Class rdf:about="&soma;StimulusRole">
  <rdfs:comment>A role classifying an object that is perceived by some agent and thus triggers some reaction (e.g., a perception event).</rdfs:comment>
  <rdfs:isDefinedBy rdf:resource="http://www.ease-crc.org/ont/SOMA-OBJ.owl"/>
  <rdfs:label xml:lang="en">Stimulus role</rdfs:label>
  <rdfs:subClassOf rdf:resource="&soma;CausativeRole"/>
</owl:Class>

<owl:Class rdf:about="&soma;Taxis">
  <rdfs:comment>An innate behavioural response such as the knee-jerk reflex or the sucking reflex of human infants.</rdfs:comment>
  <rdfs:isDefinedBy rdf:resource="http://www.ease-crc.org/ont/SOMA-PROC.owl"/>
  <rdfs:subClassOf rdf:resource="&soma;BodyMovement"/>
</owl:Class>

<owl:Class rdf:about="&soma;LookingFor">
  <rdfs:comment>A task by which an Agent uses its perception apparatus to check for the presence of an object in some specified area.</rdfs:comment>
  <rdfs:isDefinedBy rdf:resource="http://www.ease-crc.org/ont/SOMA-ACT.owl"/>
  <rdfs:label xml:lang="en">Looking for</rdfs:label>
  <rdfs:subClassOf rdf:resource="&soma;Perceiving"/>
</owl:Class>

<owl:Class rdf:about="&soma;Tool">
  <rdfs:comment>A role to classify an object used to modify or actuate others.</rdfs:comment>
  <rdfs:isDefinedBy rdf:resource="http://www.ease-crc.org/ont/SOMA-OBJ.owl"/>
  <rdfs:subClassOf rdf:resource="&soma;Instrument"/>
</owl:Class>

<owl:Class rdf:about="&soma;Orienting">
  <rdfs:comment>A task in which an Agent adjusts the orientation of an object.</rdfs:comment>
  <rdfs:isDefinedBy rdf:resource="http://www.ease-crc.org/ont/SOMA-ACT.owl"/>
  <rdfs:subClassOf rdf:resource="&soma;Positioning"/>
</owl:Class>

<owl:Class rdf:about="&soma;Enclosing">
  <rdfs:subClassOf>
    <owl:Restriction>
      <owl:allValuesFrom rdf:resource="&soma;EnclosedObject"/>
      <owl:onProperty rdf:resource="&soma;affordsTrigger"/>
    </owl:Restriction>
  </rdfs:subClassOf>
  <rdfs:subClassOf rdf:resource="&soma;Containment"/>
  <rdfs:comment>The disposition of an object (the container) to contain other objects by enclosing them to prevent their free movement.</rdfs:comment>
  <rdfs:isDefinedBy rdf:resource="http://www.ease-crc.org/ont/SOMA-OBJ.owl"/>
</owl:Class>

<owl:Class rdf:about="&soma;CoveringTheory">
  <rdfs:subClassOf>
    <owl:Restriction>
      <owl:onProperty rdf:resource="&dul;defines"/>
      <owl:someValuesFrom rdf:resource="&soma;Instrument"/>
    </owl:Restriction>
  </rdfs:subClassOf>
  <rdfs:subClassOf>
    <owl:Restriction>
      <owl:onClass rdf:resource="&soma;Patient"/>
      <owl:onProperty rdf:resource="&dul;defines"/>
      <owl:qualifiedCardinality rdf:datatype="&xsd;nonNegativeInteger">1</owl:qualifiedCardinality>
    </owl:Restriction>
  </rdfs:subClassOf>
  <rdfs:subClassOf rdf:resource="&soma;ExecutableSchematicTheory"/>
  <rdfs:comment>A schematic theory of how an agent can use an instrument to prevent access to the interior of a patient.</rdfs:comment>
  <rdfs:isDefinedBy rdf:resource="http://www.ease-crc.org/ont/SOMA-SAY.owl"/>
  <rdfs:label xml:lang="en">Covering theory</rdfs:label>
</owl:Class>

<owl:Class rdf:about="&soma;Color"
    rdfs:label="Color">
  <rdfs:subClassOf>
    <owl:Restriction>
      <owl:onProperty rdf:resource="&dul;hasRegion"/>
      <owl:someValuesFrom rdf:resource="&soma;ColorRegion"/>
    </owl:Restriction>
  </rdfs:subClassOf>
  <rdfs:subClassOf>
    <owl:Restriction>
      <owl:allValuesFrom rdf:resource="&soma;ColorRegion"/>
      <owl:onProperty rdf:resource="&dul;hasRegion"/>
    </owl:Restriction>
  </rdfs:subClassOf>
  <rdfs:subClassOf rdf:resource="&soma;Extrinsic"/>
  <rdfs:comment>The color of an object. Color regions encode the color value in some space such as RGB or HSV, and may further be used to classify the color as red, dark, etc. The color of an object may have different facets, e.g. a red and blue color.</rdfs:comment>
  <rdfs:isDefinedBy rdf:resource="http://www.ease-crc.org/ont/SOMA-OBJ.owl"/>
</owl:Class>

<owl:Class rdf:about="&soma;GraphDatabase">
  <rdfs:comment xml:lang="en">A Graph Database is a Database that uses graph structures for semantic queries with nodes, edges, and properties to represent and store data.</rdfs:comment>
  <rdfs:isDefinedBy rdf:resource="http://www.ease-crc.org/ont/SOMA-IO.owl"/>
  <rdfs:label xml:lang="en">Graph database</rdfs:label>
  <rdfs:subClassOf rdf:resource="&soma;Database"/>
</owl:Class>

<owl:Class rdf:about="&soma;SubCognitiveAgent">
  <rdfs:comment xml:lang="en">An agent that is not capable to act on its own, i.e., that is reactive. Its intentionality needs to be bestowed upon from some other agent, that it acts for.</rdfs:comment>
  <rdfs:isDefinedBy rdf:resource="http://www.ease-crc.org/ont/SOMA-IO.owl"/>
  <rdfs:label xml:lang="en">Sub-cognitive agent</rdfs:label>
  <rdfs:subClassOf rdf:resource="&dul;Agent"/>
</owl:Class>

<owl:Class rdf:about="&soma;DerivingInformation"
    rdfs:label="Deriving information">
  <rdfs:subClassOf>
    <owl:Class>
      <owl:intersectionOf rdf:parseType="Collection">

        <owl:Restriction>
          <owl:onProperty rdf:resource="&soma;isTaskOfInputRole"/>
          <owl:someValuesFrom rdf:resource="&soma;Premise"/>
        </owl:Restriction>

        <owl:Restriction>
          <owl:onProperty rdf:resource="&soma;isTaskOfOutputRole"/>
          <owl:someValuesFrom rdf:resource="&soma;Conclusion"/>
        </owl:Restriction>
      </owl:intersectionOf>
    </owl:Class>
  </rdfs:subClassOf>
  <rdfs:subClassOf rdf:resource="&soma;InformationAcquisition"/>
  <rdfs:isDefinedBy rdf:resource="http://www.ease-crc.org/ont/SOMA-ACT.owl"/>
</owl:Class>

<dul:Action rdf:about="action1">
  <soma:actionType rdf:resource="&soma;PickingUp"/>
  <soma:hasObject rdf:resource="object1"/>
  <soma:hasSource rdf:resource="location1"/>
</dul:Action>

<owl:ObjectProperty rdf:about="&soma;affordsPerformer">
  <rdfs:comment xml:lang="en">Relates a disposition to the performer role defined by the affordance describing the disposition.</rdfs:comment>
  <rdfs:domain rdf:resource="&soma;Disposition"/>
  <rdfs:isDefinedBy rdf:resource="http://www.ease-crc.org/ont/SOMA-OBJ.owl"/>
  <rdfs:label xml:lang="en">affords performer</rdfs:label>
  <rdfs:range rdf:resource="&dul;Role"/>
  <rdfs:subPropertyOf rdf:resource="&soma;affordsConcept"/>
  <owl:inverseOf rdf:resource="&soma;isPerformerAffordedBy"/>
  <owl:propertyChainAxiom rdf:parseType="Collection">
    <rdf:Description rdf:about="&dul;isDescribedBy"/>
    <rdf:Description rdf:about="&soma;definesPerformer"/>
  </owl:propertyChainAxiom>
</owl:ObjectProperty>

<owl:ObjectProperty rdf:about="&soma;isBearerDefinedIn"
    rdfs:label="is bearer defined in">
  <rdfs:comment>Relates an affordance which is a relation between a bearer and a trigger, to the role of the bearer when the affordance is manifested.</rdfs:comment>
  <rdfs:domain rdf:resource="&dul;Role"/>
  <rdfs:isDefinedBy rdf:resource="http://www.ease-crc.org/ont/SOMA-OBJ.owl"/>
  <rdfs:range rdf:resource="&soma;Affordance"/>
  <rdfs:subPropertyOf rdf:resource="&dul;isRoleDefinedIn"/>
</owl:ObjectProperty>

<owl:Class rdf:about="&soma;ArchiveText">
  <owl:equivalentClass>
    <owl:Class>
      <owl:intersectionOf rdf:parseType="Collection">
        <rdf:Description rdf:about="&soma;Structured_Text"/>
        <owl:Restriction>
          <owl:onProperty rdf:resource="&dul;expresses"/>
          <owl:someValuesFrom rdf:resource="&soma;FileConfiguration"/>
        </owl:Restriction>
      </owl:intersectionOf>
    </owl:Class>
  </owl:equivalentClass>
  <owl:equivalentClass>
    <owl:Restriction>
      <owl:onProperty rdf:resource="&soma;isGivenMeaningBy"/>
      <owl:someValuesFrom rdf:resource="&soma;ArchiveFormat"/>
    </owl:Restriction>
  </owl:equivalentClass>
  <rdfs:comment xml:lang="en">An Archive is a Structured Text that is composed of one or more Structured Texts along with metadata. Archives are used to collect multiple texts together into a single text for easier portability and storage as Archive Files, or simply to compress text to use less storage space as Computer Files. Archive often store directory structures, error detection and correction information, arbitrary comments, and sometimes use built-in encryption.

Source: https://en.wikipedia.org/wiki/Archive_file</rdfs:comment>
  <rdfs:isDefinedBy rdf:resource="http://www.ease-crc.org/ont/SOMA-IO.owl"/>
  <rdfs:label xml:lang="en">Archive Text</rdfs:label>
</owl:Class>

<owl:Class rdf:about="&soma;DesignedComponent"
    rdfs:comment="An object designed to be part or element of a larger whole."
    rdfs:label="Designed component">
  <rdfs:subClassOf>
    <owl:Restriction>
      <owl:onProperty rdf:resource="&soma;hasDisposition"/>
      <owl:someValuesFrom rdf:resource="&soma;Connectivity"/>
    </owl:Restriction>
  </rdfs:subClassOf>
  <rdfs:subClassOf rdf:resource="&soma;FunctionalPart"/>
  <rdfs:subClassOf rdf:resource="&dul;DesignedArtifact"/>
  <rdfs:isDefinedBy rdf:resource="http://www.ease-crc.org/ont/SOMA-OBJ.owl"/>
</owl:Class>

<owl:ObjectProperty rdf:about="&dul;hasPostcondition">
  <rdfs:comment>This should be taken to mean that the postcondition is the situation expected to follow the current situation. Whether the expectation is met is another issue.</rdfs:comment>
</owl:ObjectProperty>

<owl:Class rdf:about="&soma;ArchiveFormat">
  <rdfs:subClassOf>
    <owl:Restriction>
      <owl:allValuesFrom rdf:resource="&soma;ArchiveText"/>
      <owl:onProperty rdf:resource="&soma;givesMeaningTo"/>
    </owl:Restriction>
  </rdfs:subClassOf>
  <rdfs:subClassOf rdf:resource="&soma;File_format"/>
  <rdfs:comment xml:lang="en">An Archive Format is the file format of an archive file.

Source: https://en.wikipedia.org/wiki/Archive_file#Archive_formats</rdfs:comment>
  <rdfs:isDefinedBy rdf:resource="http://www.ease-crc.org/ont/SOMA-IO.owl"/>
  <rdfs:label xml:lang="en">Archive Format</rdfs:label>
</owl:Class>

<owl:Class rdf:about="&soma;Flying">
  <owl:disjointWith rdf:resource="&soma;Swimming"/>
  <owl:disjointWith rdf:resource="&soma;Walking"/>
  <rdfs:comment>A process type classifying a motion of a body that, through its own power, keeps itself aloft.</rdfs:comment>
  <rdfs:isDefinedBy rdf:resource="http://www.ease-crc.org/ont/SOMA-PROC.owl"/>
  <rdfs:subClassOf rdf:resource="&soma;Locomotion"/>
</owl:Class>

<owl:Class rdf:about="&soma;Gripper"
    rdfs:comment="A mechanical device that grasps and holds things.">
  <rdfs:isDefinedBy rdf:resource="http://www.ease-crc.org/ont/SOMA-OBJ.owl"/>
  <rdfs:subClassOf rdf:resource="&soma;PrehensileEffector"/>
</owl:Class>

<owl:ObjectProperty rdf:about="&soma;hasEndLink"
    rdfs:label="has end link">
  <rdfs:comment>Relates an object to kinematic components at the end of the kinematic chain.</rdfs:comment>
  <rdfs:domain rdf:resource="&dul;PhysicalObject"/>
  <rdfs:isDefinedBy rdf:resource="http://www.ease-crc.org/ont/SOMA-OBJ.owl"/>
  <rdfs:range rdf:resource="&dul;PhysicalObject"/>
  <rdfs:subPropertyOf rdf:resource="&soma;hasLink"/>
  <owl:inverseOf rdf:resource="&soma;isEndLinkOf"/>
</owl:ObjectProperty>

<owl:Class rdf:about="&soma;Deposit">
  <rdfs:comment>A role classifying an object ontop which others are put to e.g. store them, or to place them in a meaningful way for future activities.</rdfs:comment>
  <rdfs:isDefinedBy rdf:resource="http://www.ease-crc.org/ont/SOMA-OBJ.owl"/>
  <rdfs:subClassOf rdf:resource="&soma;Instrument"/>
</owl:Class>

<owl:Class rdf:about="&soma;AbductiveReasoning">
  <rdfs:comment>A task in which the Agent proceeds from some set of statements about a world, and attempts to obtain an explanation for these statements. This explanation is often an inferred cause, such as a final cause or intention. Further, it is often required that there be some guarantees that the explanation produced by AbductiveReasoning have some desirable property, such as being the simplest or most likely given the set of statements to explain.</rdfs:comment>
  <rdfs:isDefinedBy rdf:resource="http://www.ease-crc.org/ont/SOMA-ACT.owl"/>
  <rdfs:label xml:lang="en">Abductive reasoning</rdfs:label>
  <rdfs:subClassOf rdf:resource="&soma;Reasoning"/>
</owl:Class>

<owl:ObjectProperty rdf:about="&soma;hasDisposition"
    rdfs:comment="Associates an object to one of its dispositions."
    rdfs:label="has disposition">
  <rdfs:domain rdf:resource="&dul;Object"/>
  <rdfs:isDefinedBy rdf:resource="http://www.ease-crc.org/ont/SOMA-OBJ.owl"/>
  <rdfs:range rdf:resource="&soma;Disposition"/>
  <rdfs:subPropertyOf rdf:resource="&dul;hasQuality"/>
  <owl:inverseOf rdf:resource="&soma;isDispositionOf"/>
</owl:ObjectProperty>

<owl:Class rdf:about="&soma;StateType"
    rdfs:comment="An EventType that classifies States.">
  <rdfs:subClassOf>
    <owl:Restriction>
      <owl:allValuesFrom rdf:resource="&soma;State"/>
      <owl:onProperty rdf:resource="&dul;classifies"/>
    </owl:Restriction>
  </rdfs:subClassOf>
  <rdfs:subClassOf>
    <owl:Restriction>
      <owl:allValuesFrom rdf:resource="&soma;StateType"/>
      <owl:onProperty rdf:resource="&dul;hasPart"/>
    </owl:Restriction>
  </rdfs:subClassOf>
  <rdfs:subClassOf rdf:resource="&dul;EventType"/>
  <rdfs:isDefinedBy rdf:resource="http://www.ease-crc.org/ont/SOMA-STATE.owl"/>
  <rdfs:label xml:lang="en">State type</rdfs:label>
</owl:Class>

<owl:Class rdf:about="&soma;ThinkAloudTopic"
    rdfs:comment="A topic relevant for a think-aloud communication.">
  <rdfs:isDefinedBy rdf:resource="http://www.ease-crc.org/ont/SOMA-ACT.owl"/>
  <rdfs:label xml:lang="en">Think aloud topic</rdfs:label>
  <rdfs:subClassOf rdf:resource="&soma;CommunicationTopic"/>
</owl:Class>

<owl:ObjectProperty rdf:about="&soma;hasLocalization"
    rdfs:comment="Relates an object to its localization quality."
    rdfs:label="has localization">
  <rdfs:domain rdf:resource="&dul;PhysicalObject"/>
  <rdfs:isDefinedBy rdf:resource="http://www.ease-crc.org/ont/SOMA-OBJ.owl"/>
  <rdfs:range rdf:resource="&soma;Localization"/>
  <rdfs:subPropertyOf rdf:resource="&dul;hasQuality"/>
  <owl:inverseOf rdf:resource="&soma;isLocalizationOf"/>
</owl:ObjectProperty>

<owl:Axiom>
  <rdfs:comment>If a transition has a terminal situation then it also has a manifestation.</rdfs:comment>
  <owl:annotatedProperty rdf:resource="&rdfs;subClassOf"/>
  <owl:annotatedSource>
    <owl:Restriction>
      <rdfs:subClassOf>
        <owl:Restriction rdf:nodeID="bn6">
          <owl:onProperty rdf:resource="http://www.ease-crc.org/ont/SOMA.owl/manifestsIn"/>
          <owl:someValuesFrom rdf:resource="&dul;Event"/>
        </owl:Restriction>
      </rdfs:subClassOf>
      <owl:onProperty rdf:resource="&soma;hasTerminalSituation"/>
      <owl:someValuesFrom rdf:resource="&dul;Situation"/>
    </owl:Restriction>
  </owl:annotatedSource>
  <owl:annotatedTarget rdf:nodeID="bn6"/>
</owl:Axiom>

<owl:Class rdf:about="&soma;ForgettingIncorrectInformation">
  <rdfs:comment xml:lang="en">A mental task in which the executing agent aims to correct its present information by deleting an incorrect information.</rdfs:comment>
  <rdfs:isDefinedBy rdf:resource="http://www.ease-crc.org/ont/SOMA-ACT.owl"/>
  <rdfs:label xml:lang="en">Forgetting incorrect information</rdfs:label>
  <rdfs:subClassOf rdf:resource="&soma;InformationDismissal"/>
</owl:Class>

<owl:Class rdf:about="&soma;Instrument"
    rdfs:comment="An object used to carry out the event.">
  <rdfs:isDefinedBy rdf:resource="http://www.ease-crc.org/ont/SOMA-OBJ.owl"/>
  <rdfs:isDefinedBy rdf:resource="http://www.ease-crc.org/ont/SOMA-SAY.owl"/>
  <rdfs:subClassOf rdf:resource="&soma;ResourceRole"/>
</owl:Class>

<owl:ObjectProperty rdf:about="&soma;affordsBearer"
    rdfs:label="affords bearer">
  <rdfs:comment>Relates a disposition to the bearer role defined by the affordance describing the disposition.</rdfs:comment>
  <rdfs:domain rdf:resource="&soma;Disposition"/>
  <rdfs:isDefinedBy rdf:resource="http://www.ease-crc.org/ont/SOMA-OBJ.owl"/>
  <rdfs:range rdf:resource="&dul;Role"/>
  <rdfs:subPropertyOf rdf:resource="&soma;affordsConcept"/>
  <owl:inverseOf rdf:resource="&soma;isBearerAffordedBy"/>
  <owl:propertyChainAxiom rdf:parseType="Collection">
    <rdf:Description rdf:about="&dul;isDescribedBy"/>
    <rdf:Description rdf:about="&soma;definesBearer"/>
  </owl:propertyChainAxiom>
</owl:ObjectProperty>

<owl:ObjectProperty rdf:about="&dul;hasPrecondition">
  <rdfs:comment>This should be taken to mean: a precondition is a situation without which the current situation would not be possible.</rdfs:comment>
</owl:ObjectProperty>

<owl:Class rdf:about="&soma;FunctionalDiagnosis"
    rdfs:comment="An internal diagnosis of a system."
    rdfs:label="Functional diagnosis">
  <rdfs:isDefinedBy rdf:resource="http://www.ease-crc.org/ont/SOMA.owl"/>
  <rdfs:subClassOf rdf:resource="&dul;Diagnosis"/>
</owl:Class>

<owl:ObjectProperty rdf:about="&soma;isReplacedBy">
  <rdfs:comment xml:lang="en">The relation between a State that is replaced by another, e.g., the state of a bowl of fruits containing some objects is replaced by a new containment state when one object is taken away (in this example, we simplified the relation between the State and its type).</rdfs:comment>
  <rdfs:domain rdf:resource="&soma;State"/>
  <rdfs:isDefinedBy rdf:resource="http://www.ease-crc.org/ont/SOMA-ACT.owl"/>
  <rdfs:label xml:lang="en">is replaced by</rdfs:label>
  <rdfs:range rdf:resource="&soma;State"/>
  <rdfs:subPropertyOf rdf:resource="&soma;before"/>
  <owl:inverseOf rdf:resource="&soma;replaces"/>
  <owl:propertyChainAxiom rdf:parseType="Collection">
    <rdf:Description rdf:about="&dul;isEventIncludedIn"/>
    <rdf:Description rdf:about="&soma;isInitialSituationOf"/>
    <rdf:Description rdf:about="&soma;hasTerminalSituation"/>
    <rdf:Description rdf:about="&dul;includesEvent"/>
  </owl:propertyChainAxiom>
</owl:ObjectProperty>

<owl:AnnotationProperty rdf:about="&soma;symbol">
  <rdfs:comment>An annotation property which should be used to record by what symbols or abbreviations, if any, some relation or entity is known in scientific literature.</rdfs:comment>
  <rdfs:isDefinedBy rdf:resource="http://www.ease-crc.org/ont/SOMA.owl"/>
  <rdfs:range rdf:resource="&xsd;string"/>
</owl:AnnotationProperty>

<owl:Class rdf:about="&soma;LinkedObject"
    rdfs:comment="An object that is linked to some other object.">
  <rdfs:isDefinedBy rdf:resource="http://www.ease-crc.org/ont/SOMA-OBJ.owl"/>
  <rdfs:isDefinedBy rdf:resource="http://www.ease-crc.org/ont/SOMA-STATE.owl"/>
  <rdfs:label xml:lang="en">Linked object</rdfs:label>
  <rdfs:subClassOf rdf:resource="&soma;ConnectedObject"/>
</owl:Class>

<owl:Class rdf:about="&soma;BodyMovement">
  <rdfs:subClassOf>
    <owl:Restriction>
      <owl:allValuesFrom>
        <owl:Class>
          <owl:unionOf rdf:parseType="Collection">

            <owl:Restriction>
              <owl:onProperty rdf:resource="&dul;hasParticipant"/>
              <owl:someValuesFrom rdf:resource="&dul;PhysicalAgent"/>
            </owl:Restriction>

            <owl:Restriction>
              <owl:onProperty rdf:resource="&dul;hasParticipant"/>
              <owl:someValuesFrom>
                <owl:Class>
                  <owl:intersectionOf rdf:parseType="Collection">
                    <rdf:Description rdf:about="&dul;PhysicalObject"/>
                    <owl:Restriction>
                      <owl:onProperty rdf:resource="&dul;isPartOf"/>
                      <owl:someValuesFrom rdf:resource="&dul;PhysicalAgent"/>
                    </owl:Restriction>
                  </owl:intersectionOf>
                </owl:Class>
              </owl:someValuesFrom>
            </owl:Restriction>
          </owl:unionOf>
        </owl:Class>
      </owl:allValuesFrom>
      <owl:onProperty rdf:resource="&dul;classifies"/>
    </owl:Restriction>
  </rdfs:subClassOf>
  <rdfs:subClassOf rdf:resource="&soma;Motion"/>
  <rdfs:comment>Motion described in terms of how parts of an Agent's body move.

As such, this concept can be applied only to motions involving some PhysicalAgent, or body parts of a PhysicalAgent.</rdfs:comment>
  <rdfs:isDefinedBy rdf:resource="http://www.ease-crc.org/ont/SOMA-PROC.owl"/>
</owl:Class>

<owl:Class rdf:about="&soma;InterfaceComponentRole">
  <rdfs:isDefinedBy rdf:resource="http://www.ease-crc.org/ont/SOMA-IO.owl"/>
  <rdfs:label xml:lang="en">Interface component role</rdfs:label>
  <rdfs:subClassOf rdf:resource="&soma;SoftwareRole"/>
  <owl:equivalentClass>
    <owl:Class>
      <owl:intersectionOf rdf:parseType="Collection">
        <rdf:Description rdf:about="&soma;SoftwareRole"/>
        <owl:Restriction>
          <owl:allValuesFrom rdf:resource="&soma;InterfaceSpecification"/>
          <owl:onProperty rdf:resource="&dul;isDefinedIn"/>
        </owl:Restriction>
      </owl:intersectionOf>
    </owl:Class>
  </owl:equivalentClass>
</owl:Class>

<owl:Class rdf:about="&soma;MeshShape"
    rdfs:comment="A solid geometrical figure described in a mesh file."
    rdfs:label="Mesh shape">
  <rdfs:subClassOf>
    <owl:Restriction>
      <owl:onDataRange rdf:resource="&xsd;string"/>
      <owl:onProperty rdf:resource="&soma;hasFilePath"/>
      <owl:qualifiedCardinality rdf:datatype="&xsd;nonNegativeInteger">1</owl:qualifiedCardinality>
    </owl:Restriction>
  </rdfs:subClassOf>
  <rdfs:subClassOf>
    <owl:Restriction>
      <owl:maxQualifiedCardinality rdf:datatype="&xsd;nonNegativeInteger">1</owl:maxQualifiedCardinality>
      <owl:onDataRange rdf:resource="&soma;array_double"/>
      <owl:onProperty rdf:resource="&soma;hasShapeScale"/>
    </owl:Restriction>
  </rdfs:subClassOf>
  <rdfs:subClassOf rdf:resource="&soma;ShapeRegion"/>
  <rdfs:isDefinedBy rdf:resource="http://www.ease-crc.org/ont/SOMA-OBJ.owl"/>
</owl:Class>

<owl:ObjectProperty rdf:about="&soma;starts"
    soma:symbol="s">
  <rdf:type rdf:resource="&owl;TransitiveProperty"/>
  <rdfs:comment>`A starts B` means that A starts exactly where B starts, and that A strictly ends before B. As in "I start my day with a coffee".</rdfs:comment>
  <rdfs:domain rdf:resource="&dul;Event"/>
  <rdfs:isDefinedBy rdf:resource="http://www.ease-crc.org/ont/SOMA.owl"/>
  <rdfs:range rdf:resource="&dul;Event"/>
  <rdfs:subPropertyOf rdf:resource="&soma;coOccurs"/>
</owl:ObjectProperty>

<owl:DatatypeProperty rdf:about="&soma;hasEventBegin"
    rdfs:label="has event begin">
  <rdfs:comment>A relation recording when an Event started. In this case, we think of the Event as something unfolding over some span of time.</rdfs:comment>
  <rdfs:domain rdf:resource="&dul;Event"/>
  <rdfs:isDefinedBy rdf:resource="http://www.ease-crc.org/ont/SOMA.owl"/>
  <rdfs:range rdf:resource="&xsd;double"/>
  <rdfs:subPropertyOf rdf:resource="&soma;hasEventTime"/>
</owl:DatatypeProperty>

<owl:Class rdf:about="&soma;Tapping">
  <rdfs:comment>A motion, usually repeated several times, for example, to probe the surface of an object.</rdfs:comment>
  <rdfs:isDefinedBy rdf:resource="http://www.ease-crc.org/ont/SOMA-PROC.owl"/>
  <rdfs:subClassOf rdf:resource="&soma;DirectedMotion"/>
</owl:Class>

<owl:ObjectProperty rdf:about="&soma;replaces">
  <rdfs:comment xml:lang="en">The relation between a State that replaces another, e.g., the state of a bowl of fruits containing some objects is replaced by a new containment state when one object is taken away (in this example, we simplified the relation between the State and its type).</rdfs:comment>
  <rdfs:domain rdf:resource="&soma;State"/>
  <rdfs:isDefinedBy rdf:resource="http://www.ease-crc.org/ont/SOMA-ACT.owl"/>
  <rdfs:label xml:lang="en">replaces</rdfs:label>
  <rdfs:range rdf:resource="&soma;State"/>
  <rdfs:subPropertyOf rdf:resource="&soma;after"/>
  <owl:propertyChainAxiom rdf:parseType="Collection">
    <rdf:Description rdf:about="&dul;isEventIncludedIn"/>
    <rdf:Description rdf:about="&soma;isTerminalSituationOf"/>
    <rdf:Description rdf:about="&soma;hasInitialSituation"/>
    <rdf:Description rdf:about="&dul;includesEvent"/>
  </owl:propertyChainAxiom>
</owl:ObjectProperty>

<owl:Class rdf:about="&soma;Binding">
  <rdfs:subClassOf>
    <owl:Class>
      <owl:unionOf rdf:parseType="Collection">
        <rdf:Description rdf:about="&soma;CounterfactualBinding"/>
        <rdf:Description rdf:about="&soma;FactualBinding"/>
      </owl:unionOf>
    </owl:Class>
  </rdfs:subClassOf>
  <rdfs:subClassOf>
    <owl:Class>
      <owl:unionOf rdf:parseType="Collection">
        <rdf:Description rdf:about="&soma;RoleFillerBinding"/>
        <rdf:Description rdf:about="&soma;RoleRoleBinding"/>
      </owl:unionOf>
    </owl:Class>
  </rdfs:subClassOf>
  <rdfs:subClassOf>
    <owl:Restriction>
      <owl:onProperty>
        <rdf:Description>
          <owl:inverseOf rdf:resource="&soma;hasBinding"/>
        </rdf:Description>
      </owl:onProperty>
      <owl:someValuesFrom rdf:resource="&dul;Description"/>
    </owl:Restriction>
  </rdfs:subClassOf>
  <rdfs:subClassOf>
    <owl:Restriction>
      <owl:onClass rdf:resource="&dul;Entity"/>
      <owl:onProperty rdf:resource="&soma;hasBindingFiller"/>
      <owl:qualifiedCardinality rdf:datatype="&xsd;nonNegativeInteger">1</owl:qualifiedCardinality>
    </owl:Restriction>
  </rdfs:subClassOf>
  <rdfs:subClassOf>
    <owl:Restriction>
      <owl:onClass>
        <owl:Class>
          <owl:unionOf rdf:parseType="Collection">
            <rdf:Description rdf:about="&dul;Parameter"/>
            <rdf:Description rdf:about="&dul;Role"/>
          </owl:unionOf>
        </owl:Class>
      </owl:onClass>
      <owl:onProperty rdf:resource="&soma;hasBindingRole"/>
      <owl:qualifiedCardinality rdf:datatype="&xsd;nonNegativeInteger">1</owl:qualifiedCardinality>
    </owl:Restriction>
  </rdfs:subClassOf>
  <rdfs:subClassOf rdf:resource="&dul;Relation"/>
  <rdfs:comment>A Relation between Roles/Parameters and their fillers that holds in a particular descriptive context, such as a Workflow or Narrative.

It covers two conceptually related, but somewhat ontologically distinct situations:

-- a binding between two Roles, or two Parameters, with the meaning that in the particular descriptive context where the Binding holds, a filler for one Role/Parameter is also a filler for the other
-- a binding between a Role/Parameter and an Entity able to fill that Role/Parameter, with the meaning that in the particular descriptive context where the Binding holds, the Entity fills the Role/Parameter.

Note: in the second case, the Entity filling the Role/Parameter may be a Role or Parameter itself. This however does NOT reduce to the first case. Consider these examples:

-- (first situation) The accountant is also the lawyer. In this case, there are two roles, and there is a person filling both of them. This is a factual, role-role binding.
-- (second situation, linking to a generic Entity) The accountant is Bob. In this case, there is a factual, role-filler binding asserting who fills the accountant role.
-- (second situation, linking to a role) The newly opened job is accountant. In this case, there is a factual, role-filler binding asserting that some role is filled by another, without making any assertion about the filler of this second role. It is not known, and not important, whether an accountant exists at this time.

There is a further, orthogonal distinction made between:
-- factual: the Binding is asserted to hold in the descriptive context
-- counterfactual: the Binding is used to express conditions in the descriptive context. A counterfactual Binding is not meant as an assertion that the Binding actually holds.</rdfs:comment>
  <rdfs:isDefinedBy rdf:resource="http://www.ease-crc.org/ont/SOMA-WF.owl"/>
</owl:Class>

<owl:Class rdf:about="&soma;DestroyedObject"
    rdfs:comment="An object that is detroyed.">
  <rdfs:isDefinedBy rdf:resource="http://www.ease-crc.org/ont/SOMA-OBJ.owl"/>
  <rdfs:isDefinedBy rdf:resource="http://www.ease-crc.org/ont/SOMA-PROC.owl"/>
  <rdfs:label xml:lang="en">Destroyed object</rdfs:label>
  <rdfs:subClassOf rdf:resource="&soma;Patient"/>
</owl:Class>

<owl:ObjectProperty rdf:about="&soma;finishes"
    soma:symbol="f">
  <rdf:type rdf:resource="&owl;TransitiveProperty"/>
  <rdfs:comment>`A finishes B` means that A ends exactly where B ends, and that B strictly starts before A.  As in "I finish my day by taking a shower".</rdfs:comment>
  <rdfs:domain rdf:resource="&dul;Event"/>
  <rdfs:isDefinedBy rdf:resource="http://www.ease-crc.org/ont/SOMA.owl"/>
  <rdfs:range rdf:resource="&dul;Event"/>
  <rdfs:subPropertyOf rdf:resource="&soma;coOccurs"/>
</owl:ObjectProperty>

<owl:Class rdf:about="&dul;InformationObject">
  <rdfs:comment>In SOMA-compliant systems, the way to use InformationObjects to specify extra data about an individual entity is to employ the 'is about' and 'expresses' properties (or their inverses 'is reference of' and 'is expressed by') and to supply a persistent identifier for a realization of the InformationObject.

As a prototypical example, consider an individual called Action_XYZ, about which we have some data for which the meaning is described by Description_ABC. The data would be an individual InformationObject_DEF, and the following property assertions would hold:

InformationObject_DEF 'is about' Action_XYZ
InformationObject_DEF expresses Description_ABC


Usually, an individual InformationObject would be connected to (at least) an InformationRealization individual. For example, suppose there is such an InformationRealization individual, InformationRealization_123. Then, this individual will have data properties describing its format and persistent identifier

InformationRealization_123 hasPersistentIdentifier 'doi'
InformationRealization_123 hasDataFormat 'urdf'</rdfs:comment>
</owl:Class>

<owl:Class rdf:about="&soma;Feature">
  <rdfs:subClassOf>
    <owl:Restriction>
      <owl:allValuesFrom rdf:resource="&soma;Feature"/>
      <owl:onProperty rdf:resource="&dul;hasPart"/>
    </owl:Restriction>
  </rdfs:subClassOf>
  <rdfs:subClassOf>
    <owl:Restriction>
      <owl:onClass rdf:resource="&dul;PhysicalObject"/>
      <owl:onProperty rdf:resource="&soma;isFeatureOf"/>
      <owl:qualifiedCardinality rdf:datatype="&xsd;nonNegativeInteger">1</owl:qualifiedCardinality>
    </owl:Restriction>
  </rdfs:subClassOf>
  <rdfs:subClassOf rdf:resource="&dul;Object"/>
  <owl:disjointWith rdf:resource="&dul;Agent"/>
  <owl:disjointWith rdf:resource="&dul;PhysicalObject"/>
  <owl:disjointWith rdf:resource="&dul;SocialObject"/>
  <rdfs:comment>Features are 'parasitic' entities that only exist insofar their host exists. Typical examples are holes, bumps, boundaries, or spots of color.</rdfs:comment>
  <rdfs:isDefinedBy rdf:resource="http://www.ease-crc.org/ont/SOMA-OBJ.owl"/>
</owl:Class>

<owl:Class rdf:about="&soma;Infeasibility">
  <rdfs:comment>A description of a situation with a goal that is impossible to achieve in some situational context.</rdfs:comment>
  <rdfs:isDefinedBy rdf:resource="http://www.ease-crc.org/ont/SOMA.owl"/>
  <rdfs:subClassOf rdf:resource="&soma;Unsuccessfulness"/>
</owl:Class>

<owl:Class rdf:about="&soma;RelationalQueryLanguage">
  <rdfs:comment xml:lang="en">A Query Language that is designed for communication with some Relational Database.</rdfs:comment>
  <rdfs:isDefinedBy rdf:resource="http://www.ease-crc.org/ont/SOMA-IO.owl"/>
  <rdfs:label xml:lang="en">Relational query language</rdfs:label>
  <rdfs:subClassOf rdf:resource="&soma;QueryLanguage"/>
</owl:Class>

<owl:Class rdf:about="&soma;AreaSurveying">
  <rdfs:comment>A task in which an Agent uses its perception apparatus to gain information about some location.</rdfs:comment>
  <rdfs:isDefinedBy rdf:resource="http://www.ease-crc.org/ont/SOMA-ACT.owl"/>
  <rdfs:label xml:lang="en">Area surveying</rdfs:label>
  <rdfs:subClassOf rdf:resource="&soma;Perceiving"/>
</owl:Class>

<owl:ObjectProperty rdf:about="&soma;hasMassAttribute"
    rdfs:comment="A relation between physical objects and their mass."
    rdfs:label="has mass attribute">
  <rdfs:domain rdf:resource="&dul;PhysicalObject"/>
  <rdfs:isDefinedBy rdf:resource="http://www.ease-crc.org/ont/SOMA-OBJ.owl"/>
  <rdfs:range rdf:resource="&soma;MassAttribute"/>
  <rdfs:subPropertyOf rdf:resource="&dul;hasRegion"/>
  <owl:inverseOf rdf:resource="&soma;isMassAttributeOf"/>
</owl:ObjectProperty>

<owl:ObjectProperty rdf:about="&soma;isGivenMeaningBy">
  <rdfs:comment xml:lang="en">The relation between an Information Object and a System that gives meaning to said object, e.g., a word, sentence, text, etc. might be given meaning by a Language and without the knowledge of said System (Language), the text will not make sense to a reader.</rdfs:comment>
  <rdfs:domain rdf:resource="&dul;InformationObject"/>
  <rdfs:isDefinedBy rdf:resource="http://www.ease-crc.org/ont/SOMA-IO.owl"/>
  <rdfs:label xml:lang="en">is given meaning by</rdfs:label>
  <rdfs:range rdf:resource="&soma;System"/>
  <rdfs:subPropertyOf rdf:resource="&dul;associatedWith"/>
</owl:ObjectProperty>

<owl:Class rdf:about="&soma;PlanarJoint"
    rdfs:label="Planar joint">
  <rdfs:comment>A joint that allows motion in a plane perpendicular to an axis.</rdfs:comment>
  <rdfs:isDefinedBy rdf:resource="http://www.ease-crc.org/ont/SOMA-OBJ.owl"/>
  <rdfs:subClassOf rdf:resource="&soma;MovableJoint"/>
</owl:Class>

<owl:Class rdf:about="&soma;Driving">
  <owl:disjointWith rdf:resource="&soma;Flying"/>
  <owl:disjointWith rdf:resource="&soma;Swimming"/>
  <owl:disjointWith rdf:resource="&soma;Walking"/>
  <rdfs:comment>A process type classifying a motion of a body that exists because this body is attached to and controls some other moving body, usually a vehicle.</rdfs:comment>
  <rdfs:isDefinedBy rdf:resource="http://www.ease-crc.org/ont/SOMA-PROC.owl"/>
  <rdfs:subClassOf rdf:resource="&soma;Locomotion"/>
</owl:Class>

<owl:ObjectProperty rdf:about="&soma;isPerformerAffordedBy">
  <rdfs:label xml:lang="en">Relates a disposition to the performer role defined by the affordance describing the disposition.</rdfs:label>
  <rdfs:label xml:lang="en">is performer afforded by</rdfs:label>
  <rdfs:domain rdf:resource="&dul;Role"/>
  <rdfs:isDefinedBy rdf:resource="http://www.ease-crc.org/ont/SOMA-OBJ.owl"/>
  <rdfs:range rdf:resource="&soma;Disposition"/>
  <rdfs:subPropertyOf rdf:resource="&soma;isConceptAffordedBy"/>
  <owl:propertyChainAxiom rdf:parseType="Collection">
    <rdf:Description rdf:about="&soma;isPerformerDefinedIn"/>
    <rdf:Description rdf:about="&dul;describes"/>
  </owl:propertyChainAxiom>
</owl:ObjectProperty>

<owl:ObjectProperty rdf:about="&dul;isParameterFor"/>

<owl:ObjectProperty rdf:about="&dul;isTaskDefinedIn">
  <rdfs:subPropertyOf rdf:resource="&soma;isEventTypeDefinedIn"/>
</owl:ObjectProperty>

<owl:Class rdf:about="&soma;Conclusion"
    rdfs:label="Conclusions">
  <rdfs:subClassOf rdf:resource="&soma;CreatedObject"/>
  <rdfs:subClassOf rdf:resource="&soma;Knowledge"/>
  <rdfs:comment>An object that is derived from some premise using some inference rules.</rdfs:comment>
  <rdfs:isDefinedBy rdf:resource="http://www.ease-crc.org/ont/SOMA-ACT.owl"/>
</owl:Class>

<owl:Class rdf:about="&soma;OrderedElement">
  <rdfs:subClassOf>
    <owl:Restriction>
      <owl:allValuesFrom rdf:resource="&soma;OrderedElement"/>
      <owl:onProperty rdf:resource="&dul;follows"/>
    </owl:Restriction>
  </rdfs:subClassOf>
  <rdfs:subClassOf>
    <owl:Restriction>
      <owl:allValuesFrom rdf:resource="&soma;OrderedElement"/>
      <owl:onProperty rdf:resource="&dul;precedes"/>
    </owl:Restriction>
  </rdfs:subClassOf>
  <rdfs:subClassOf>
    <owl:Restriction>
      <owl:onClass rdf:resource="&soma;Order"/>
      <owl:onProperty rdf:resource="&soma;isOrderedBy"/>
      <owl:qualifiedCardinality rdf:datatype="&xsd;nonNegativeInteger">1</owl:qualifiedCardinality>
    </owl:Restriction>
  </rdfs:subClassOf>
  <rdfs:subClassOf rdf:resource="&soma;Singleton"/>
  <rdfs:comment xml:lang="en">A 'Singleton' of an entity that 'is ordered by' some 'Order'. An 'Order item' can only 'precede' or 'follow' another 'Order item', encoding the sortation of the entities contained within the 'Order items'. Different 'Order's need to use different 'Order item's.</rdfs:comment>
  <rdfs:isDefinedBy rdf:resource="http://www.ease-crc.org/ont/SOMA-AGENT.owl"/>
  <rdfs:label xml:lang="en">Ordered element</rdfs:label>
</owl:Class>

<owl:Class rdf:about="&soma;Squeezing">
  <rdfs:comment>A task in which an Agent applies pressure to an object they have in their grasp.</rdfs:comment>
  <rdfs:isDefinedBy rdf:resource="http://www.ease-crc.org/ont/SOMA-ACT.owl"/>
  <rdfs:subClassOf rdf:resource="&soma;Actuating"/>
</owl:Class>

<owl:Restriction>
  <rdfs:subClassOf>
    <owl:Class>
      <owl:complementOf>
        <owl:Class>
          <owl:intersectionOf rdf:parseType="Collection">

            <owl:Restriction>
              <owl:onProperty rdf:resource="&dul;hasPrecondition"/>
              <owl:someValuesFrom rdf:resource="http://www.ease-crc.org/ont/SOMA.owl/NonmanifestedSituation"/>
            </owl:Restriction>
          </owl:intersectionOf>
        </owl:Class>
      </owl:complementOf>
    </owl:Class>
  </rdfs:subClassOf>
  <owl:onProperty rdf:resource="http://www.ease-crc.org/ont/SOMA.owl/manifestsIn"/>
  <owl:someValuesFrom rdf:resource="&dul;Event"/>
</owl:Restriction>

<owl:Class rdf:about="&soma;Simulating">
  <rdfs:comment>A Mental task in which the Agent endeavours to create representations of a sequence of states of affairs in the world. Simulation commits itself to some degree of transition accuracy: supposing the actual state of the world was the initial state of the simulation, the world state and simulation state should evolve to some degree similarly.

Simulation does not commit itself to state accuracy: the initial state of the simulation is not constrained to be faithful to the actual state of the world in which the Agent is embodied. Counterfactual simulation ("what would happen if--?") is possible.</rdfs:comment>
  <rdfs:isDefinedBy rdf:resource="http://www.ease-crc.org/ont/SOMA-ACT.owl"/>
  <rdfs:subClassOf rdf:resource="&soma;Prospecting"/>
</owl:Class>

<owl:ObjectProperty rdf:about="&soma;isColorOf"
    rdfs:comment="Relates a color quality to the object the color belongs to."
    rdfs:label="is color of">
  <rdfs:domain rdf:resource="&soma;Color"/>
  <rdfs:isDefinedBy rdf:resource="http://www.ease-crc.org/ont/SOMA-OBJ.owl"/>
  <rdfs:range rdf:resource="&dul;PhysicalObject"/>
  <rdfs:subPropertyOf rdf:resource="&dul;isQualityOf"/>
</owl:ObjectProperty>

<owl:ObjectProperty rdf:about="&dul;hasQuality">
  <rdfs:isDefinedBy rdf:resource="http://www.ease-crc.org/ont/SOMA-OBJ.owl"/>
  <rdfs:isDefinedBy rdf:resource="http://www.ease-crc.org/ont/SOMA.owl"/>
</owl:ObjectProperty>

<owl:Class rdf:about="&soma;PrismaticJoint"
    rdfs:label="Prismatic joint">
  <rdfs:subClassOf>
    <owl:Restriction>
      <owl:onClass rdf:resource="&soma;JointLimit"/>
      <owl:onProperty rdf:resource="&soma;hasJointLimit"/>
      <owl:qualifiedCardinality rdf:datatype="&xsd;nonNegativeInteger">1</owl:qualifiedCardinality>
    </owl:Restriction>
  </rdfs:subClassOf>
  <rdfs:subClassOf rdf:resource="&soma;MovableJoint"/>
  <rdfs:comment>A sliding joint that slides along an axis, and has a limited range specified by the upper and lower limits.</rdfs:comment>
  <rdfs:isDefinedBy rdf:resource="http://www.ease-crc.org/ont/SOMA-OBJ.owl"/>
</owl:Class>

<owl:DatatypeProperty rdf:about="&soma;hasPersistentIdentifier">
  <rdfs:comment>A property linking an InformationRealization to a persistent identifier such as a DOI, which can then be used to obtain an address at which the realization (i.e. digital file) can be retrieved.</rdfs:comment>
  <rdfs:domain rdf:resource="&dul;InformationRealization"/>
  <rdfs:isDefinedBy rdf:resource="http://www.ease-crc.org/ont/SOMA.owl"/>
  <rdfs:range rdf:resource="&xsd;string"/>
  <rdfs:subPropertyOf rdf:resource="&dul;hasDataValue"/>
</owl:DatatypeProperty>

<owl:Class rdf:about="&soma;BoxShape"
    rdfs:label="Box shape">
  <rdfs:subClassOf>
    <owl:Restriction>
      <owl:onDataRange rdf:resource="&xsd;float"/>
      <owl:onProperty rdf:resource="&soma;hasHeight"/>
      <owl:qualifiedCardinality rdf:datatype="&xsd;nonNegativeInteger">1</owl:qualifiedCardinality>
    </owl:Restriction>
  </rdfs:subClassOf>
  <rdfs:subClassOf>
    <owl:Restriction>
      <owl:onDataRange rdf:resource="&xsd;float"/>
      <owl:onProperty rdf:resource="&soma;hasLength"/>
      <owl:qualifiedCardinality rdf:datatype="&xsd;nonNegativeInteger">1</owl:qualifiedCardinality>
    </owl:Restriction>
  </rdfs:subClassOf>
  <rdfs:subClassOf>
    <owl:Restriction>
      <owl:onDataRange rdf:resource="&xsd;float"/>
      <owl:onProperty rdf:resource="&soma;hasWidth"/>
      <owl:qualifiedCardinality rdf:datatype="&xsd;nonNegativeInteger">1</owl:qualifiedCardinality>
    </owl:Restriction>
  </rdfs:subClassOf>
  <rdfs:subClassOf rdf:resource="&soma;ShapeRegion"/>
  <rdfs:comment>A symmetrical shape, either solid or hollow, contained by six rectangles.</rdfs:comment>
  <rdfs:isDefinedBy rdf:resource="http://www.ease-crc.org/ont/SOMA-OBJ.owl"/>
</owl:Class>

<owl:Class rdf:about="&soma;Cleanliness"
    rdfs:comment="The quality of being clean.">
  <rdfs:subClassOf>
    <owl:Restriction>
      <owl:onProperty rdf:resource="&dul;hasRegion"/>
      <owl:someValuesFrom rdf:resource="&soma;CleanlinessRegion"/>
    </owl:Restriction>
  </rdfs:subClassOf>
  <rdfs:subClassOf>
    <owl:Restriction>
      <owl:allValuesFrom rdf:resource="&soma;CleanlinessRegion"/>
      <owl:onProperty rdf:resource="&dul;hasRegion"/>
    </owl:Restriction>
  </rdfs:subClassOf>
  <rdfs:subClassOf rdf:resource="&soma;SocialQuality"/>
  <rdfs:isDefinedBy rdf:resource="http://www.ease-crc.org/ont/SOMA-OBJ.owl"/>
</owl:Class>

<owl:Class rdf:about="&dul;Entity">
  <rdfs:isDefinedBy rdf:resource="http://www.ease-crc.org/ont/SOMA-WF.owl"/>
</owl:Class>

<owl:Class rdf:about="&soma;SettingGripper">
  <rdfs:comment>A task by which an Agent arranges one/some/all of its grippers in some configuration.</rdfs:comment>
  <rdfs:isDefinedBy rdf:resource="http://www.ease-crc.org/ont/SOMA-ACT.owl"/>
  <rdfs:label xml:lang="en">Setting gripper</rdfs:label>
  <rdfs:subClassOf rdf:resource="&soma;AssumingPose"/>
</owl:Class>

<owl:Class rdf:about="&soma;Ontology">
  <rdfs:comment xml:lang="en">An ontology encompasses a representation, formal naming, and definition of the categories, properties, and relations between the concepts, data, and entities that substantiate one, many, or all domains of discourse. More simply, an ontology is a way of showing the properties of a subject area and how they are related, by defining a set of concepts and categories that represent the subject.

From Wikipedia: https://en.wikipedia.org/wiki/Ontology_(information_science)</rdfs:comment>
  <rdfs:isDefinedBy rdf:resource="http://www.ease-crc.org/ont/SOMA-IO.owl"/>
  <rdfs:subClassOf rdf:resource="&soma;Structured_Text"/>
  <owl:equivalentClass>
    <owl:Class>
      <owl:intersectionOf rdf:parseType="Collection">
        <rdf:Description rdf:about="&soma;Structured_Text"/>
        <owl:Restriction>
          <owl:onProperty rdf:resource="&soma;isGivenMeaningBy"/>
          <owl:someValuesFrom rdf:resource="&soma;Ontology_Language"/>
        </owl:Restriction>
      </owl:intersectionOf>
    </owl:Class>
  </owl:equivalentClass>
</owl:Class>

<owl:Class rdf:about="&soma;Phrase">
  <rdfs:isDefinedBy rdf:resource="http://www.ease-crc.org/ont/SOMA-SAY.owl"/>
  <rdfs:isDefinedBy rdf:resource="http://www.ontologydesignpatterns.org/ont/dul/IOLite.owl"/>
  <rdfs:subClassOf rdf:resource="&soma;LinguisticObject"/>
</owl:Class>

<owl:Class rdf:about="&soma;Perceiving">
  <rdfs:comment>A task in which the Agent gathers and interprets sensor information about its surroundings.</rdfs:comment>
  <rdfs:isDefinedBy rdf:resource="http://www.ease-crc.org/ont/SOMA-ACT.owl"/>
  <rdfs:subClassOf>
    <owl:Class>
      <owl:intersectionOf rdf:parseType="Collection">
        <rdf:Description rdf:about="&soma;InformationAcquisition"/>
        <rdf:Description rdf:about="&soma;PhysicalTask"/>
      </owl:intersectionOf>
    </owl:Class>
  </rdfs:subClassOf>
</owl:Class>

<owl:ObjectProperty rdf:about="&soma;isTaskOfOutputRole"
    rdfs:comment="A relation between a Task and one of its output roles.">
  <rdfs:domain rdf:resource="&dul;Task"/>
  <rdfs:isDefinedBy rdf:resource="http://www.ease-crc.org/ont/SOMA.owl"/>
  <rdfs:label xml:lang="en">is task of output role</rdfs:label>
  <rdfs:range rdf:resource="&dul;Role"/>
  <rdfs:subPropertyOf rdf:resource="&dul;isTaskOf"/>
</owl:ObjectProperty>

<owl:ObjectProperty rdf:about="&soma;affordsTrigger"
    rdfs:label="affords trigger">
  <rdfs:comment>Relates a disposition to the trigger role defined by the affordance describing the disposition.</rdfs:comment>
  <rdfs:domain rdf:resource="&soma;Disposition"/>
  <rdfs:isDefinedBy rdf:resource="http://www.ease-crc.org/ont/SOMA-OBJ.owl"/>
  <rdfs:range rdf:resource="&dul;Role"/>
  <rdfs:subPropertyOf rdf:resource="&soma;affordsConcept"/>
  <owl:inverseOf rdf:resource="&soma;isTriggerAffordedBy"/>
  <owl:propertyChainAxiom rdf:parseType="Collection">
    <rdf:Description rdf:about="&dul;isDescribedBy"/>
    <rdf:Description rdf:about="&soma;definesTrigger"/>
  </owl:propertyChainAxiom>
</owl:ObjectProperty>

<owl:AnnotationProperty rdf:about="&soma;UsageGuideline">
  <rdfs:comment>Provides a definition, or usage guideline, aimed at a particular community of the ontology's users. The community is identified by the subproperty of UsageGuideline.

A style recommendation for usage guidelines is that they should be brief. In contrast to usual concept annotations that can, and should be detailed about the reasons behind modelling decisions, usage guidelines are simply meant to answer questions about when it is appropriate to use a concept, and they must be a practical, easy to query and understand resource.</rdfs:comment>
  <rdfs:isDefinedBy rdf:resource="http://www.ease-crc.org/ont/SOMA.owl"/>
</owl:AnnotationProperty>

<rdf:Property rdf:about="&soma;location">
  <rdfs:domain rdf:resource="&soma;Location"/>
  <rdfs:range rdf:resource="&xsd;string"/>
</rdf:Property>

<owl:Class rdf:about="&soma;PushingDown"
    rdfs:comment="A task in which an Agent pushes an object downwards.">
  <rdfs:isDefinedBy rdf:resource="http://www.ease-crc.org/ont/SOMA-ACT.owl"/>
  <rdfs:label xml:lang="en">Pushing down</rdfs:label>
  <rdfs:subClassOf rdf:resource="&soma;Pushing"/>
</owl:Class>

<owl:ObjectProperty rdf:about="&soma;isArtifactInvolvedIn"
    rdfs:comment="Artifact participation."
    rdfs:label="is artifact involved in">
  <rdfs:domain rdf:resource="&dul;PhysicalArtifact"/>
  <rdfs:isDefinedBy rdf:resource="http://www.ease-crc.org/ont/SOMA.owl"/>
  <rdfs:range rdf:resource="&dul;Event"/>
  <rdfs:subPropertyOf rdf:resource="&dul;isParticipantIn"/>
</owl:ObjectProperty>

<owl:ObjectProperty rdf:about="&dul;classifies">
  <rdfs:isDefinedBy rdf:resource="http://www.ease-crc.org/ont/SOMA-PROC.owl"/>
  <rdfs:isDefinedBy rdf:resource="http://www.ease-crc.org/ont/SOMA-STATE.owl"/>
</owl:ObjectProperty>

<owl:Class rdf:about="&soma;Receiver">
  <rdfs:subClassOf>
    <owl:Restriction>
      <owl:onProperty rdf:resource="&dul;hasTask"/>
      <owl:someValuesFrom rdf:resource="&soma;CommunicationTask"/>
    </owl:Restriction>
  </rdfs:subClassOf>
  <rdfs:subClassOf rdf:resource="&soma;ExperiencerRole"/>
  <rdfs:comment xml:lang="en">The role played by an Agent in a Communication Task that perceives and interpretes some incoming Message.</rdfs:comment>
  <rdfs:isDefinedBy rdf:resource="http://www.ease-crc.org/ont/SOMA-ACT.owl"/>
  <rdfs:label xml:lang="en">Receiver</rdfs:label>
</owl:Class>

<owl:Class rdf:about="&soma;LookingAt"
    rdfs:comment="better: Gazing">
  <rdfs:isDefinedBy rdf:resource="http://www.ease-crc.org/ont/SOMA-ACT.owl"/>
  <rdfs:subClassOf rdf:resource="&soma;PhysicalTask"/>
</owl:Class>

<owl:Class rdf:about="&soma;MetaCognitionMemoryTopic"
    rdfs:label="Meta cognition memory topic">
  <rdfs:comment>A topic used while an Agent describes its own cognitive processes and actions, and which covers descriptions of what memories are involved in them.</rdfs:comment>
  <rdfs:isDefinedBy rdf:resource="http://www.ease-crc.org/ont/SOMA-ACT.owl"/>
  <rdfs:subClassOf rdf:resource="&soma;MetaCognitionTopic"/>
</owl:Class>

<owl:Class rdf:about="&soma;ExcludedObject"
    rdfs:label="Excluded object">
  <rdfs:comment>An object that is not contained in something. This is meant very general and includes, e.g., elements excluded from a set, or things that are spatially excluded from the boundaries of some object.</rdfs:comment>
  <rdfs:isDefinedBy rdf:resource="http://www.ease-crc.org/ont/SOMA-OBJ.owl"/>
  <rdfs:subClassOf rdf:resource="&soma;Patient"/>
</owl:Class>

<owl:Class rdf:about="&soma;Shifting">
  <rdfs:subClassOf>
    <owl:Restriction>
      <owl:allValuesFrom>
        <owl:Restriction>
          <owl:allValuesFrom rdf:resource="&soma;Localization"/>
          <owl:onProperty rdf:resource="&dul;classifies"/>
        </owl:Restriction>
      </owl:allValuesFrom>
      <owl:onProperty rdf:resource="&soma;affordsSetpoint"/>
    </owl:Restriction>
  </rdfs:subClassOf>
  <rdfs:subClassOf>
    <owl:Restriction>
      <owl:allValuesFrom rdf:resource="&soma;MovedObject"/>
      <owl:onProperty rdf:resource="&soma;affordsTrigger"/>
    </owl:Restriction>
  </rdfs:subClassOf>
  <rdfs:subClassOf rdf:resource="&soma;Variability"/>
  <rdfs:comment>The disposition of an object (the tool) to change the localization of others.</rdfs:comment>
  <rdfs:isDefinedBy rdf:resource="http://www.ease-crc.org/ont/SOMA-OBJ.owl"/>
</owl:Class>

<owl:Class rdf:about="&soma;Predilection">
  <rdfs:label>Predilection</rdfs:label>
  <rdfs:label xml:lang="en">The relation between a 'Preference' and the 'Order' that the 'Preference' defines over Situations.

For the complete model, see 'Preference'.</rdfs:label>
  <rdfs:subClassOf>
    <owl:Restriction>
      <owl:allValuesFrom>
        <owl:Class>
          <owl:unionOf rdf:parseType="Collection">
            <rdf:Description rdf:about="&soma;Preference"/>
            <owl:Class>
              <owl:intersectionOf rdf:parseType="Collection">
                <rdf:Description rdf:about="&soma;Order"/>
                <owl:Restriction>
                  <owl:allValuesFrom>
                    <owl:Restriction>
                      <owl:allValuesFrom rdf:resource="&dul;Situation"/>
                      <owl:onProperty rdf:resource="&soma;encapsulates"/>
                    </owl:Restriction>
                  </owl:allValuesFrom>
                  <owl:onProperty rdf:resource="&soma;orders"/>
                </owl:Restriction>
              </owl:intersectionOf>
            </owl:Class>
          </owl:unionOf>
        </owl:Class>
      </owl:allValuesFrom>
      <owl:onProperty rdf:resource="&dul;describes"/>
    </owl:Restriction>
  </rdfs:subClassOf>
  <rdfs:subClassOf rdf:resource="&dul;SocialRelation"/>
  <rdfs:isDefinedBy rdf:resource="http://www.ease-crc.org/ont/SOMA-AGENT.owl"/>
</owl:Class>

<owl:Class rdf:about="&soma;ArtificialAgent"
    rdfs:label="Artificial agent">
  <rdfs:comment>A physical object with artificial characteristics, which can perform actions to achieve desired goals, and typically has sensors and/or actuators.

There can be non-physical artificial agents such as software programs but they are not considered here in the scope of artificial agent.</rdfs:comment>
  <rdfs:isDefinedBy rdf:resource="http://www.ease-crc.org/ont/SOMA-OBJ.owl"/>
  <rdfs:subClassOf rdf:resource="&dul;PhysicalAgent"/>
</owl:Class>

<owl:Class rdf:about="&soma;PreservativeInteraction"
    rdfs:label="Preservative interaction">
  <rdfs:comment>A force interaction where the agonist has a tendency to keep another object still. An example is 'holding a door closed' where some object interacts with the door to neutralize forces that could set the door into motion.</rdfs:comment>
  <rdfs:isDefinedBy rdf:resource="http://www.ease-crc.org/ont/SOMA-PROC.owl"/>
  <rdfs:subClassOf rdf:resource="&soma;ForceInteraction"/>
</owl:Class>

<owl:ObjectProperty rdf:about="&soma;affordsTask"
    rdfs:label="affords task">
  <rdfs:comment>Relates a disposition to the task defined by the affordance describing the disposition.</rdfs:comment>
  <rdfs:domain rdf:resource="&soma;Disposition"/>
  <rdfs:isDefinedBy rdf:resource="http://www.ease-crc.org/ont/SOMA-OBJ.owl"/>
  <rdfs:range rdf:resource="&dul;Task"/>
  <rdfs:subPropertyOf rdf:resource="&soma;affordsConcept"/>
  <owl:inverseOf rdf:resource="&soma;isTaskAffordedBy"/>
  <owl:propertyChainAxiom rdf:parseType="Collection">
    <rdf:Description rdf:about="&dul;isDescribedBy"/>
    <rdf:Description rdf:about="&soma;affordanceDefinesTask"/>
  </owl:propertyChainAxiom>
</owl:ObjectProperty>

<owl:Class rdf:about="&soma;Deciding">
  <rdfs:isDefinedBy rdf:resource="http://www.ease-crc.org/ont/SOMA-ACT.owl"/>
  <rdfs:isDefinedBy xml:lang="en">A mental task in where an agent makes some decision, that is, selecting some Information object; usually on the basis of others.</rdfs:isDefinedBy>
  <rdfs:label xml:lang="en">Deciding</rdfs:label>
  <rdfs:subClassOf rdf:resource="&soma;DerivingInformation"/>
</owl:Class>

<owl:Class rdf:about="&soma;Software_Configuration">
  <rdfs:label xml:lang="en">Software Configuration</rdfs:label>
  <rdfs:label xml:lang="en">The part-whole relationship of Software and its components. Every Software has (at least 1) such configuration that exactly describes all Resources that make up the software (i.e., that are needed for the Software to function).
We support seperate views:
1. The Software Configuration describes all the necessary files, in which it should also be a File Configuration
2. It describes a Software Suit, e.g., 'Open Office' consists of Writer, Calc, Impress etc. Note that thus. Software can consist of other Software - this pattern may also be useful when describing Software Components, e.g., that some Software relies on a Database Software.
3. It describes not the files, but their content (the program code), which can also be seen as the part-whole relationship if one abstracts away from the files.</rdfs:label>
  <rdfs:subClassOf>
    <owl:Restriction>
      <owl:onClass rdf:resource="&soma;Software"/>
      <owl:onProperty rdf:resource="&dul;isDescribedBy"/>
      <owl:qualifiedCardinality rdf:datatype="&xsd;nonNegativeInteger">1</owl:qualifiedCardinality>
    </owl:Restriction>
  </rdfs:subClassOf>
  <rdfs:subClassOf rdf:resource="&dul;Configuration"/>
  <rdfs:isDefinedBy rdf:resource="http://www.ease-crc.org/ont/SOMA-IO.owl"/>
</owl:Class>

<owl:ObjectProperty rdf:about="&soma;isCausedByEvent"
    rdfs:label="is caused by event">
  <rdfs:comment>A relation recording that a Transition is the result of some Event.</rdfs:comment>
  <rdfs:domain rdf:resource="&dul;Transition"/>
  <rdfs:isDefinedBy rdf:resource="http://www.ease-crc.org/ont/SOMA.owl"/>
  <rdfs:range rdf:resource="&dul;Event"/>
  <rdfs:subPropertyOf rdf:resource="&dul;includesEvent"/>
</owl:ObjectProperty>

<owl:Class rdf:about="&soma;MovingAway">
  <rdfs:comment>A process type classifying a motion by which some Agent puts distance between itself and another object or location.</rdfs:comment>
  <rdfs:isDefinedBy rdf:resource="http://www.ease-crc.org/ont/SOMA-PROC.owl"/>
  <rdfs:subClassOf rdf:resource="&soma;Locomotion"/>
</owl:Class>

<owl:Class rdf:about="&soma;Rubbing">
  <rdfs:comment>The motion of an object sliding along the surface of another, for example, to clean the surface.</rdfs:comment>
  <rdfs:isDefinedBy rdf:resource="http://www.ease-crc.org/ont/SOMA-PROC.owl"/>
  <rdfs:subClassOf rdf:resource="&soma;DirectedMotion"/>
</owl:Class>

<owl:Class rdf:about="&soma;MeshShapeData">
  <rdfs:subClassOf>
    <owl:Restriction>
      <owl:allValuesFrom rdf:resource="&dul;PhysicalObject"/>
      <owl:onProperty rdf:resource="&dul;isAbout"/>
    </owl:Restriction>
  </rdfs:subClassOf>
  <rdfs:subClassOf rdf:resource="&dul;InformationObject"/>
  <rdfs:comment>An InformationObject containing data about the geometry of a physical object.</rdfs:comment>
  <rdfs:isDefinedBy rdf:resource="http://www.ease-crc.org/ont/SOMA-NEEM.owl"/>
  <rdfs:label xml:lang="en">Mesh-shape data</rdfs:label>
</owl:Class>

<owl:Class rdf:about="&soma;PluginSpecification">
  <rdfs:subClassOf>
    <owl:Class>
      <owl:intersectionOf rdf:parseType="Collection">

        <owl:Restriction>
          <owl:onProperty rdf:resource="&dul;definesRole"/>
          <owl:someValuesFrom rdf:resource="&soma;HostRole"/>
        </owl:Restriction>

        <owl:Restriction>
          <owl:onProperty rdf:resource="&dul;definesRole"/>
          <owl:someValuesFrom rdf:resource="&soma;PluginRole"/>
        </owl:Restriction>
      </owl:intersectionOf>
    </owl:Class>
  </rdfs:subClassOf>
  <rdfs:subClassOf rdf:resource="&soma;API_Specification"/>
  <rdfs:comment xml:lang="en">The Specification of a Plugin interface defines how a Host and a Plug-in function together and exchange information.</rdfs:comment>
  <rdfs:isDefinedBy rdf:resource="http://www.ease-crc.org/ont/SOMA-IO.owl"/>
  <rdfs:label xml:lang="en">Plugin Specification</rdfs:label>
</owl:Class>

<owl:Class rdf:about="&soma;Constructing">
  <rdfs:comment xml:lang="en">A task in which an Agent creates a new physical object.</rdfs:comment>
  <rdfs:isDefinedBy rdf:resource="http://www.ease-crc.org/ont/SOMA-ACT.owl"/>
  <rdfs:subClassOf rdf:resource="&soma;PhysicalTask"/>
  <owl:disjointWith rdf:resource="&soma;ModifyingPhysicalObject"/>
</owl:Class>

<owl:Class rdf:about="&soma;GraspingMotion"
    rdfs:label="Grasping motion">
  <rdfs:comment>A process type classifying a motion by which some end effector acquires kinematic control over some other object.</rdfs:comment>
  <rdfs:isDefinedBy rdf:resource="http://www.ease-crc.org/ont/SOMA-PROC.owl"/>
  <rdfs:subClassOf rdf:resource="&soma;PrehensileMotion"/>
  <owl:disjointWith rdf:resource="&soma;ReleasingMotion"/>
  <owl:equivalentClass>
    <owl:Class>
      <owl:unionOf rdf:parseType="Collection">
        <rdf:Description rdf:about="&soma;IntermediateGrasp"/>
        <rdf:Description rdf:about="&soma;PowerGrasp"/>
        <rdf:Description rdf:about="&soma;PrecisionGrasp"/>
      </owl:unionOf>
    </owl:Class>
  </owl:equivalentClass>
</owl:Class>

<owl:ObjectProperty rdf:about="&soma;isMovedByAgent">
  <rdfs:comment>A relation from an object to an agent who causes it to move.</rdfs:comment>
  <rdfs:domain rdf:resource="&dul;PhysicalObject"/>
  <rdfs:isDefinedBy rdf:resource="http://www.ease-crc.org/ont/SOMA-SAY.owl"/>
  <rdfs:range rdf:resource="&dul;Agent"/>
  <rdfs:subPropertyOf rdf:resource="&soma;interactsWith"/>
  <owl:inverseOf rdf:resource="&soma;movesObject"/>
</owl:ObjectProperty>

<owl:ObjectProperty rdf:about="&dul;overlaps"/>

<owl:Class rdf:about="&soma;Setpoint"
    rdfs:comment="Classifies some dedicated goal region.">
  <rdfs:isDefinedBy rdf:resource="http://www.ease-crc.org/ont/SOMA-OBJ.owl"/>
  <rdfs:subClassOf rdf:resource="&dul;Parameter"/>
</owl:Class>

<soma:StatusFailure rdf:about="&soma;FailWFUninterpretableTask">
  <rdf:type rdf:resource="&owl;NamedIndividual"/>
  <rdfs:comment>A particular kind of failure: a task is not recognized and not associated to anything that could execute it, nor to a workflow that could detail its structure into simpler structure.</rdfs:comment>
  <rdfs:isDefinedBy rdf:resource="http://www.ease-crc.org/ont/SOMA-WF.owl"/>
</soma:StatusFailure>

<owl:ObjectProperty rdf:about="&dul;isObjectIncludedIn"/>

<owl:Class rdf:about="&soma;ContinuousJoint"
    rdfs:label="Continuous joint">
  <rdfs:comment>A continuous hinge joint that rotates around an axis and has no upper and lower limits.</rdfs:comment>
  <rdfs:isDefinedBy rdf:resource="http://www.ease-crc.org/ont/SOMA-OBJ.owl"/>
  <rdfs:subClassOf rdf:resource="&soma;HingeJoint"/>
</owl:Class>

<owl:DatatypeProperty rdf:about="&soma;hasHSVValue"
    rdfs:label="has hsv value">
  <rdfs:comment>Associates a ColorRegion to numerical data describing the color. This data uses the Hue-Saturation-Value color space.</rdfs:comment>
  <rdfs:domain rdf:resource="&soma;ColorRegion"/>
  <rdfs:isDefinedBy rdf:resource="http://www.ease-crc.org/ont/SOMA-OBJ.owl"/>
  <rdfs:range rdf:resource="&xsd;string"/>
  <rdfs:subPropertyOf rdf:resource="&soma;hasColorValue"/>
</owl:DatatypeProperty>

<owl:ObjectProperty rdf:about="&soma;directlyDerivedFrom"
    rdfs:label="directly derived from">
  <rdfs:comment>The relation between an information object and another which it has been derived from.</rdfs:comment>
  <rdfs:isDefinedBy rdf:resource="http://www.ease-crc.org/ont/SOMA.owl"/>
  <rdfs:subPropertyOf rdf:resource="&soma;derivedFrom"/>
  <owl:inverseOf rdf:resource="&soma;isDirectSourceFor"/>
</owl:ObjectProperty>

<owl:Class rdf:about="&soma;Reasoning">
  <rdfs:comment>A Mental task in which an Agent endeavours to obtain new knowledge from knowledge it already possesses.</rdfs:comment>
  <rdfs:comment>todo: a taxonomy of reasoning is not trivial. Classical theory distinguishes Deductive, Inductive, and with a stretch Abductive reasoning. However, modern practice distinguishes other categories that overlap with these, e.g. Probabilistic and Non-monotonic.

Both Abductive and Inductive inference may, and often do, use Probabilistic methods. Probabilistic inference is, by its nature, most opposed to Deductive inference which, classically, requires logical certainty.

Any of the Abductive/Deductive/Inductive triad can be further affected by the Monotone/Non-monotone distinction. There are preferences (Inductive and Abductive reasoning is probably most often non-monotonic; most of Deductive reasoning is probably done in monotonic formalisms), but it is certainly the case that, e.g., non-monotone Deduction is possible.

Note, this classification has nothing to do with reasoning domain (e.g. SpatialReasoning, TemporalReasoning, ...) and merely with techniques/logical-mathematical underpinnings.</rdfs:comment>
  <rdfs:isDefinedBy rdf:resource="http://www.ease-crc.org/ont/SOMA-ACT.owl"/>
  <rdfs:subClassOf rdf:resource="&soma;DerivingInformation"/>
</owl:Class>

<owl:Class rdf:about="&soma;ExtractedObject"
    rdfs:comment="An object that is removed from a container or system.">
  <rdfs:isDefinedBy rdf:resource="http://www.ease-crc.org/ont/SOMA-OBJ.owl"/>
  <rdfs:label xml:lang="en">Extracted object</rdfs:label>
  <rdfs:subClassOf rdf:resource="&soma;Patient"/>
</owl:Class>

<owl:Class rdf:about="&soma;FileConfiguration">
  <rdfs:comment xml:lang="en">A configuration whose members are all files. Used to model, e.g., concrete collections of zip- and jar-files (and so on).</rdfs:comment>
  <rdfs:isDefinedBy rdf:resource="http://www.ease-crc.org/ont/SOMA-IO.owl"/>
  <rdfs:label xml:lang="en">File Configuration</rdfs:label>
  <owl:equivalentClass>
    <owl:Class>
      <owl:intersectionOf rdf:parseType="Collection">
        <rdf:Description rdf:about="&dul;Configuration"/>
        <owl:Restriction>
          <owl:allValuesFrom rdf:resource="&soma;Digital_File"/>
          <owl:onProperty rdf:resource="&dul;hasMember"/>
        </owl:Restriction>
      </owl:intersectionOf>
    </owl:Class>
  </owl:equivalentClass>
</owl:Class>

<owl:Class rdf:about="&soma;StatisticalReasoner">
  <rdfs:label xml:lang="en">A Statistical Reasoner is a Reasoner that uses statistical or stochastical data to infer implicit information from explicit information. Examples are Hidden Markov Models and Neural Networks.</rdfs:label>
  <rdfs:label xml:lang="en">Statistical reasoner</rdfs:label>
  <rdfs:isDefinedBy rdf:resource="http://www.ease-crc.org/ont/SOMA-IO.owl"/>
  <rdfs:subClassOf rdf:resource="&soma;Reasoner"/>
</owl:Class>

<owl:ObjectProperty rdf:about="&dul;actsFor"/>

<rdfs:Datatype rdf:about="&soma;array_uint">
  <rdfs:isDefinedBy rdf:resource="http://www.ease-crc.org/ont/SOMA.owl"/>
  <owl:equivalentClass rdf:resource="&xsd;string"/>
</rdfs:Datatype>

<owl:Class rdf:about="&soma;Succedence">
  <rdfs:comment>A relation that holds in some descriptive context such as a Workflow, between two TaskInvocations belonging to that same Workflow. It means that one task invocation should follow the other.

Note: a successor relation implemented as an OWL object property is sometimes enough, but not in general; in particular, when there are conditions imposed on the succession.

As a result, a reification pattern was applied here.</rdfs:comment>
  <rdfs:comment>Note: it is possible for a Succedence relation to exist between a TaskInvocation and itself; in this case, both the hasPredecessor and hasSuccessor roles are filled by the same TaskInvocation individual.

Care must be taken with this however, as a natural interpretation of this situation is an infinite loop.</rdfs:comment>
  <rdfs:subClassOf>
    <owl:Restriction>
      <owl:onProperty>
        <rdf:Description>
          <owl:inverseOf rdf:resource="&soma;hasSuccedence"/>
        </rdf:Description>
      </owl:onProperty>
      <owl:someValuesFrom rdf:resource="&dul;Description"/>
    </owl:Restriction>
  </rdfs:subClassOf>
  <rdfs:subClassOf>
    <owl:Restriction>
      <owl:onClass rdf:resource="&soma;TaskInvocation"/>
      <owl:onProperty rdf:resource="&soma;hasPredecessor"/>
      <owl:qualifiedCardinality rdf:datatype="&xsd;nonNegativeInteger">1</owl:qualifiedCardinality>
    </owl:Restriction>
  </rdfs:subClassOf>
  <rdfs:subClassOf>
    <owl:Restriction>
      <owl:onClass rdf:resource="&soma;TaskInvocation"/>
      <owl:onProperty rdf:resource="&soma;hasSuccessor"/>
      <owl:qualifiedCardinality rdf:datatype="&xsd;nonNegativeInteger">1</owl:qualifiedCardinality>
    </owl:Restriction>
  </rdfs:subClassOf>
  <rdfs:subClassOf rdf:resource="&dul;Relation"/>
  <rdfs:isDefinedBy rdf:resource="http://www.ease-crc.org/ont/SOMA-WF.owl"/>
</owl:Class>

<owl:ObjectProperty rdf:about="&dul;hasLocation"/>

<owl:ObjectProperty rdf:about="&dul;expresses">
  <rdfs:subPropertyOf rdf:resource="&dul;isAbout"/>
</owl:ObjectProperty>

<owl:Class rdf:about="&soma;Agonist">
  <rdfs:comment>A role that classifies entities with a tendency to either cause an alteration or to preserve some state.</rdfs:comment>
  <rdfs:isDefinedBy rdf:resource="http://www.ease-crc.org/ont/SOMA-PROC.owl"/>
  <rdfs:subClassOf rdf:resource="&soma;Patient"/>
</owl:Class>

<owl:Class rdf:about="&soma;DeviceTurnedOff"
    rdfs:comment="A value indicating a device is not in operation.">
  <rdfs:isDefinedBy rdf:resource="http://www.ease-crc.org/ont/SOMA-OBJ.owl"/>
  <rdfs:label xml:lang="en">Device turned off</rdfs:label>
  <rdfs:subClassOf rdf:resource="&soma;DeviceStateRange"/>
</owl:Class>

<owl:ObjectProperty rdf:about="&soma;hasInitialState"
    rdfs:label="has initial state">
  <rdfs:comment>A relation which connects a Transition to the Situation it starts from.</rdfs:comment>
  <rdfs:domain rdf:resource="&dul;Transition"/>
  <rdfs:isDefinedBy rdf:resource="http://www.ease-crc.org/ont/SOMA.owl"/>
  <rdfs:range rdf:resource="&dul;Situation"/>
  <rdfs:subPropertyOf rdf:resource="&soma;includesSituation"/>
  <owl:inverseOf rdf:resource="&soma;isInitialStateOf"/>
</owl:ObjectProperty>

<owl:Class rdf:about="&soma;ThinkAloudKnowledgeTopic"
    rdfs:label="Think aloud knowledge topic">
  <rdfs:comment>A topic used when an Agent states some item of knowledge. This knowledge can be general, or specific to the environment and task at hand.</rdfs:comment>
  <rdfs:isDefinedBy rdf:resource="http://www.ease-crc.org/ont/SOMA-ACT.owl"/>
  <rdfs:subClassOf rdf:resource="&soma;ThinkAloudTopic"/>
</owl:Class>

<owl:ObjectProperty rdf:about="&soma;isTerminalSituationOf">
  <rdfs:comment>A relation between SituationTransitions and Situations, which identifies the Situation the transition ends at.</rdfs:comment>
  <rdfs:domain rdf:resource="&dul;Situation"/>
  <rdfs:isDefinedBy rdf:resource="http://www.ease-crc.org/ont/SOMA-ACT.owl"/>
  <rdfs:label xml:lang="en">is terminal situation of</rdfs:label>
  <rdfs:range rdf:resource="&soma;SituationTransition"/>
  <rdfs:subPropertyOf rdf:resource="&soma;isTerminalStateOf"/>
</owl:ObjectProperty>

<owl:Class rdf:about="&soma;ThinkAloudGeneralKnowledgeTopic"
    rdfs:label="Think aloud general knowledge topic">
  <rdfs:comment>A topic used when an Agent states general knowledge they have.</rdfs:comment>
  <rdfs:isDefinedBy rdf:resource="http://www.ease-crc.org/ont/SOMA-ACT.owl"/>
  <rdfs:subClassOf rdf:resource="&soma;ThinkAloudKnowledgeTopic"/>
</owl:Class>

<owl:Class rdf:about="&soma;CutObject"
    rdfs:comment="An object being cut down into pieces."
    rdfs:label="Cut object">
  <rdfs:isDefinedBy rdf:resource="http://www.ease-crc.org/ont/SOMA-OBJ.owl"/>
  <rdfs:subClassOf rdf:resource="&soma;AlteredObject"/>
</owl:Class>

<owl:DatatypeProperty rdf:about="&soma;hasJointPositionMax"
    rdfs:label="has joint position max">
  <rdfs:comment>The maximum position of a joint given in m (prismatic joints) or rad (hinged joints).</rdfs:comment>
  <rdfs:domain rdf:resource="&soma;JointLimit"/>
  <rdfs:isDefinedBy rdf:resource="http://www.ease-crc.org/ont/SOMA-OBJ.owl"/>
  <rdfs:range rdf:resource="&xsd;double"/>
  <rdfs:subPropertyOf rdf:resource="&soma;hasJointParameter"/>
</owl:DatatypeProperty>

<owl:ObjectProperty rdf:about="&soma;isInitialSceneOf"
    rdfs:label="is initial scene of">
  <rdfs:comment>A relation between StateTransitions and Scenes, which identifies the scene the transition starts from.</rdfs:comment>
  <rdfs:domain rdf:resource="&soma;Scene"/>
  <rdfs:isDefinedBy rdf:resource="http://www.ease-crc.org/ont/SOMA.owl"/>
  <rdfs:range rdf:resource="&soma;StateTransition"/>
  <rdfs:subPropertyOf rdf:resource="&soma;isInitialStateOf"/>
</owl:ObjectProperty>

<owl:Class rdf:about="&soma;Replanning">
  <rdfs:comment xml:lang="en">A mental task, in which an agent reconfigures some plan that has been put together before.</rdfs:comment>
  <rdfs:isDefinedBy rdf:resource="http://www.ease-crc.org/ont/SOMA-ACT.owl"/>
  <rdfs:label xml:lang="en">Replanning</rdfs:label>
  <rdfs:subClassOf rdf:resource="&soma;Planning"/>
</owl:Class>

<owl:Class rdf:about="&dul;Role">
  <rdfs:isDefinedBy rdf:resource="http://www.ease-crc.org/ont/SOMA-PROC.owl"/>
  <rdfs:isDefinedBy rdf:resource="http://www.ease-crc.org/ont/SOMA-STATE.owl"/>
  <rdfs:isDefinedBy rdf:resource="http://www.ease-crc.org/ont/SOMA-WF.owl"/>
</owl:Class>

<owl:DatatypeProperty rdf:about="&soma;hasIntervalEnd"
    rdfs:comment="A relation recording when a TimeInterval ended."
    rdfs:label="has interval end">
  <rdfs:domain rdf:resource="&dul;TimeInterval"/>
  <rdfs:isDefinedBy rdf:resource="http://www.ease-crc.org/ont/SOMA.owl"/>
  <rdfs:range rdf:resource="&xsd;float"/>
  <rdfs:subPropertyOf rdf:resource="&soma;hasIntervalTime"/>
</owl:DatatypeProperty>

<owl:Class rdf:about="&soma;Memorizing">
  <rdfs:comment xml:lang="en">An atomic mental task in which an Agent saves some (declarative) information for later retrieval.

Examples include a student learning vocabularies or a computer saving some information to a database.</rdfs:comment>
  <rdfs:isDefinedBy rdf:resource="http://www.ease-crc.org/ont/SOMA-ACT.owl"/>
  <rdfs:label xml:lang="en">Memorizing</rdfs:label>
  <rdfs:subClassOf rdf:resource="&soma;Learning"/>
</owl:Class>

<owl:Class rdf:about="&soma;Cutting">
  <rdfs:comment>The goal of this task is to separate one or more pieces from some target object by means of cutting into its constituent material. Unlike a disassembly, a cut is usually not easily reversible.</rdfs:comment>
  <rdfs:isDefinedBy rdf:resource="http://www.ease-crc.org/ont/SOMA-ACT.owl"/>
  <rdfs:subClassOf rdf:resource="&soma;ModifyingPhysicalObject"/>
</owl:Class>

<owl:Class rdf:about="&soma;Leg"
    rdfs:comment="A limb on which an agent walks or stands.">
  <rdfs:isDefinedBy rdf:resource="http://www.ease-crc.org/ont/SOMA-OBJ.owl"/>
  <rdfs:subClassOf rdf:resource="&soma;Limb"/>
</owl:Class>

<owl:Class rdf:about="&soma;Mixing">
  <rdfs:comment>A task by which an Agent combines several entities, such that the combination is difficult or in practice impossible to reverse.</rdfs:comment>
  <rdfs:isDefinedBy rdf:resource="http://www.ease-crc.org/ont/SOMA-ACT.owl"/>
  <rdfs:subClassOf rdf:resource="&soma;Constructing"/>
</owl:Class>

<owl:ObjectProperty rdf:about="&soma;includesRecord">
  <rdfs:comment>A relationship indicating that an Event has been recorded by an InformationObject</rdfs:comment>
  <rdfs:domain rdf:resource="&dul;Event"/>
  <rdfs:isDefinedBy rdf:resource="http://www.ease-crc.org/ont/SOMA.owl"/>
  <rdfs:range rdf:resource="&dul;InformationObject"/>
  <rdfs:subPropertyOf rdf:resource="&dul;isReferenceOf"/>
  <owl:inverseOf rdf:resource="&soma;isRecordIncludedBy"/>
</owl:ObjectProperty>

<owl:ObjectProperty rdf:about="&soma;isDirectReactionTo">
  <rdfs:comment xml:lang="en">Non-transitive version of "is reaction to".</rdfs:comment>
  <rdfs:domain rdf:resource="&dul;Event"/>
  <rdfs:isDefinedBy rdf:resource="http://www.ease-crc.org/ont/SOMA-ACT.owl"/>
  <rdfs:label xml:lang="en">is direct reaction to</rdfs:label>
  <rdfs:range rdf:resource="&dul;Event"/>
  <rdfs:subPropertyOf rdf:resource="&soma;isReactionTo"/>
</owl:ObjectProperty>

<owl:Class rdf:about="&soma;Instructions"
    rdfs:comment="The role of a plan to follow during an execution task."
    rdfs:label="Instructions">
  <rdfs:isDefinedBy rdf:resource="http://www.ease-crc.org/ont/SOMA-ACT.owl"/>
  <rdfs:subClassOf rdf:resource="&soma;Item"/>
</owl:Class>

<rdf:Property rdf:about="&soma;type">
  <rdfs:domain rdf:resource="&soma;Object"/>
  <rdfs:range rdf:resource="&xsd;string"/>
</rdf:Property>

<owl:Class rdf:about="&soma;Clean"
    rdfs:comment="A cleanliness region with values considered as clean.">
  <rdfs:isDefinedBy rdf:resource="http://www.ease-crc.org/ont/SOMA-OBJ.owl"/>
  <rdfs:subClassOf rdf:resource="&soma;CleanlinessRegion"/>
</owl:Class>

<owl:Class rdf:about="&soma;Classifier">
  <rdfs:isDefinedBy rdf:resource="http://www.ease-crc.org/ont/SOMA-IO.owl"/>
  <rdfs:label xml:lang="en">Classifier</rdfs:label>
  <rdfs:subClassOf rdf:resource="&soma;StatisticalReasoner"/>
</owl:Class>

<owl:ObjectProperty rdf:about="&soma;transitionsTo">
  <rdfs:comment>A property which relates a Transient to an Object it changes into. This is useful to model objects which, through participation in a process, transform themselves so that an ontological reclassification is necessary. An example of this is baked dough eventually becoming bread by completing a baking process.</rdfs:comment>
  <rdfs:domain rdf:resource="&soma;Transient"/>
  <rdfs:isDefinedBy rdf:resource="http://www.ease-crc.org/ont/SOMA-OBJ.owl"/>
  <rdfs:label xml:lang="en">transitions to</rdfs:label>
  <rdfs:range rdf:resource="&dul;Object"/>
  <rdfs:subPropertyOf rdf:resource="&dul;hasCommonBoundary"/>
</owl:ObjectProperty>

<owl:Class rdf:about="&soma;Supporter"
    rdfs:comment="A role classifying an object used to support others.">
  <rdfs:isDefinedBy rdf:resource="http://www.ease-crc.org/ont/SOMA-OBJ.owl"/>
  <rdfs:isDefinedBy rdf:resource="http://www.ease-crc.org/ont/SOMA-STATE.owl"/>
  <rdfs:subClassOf rdf:resource="&soma;Restrictor"/>
</owl:Class>

<owl:ObjectProperty rdf:about="&soma;isSituationIncludedIn"
    rdfs:label="is situation included in">
  <rdfs:comment>A relation recording that a Situation participates in another in some role, or can be considered as a subsituation of the other.</rdfs:comment>
  <rdfs:domain rdf:resource="&dul;Situation"/>
  <rdfs:isDefinedBy rdf:resource="http://www.ease-crc.org/ont/SOMA.owl"/>
  <rdfs:range rdf:resource="&dul;Situation"/>
  <rdfs:subPropertyOf rdf:resource="&dul;hasSetting"/>
</owl:ObjectProperty>

<owl:ObjectProperty rdf:about="&dul;hasTask"/>

<owl:Class rdf:about="&soma;FactualBinding">
  <rdfs:comment>FactualBindings are used in a workflow to assert that:

-- task- or workflow-defined roles share fillers (RoleRoleBindings). Example, the instrument of a cutting task may be the actee of a grasping task;
-- task- or workflow-defined roles are filled by a particular entity (RoleFillerBindings). This is typically the case when roles, and especially parameters, can be assigned to constants. Example, the waiting time to cook soft eggs is 3 minutes.</rdfs:comment>
  <rdfs:isDefinedBy rdf:resource="http://www.ease-crc.org/ont/SOMA-WF.owl"/>
  <rdfs:label xml:lang="en">Factial binding</rdfs:label>
  <rdfs:subClassOf rdf:resource="&soma;Binding"/>
</owl:Class>

<owl:ObjectProperty rdf:about="&dul;isDefinedIn">
  <rdfs:isDefinedBy rdf:resource="http://www.ease-crc.org/ont/SOMA-PROC.owl"/>
</owl:ObjectProperty>

<owl:Class rdf:about="&soma;Localization">
  <rdfs:subClassOf>
    <owl:Restriction>
      <owl:onProperty rdf:resource="&dul;hasRegion"/>
      <owl:someValuesFrom rdf:resource="&dul;SpaceRegion"/>
    </owl:Restriction>
  </rdfs:subClassOf>
  <rdfs:subClassOf>
    <owl:Restriction>
      <owl:allValuesFrom rdf:resource="&dul;SpaceRegion"/>
      <owl:onProperty rdf:resource="&dul;hasRegion"/>
    </owl:Restriction>
  </rdfs:subClassOf>
  <rdfs:subClassOf rdf:resource="&soma;Extrinsic"/>
  <rdfs:comment>The localization of an object. The region of this quality encodes values to localize the object in a dimensional space, e.g. Euclidean positions that localize the object in Euclidean space.</rdfs:comment>
  <rdfs:isDefinedBy rdf:resource="http://www.ease-crc.org/ont/SOMA-OBJ.owl"/>
</owl:Class>

<owl:Class rdf:about="&soma;SphereShape"
    rdfs:label="Sphere shape">
  <rdfs:subClassOf>
    <owl:Restriction>
      <owl:onDataRange rdf:resource="&xsd;float"/>
      <owl:onProperty rdf:resource="&soma;hasRadius"/>
      <owl:qualifiedCardinality rdf:datatype="&xsd;nonNegativeInteger">1</owl:qualifiedCardinality>
    </owl:Restriction>
  </rdfs:subClassOf>
  <rdfs:subClassOf rdf:resource="&soma;ShapeRegion"/>
  <rdfs:comment>A round solid figure with every point on its surface equidistant from its centre.</rdfs:comment>
  <rdfs:isDefinedBy rdf:resource="http://www.ease-crc.org/ont/SOMA-OBJ.owl"/>
</owl:Class>

<owl:ObjectProperty rdf:about="&soma;hasLink"
    rdfs:comment="Relates an object to its kinematic components."
    rdfs:label="has link">
  <rdfs:domain rdf:resource="&dul;PhysicalObject"/>
  <rdfs:isDefinedBy rdf:resource="http://www.ease-crc.org/ont/SOMA-OBJ.owl"/>
  <rdfs:range rdf:resource="&dul;PhysicalObject"/>
  <rdfs:subPropertyOf rdf:resource="&dul;hasComponent"/>
  <owl:inverseOf rdf:resource="&soma;isLinkOf"/>
</owl:ObjectProperty>

<owl:Class rdf:about="&soma;API_Specification">
  <rdfs:comment xml:lang="en">An application programming interface (API) is a way for two or more computer programs to communicate with each other. It is a type of software interface, offering a service to other pieces of software. A document or standard that describes how to build or use an API is called an API specification.

Source: https://en.wikipedia.org/wiki/API</rdfs:comment>
  <rdfs:isDefinedBy rdf:resource="http://www.ease-crc.org/ont/SOMA-IO.owl"/>
  <rdfs:label xml:lang="en">API Specification</rdfs:label>
  <rdfs:subClassOf rdf:resource="&soma;InterfaceSpecification"/>
</owl:Class>

<owl:Class rdf:about="&soma;ContainmentTheory">
  <rdfs:comment>A schematic theory that describes a functional relation which ensures that the location of some entity, the locatum, is constrained to be within some region which is the interior of some other entity, the relatum.

This is also known as FunctionalControlInternal in GUM-4-space (Bateman et al. 2010).

Let xL, xR be objects filling the locatum, relatum roles of this schema. Then one can infer that xL isInsideOf xR.</rdfs:comment>
  <rdfs:isDefinedBy rdf:resource="http://www.ease-crc.org/ont/SOMA-SAY.owl"/>
  <rdfs:label xml:lang="en">Containment theory</rdfs:label>
  <rdfs:subClassOf rdf:resource="&soma;ControlTheory"/>
</owl:Class>

<owl:ObjectProperty rdf:about="&soma;hasShape"
    rdfs:comment="Relates an object to its shape quality."
    rdfs:label="has shape">
  <rdfs:domain rdf:resource="&dul;PhysicalObject"/>
  <rdfs:isDefinedBy rdf:resource="http://www.ease-crc.org/ont/SOMA-OBJ.owl"/>
  <rdfs:range rdf:resource="&soma;Shape"/>
  <rdfs:subPropertyOf rdf:resource="&dul;hasQuality"/>
  <owl:inverseOf rdf:resource="&soma;isShapeOf"/>
</owl:ObjectProperty>

<owl:Class rdf:about="&soma;SupportTheory">
  <rdfs:comment>An image schematic theory that describes the reified functional relation holding between two spatial objects x and y, such that x physically supports y in the presence of gravity; x and y need not be in contact. An example of such an expression is "The bowl is on the table".

This is also known as FunctionalControlExternal in GUM (Bateman et al. 2010).

Let xL, xR be objects filling the locatum, relatum roles of this schema. Then one can infer that xL isSupportedBy xR.</rdfs:comment>
  <rdfs:isDefinedBy rdf:resource="http://www.ease-crc.org/ont/SOMA-SAY.owl"/>
  <rdfs:label xml:lang="en">Support theory</rdfs:label>
  <rdfs:subClassOf rdf:resource="&soma;ControlTheory"/>
</owl:Class>

<owl:ObjectProperty rdf:about="&soma;isShapeRegionOf"
    rdfs:comment="Relates a shape to a physical object that has it."
    rdfs:label="is shape region of">
  <rdfs:domain rdf:resource="&soma;ShapeRegion"/>
  <rdfs:isDefinedBy rdf:resource="http://www.ease-crc.org/ont/SOMA-OBJ.owl"/>
  <rdfs:range>
    <owl:Class>
      <owl:unionOf rdf:parseType="Collection">
        <rdf:Description rdf:about="&soma;Shape"/>
        <rdf:Description rdf:about="&dul;PhysicalObject"/>
      </owl:unionOf>
    </owl:Class>
  </rdfs:range>
  <rdfs:subPropertyOf rdf:resource="&dul;isRegionFor"/>
</owl:ObjectProperty>

<owl:Class rdf:about="&soma;ProcessType"
    rdfs:comment="An EventType that classifies Processes."
    rdfs:label="Process type">
  <rdfs:subClassOf>
    <owl:Restriction>
      <owl:allValuesFrom rdf:resource="&dul;Process"/>
      <owl:onProperty rdf:resource="&dul;classifies"/>
    </owl:Restriction>
  </rdfs:subClassOf>
  <rdfs:subClassOf>
    <owl:Restriction>
      <owl:allValuesFrom rdf:resource="&soma;ProcessType"/>
      <owl:onProperty rdf:resource="&dul;hasPart"/>
    </owl:Restriction>
  </rdfs:subClassOf>
  <rdfs:subClassOf>
    <owl:Restriction>
      <owl:allValuesFrom rdf:resource="&dul;Description"/>
      <owl:onProperty rdf:resource="&dul;isDefinedIn"/>
    </owl:Restriction>
  </rdfs:subClassOf>
  <rdfs:subClassOf rdf:resource="&dul;EventType"/>
  <rdfs:isDefinedBy rdf:resource="http://www.ease-crc.org/ont/SOMA-PROC.owl"/>
</owl:Class>

<owl:Class rdf:about="&soma;InformationDismissal">
  <rdfs:subClassOf>
    <owl:Restriction>
      <owl:onProperty rdf:resource="&soma;isTaskOfInputRole"/>
      <owl:someValuesFrom>
        <owl:Class>
          <owl:intersectionOf rdf:parseType="Collection">
            <rdf:Description rdf:about="&soma;ExcludedObject"/>
            <rdf:Description rdf:about="&soma;Knowledge"/>
          </owl:intersectionOf>
        </owl:Class>
      </owl:someValuesFrom>
    </owl:Restriction>
  </rdfs:subClassOf>
  <rdfs:subClassOf rdf:resource="&soma;MentalTask"/>
  <rdfs:comment xml:lang="en">A mental task in which the executing agent dismisses some information.

An example is forgetting some knowledge.</rdfs:comment>
  <rdfs:isDefinedBy rdf:resource="http://www.ease-crc.org/ont/SOMA-ACT.owl"/>
  <rdfs:label xml:lang="en">Information dismissal</rdfs:label>
</owl:Class>

<owl:Class rdf:about="&soma;AlteredObject"
    rdfs:comment="An object undergoing modifications.">
  <rdfs:isDefinedBy rdf:resource="http://www.ease-crc.org/ont/SOMA-OBJ.owl"/>
  <rdfs:isDefinedBy rdf:resource="http://www.ease-crc.org/ont/SOMA-PROC.owl"/>
  <rdfs:label xml:lang="en">Altered object</rdfs:label>
  <rdfs:subClassOf rdf:resource="&soma;Patient"/>
</owl:Class>

<owl:ObjectProperty rdf:about="&dul;hasCommonBoundary"/>

<owl:Class rdf:about="&soma;Query">
  <rdfs:comment xml:lang="en">A role played by some Information Realization that carries meaning, where this meaning is a query of some sort.</rdfs:comment>
  <rdfs:isDefinedBy rdf:resource="http://www.ease-crc.org/ont/SOMA-ACT.owl"/>
  <rdfs:label xml:lang="en">Query</rdfs:label>
  <rdfs:subClassOf rdf:resource="&soma;Message"/>
</owl:Class>

<owl:Class rdf:about="&soma;InformationStorage">
  <rdfs:subClassOf>
    <owl:Restriction>
      <owl:onProperty rdf:resource="&soma;isTaskOfInputRole"/>
      <owl:someValuesFrom>
        <owl:Class>
          <owl:intersectionOf rdf:parseType="Collection">
            <rdf:Description rdf:about="&soma;Knowledge"/>
            <rdf:Description rdf:about="&soma;StoredObject"/>
          </owl:intersectionOf>
        </owl:Class>
      </owl:someValuesFrom>
    </owl:Restriction>
  </rdfs:subClassOf>
  <rdfs:subClassOf rdf:resource="&soma;MentalTask"/>
  <rdfs:comment xml:lang="en">A mental task in which the executing agent persists some information for later recall, if necessary.

An example is learning new knowledge.</rdfs:comment>
  <rdfs:isDefinedBy rdf:resource="http://www.ease-crc.org/ont/SOMA-ACT.owl"/>
  <rdfs:label xml:lang="en">Information storage</rdfs:label>
</owl:Class>

<owl:Class rdf:about="&soma;ExecutableSoftware">
  <rdfs:comment xml:lang="en">Executable Software is Software that can directly be executed, in comparison to a Software Library, which might only contain functionality via interfaces, but offers no execution entry point.</rdfs:comment>
  <rdfs:isDefinedBy rdf:resource="http://www.ease-crc.org/ont/SOMA-IO.owl"/>
  <rdfs:label xml:lang="en">Executable Software</rdfs:label>
  <owl:equivalentClass>
    <owl:Class>
      <owl:intersectionOf rdf:parseType="Collection">
        <rdf:Description rdf:about="&soma;Software"/>
        <owl:Restriction>
          <owl:onProperty rdf:resource="&dul;hasMember"/>
          <owl:someValuesFrom rdf:resource="&soma;ExecutableFile"/>
        </owl:Restriction>
      </owl:intersectionOf>
    </owl:Class>
  </owl:equivalentClass>
</owl:Class>

<owl:ObjectProperty rdf:about="&soma;isEventTypeDefinedIn">
  <rdfs:comment xml:lang="en">A relation between an event type and a description, e.g. an event that is described by the Affordance of an object to be cut with a knife.

The distinction to 'is task defined in' is necessary to let Dispositions and Affordances not only describe which tasks might be afforded by objects, but also whihc processes (where there is no agent). For example, the fall of a knife from a shelf slicing a loaf of bread on impact is , in the absence of an executing agent, not a task but merely a process, the possibility of which is nevertheless described by the dispositions of the knife and the loaf.</rdfs:comment>
  <rdfs:domain rdf:resource="&dul;EventType"/>
  <rdfs:isDefinedBy rdf:resource="http://www.ease-crc.org/ont/SOMA-ACT.owl"/>
  <rdfs:label xml:lang="en">is event type defined in</rdfs:label>
  <rdfs:range rdf:resource="&dul;Description"/>
  <rdfs:subPropertyOf rdf:resource="&dul;isDefinedIn"/>
</owl:ObjectProperty>

<owl:ObjectProperty rdf:about="&soma;isSetpointAffordedBy"
    rdfs:label="is setpoint afforded by">
  <rdfs:comment>Relates a disposition to the setpoint parameter defined by the affordance describing the disposition.</rdfs:comment>
  <rdfs:domain rdf:resource="&soma;Setpoint"/>
  <rdfs:isDefinedBy rdf:resource="http://www.ease-crc.org/ont/SOMA-OBJ.owl"/>
  <rdfs:range rdf:resource="&soma;Disposition"/>
  <rdfs:subPropertyOf rdf:resource="&soma;isConceptAffordedBy"/>
  <owl:propertyChainAxiom rdf:parseType="Collection">
    <rdf:Description rdf:about="&soma;isSetpointDefinedIn"/>
    <rdf:Description rdf:about="&dul;describes"/>
  </owl:propertyChainAxiom>
</owl:ObjectProperty>

<rdf:Property rdf:about="&soma;texture">
  <rdfs:domain rdf:resource="&soma;Object"/>
  <rdfs:range rdf:resource="&xsd;string"/>
</rdf:Property>

<owl:ObjectProperty rdf:about="&dul;hasParticipant">
  <rdfs:isDefinedBy rdf:resource="http://www.ease-crc.org/ont/SOMA-PROC.owl"/>
  <rdfs:isDefinedBy rdf:resource="http://www.ease-crc.org/ont/SOMA-STATE.owl"/>
  <rdfs:isDefinedBy rdf:resource="http://www.ease-crc.org/ont/SOMA.owl"/>
</owl:ObjectProperty>

<rdfs:Datatype rdf:about="&soma;array_boolean">
  <rdfs:isDefinedBy rdf:resource="http://www.ease-crc.org/ont/SOMA.owl"/>
  <owl:equivalentClass rdf:resource="&xsd;string"/>
</rdfs:Datatype>

<owl:Class rdf:about="&soma;Preference">
  <rdfs:subClassOf>
    <owl:Restriction>
      <owl:allValuesFrom rdf:resource="&dul;Agent"/>
      <owl:onProperty rdf:resource="&soma;isPreferenceOf"/>
    </owl:Restriction>
  </rdfs:subClassOf>
  <rdfs:subClassOf rdf:resource="&soma;SocialQuality"/>
  <rdfs:comment xml:lang="en">A 'Preference' is a 'Quality' of an 'Agent' that orders 'Situation's by some heuristic based on the happiness, satisfaction, gratification, morality, enjoyment, and utility (see alse https://en.wikipedia.org/wiki/Preference) they provide to their bearing Agent.

The pattern is as follows: A 'Preference' 'is described by' a 'Predilection', which also 'describes' an 'Order' that 'orders' 'Order item's that contain only 'Situation's. The 'Situation's then are modeled according to what the preference entails.

That a 'Preference' orders 'Situation's might be unintuitive, but makes the model very general. A few examples:

Example 1

"Peter likes coffee and dislikes tea".
Here, between different hypothetical situations where he plays the role of a performer in a drinking task, Peter prefers the situations in which role of the drunken object is played by some coffee (vs. some tea). Note that the coffe and tea are hypothetical objects as well and could, for example, be represented via reified Concepts.

Example 2

"Would you like this pot of coffee, or this pot of tea, Peter?"
Here, as opposed to Example 1, the pot of coffee and the pot of tea are not hypothetical, but concrete.

Example 3

"Would you like this pot of coffee, or should I brew you some tea?"
Here, the pot of coffee is concrete and the tea is not.

Example 4

Situations are not restricted to Tasks; other event types are possible as well.
For example, Peter might prefer the Containment State of a tiger being inside a cage vs. the Containment State of the tiger being outside of the cage.</rdfs:comment>
  <rdfs:isDefinedBy rdf:resource="http://www.ease-crc.org/ont/SOMA-AGENT.owl"/>
  <rdfs:label xml:lang="en">Preference</rdfs:label>
</owl:Class>

<owl:ObjectProperty rdf:about="&soma;hasColor"
    rdfs:comment="Relates an object to its color quality."
    rdfs:label="has color">
  <rdfs:domain rdf:resource="&dul;PhysicalObject"/>
  <rdfs:isDefinedBy rdf:resource="http://www.ease-crc.org/ont/SOMA-OBJ.owl"/>
  <rdfs:range rdf:resource="&soma;Color"/>
  <rdfs:subPropertyOf rdf:resource="&dul;hasQuality"/>
  <owl:inverseOf rdf:resource="&soma;isColorOf"/>
</owl:ObjectProperty>

<owl:Class rdf:about="&soma;Destruction"
    rdfs:label="Destruction">
  <rdfs:subClassOf>
    <owl:Restriction>
      <owl:onProperty rdf:resource="&soma;isProcessTypeOf"/>
      <owl:someValuesFrom rdf:resource="&soma;DestroyedObject"/>
    </owl:Restriction>
  </rdfs:subClassOf>
  <rdfs:subClassOf rdf:resource="&soma;ProcessType"/>
  <rdfs:comment>A process by which a physical Entity is destroyed.

Note, most of the physical Entities we are concerned with are actually arrangements of many smaller physical Entities, so another way to look at this is that a 'Physical destruction' is a process by which an arrangement of physical Entities, which was previously itself considered a physical Entity, is changed to such an extent that it is no longer recognized as continuing to exist.</rdfs:comment>
  <rdfs:isDefinedBy rdf:resource="http://www.ease-crc.org/ont/SOMA-PROC.owl"/>
</owl:Class>

<owl:Class rdf:about="&soma;SourceMaterialRole">
  <rdfs:comment>A role classifying a substance or object that enters a process of transformation intended to create some other object.</rdfs:comment>
  <rdfs:isDefinedBy rdf:resource="http://www.ease-crc.org/ont/SOMA-OBJ.owl"/>
  <rdfs:label xml:lang="en">Source material role</rdfs:label>
  <rdfs:subClassOf rdf:resource="&soma;ResourceRole"/>
</owl:Class>

<owl:Class rdf:about="&soma;InformationAcquisition">
  <rdfs:comment xml:lang="en">A mental task in which the executing agent acquires some information that was not immediately available to it before.
A synonym might be "Thinking".

Examples include recalling knowledge or inferring some information from other information.</rdfs:comment>
  <rdfs:isDefinedBy rdf:resource="http://www.ease-crc.org/ont/SOMA-ACT.owl"/>
  <rdfs:label xml:lang="en">Information acquisition</rdfs:label>
  <owl:equivalentClass>
    <owl:Class>
      <owl:intersectionOf rdf:parseType="Collection">
        <rdf:Description rdf:about="&soma;MentalTask"/>
        <owl:Restriction>
          <owl:onProperty rdf:resource="&soma;isTaskOfOutputRole"/>
          <owl:someValuesFrom rdf:resource="&soma;Knowledge"/>
        </owl:Restriction>
      </owl:intersectionOf>
    </owl:Class>
  </owl:equivalentClass>
</owl:Class>

<owl:Class rdf:about="&soma;Source_Code">
  <rdfs:comment xml:lang="en">The Source Code itself (the specific set of instruction in a human-readable Programming Language), not the file that it is contained in nor the implemented algorithm!</rdfs:comment>
  <rdfs:isDefinedBy rdf:resource="http://www.ease-crc.org/ont/SOMA-IO.owl"/>
  <rdfs:label xml:lang="en">Source code</rdfs:label>
  <rdfs:subClassOf rdf:resource="&soma;Computer_Program"/>
  <owl:equivalentClass>
    <owl:Class>
      <owl:intersectionOf rdf:parseType="Collection">
        <rdf:Description rdf:about="&soma;Computer_Program"/>
        <owl:Restriction>
          <owl:onProperty rdf:resource="&soma;isGivenMeaningBy"/>
          <owl:someValuesFrom rdf:resource="&soma;Human-readable_Programming_Language"/>
        </owl:Restriction>
      </owl:intersectionOf>
    </owl:Class>
  </owl:equivalentClass>
</owl:Class>

<owl:ObjectProperty rdf:about="&dul;isConstituentOf"/>

<owl:ObjectProperty rdf:about="&soma;hasFirstStep"
    rdfs:comment="A relation from a Workflow to its first Task."
    rdfs:label="has first step">
  <rdfs:domain rdf:resource="&dul;Workflow"/>
  <rdfs:isDefinedBy rdf:resource="http://www.ease-crc.org/ont/SOMA-WF.owl"/>
  <rdfs:range rdf:resource="&dul;Task"/>
  <rdfs:subPropertyOf rdf:resource="&soma;hasStep"/>
  <owl:inverseOf rdf:resource="&soma;isFirstStepOf"/>
</owl:ObjectProperty>

<owl:DatatypeProperty rdf:about="&soma;hasSpaceParameter"
    rdfs:label="has space parameter">
  <rdfs:comment>Associates a SpaceRegion to some parameter value describing it. This is a fairly generic property, and to capture the semantics of the information associated to the SpaceRegion, its more specific subproperties should be used.</rdfs:comment>
  <rdfs:domain rdf:resource="&dul;SpaceRegion"/>
  <rdfs:isDefinedBy rdf:resource="http://www.ease-crc.org/ont/SOMA-OBJ.owl"/>
  <rdfs:subPropertyOf rdf:resource="&dul;hasRegionDataValue"/>
</owl:DatatypeProperty>

<owl:ObjectProperty rdf:about="&soma;relatesToAnotherRole"
    rdfs:comment="Simple top-level property for relations between two roles."
    rdfs:label="relates to another role">
  <rdf:type rdf:resource="&owl;SymmetricProperty"/>
  <rdfs:domain rdf:resource="&dul;Role"/>
  <rdfs:isDefinedBy rdf:resource="http://www.ease-crc.org/ont/SOMA-ACT.owl"/>
  <rdfs:range rdf:resource="&dul;Role"/>
  <rdfs:subPropertyOf rdf:resource="&dul;associatedWith"/>
</owl:ObjectProperty>

<owl:ObjectProperty rdf:about="&soma;isStepOf"
    rdfs:comment="A relation stating that a task is a step in a workflow."
    rdfs:label="is step of">
  <rdfs:domain rdf:resource="&dul;Task"/>
  <rdfs:isDefinedBy rdf:resource="http://www.ease-crc.org/ont/SOMA-WF.owl"/>
  <rdfs:range rdf:resource="&dul;Workflow"/>
  <rdfs:subPropertyOf rdf:resource="&dul;isTaskDefinedIn"/>
</owl:ObjectProperty>

<owl:Class rdf:about="&soma;Reasoner">
  <rdfs:comment xml:lang="en">A Reasoner is some Software that can infer new, implicit knowlegde from explicitly stated knowledge.

This definition is broad and we consider any System fitting the above description as reasoners. For example, the following can be seen as Reasoners:
* A simulation, where the explicit knowledge corresponds to the initial situation, and the implicit knowlegde corresponds to the situation that is derived from that by simulating some unfolding processes.
* A machine learning algorithm, e.g., an image classifier: The explicit knowledge is the visual content of a picture (even down to the pixel), the implicit knowledge is the derived classification.
* A logic based rule engine, where initial facts are the explicit knowledge, and derived facts are the implicit knowledge.</rdfs:comment>
  <rdfs:isDefinedBy rdf:resource="http://www.ease-crc.org/ont/SOMA-IO.owl"/>
  <rdfs:subClassOf rdf:resource="&soma;SoftwareRole"/>
</owl:Class>

<owl:Class rdf:about="&soma;FunctionalDesign"
    rdfs:label="Functional Design">
  <rdfs:comment>The design of an object from functionality point of view. A functional design is useful to develop complex modular objects with components that have a specific purpose, and can function with minimum side effect on other components of that object. </rdfs:comment>
  <rdfs:isDefinedBy rdf:resource="http://www.ease-crc.org/ont/SOMA-OBJ.owl"/>
  <rdfs:subClassOf rdf:resource="&dul;Design"/>
</owl:Class>

<owl:ObjectProperty rdf:about="&soma;definesProcess"
    rdfs:comment="A relation between a description and a process type."
    rdfs:label="defines process">
  <rdfs:domain rdf:resource="&dul;Description"/>
  <rdfs:isDefinedBy rdf:resource="http://www.ease-crc.org/ont/SOMA-PROC.owl"/>
  <rdfs:range rdf:resource="&soma;ProcessType"/>
  <rdfs:subPropertyOf rdf:resource="&dul;defines"/>
  <owl:inverseOf rdf:resource="&soma;isProcessDefinedIn"/>
</owl:ObjectProperty>

<owl:Class rdf:about="&soma;JointState"
    rdfs:label="Joint state">
  <rdfs:subClassOf>
    <owl:Restriction>
      <owl:onDataRange rdf:resource="&xsd;double"/>
      <owl:onProperty rdf:resource="&soma;hasJointPosition"/>
      <owl:qualifiedCardinality rdf:datatype="&xsd;nonNegativeInteger">1</owl:qualifiedCardinality>
    </owl:Restriction>
  </rdfs:subClassOf>
  <rdfs:subClassOf>
    <owl:Restriction>
      <owl:onDataRange rdf:resource="&xsd;double"/>
      <owl:onProperty rdf:resource="&soma;hasJointVelocity"/>
      <owl:qualifiedCardinality rdf:datatype="&xsd;nonNegativeInteger">1</owl:qualifiedCardinality>
    </owl:Restriction>
  </rdfs:subClassOf>
  <rdfs:subClassOf>
    <owl:Restriction>
      <owl:maxQualifiedCardinality rdf:datatype="&xsd;nonNegativeInteger">1</owl:maxQualifiedCardinality>
      <owl:onDataRange rdf:resource="&xsd;double"/>
      <owl:onProperty rdf:resource="&soma;hasJointEffort"/>
    </owl:Restriction>
  </rdfs:subClassOf>
  <rdfs:subClassOf rdf:resource="&dul;PhysicalAttribute"/>
  <rdfs:comment>The state of a joint in terms of position, velocity of the joint and effort applied to it.</rdfs:comment>
  <rdfs:isDefinedBy rdf:resource="http://www.ease-crc.org/ont/SOMA-OBJ.owl"/>
</owl:Class>

<owl:Class rdf:about="&dul;Event">
  <rdfs:isDefinedBy rdf:resource="http://www.ease-crc.org/ont/SOMA-STATE.owl"/>
</owl:Class>

<owl:Class rdf:about="&soma;ThinkAloudPerceptionTopic"
    rdfs:label="Think aloud perception topic">
  <rdfs:comment>A topic used when an Agent describes what they currently perceive.</rdfs:comment>
  <rdfs:isDefinedBy rdf:resource="http://www.ease-crc.org/ont/SOMA-ACT.owl"/>
  <rdfs:subClassOf rdf:resource="&soma;ThinkAloudTopic"/>
</owl:Class>

<owl:Class rdf:about="&dul;PhysicalPlace"/>

<owl:ObjectProperty rdf:about="&soma;encodes">
  <rdf:type rdf:resource="&owl;SymmetricProperty"/>
  <rdfs:comment xml:lang="en">The relation between two Information Objects that have the same meaning, but are formatted differently. E.g., a text written in UTF-8 encodes a text in a natural writing system (letters) and vice versa.</rdfs:comment>
  <rdfs:domain rdf:resource="&dul;InformationObject"/>
  <rdfs:isDefinedBy rdf:resource="http://www.ease-crc.org/ont/SOMA-IO.owl"/>
  <rdfs:range rdf:resource="&dul;InformationObject"/>
  <rdfs:subPropertyOf rdf:resource="&dul;associatedWith"/>
</owl:ObjectProperty>

<owl:Class rdf:about="&soma;SupportState">
  <rdfs:subClassOf>
    <owl:Restriction>
      <owl:onProperty rdf:resource="&soma;isStateTypeOf"/>
      <owl:someValuesFrom>
        <owl:Class>
          <owl:intersectionOf rdf:parseType="Collection">
            <rdf:Description rdf:about="&soma;Supporter"/>
            <owl:Restriction>
              <owl:allValuesFrom>
                <owl:Restriction>
                  <owl:onProperty rdf:resource="&soma;hasDisposition"/>
                  <owl:someValuesFrom rdf:resource="&soma;Deposition"/>
                </owl:Restriction>
              </owl:allValuesFrom>
              <owl:onProperty rdf:resource="&dul;classifies"/>
            </owl:Restriction>
          </owl:intersectionOf>
        </owl:Class>
      </owl:someValuesFrom>
    </owl:Restriction>
  </rdfs:subClassOf>
  <rdfs:subClassOf rdf:resource="&soma;FunctionalControl"/>
  <rdfs:comment>Classifies States in which an object is not able to move under gravity because of its placement relative to some other object.</rdfs:comment>
  <rdfs:isDefinedBy rdf:resource="http://www.ease-crc.org/ont/SOMA-STATE.owl"/>
  <rdfs:label xml:lang="en">Support state</rdfs:label>
</owl:Class>

<owl:Class rdf:about="&soma;Protector">
  <rdfs:comment>A role classifying an object that protects another by preventing other entities from coming in contact with the protected object.</rdfs:comment>
  <rdfs:isDefinedBy rdf:resource="http://www.ease-crc.org/ont/SOMA-OBJ.owl"/>
  <rdfs:subClassOf rdf:resource="&soma;Restrictor"/>
</owl:Class>

<owl:Class rdf:about="&dul;Task">
  <rdfs:isDefinedBy rdf:resource="http://www.ease-crc.org/ont/SOMA-WF.owl"/>
</owl:Class>

<owl:DatatypeProperty rdf:about="&soma;hasMassValue"
    rdfs:comment="The mass value of a physical object in kilogram."
    rdfs:label="has mass value">
  <rdfs:domain rdf:resource="&soma;MassAttribute"/>
  <rdfs:isDefinedBy rdf:resource="http://www.ease-crc.org/ont/SOMA-OBJ.owl"/>
  <rdfs:range rdf:resource="&xsd;double"/>
  <rdfs:subPropertyOf rdf:resource="&dul;hasRegionDataValue"/>
</owl:DatatypeProperty>

<owl:ObjectProperty rdf:about="&soma;isPlaceInvolvedIn"
    rdfs:label="is place involved in">
  <rdfs:comment>A relation recording that a PhysicalPlace is involved in some Event; typically, this is where the Event is located.</rdfs:comment>
  <rdfs:domain rdf:resource="&dul;PhysicalPlace"/>
  <rdfs:isDefinedBy rdf:resource="http://www.ease-crc.org/ont/SOMA.owl"/>
  <rdfs:range rdf:resource="&dul;Event"/>
  <rdfs:subPropertyOf rdf:resource="&dul;isParticipantIn"/>
</owl:ObjectProperty>

<owl:Class rdf:about="&soma;AgentRole">
  <rdfs:isDefinedBy rdf:resource="http://www.ease-crc.org/ont/SOMA-AGENT.owl"/>
  <rdfs:isDefinedBy rdf:resource="http://www.ease-crc.org/ont/SOMA-OBJ.owl"/>
  <rdfs:subClassOf>
    <owl:Restriction>
      <owl:allValuesFrom rdf:resource="&dul;Agent"/>
      <owl:onProperty rdf:resource="&dul;classifies"/>
    </owl:Restriction>
  </rdfs:subClassOf>
  <rdfs:subClassOf rdf:resource="&soma;CausativeRole"/>
  <rdfs:comment>A role classifying an Agent responsible for performing an Action.

The entity playing an AgentRole is endowed with sentience and the capacity to deliberately choose actions in pursuit of goals. This distinguishes Agents from other causes that could bring an event about.</rdfs:comment>
  <rdfs:label xml:lang="en">Agent role</rdfs:label>
</owl:Class>

<owl:Class rdf:about="&soma;Pourable">
  <rdfs:subClassOf>
    <owl:Restriction>
      <owl:allValuesFrom rdf:resource="&soma;PouredObject"/>
      <owl:onProperty rdf:resource="&soma;affordsBearer"/>
    </owl:Restriction>
  </rdfs:subClassOf>
  <rdfs:subClassOf rdf:resource="&soma;Disposition"/>
  <rdfs:comment>The disposition of a fluid or substance which makes it possible to pour it out of a container and into or onto other objects.</rdfs:comment>
  <rdfs:isDefinedBy rdf:resource="http://www.ease-crc.org/ont/SOMA-OBJ.owl"/>
</owl:Class>

<owl:ObjectProperty rdf:about="&soma;isRecordIncludedBy">
  <rdfs:comment>A relationship indicating that an InformationObject is a recording of an Event.</rdfs:comment>
  <rdfs:domain rdf:resource="&dul;InformationObject"/>
  <rdfs:isDefinedBy rdf:resource="http://www.ease-crc.org/ont/SOMA.owl"/>
  <rdfs:range rdf:resource="&dul;Event"/>
  <rdfs:subPropertyOf rdf:resource="&dul;isAbout"/>
</owl:ObjectProperty>

<owl:Class rdf:about="&soma;LinkageState">
  <rdfs:subClassOf>
    <owl:Restriction>
      <owl:onProperty rdf:resource="&soma;isStateTypeOf"/>
      <owl:someValuesFrom rdf:resource="&soma;LinkedObject"/>
    </owl:Restriction>
  </rdfs:subClassOf>
  <rdfs:subClassOf rdf:resource="&soma;StateType"/>
  <rdfs:comment>Classifies States in which two objects are in a rigid connection, such that the movement of one determines the movement of the other.</rdfs:comment>
  <rdfs:isDefinedBy rdf:resource="http://www.ease-crc.org/ont/SOMA-STATE.owl"/>
  <rdfs:label xml:lang="en">Linkage state</rdfs:label>
</owl:Class>

<owl:Class rdf:about="&soma;MetacognitiveControlling"
    rdfs:label="Metacognitive controlling">
  <rdfs:comment>The concious or subconcious task to control the own mental processes, e.g., evaluating them and instructing the own mind to shift attention.</rdfs:comment>
  <rdfs:isDefinedBy rdf:resource="http://www.ease-crc.org/ont/SOMA-ACT.owl"/>
  <rdfs:subClassOf rdf:resource="&soma;MentalTask"/>
</owl:Class>

<owl:ObjectProperty rdf:about="&soma;isProcessTypeOf"
    rdfs:label="is process type of">
  <rdfs:comment>A relation between roles and process types, e.g. a catalysator is needed to trigger some chemical reaction.</rdfs:comment>
  <rdfs:domain rdf:resource="&soma;ProcessType"/>
  <rdfs:isDefinedBy rdf:resource="http://www.ease-crc.org/ont/SOMA-PROC.owl"/>
  <rdfs:range rdf:resource="&dul;Role"/>
  <rdfs:subPropertyOf rdf:resource="&dul;isRelatedToConcept"/>
</owl:ObjectProperty>

<owl:ObjectProperty rdf:about="&soma;containsEvent"
    soma:symbol="di"
    rdfs:label="contains event">
  <rdfs:subPropertyOf rdf:resource="&soma;coOccurs"/>
  <rdfs:subPropertyOf rdf:resource="&soma;contains"/>
  <rdf:type rdf:resource="&owl;TransitiveProperty"/>
  <rdfs:comment>`A contains event B` means that A strictly starts before, and ends after B, i.e. B is wholly contained in A.</rdfs:comment>
  <rdfs:domain rdf:resource="&dul;Event"/>
  <rdfs:isDefinedBy rdf:resource="http://www.ease-crc.org/ont/SOMA.owl"/>
  <rdfs:range rdf:resource="&dul;Event"/>
  <owl:inverseOf rdf:resource="&soma;during"/>
</owl:ObjectProperty>

<owl:ObjectProperty rdf:about="&soma;isTerminatedBy">
  <rdfs:comment xml:lang="en">The association between an Event that is terminated by another Event, e.g., the Action of picking an apple from a bowl of fruits terminates the State of containment between the apple and the bowl.</rdfs:comment>
  <rdfs:domain rdf:resource="&dul;Event"/>
  <rdfs:isDefinedBy rdf:resource="http://www.ease-crc.org/ont/SOMA-ACT.owl"/>
  <rdfs:label xml:lang="en">is terminated by</rdfs:label>
  <rdfs:range rdf:resource="&dul;Event"/>
  <rdfs:subPropertyOf rdf:resource="&dul;associatedWith"/>
  <owl:inverseOf rdf:resource="&soma;terminates"/>
</owl:ObjectProperty>

<owl:ObjectProperty rdf:about="&soma;hasAlterationResult"
    rdfs:label="has alteration result">
  <rdfs:comment>Relates an action that alters an object to the region that the alteration reached during the action.</rdfs:comment>
  <rdfs:domain rdf:resource="&dul;Action"/>
  <rdfs:isDefinedBy rdf:resource="http://www.ease-crc.org/ont/SOMA-OBJ.owl"/>
  <rdfs:range rdf:resource="&dul;Region"/>
  <rdfs:subPropertyOf rdf:resource="&dul;hasRegion"/>
  <owl:inverseOf rdf:resource="&soma;isAlterationResultOf"/>
</owl:ObjectProperty>

<owl:Class rdf:about="&soma;AvoidedObject"
    rdfs:comment="An object that is avoided.">
  <rdfs:isDefinedBy rdf:resource="http://www.ease-crc.org/ont/SOMA-OBJ.owl"/>
  <rdfs:label xml:lang="en">Avoided object</rdfs:label>
  <rdfs:subClassOf rdf:resource="&soma;Patient"/>
</owl:Class>

<owl:Class rdf:about="&soma;ThinkAloudOpinionTopic"
    rdfs:label="Think aloud opinion topic">
  <rdfs:comment>A topic used when an Agent expresses an opinion about the action they perform or the environment they are in.</rdfs:comment>
  <rdfs:isDefinedBy rdf:resource="http://www.ease-crc.org/ont/SOMA-ACT.owl"/>
  <rdfs:subClassOf rdf:resource="&soma;ThinkAloudTopic"/>
</owl:Class>

<owl:Class rdf:about="&soma;SelectingItem">
  <rdfs:subClassOf>
    <owl:Restriction>
      <owl:onProperty rdf:resource="&soma;isTaskOfOutputRole"/>
      <owl:someValuesFrom>
        <owl:Class>
          <owl:intersectionOf rdf:parseType="Collection">
            <rdf:Description rdf:about="&soma;SelectedObject"/>
            <owl:Restriction>
              <owl:allValuesFrom rdf:resource="&dul;PhysicalObject"/>
              <owl:onProperty rdf:resource="&dul;classifies"/>
            </owl:Restriction>
          </owl:intersectionOf>
        </owl:Class>
      </owl:someValuesFrom>
    </owl:Restriction>
  </rdfs:subClassOf>
  <rdfs:subClassOf rdf:resource="&soma;GetTaskParameter"/>
  <rdfs:comment>A task in which an Agent selects some object to use for a subsequent task.</rdfs:comment>
  <rdfs:isDefinedBy rdf:resource="http://www.ease-crc.org/ont/SOMA-ACT.owl"/>
  <rdfs:label xml:lang="en">Selecting item</rdfs:label>
</owl:Class>

<owl:ObjectProperty rdf:about="&soma;isOntopOf"
    rdfs:label="is ontop of">
  <rdfs:comment>A spatial relation holding between an object (the deposit), and objects that are located ontop of it.</rdfs:comment>
  <rdfs:domain rdf:resource="&dul;PhysicalObject"/>
  <rdfs:isDefinedBy rdf:resource="http://www.ease-crc.org/ont/SOMA-OBJ.owl"/>
  <rdfs:range rdf:resource="&dul;PhysicalObject"/>
  <rdfs:subPropertyOf rdf:resource="&dul;hasLocation"/>
</owl:ObjectProperty>

<owl:Class rdf:about="&soma;SuccessDiagnosis"
    rdfs:label="Success diagnosis">
  <rdfs:comment>A diagnosis of the fullfilment of a goal that motivates the behavior of a system.</rdfs:comment>
  <rdfs:isDefinedBy rdf:resource="http://www.ease-crc.org/ont/SOMA.owl"/>
  <rdfs:subClassOf rdf:resource="&soma;BehavioralDiagnosis"/>
</owl:Class>

<owl:Class rdf:about="&soma;Capacity"
    rdfs:comment="The maximum amount an object can contain.">
  <rdfs:isDefinedBy rdf:resource="http://www.ease-crc.org/ont/SOMA-OBJ.owl"/>
  <rdfs:subClassOf rdf:resource="&soma;Intrinsic"/>
</owl:Class>

<owl:Class rdf:about="&soma;Scene">
  <rdfs:isDefinedBy rdf:resource="http://www.ease-crc.org/ont/SOMA-SAY.owl"/>
  <rdfs:isDefinedBy rdf:resource="http://www.ease-crc.org/ont/SOMA.owl"/>
  <rdfs:subClassOf>
    <owl:Restriction>
      <owl:onProperty rdf:resource="&dul;includesEvent"/>
      <owl:someValuesFrom rdf:resource="&soma;State"/>
    </owl:Restriction>
  </rdfs:subClassOf>
  <rdfs:subClassOf>
    <owl:Restriction>
      <owl:onProperty rdf:resource="&dul;satisfies"/>
      <owl:someValuesFrom rdf:resource="&soma;ImageSchemaTheory"/>
    </owl:Restriction>
  </rdfs:subClassOf>
  <rdfs:subClassOf rdf:resource="&dul;Situation"/>
  <rdfs:comment>Scenes are Situations which interpret a State in terms of its conformance to some qualitative, image schematic description. I.e., the scene is described in terms of qualitative functional and spatial relations existing between participating objects.</rdfs:comment>
</owl:Class>

<owl:Class rdf:about="&soma;Placing">
  <rdfs:comment>Distinguished from Positioning in that this task is more about placing an object at a functionally specified location (e.g., place the cup on the table) as opposed to positioning an object at a location defined by coordinates or a region of coordinates (position the cup at xyz).</rdfs:comment>
  <rdfs:isDefinedBy rdf:resource="http://www.ease-crc.org/ont/SOMA-ACT.owl"/>
  <rdfs:subClassOf rdf:resource="&soma;PhysicalTask"/>
</owl:Class>

<owl:DatatypeProperty rdf:about="&soma;hasRadius"
    rdfs:comment="The radius of a circular or oval shape."
    rdfs:label="has radius">
  <rdfs:domain rdf:resource="&soma;ShapeRegion"/>
  <rdfs:isDefinedBy rdf:resource="http://www.ease-crc.org/ont/SOMA-OBJ.owl"/>
  <rdfs:range rdf:resource="&xsd;float"/>
  <rdfs:subPropertyOf rdf:resource="&soma;hasShapeParameter"/>
</owl:DatatypeProperty>

<owl:ObjectProperty rdf:about="&dul;hasRegion">
  <rdfs:isDefinedBy rdf:resource="http://www.ease-crc.org/ont/SOMA.owl"/>
</owl:ObjectProperty>

<owl:Class rdf:about="&soma;Dropping">
  <rdfs:comment>The dropped object falls mainly under the influence of gravity. However, an agent may also drop something during navigation. The difference to 'Throwing' is that there is no 'Limb motion' which is a constitiuent of the action.

'Dropping' is intentional. Dropping by accident may not has a phase to release the grasp. It could be that the grasp was not strong enough and the objects "slips" away.</rdfs:comment>
  <rdfs:isDefinedBy rdf:resource="http://www.ease-crc.org/ont/SOMA-ACT.owl"/>
  <rdfs:subClassOf rdf:resource="&soma;Actuating"/>
  <owl:disjointWith rdf:resource="&soma;Placing"/>
</owl:Class>

<owl:ObjectProperty rdf:about="&soma;hasAnswer"
    rdfs:comment="The relation between a message and its answer."
    rdfs:label="has answer">
  <rdfs:domain rdf:resource="&soma;Message"/>
  <rdfs:isDefinedBy rdf:resource="http://www.ease-crc.org/ont/SOMA-ACT.owl"/>
  <rdfs:range rdf:resource="&soma;Answer"/>
  <rdfs:subPropertyOf rdf:resource="&soma;relatesToAnotherRole"/>
</owl:ObjectProperty>

<owl:ObjectProperty rdf:about="&soma;hasStatus"
    rdfs:label="has status">
  <rdfs:comment>A relation from an Entity to a Quality that is indicative of the Entity's state, e.g. if it is a device, its state of operation.</rdfs:comment>
  <rdfs:isDefinedBy rdf:resource="http://www.ease-crc.org/ont/SOMA.owl"/>
  <rdfs:subPropertyOf rdf:resource="&dul;hasQuality"/>
</owl:ObjectProperty>

<owl:Class rdf:about="&soma;Imagining">
  <rdfs:comment>A Mental task in which the Agent constructs a mental representation of a possible world. An Agent performing an Imagining activity does not aim to construct a representation that aspires to be faithful to some past, present, or future state of affairs of the actual world it is embodied in.</rdfs:comment>
  <rdfs:isDefinedBy rdf:resource="http://www.ease-crc.org/ont/SOMA-ACT.owl"/>
  <rdfs:subClassOf rdf:resource="&soma;InformationAcquisition"/>
</owl:Class>

<owl:Class rdf:about="&soma;MovedObject"
    rdfs:comment="An object undergoing location change.">
  <rdfs:isDefinedBy rdf:resource="http://www.ease-crc.org/ont/SOMA-OBJ.owl"/>
  <rdfs:isDefinedBy rdf:resource="http://www.ease-crc.org/ont/SOMA-PROC.owl"/>
  <rdfs:subClassOf>
    <owl:Restriction>
      <owl:onProperty rdf:resource="&soma;isTriggerDefinedIn"/>
      <owl:someValuesFrom>
        <owl:Restriction>
          <owl:allValuesFrom rdf:resource="&soma;Localization"/>
          <owl:onProperty rdf:resource="&soma;describesQuality"/>
        </owl:Restriction>
      </owl:someValuesFrom>
    </owl:Restriction>
  </rdfs:subClassOf>
  <rdfs:subClassOf>
    <owl:Restriction>
      <owl:allValuesFrom>
        <owl:Restriction>
          <owl:onProperty rdf:resource="&dul;hasQuality"/>
          <owl:someValuesFrom rdf:resource="&soma;Localization"/>
        </owl:Restriction>
      </owl:allValuesFrom>
      <owl:onProperty rdf:resource="&dul;classifies"/>
    </owl:Restriction>
  </rdfs:subClassOf>
  <rdfs:subClassOf rdf:resource="&soma;AlteredObject"/>
  <rdfs:label xml:lang="en">Moved object</rdfs:label>
</owl:Class>

<owl:Class rdf:about="&soma;Head">
  <rdfs:comment>A functional part of the body responsible for carrying high bandwidth sensors, i.e., camera.</rdfs:comment>
  <rdfs:isDefinedBy rdf:resource="http://www.ease-crc.org/ont/SOMA-OBJ.owl"/>
  <rdfs:subClassOf rdf:resource="&soma;FunctionalPart"/>
</owl:Class>

<owl:Class rdf:about="&soma;SymbolicReasoner">
  <rdfs:comment xml:lang="en">A Symbolic Reasoner, is a piece of software able to infer logical consequences from a set of asserted facts or axioms.

Source: https://en.wikipedia.org/wiki/Semantic_reasoner</rdfs:comment>
  <rdfs:isDefinedBy rdf:resource="http://www.ease-crc.org/ont/SOMA-IO.owl"/>
  <rdfs:label xml:lang="en">Symbolic reasoner</rdfs:label>
  <rdfs:subClassOf rdf:resource="&soma;Reasoner"/>
</owl:Class>

<owl:ObjectProperty rdf:about="&soma;isCreatedOutputOf"
    rdfs:label="is created output of">
  <rdfs:comment>A relation between a created output role and its Task. The difference to isOutputRoleOf is that the latter is also applicable, e.g., for Deciding between objects, where the selected object is not created, but still an outcome of that task.</rdfs:comment>
  <rdfs:domain rdf:resource="&dul;Role"/>
  <rdfs:isDefinedBy rdf:resource="http://www.ease-crc.org/ont/SOMA-ACT.owl"/>
  <rdfs:range rdf:resource="&dul;Task"/>
  <rdfs:subPropertyOf rdf:resource="&soma;isOutputRoleOf"/>
  <owl:inverseOf rdf:resource="&soma;isTaskOfCreatedRole"/>
</owl:ObjectProperty>

<owl:Class rdf:about="&soma;Distancing">
  <rdfs:comment>A task in which an Agent increases its distance from some location.</rdfs:comment>
  <rdfs:isDefinedBy rdf:resource="http://www.ease-crc.org/ont/SOMA-ACT.owl"/>
  <rdfs:subClassOf rdf:resource="&soma;Navigating"/>
</owl:Class>

<owl:Class rdf:about="&soma;FunctionalPart"
    rdfs:label="Functional part">
  <rdfs:subClassOf>
    <owl:Restriction>
      <owl:allValuesFrom>
        <owl:Class>
          <owl:unionOf rdf:parseType="Collection">
            <rdf:Description rdf:about="&dul;Agent"/>
            <rdf:Description rdf:about="&dul;DesignedArtifact"/>
          </owl:unionOf>
        </owl:Class>
      </owl:allValuesFrom>
      <owl:onProperty rdf:resource="&dul;isComponentOf"/>
    </owl:Restriction>
  </rdfs:subClassOf>
  <rdfs:subClassOf rdf:resource="&dul;PhysicalBody"/>
  <rdfs:comment>Parts of an agent or an artifact are considered as functional parts.</rdfs:comment>
  <rdfs:isDefinedBy rdf:resource="http://www.ease-crc.org/ont/SOMA-OBJ.owl"/>
</owl:Class>

<owl:Class rdf:about="&soma;InferenceRules"
    rdfs:label="Inference rules">
  <rdfs:comment>The role of an object that is used to derive a conclusion from some premises.</rdfs:comment>
  <rdfs:isDefinedBy rdf:resource="http://www.ease-crc.org/ont/SOMA-ACT.owl"/>
  <rdfs:subClassOf rdf:resource="&soma;Knowledge"/>
</owl:Class>

<owl:ObjectProperty rdf:about="&soma;definesOutput">
  <rdfs:comment>Defines an "output" participant:

- an Entity (Object or state of affairs) that exists as a result of the execution of a Task;
- a Region/value that has been demarcated/computed as a result of the execution of a Task.</rdfs:comment>
  <rdfs:domain rdf:resource="&dul;Description"/>
  <rdfs:isDefinedBy rdf:resource="http://www.ease-crc.org/ont/SOMA-WF.owl"/>
  <rdfs:range>
    <owl:Class>
      <owl:unionOf rdf:parseType="Collection">
        <rdf:Description rdf:about="&dul;Parameter"/>
        <rdf:Description rdf:about="&dul;Role"/>
      </owl:unionOf>
    </owl:Class>
  </rdfs:range>
  <rdfs:subPropertyOf rdf:resource="&soma;definesParticipant"/>
</owl:ObjectProperty>

<owl:Class rdf:about="&soma;Leaning"
    rdfs:comment="An Agent pitches its body in some direction.">
  <rdfs:isDefinedBy rdf:resource="http://www.ease-crc.org/ont/SOMA-PROC.owl"/>
  <rdfs:subClassOf rdf:resource="&soma;PosturalMoving"/>
</owl:Class>

<owl:DatatypeProperty rdf:about="&soma;hasIntervalBegin"
    rdfs:comment="A relation recording when some TimeInterval started."
    rdfs:label="has interval begin">
  <rdfs:domain rdf:resource="&dul;TimeInterval"/>
  <rdfs:isDefinedBy rdf:resource="http://www.ease-crc.org/ont/SOMA.owl"/>
  <rdfs:range rdf:resource="&xsd;float"/>
  <rdfs:subPropertyOf rdf:resource="&soma;hasIntervalTime"/>
</owl:DatatypeProperty>

<owl:ObjectProperty rdf:about="&soma;definesPerformer">
  <rdfs:comment xml:lang="en">Relates an affordance which is a relation between a bearer and a trigger, to the role of the performer when the affordance is manifested.</rdfs:comment>
  <rdfs:domain rdf:resource="&soma;Affordance"/>
  <rdfs:isDefinedBy rdf:resource="http://www.ease-crc.org/ont/SOMA-OBJ.owl"/>
  <rdfs:label xml:lang="en">defines performer</rdfs:label>
  <rdfs:range rdf:resource="&dul;Role"/>
  <rdfs:subPropertyOf rdf:resource="&dul;definesRole"/>
  <owl:inverseOf rdf:resource="&soma;isPerformerDefinedIn"/>
</owl:ObjectProperty>

<owl:Class rdf:about="&dul;PhysicalObject">
  <rdfs:isDefinedBy rdf:resource="http://www.ease-crc.org/ont/SOMA-PROC.owl"/>
  <rdfs:isDefinedBy rdf:resource="http://www.ease-crc.org/ont/SOMA-STATE.owl"/>
</owl:Class>

<owl:Class rdf:about="&soma;PhaseTransition"
    rdfs:label="Phase transition">
  <rdfs:comment>An EventType that classifies processes by which matter changes from some distinguishable phase to another. We will use this to refer to the classical phase transitions between Solid, Liquid, Gaseous, Plasma etc. phases.</rdfs:comment>
  <rdfs:isDefinedBy rdf:resource="http://www.ease-crc.org/ont/SOMA-PROC.owl"/>
  <rdfs:seeAlso>The phase transition concept has also been more or less metaphorically applied in other contexts. An example from physics is the "jamming transition", and sometimes "phase transitions" are spoken of when describing problem spaces such as 3SAT.

In all these cases, the metaphor points to the existence of several regions of qualitatively different behavior (unimpeded passage of solid grains vs deadlock in a corridor; problem instances where the answer NO is trivial to prove vs. problem instances where the answer YES is trivial to prove), separated fairly sharply when some quantity reaches a threshold.</rdfs:seeAlso>
  <rdfs:subClassOf rdf:resource="&soma;Alteration"/>
</owl:Class>

<owl:Class rdf:about="&soma;ShapedObject"
    rdfs:comment="An object undergoing shape change.">
  <rdfs:isDefinedBy rdf:resource="http://www.ease-crc.org/ont/SOMA-OBJ.owl"/>
  <rdfs:isDefinedBy rdf:resource="http://www.ease-crc.org/ont/SOMA-PROC.owl"/>
  <rdfs:subClassOf>
    <owl:Restriction>
      <owl:onProperty rdf:resource="&soma;isTriggerDefinedIn"/>
      <owl:someValuesFrom>
        <owl:Restriction>
          <owl:allValuesFrom rdf:resource="&soma;Shape"/>
          <owl:onProperty rdf:resource="&soma;describesQuality"/>
        </owl:Restriction>
      </owl:someValuesFrom>
    </owl:Restriction>
  </rdfs:subClassOf>
  <rdfs:subClassOf>
    <owl:Restriction>
      <owl:allValuesFrom>
        <owl:Restriction>
          <owl:onProperty rdf:resource="&dul;hasQuality"/>
          <owl:someValuesFrom rdf:resource="&soma;Shape"/>
        </owl:Restriction>
      </owl:allValuesFrom>
      <owl:onProperty rdf:resource="&dul;classifies"/>
    </owl:Restriction>
  </rdfs:subClassOf>
  <rdfs:subClassOf rdf:resource="&soma;AlteredObject"/>
  <rdfs:label xml:lang="en">Shaped object</rdfs:label>
</owl:Class>

<owl:Class rdf:about="&soma;CleanlinessRegion"
    rdfs:comment="Encodes the cleanliness of an object.">
  <rdfs:isDefinedBy rdf:resource="http://www.ease-crc.org/ont/SOMA-OBJ.owl"/>
  <rdfs:label xml:lang="en">Cleanliness region</rdfs:label>
  <rdfs:subClassOf rdf:resource="&dul;Region"/>
</owl:Class>

<owl:Axiom>
  <rdfs:comment>If a SituationTransition manifests in some Event, then it also has an initial Situation and a terminal one.</rdfs:comment>
  <owl:annotatedProperty rdf:resource="&rdfs;subClassOf"/>
  <owl:annotatedSource>
    <owl:Class>
      <rdfs:subClassOf>
        <owl:Class rdf:nodeID="bn7">
          <owl:intersectionOf rdf:parseType="Collection">

            <owl:Restriction>
              <owl:onProperty rdf:resource="&soma;hasInitialSituation"/>
              <owl:someValuesFrom rdf:resource="&dul;Situation"/>
            </owl:Restriction>

            <owl:Restriction>
              <owl:onProperty rdf:resource="&soma;hasTerminalSituation"/>
              <owl:someValuesFrom rdf:resource="&dul;Situation"/>
            </owl:Restriction>
          </owl:intersectionOf>
        </owl:Class>
      </rdfs:subClassOf>
      <owl:intersectionOf rdf:parseType="Collection">
        <rdf:Description rdf:about="&soma;SituationTransition"/>
        <owl:Restriction>
          <owl:onProperty rdf:resource="http://www.ease-crc.org/ont/SOMA.owl/manifestsIn"/>
          <owl:someValuesFrom rdf:resource="&dul;Event"/>
        </owl:Restriction>
      </owl:intersectionOf>
    </owl:Class>
  </owl:annotatedSource>
  <owl:annotatedTarget rdf:nodeID="bn7"/>
</owl:Axiom>

<owl:ObjectProperty rdf:about="&soma;isOrderedBy">
  <rdfs:comment xml:lang="en">The relation between an 'Order item' and the 'Order' that sorts them (via the relations 'precedes' and 'follows')</rdfs:comment>
  <rdfs:domain rdf:resource="&soma;OrderedElement"/>
  <rdfs:isDefinedBy rdf:resource="http://www.ease-crc.org/ont/SOMA-AGENT.owl"/>
  <rdfs:label xml:lang="en">is ordered by</rdfs:label>
  <rdfs:range rdf:resource="&soma;Order"/>
  <rdfs:subPropertyOf rdf:resource="&dul;associatedWith"/>
  <owl:inverseOf rdf:resource="&soma;orders"/>
</owl:ObjectProperty>

<owl:Class rdf:about="&soma;Appliance">
  <rdfs:comment>A device designed to perform a specific task, and that can be operated in some way.</rdfs:comment>
  <rdfs:isDefinedBy rdf:resource="http://www.ease-crc.org/ont/SOMA-OBJ.owl"/>
  <rdfs:subClassOf rdf:resource="&dul;DesignedArtifact"/>
</owl:Class>

<owl:ObjectProperty rdf:about="&soma;isDesignedBy">
  <rdfs:comment xml:lang="en">A special relation between a Design and an Object, to indicate that the Object is described by the Design.</rdfs:comment>
  <rdfs:domain rdf:resource="&dul;Object"/>
  <rdfs:isDefinedBy rdf:resource="http://www.ease-crc.org/ont/SOMA-IO.owl"/>
  <rdfs:label xml:lang="en">is designed by</rdfs:label>
  <rdfs:range rdf:resource="&dul;Design"/>
  <rdfs:subPropertyOf rdf:resource="&dul;isDescribedBy"/>
</owl:ObjectProperty>

<owl:Class rdf:about="&dul;SocialRelation"/>

<owl:Class rdf:about="&soma;DeviceState">
  <rdfs:comment>A quality belonging to a device which indicates its overall functional state.</rdfs:comment>
  <rdfs:isDefinedBy rdf:resource="http://www.ease-crc.org/ont/SOMA-OBJ.owl"/>
  <rdfs:subClassOf rdf:resource="&soma;Intrinsic"/>
</owl:Class>

<owl:DatatypeProperty rdf:about="&soma;hasEventTime"
    rdfs:label="has event time">
  <rdfs:comment>Superproperty of hasEventBegin and hasEventEnd, records that an Event happened, or was happening, at a particular time. Using the subproperties captures the richer semantics of that time relative to the event. Using only this superproperty may be appropriate when the Event is construed to take place at a single instant of time.</rdfs:comment>
  <rdfs:domain rdf:resource="&dul;Event"/>
  <rdfs:isDefinedBy rdf:resource="http://www.ease-crc.org/ont/SOMA.owl"/>
  <rdfs:range rdf:resource="&xsd;double"/>
  <rdfs:subPropertyOf rdf:resource="&dul;hasDataValue"/>
</owl:DatatypeProperty>

<owl:Class rdf:about="&soma;ProximalTheory">
  <rdfs:subClassOf>
    <owl:Restriction>
      <owl:onProperty rdf:resource="&dul;defines"/>
      <owl:someValuesFrom rdf:resource="&soma;LocatumRole"/>
    </owl:Restriction>
  </rdfs:subClassOf>
  <rdfs:subClassOf>
    <owl:Restriction>
      <owl:onProperty rdf:resource="&dul;defines"/>
      <owl:someValuesFrom rdf:resource="&soma;RelatumRole"/>
    </owl:Restriction>
  </rdfs:subClassOf>
  <rdfs:subClassOf rdf:resource="&soma;ImageSchemaTheory"/>
  <rdfs:comment>An image schematic theory that describes a qualitative spatial relation indicating relative proximity, as expressed by the prepositions 'near', 'close to', 'next to', etc.

It may seem that proximity is a very simple notion, requiring no sophisticated theoretical underpinnings. However, proximity is an extremely object- and purpose-dependent relation. A store next door is in a closeness relation to a person, and so is the Sun in the sky, despite the physical distances being different by several orders of magnitude.

As such, a theory, i.e. a description of what a particular kind of closeness means and in which contexts it applies, is necessary.

Adopted from GUM-4-space (Bateman et al. 2010).

Let xL, xR be objects filling the locatum, relatum roles of this schema. Then one can infer that xL 'near to' xR.</rdfs:comment>
  <rdfs:isDefinedBy rdf:resource="http://www.ease-crc.org/ont/SOMA-SAY.owl"/>
  <rdfs:label xml:lang="en">Proximal theory</rdfs:label>
</owl:Class>

<owl:ObjectProperty rdf:about="&soma;isPlanFor">
  <rdfs:isDefinedBy rdf:resource="http://www.ease-crc.org/ont/SOMA-WF.owl"/>
  <rdfs:isDefinedBy rdf:resource="http://www.ease-crc.org/ont/SOMA.owl"/>
  <rdfs:comment>A special relation between a Plan and a Task, to indicate that the Plan describes a way to achieve the Task.</rdfs:comment>
  <rdfs:domain rdf:resource="&dul;Plan"/>
  <rdfs:label xml:lang="en">is plan for</rdfs:label>
  <rdfs:range rdf:resource="&dul;Task"/>
  <rdfs:seeAlso>Note that DUL already says Plans can define Tasks, but that relation is used differently: a Plan defines a Task because it contains it as a step.</rdfs:seeAlso>
  <rdfs:subPropertyOf rdf:resource="&dul;describes"/>
</owl:ObjectProperty>

<owl:ObjectProperty rdf:about="&soma;hasTask">
  <rdfs:comment>A relation to indicate that a Task is part of a Workflow or ordering Relation: that is, the task may be executed during the execution of the Workflow, or there exists some Relation between the Tasks that informs how their executions are to be located in time.</rdfs:comment>
  <rdfs:domain>
    <owl:Class>
      <owl:unionOf rdf:parseType="Collection">
        <rdf:Description rdf:about="&dul;Relation"/>
        <rdf:Description rdf:about="&dul;Workflow"/>
      </owl:unionOf>
    </owl:Class>
  </rdfs:domain>
  <rdfs:isDefinedBy rdf:resource="http://www.ease-crc.org/ont/SOMA-WF.owl"/>
  <rdfs:label xml:lang="en">has task</rdfs:label>
  <rdfs:range rdf:resource="&dul;Task"/>
  <rdfs:subPropertyOf rdf:resource="&dul;hasPart"/>
</owl:ObjectProperty>

<owl:Class rdf:about="&soma;LocatumRole">
  <rdfs:subClassOf>
    <owl:Restriction>
      <owl:allValuesFrom rdf:resource="&dul;PhysicalObject"/>
      <owl:onProperty rdf:resource="&dul;classifies"/>
    </owl:Restriction>
  </rdfs:subClassOf>
  <rdfs:subClassOf rdf:resource="&soma;SpatialRelationRole"/>
  <rdfs:comment>Denotes the object with primary focal prominence in a spatial or spatio-temporal schema. Terminological variants that appear in the literature on cognitive linguistics include Figure (Talmy 1983) and Trajector (Langacker 1986).</rdfs:comment>
  <rdfs:isDefinedBy rdf:resource="http://www.ease-crc.org/ont/SOMA-OBJ.owl"/>
  <rdfs:label xml:lang="en">Locatum role</rdfs:label>
</owl:Class>

<owl:Class rdf:about="&soma;EndEffectorPositioning">
  <rdfs:comment>A task in which an Agent places its end effectors at particular poses.</rdfs:comment>
  <rdfs:isDefinedBy rdf:resource="http://www.ease-crc.org/ont/SOMA-ACT.owl"/>
  <rdfs:label xml:lang="en">End effector positioning</rdfs:label>
  <rdfs:subClassOf rdf:resource="&soma;Manipulating"/>
</owl:Class>

<owl:Class rdf:about="&soma;Actuating">
  <rdfs:comment>Tasks where the goal is to move an object.

Usually, an agent will use their prehensile effectors, ie. hands, for this purpose, so there is a lot of conceptual overlap between Actuating and Manipulating.

However, these categories are nonetheless distinguished in that there are more ways to actuate objects than simply manipulating them; for example, some tool like a net or frying pan might be used to catch an object.

Another way to look at the difference between Actuating and Manipulating is in what they "profile", ie. focus on as important.

For Actuating, it is the object's motion that is paramount.

For Manipulating, it is the movement of the hand(s) and the change in functional relationships (such as kinematic control) between the hand(s) and the manipulated object(s).</rdfs:comment>
  <rdfs:comment>todo: think about use of tools. force events are generated between artifacts then. also not only the tool would be the 'salient artifact' here.</rdfs:comment>
  <rdfs:isDefinedBy rdf:resource="http://www.ease-crc.org/ont/SOMA-ACT.owl"/>
  <rdfs:subClassOf rdf:resource="&soma;PhysicalTask"/>
</owl:Class>

<owl:Class rdf:about="&soma;StaticFrictionAttribute"
    rdfs:label="Static friction attribute">
  <rdfs:comment>Friction between two touching objects that do not move relative to each other.</rdfs:comment>
  <rdfs:isDefinedBy rdf:resource="http://www.ease-crc.org/ont/SOMA-OBJ.owl"/>
  <rdfs:subClassOf rdf:resource="&soma;FrictionAttribute"/>
</owl:Class>

<owl:ObjectProperty rdf:about="&dul;hasRole"/>

<owl:ObjectProperty rdf:about="&soma;isQualityDescribedBy"
    rdfs:comment="Relates a description to a quality it describes."
    rdfs:label="is quality described by">
  <rdfs:domain rdf:resource="&dul;Quality"/>
  <rdfs:isDefinedBy rdf:resource="http://www.ease-crc.org/ont/SOMA-OBJ.owl"/>
  <rdfs:range rdf:resource="&dul;Description"/>
  <rdfs:subPropertyOf rdf:resource="&dul;isDescribedBy"/>
</owl:ObjectProperty>

<owl:Class rdf:about="&soma;LinguisticObject">
  <rdfs:isDefinedBy rdf:resource="http://www.ease-crc.org/ont/SOMA-ACT.owl"/>
  <rdfs:isDefinedBy rdf:resource="http://www.ease-crc.org/ont/SOMA-SAY.owl"/>
  <rdfs:isDefinedBy rdf:resource="http://www.ontologydesignpatterns.org/ont/dul/IOLite.owl"/>
  <rdfs:label xml:lang="en">Linguistic object</rdfs:label>
  <rdfs:subClassOf rdf:resource="&dul;InformationObject"/>
</owl:Class>

<owl:ObjectProperty rdf:about="&dul;hasSetting"/>

<owl:Class rdf:about="&dul;Set"/>

<owl:Class rdf:about="&soma;Swimming">
  <rdfs:comment>A motion of some body through water. The body provides the power for the motion.</rdfs:comment>
  <rdfs:isDefinedBy rdf:resource="http://www.ease-crc.org/ont/SOMA-PROC.owl"/>
  <rdfs:subClassOf rdf:resource="&soma;Locomotion"/>
  <owl:disjointWith rdf:resource="&soma;Walking"/>
</owl:Class>

<owl:Class rdf:about="&soma;Simulation_Reasoner">
  <rdfs:comment xml:lang="en">A Simulation-based Reasoner is a simulation that is used as a reasoner, where the explicit knowledge corresponds to the initial situation, and the implicit knowlegde corresponds to the situation that is derived from that by simulating some unfolding processes.</rdfs:comment>
  <rdfs:isDefinedBy rdf:resource="http://www.ease-crc.org/ont/SOMA-IO.owl"/>
  <rdfs:label xml:lang="en">Simulation-based reasoner</rdfs:label>
  <rdfs:subClassOf rdf:resource="&soma;Reasoner"/>
</owl:Class>

<owl:Class rdf:about="&soma;PhysicalExistence">
  <rdfs:comment>A State in which an Entity is said to exist in the physical world.</rdfs:comment>
  <rdfs:isDefinedBy rdf:resource="http://www.ease-crc.org/ont/SOMA-STATE.owl"/>
  <rdfs:label xml:lang="en">Physical Existince</rdfs:label>
  <rdfs:subClassOf rdf:resource="&soma;PhysicalState"/>
</owl:Class>

<owl:Class rdf:about="&soma;Graspability">
  <rdfs:comment>The disposition of an object (e.g. the handle) to afford grasping the object.</rdfs:comment>
  <rdfs:isDefinedBy rdf:resource="http://www.ease-crc.org/ont/SOMA-OBJ.owl"/>
  <rdfs:subClassOf rdf:resource="&soma;Disposition"/>
</owl:Class>

<owl:Class rdf:about="&dul;Process">
  <rdfs:isDefinedBy rdf:resource="http://www.ease-crc.org/ont/SOMA-PROC.owl"/>
</owl:Class>

<owl:Class rdf:about="&soma;ExecutableFile">
  <rdfs:comment xml:lang="en">An Executable File, sometimes simply referred to as an executable or binary, causes a computer "to perform indicated tasks according to encoded instructions", as opposed to a data file that must be interpreted (parsed) by a program to be meaningful.

The exact interpretation depends upon the use. "Instructions" is traditionally taken to mean machine code instructions for a physical CPU. In some contexts, a file containing scripting instructions (such as bytecode) may also be considered executable.</rdfs:comment>
  <rdfs:isDefinedBy rdf:resource="http://www.ease-crc.org/ont/SOMA-IO.owl"/>
  <rdfs:label xml:lang="en">Executable File</rdfs:label>
  <owl:equivalentClass>
    <owl:Class>
      <owl:intersectionOf rdf:parseType="Collection">
        <rdf:Description rdf:about="&soma;Digital_File"/>
        <owl:Restriction>
          <owl:onProperty rdf:resource="&dul;realizes"/>
          <owl:someValuesFrom rdf:resource="&soma;Executable_Code"/>
        </owl:Restriction>
      </owl:intersectionOf>
    </owl:Class>
  </owl:equivalentClass>
</owl:Class>

<owl:ObjectProperty rdf:about="&dul;isQualityOf"/>

<owl:Class rdf:about="&soma;Learning"
    rdfs:label="Learning">
  <rdfs:comment>The mental task of storing information for later use.

This is more general than memorizing, as the later only captures declarative knowledge.</rdfs:comment>
  <rdfs:isDefinedBy rdf:resource="http://www.ease-crc.org/ont/SOMA-ACT.owl"/>
  <rdfs:subClassOf rdf:resource="&soma;InformationStorage"/>
</owl:Class>

<owl:Class rdf:about="&soma;Deposition"
    rdfs:comment="The disposition to support objects.">
  <rdfs:subClassOf>
    <owl:Restriction>
      <owl:allValuesFrom rdf:resource="&soma;Deposit"/>
      <owl:onProperty rdf:resource="&soma;affordsBearer"/>
    </owl:Restriction>
  </rdfs:subClassOf>
  <rdfs:subClassOf>
    <owl:Restriction>
      <owl:allValuesFrom rdf:resource="&soma;DepositedObject"/>
      <owl:onProperty rdf:resource="&soma;affordsTrigger"/>
    </owl:Restriction>
  </rdfs:subClassOf>
  <rdfs:subClassOf rdf:resource="&soma;Disposition"/>
  <rdfs:isDefinedBy rdf:resource="http://www.ease-crc.org/ont/SOMA-OBJ.owl"/>
</owl:Class>

<owl:Class rdf:about="&soma;NetForce"
    rdfs:comment="The accumulated force acting upon an object."
    rdfs:label="Net force">
  <rdfs:isDefinedBy rdf:resource="http://www.ease-crc.org/ont/SOMA-OBJ.owl"/>
  <rdfs:subClassOf rdf:resource="&soma;ForceAttribute"/>
</owl:Class>

<owl:Class rdf:about="&soma;Markup_Language">
  <rdfs:comment xml:lang="en">Markup refers to data included in an electronic document which is distinct from the document's content in that it is typically not included in representations of the document for end users, for example on paper or a computer screen, or in an audio stream. Markup is often used to control the display of the document or to enrich its content to facilitate automated processing. A markup language is a set of rules governing what markup information may be included in a document and how it is combined with the content of the document in a way to facilitate use by humans and computer programs.

From Wikipedia: https://en.wikipedia.org/wiki/Markup_language</rdfs:comment>
  <rdfs:isDefinedBy rdf:resource="http://www.ease-crc.org/ont/SOMA-IO.owl"/>
  <rdfs:label xml:lang="en">Markup Language</rdfs:label>
  <rdfs:subClassOf rdf:resource="&soma;Computer_Language"/>
</owl:Class>

<owl:Class rdf:about="&soma;Focusing"
    rdfs:comment="The mental task to center the attention to some subject."
    rdfs:label="Focusing">
  <rdfs:isDefinedBy rdf:resource="http://www.ease-crc.org/ont/SOMA-ACT.owl"/>
  <rdfs:subClassOf rdf:resource="&soma;AttentionShift"/>
</owl:Class>

<owl:DatatypeProperty rdf:about="&soma;hasJointPositionMin"
    rdfs:label="has joint position min">
  <rdfs:comment>The minimum position of a joint given in m (prismatic joints) or rad (hinged joints).</rdfs:comment>
  <rdfs:domain rdf:resource="&soma;JointLimit"/>
  <rdfs:isDefinedBy rdf:resource="http://www.ease-crc.org/ont/SOMA-OBJ.owl"/>
  <rdfs:range rdf:resource="&xsd;double"/>
  <rdfs:subPropertyOf rdf:resource="&soma;hasJointParameter"/>
</owl:DatatypeProperty>

<owl:Class rdf:about="&soma;Effort">
  <rdfs:comment>A parameter describing the amount of force to be exerted by some actuator.</rdfs:comment>
  <rdfs:isDefinedBy rdf:resource="http://www.ease-crc.org/ont/SOMA-OBJ.owl"/>
  <rdfs:subClassOf rdf:resource="&dul;Parameter"/>
</owl:Class>

<owl:Class rdf:about="&soma;SpatialRelationRole">
  <rdfs:comment>Roles classifying entities participating in some spatial relation.</rdfs:comment>
  <rdfs:isDefinedBy rdf:resource="http://www.ease-crc.org/ont/SOMA-OBJ.owl"/>
  <rdfs:label xml:lang="en">Spatial relation role</rdfs:label>
  <rdfs:subClassOf rdf:resource="&soma;RelationAdjacentRole"/>
</owl:Class>

<owl:Class rdf:about="&soma;SelectedObject"
    rdfs:comment="An object chosen as the result of some selection task.">
  <rdfs:isDefinedBy rdf:resource="http://www.ease-crc.org/ont/SOMA-OBJ.owl"/>
  <rdfs:label xml:lang="en">Selected object</rdfs:label>
  <rdfs:subClassOf rdf:resource="&dul;Role"/>
</owl:Class>

<owl:ObjectProperty rdf:about="&dul;isRelatedToConcept">
  <rdfs:isDefinedBy rdf:resource="http://www.ease-crc.org/ont/SOMA-PROC.owl"/>
  <rdfs:isDefinedBy rdf:resource="http://www.ease-crc.org/ont/SOMA-STATE.owl"/>
</owl:ObjectProperty>

<owl:Class rdf:about="http://www.ease-crc.org/ont/SOMA.owl#3DPosition"
    rdfs:comment="A point in three dimensional space, given as translation.">
  <rdfs:subClassOf>
    <owl:Restriction>
      <owl:onDataRange rdf:resource="&xsd;string"/>
      <owl:onProperty rdf:resource="&soma;hasPositionData"/>
      <owl:qualifiedCardinality rdf:datatype="&xsd;nonNegativeInteger">1</owl:qualifiedCardinality>
    </owl:Restriction>
  </rdfs:subClassOf>
  <rdfs:subClassOf rdf:resource="&dul;SpaceRegion"/>
  <rdfs:isDefinedBy rdf:resource="http://www.ease-crc.org/ont/SOMA-OBJ.owl"/>
  <rdfs:label xml:lang="en">3D position</rdfs:label>
</owl:Class>

<owl:ObjectProperty rdf:about="&soma;isFeatureOf"
    rdfs:comment="Associates a feature to the physical object it belongs to."
    rdfs:label="is feature of">
  <rdfs:domain rdf:resource="&soma;Feature"/>
  <rdfs:isDefinedBy rdf:resource="http://www.ease-crc.org/ont/SOMA-OBJ.owl"/>
  <rdfs:range rdf:resource="&dul;PhysicalObject"/>
  <rdfs:subPropertyOf rdf:resource="&dul;isConstituentOf"/>
</owl:ObjectProperty>

<owl:Class rdf:about="&soma;Throwing">
  <rdfs:subClassOf rdf:resource="&soma;Actuating"/>
  <rdfs:subClassOf rdf:resource="&soma;Manipulating"/>
  <rdfs:comment>A task in which an Agent imparts momentum to an object before releasing it so that it flies for some distance unsupported.</rdfs:comment>
  <rdfs:isDefinedBy rdf:resource="http://www.ease-crc.org/ont/SOMA-ACT.owl"/>
</owl:Class>

<owl:Class rdf:about="&soma;DexterityDiagnosis"
    rdfs:label="Dexterity diagnosis">
  <rdfs:comment>A description of the dexterity of a system, possibly in comparison to another system.</rdfs:comment>
  <rdfs:isDefinedBy rdf:resource="http://www.ease-crc.org/ont/SOMA.owl"/>
  <rdfs:subClassOf rdf:resource="&soma;BehavioralDiagnosis"/>
</owl:Class>

<owl:ObjectProperty rdf:about="&soma;isInitialSituationOf">
  <rdfs:comment>A relation between SituationTransitions and Situations, which identifies the Situation the transition starts from.</rdfs:comment>
  <rdfs:domain rdf:resource="&dul;Situation"/>
  <rdfs:isDefinedBy rdf:resource="http://www.ease-crc.org/ont/SOMA-ACT.owl"/>
  <rdfs:label xml:lang="en">is initial situation of</rdfs:label>
  <rdfs:range rdf:resource="&soma;SituationTransition"/>
  <rdfs:subPropertyOf rdf:resource="&soma;isInitialStateOf"/>
</owl:ObjectProperty>

<owl:Class rdf:about="&soma;Obstacle">
  <rdfs:comment>An object used to restrict access to a protected space or group.</rdfs:comment>
  <rdfs:isDefinedBy rdf:resource="http://www.ease-crc.org/ont/SOMA-OBJ.owl"/>
  <rdfs:subClassOf rdf:resource="&soma;Barrier"/>
</owl:Class>

<owl:Class rdf:about="&soma;ForceInteraction"
    rdfs:label="Force interaction">
  <rdfs:subClassOf>
    <owl:Restriction>
      <owl:onProperty rdf:resource="&soma;isProcessTypeOf"/>
      <owl:someValuesFrom rdf:resource="&soma;Agonist"/>
    </owl:Restriction>
  </rdfs:subClassOf>
  <rdfs:subClassOf>
    <owl:Restriction>
      <owl:onProperty rdf:resource="&soma;isProcessTypeOf"/>
      <owl:someValuesFrom rdf:resource="&soma;Antagonist"/>
    </owl:Restriction>
  </rdfs:subClassOf>
  <rdfs:subClassOf rdf:resource="&soma;ProcessType"/>
  <rdfs:comment>Classifies events in which two entities interact with each other with a reference to force. One of the entities, the agonist, has a tendency to either set the other entity (the antagonist) into motion, or to keep it still under the influence of some other force. The tendency only manifests in case the agonist is the "stronger entity".</rdfs:comment>
  <rdfs:isDefinedBy rdf:resource="http://www.ease-crc.org/ont/SOMA-PROC.owl"/>
  <rdfs:seeAlso>Talmy, Leonard (1981) ‘Force Dynamics’. Language and Mental Imagery. May 1981, University of California, Berkeley.</rdfs:seeAlso>
  <owl:equivalentClass>
    <owl:Class>
      <owl:unionOf rdf:parseType="Collection">
        <rdf:Description rdf:about="&soma;AlterativeInteraction"/>
        <rdf:Description rdf:about="&soma;PreservativeInteraction"/>
      </owl:unionOf>
    </owl:Class>
  </owl:equivalentClass>
</owl:Class>

<owl:ObjectProperty rdf:about="&soma;isInputRoleOf"
    rdfs:comment="A relation between an input roles and its Task.">
  <rdfs:domain rdf:resource="&dul;Role"/>
  <rdfs:isDefinedBy rdf:resource="http://www.ease-crc.org/ont/SOMA.owl"/>
  <rdfs:label xml:lang="en">is input role of</rdfs:label>
  <rdfs:range rdf:resource="&dul;Task"/>
  <rdfs:subPropertyOf rdf:resource="&dul;hasTask"/>
  <owl:inverseOf rdf:resource="&soma;isTaskOfInputRole"/>
</owl:ObjectProperty>

<owl:Class rdf:about="&soma;LocutionaryAction">
  <rdfs:comment xml:lang="en">A Locutionary Act is the performance of an utterance (source: https://en.wikipedia.org/wiki/Locutionary_act).

We additionally require a Locutionary Act to be performed by an Agent, not an Actor - this is what sets it apart from a Communication Action.</rdfs:comment>
  <rdfs:isDefinedBy rdf:resource="http://www.ease-crc.org/ont/SOMA-SAY.owl"/>
  <rdfs:label xml:lang="en">Locutionary action</rdfs:label>
  <owl:equivalentClass>
    <owl:Class>
      <owl:intersectionOf rdf:parseType="Collection">
        <rdf:Description rdf:about="&soma;CommunicationAction"/>
        <owl:Restriction>
          <owl:onProperty rdf:resource="&dul;hasParticipant"/>
          <owl:someValuesFrom rdf:resource="&dul;Agent"/>
        </owl:Restriction>
      </owl:intersectionOf>
    </owl:Class>
  </owl:equivalentClass>
</owl:Class>

<owl:ObjectProperty rdf:about="&dul;hasMember"/>

<owl:Class rdf:about="&soma;Programming_Language">
  <rdfs:subClassOf>
    <owl:Restriction>
      <owl:allValuesFrom rdf:resource="&soma;Computer_Program"/>
      <owl:onProperty rdf:resource="&soma;givesMeaningTo"/>
    </owl:Restriction>
  </rdfs:subClassOf>
  <rdfs:subClassOf rdf:resource="&soma;Computer_Language"/>
  <rdfs:comment xml:lang="en">Any Programming Language, including both human-readable like Java and non-human-readable languages like binary machine code.</rdfs:comment>
  <rdfs:isDefinedBy rdf:resource="http://www.ease-crc.org/ont/SOMA-IO.owl"/>
  <rdfs:label xml:lang="en">Programming language</rdfs:label>
</owl:Class>

<owl:ObjectProperty rdf:about="&soma;isConceptAffordedBy"
    rdfs:label="is concept afforded by">
  <rdfs:comment>A relation between a disposition and a concept defined in the affordance that describes the disposition.</rdfs:comment>
  <rdfs:domain rdf:resource="&dul;Concept"/>
  <rdfs:isDefinedBy rdf:resource="http://www.ease-crc.org/ont/SOMA-OBJ.owl"/>
  <rdfs:range rdf:resource="&soma;Disposition"/>
  <rdfs:subPropertyOf rdf:resource="&dul;associatedWith"/>
  <owl:propertyChainAxiom rdf:parseType="Collection">
    <rdf:Description rdf:about="&soma;isDefinedInAffordance"/>
    <rdf:Description rdf:about="&dul;describes"/>
  </owl:propertyChainAxiom>
</owl:ObjectProperty>

<owl:Class rdf:about="&soma;Text">
  <rdfs:comment xml:lang="en">Any Information Object defined using a Language that, when realized through a symbolic writing system, can be read and made sense of.

One may define Text as anything that can be made sense of, including e.g., Speech or Paintings.

However, the argument can be made that Speech or Paintings are not considered Text as they cannot be EXACTLY realized by a symbolic writing system: Speech may loose punctuation, Paintings their original appearance.
On the other hand, this might not be true as both could be encoded in a binary format that can be interpreted using a language (eg., mp3, png).</rdfs:comment>
  <rdfs:isDefinedBy rdf:resource="http://www.ease-crc.org/ont/SOMA-IO.owl"/>
  <rdfs:label xml:lang="en">Text</rdfs:label>
  <owl:equivalentClass>
    <owl:Class>
      <owl:intersectionOf rdf:parseType="Collection">
        <rdf:Description rdf:about="&dul;InformationObject"/>
        <owl:Restriction>
          <owl:onProperty rdf:resource="&soma;isGivenMeaningBy"/>
          <owl:someValuesFrom rdf:resource="&soma;Language"/>
        </owl:Restriction>
      </owl:intersectionOf>
    </owl:Class>
  </owl:equivalentClass>
</owl:Class>

<owl:ObjectProperty rdf:about="&soma;isBearerAffordedBy"
    rdfs:label="is bearer afforded by">
  <rdfs:comment>Relates a disposition to the bearer role defined by the affordance describing the disposition.</rdfs:comment>
  <rdfs:domain rdf:resource="&dul;Role"/>
  <rdfs:isDefinedBy rdf:resource="http://www.ease-crc.org/ont/SOMA-OBJ.owl"/>
  <rdfs:range rdf:resource="&soma;Disposition"/>
  <rdfs:subPropertyOf rdf:resource="&soma;isConceptAffordedBy"/>
  <owl:propertyChainAxiom rdf:parseType="Collection">
    <rdf:Description rdf:about="&soma;isBearerDefinedIn"/>
    <rdf:Description rdf:about="&dul;describes"/>
  </owl:propertyChainAxiom>
</owl:ObjectProperty>

<owl:Class rdf:about="&soma;Pouring">
  <rdfs:subClassOf>
    <owl:Restriction>
      <owl:onProperty rdf:resource="&soma;isTaskAffordedBy"/>
      <owl:someValuesFrom rdf:resource="&soma;Pourable"/>
    </owl:Restriction>
  </rdfs:subClassOf>
  <rdfs:subClassOf rdf:resource="&soma;Actuating"/>
  <rdfs:comment>A task in which an agent lets liquid substance to flow out of an object. The agent has a kinematic control over the object.</rdfs:comment>
  <rdfs:isDefinedBy rdf:resource="http://www.ease-crc.org/ont/SOMA-ACT.owl"/>
</owl:Class>

<owl:ObjectProperty rdf:about="&soma;includesSituation"
    rdfs:label="includes situation">
  <rdfs:comment>A relation recording that a Situation has a (sub) Situation as participant in some role.</rdfs:comment>
  <rdfs:domain rdf:resource="&dul;Situation"/>
  <rdfs:isDefinedBy rdf:resource="http://www.ease-crc.org/ont/SOMA.owl"/>
  <rdfs:range rdf:resource="&dul;Situation"/>
  <rdfs:subPropertyOf rdf:resource="&dul;isSettingFor"/>
  <owl:inverseOf rdf:resource="&soma;isSituationIncludedIn"/>
</owl:ObjectProperty>

<owl:Class rdf:about="&soma;PrehensileMotion"
    rdfs:comment="A motion of a prehensile effector."
    rdfs:label="Prehensile motion">
  <rdfs:subClassOf>
    <owl:Restriction>
      <owl:onProperty rdf:resource="&soma;isProcessTypeOf"/>
      <owl:someValuesFrom>
        <owl:Class>
          <owl:intersectionOf rdf:parseType="Collection">
            <rdf:Description rdf:about="&soma;MovedObject"/>
            <owl:Restriction>
              <owl:allValuesFrom rdf:resource="&soma;PrehensileEffector"/>
              <owl:onProperty rdf:resource="&dul;classifies"/>
            </owl:Restriction>
          </owl:intersectionOf>
        </owl:Class>
      </owl:someValuesFrom>
    </owl:Restriction>
  </rdfs:subClassOf>
  <rdfs:subClassOf rdf:resource="&soma;DirectedMotion"/>
  <rdfs:isDefinedBy rdf:resource="http://www.ease-crc.org/ont/SOMA-PROC.owl"/>
  <owl:equivalentClass>
    <owl:Class>
      <owl:unionOf rdf:parseType="Collection">
        <rdf:Description rdf:about="&soma;GraspingMotion"/>
        <rdf:Description rdf:about="&soma;ReleasingMotion"/>
      </owl:unionOf>
    </owl:Class>
  </owl:equivalentClass>
</owl:Class>

<owl:Class rdf:about="&soma;AlterativeInteraction"
    rdfs:label="Alterative interaction">
  <rdfs:comment>A force interaction where the agonist has the tendency to set another object into motion. An example is 'opening a door' where some object interacts with the door such that it moves out of its frame.</rdfs:comment>
  <rdfs:isDefinedBy rdf:resource="http://www.ease-crc.org/ont/SOMA-PROC.owl"/>
  <rdfs:subClassOf rdf:resource="&soma;ForceInteraction"/>
  <owl:disjointWith rdf:resource="&soma;PreservativeInteraction"/>
</owl:Class>

<owl:Class rdf:about="&soma;Limb"
    rdfs:comment="An arm or leg of an embodied agent.">
  <rdfs:isDefinedBy rdf:resource="http://www.ease-crc.org/ont/SOMA-OBJ.owl"/>
  <rdfs:isDefinedBy rdf:resource="http://www.ease-crc.org/ont/SOMA-PROC.owl"/>
  <rdfs:subClassOf rdf:resource="&soma;PhysicalEffector"/>
  <owl:equivalentClass>
    <owl:Class>
      <owl:unionOf rdf:parseType="Collection">
        <rdf:Description rdf:about="&soma;Arm"/>
        <rdf:Description rdf:about="&soma;Leg"/>
      </owl:unionOf>
    </owl:Class>
  </owl:equivalentClass>
</owl:Class>

<owl:Class rdf:about="&soma;SourcePathGoalTheory">
  <rdfs:subClassOf>
    <owl:Restriction>
      <owl:onProperty rdf:resource="&dul;defines"/>
      <owl:someValuesFrom rdf:resource="&soma;Destination"/>
    </owl:Restriction>
  </rdfs:subClassOf>
  <rdfs:subClassOf>
    <owl:Restriction>
      <owl:onProperty rdf:resource="&dul;defines"/>
      <owl:someValuesFrom rdf:resource="&soma;Origin"/>
    </owl:Restriction>
  </rdfs:subClassOf>
  <rdfs:subClassOf>
    <owl:Restriction>
      <owl:onProperty rdf:resource="&dul;defines"/>
      <owl:someValuesFrom rdf:resource="&soma;PathRole"/>
    </owl:Restriction>
  </rdfs:subClassOf>
  <rdfs:subClassOf rdf:resource="&soma;ImageSchemaTheory"/>
  <rdfs:comment>A very general image-schema of the Path family, this schema describes movement along a path from a source towards a goal.

Note: in cognitive linguistics literature, the roles of this schema are Source, Path, Goal. However, to avoid overloading some other terminology in SOMA, we renamed Source to Origin and Goal to Destination.

As yet, this schema is not associated to any object property.</rdfs:comment>
  <rdfs:isDefinedBy rdf:resource="http://www.ease-crc.org/ont/SOMA-SAY.owl"/>
  <rdfs:label xml:lang="en">Source-path-goal theory</rdfs:label>
</owl:Class>

<owl:Class rdf:about="&soma;Structured_Text">
  <rdfs:comment xml:lang="en">Any Text that adheres to some rules that are in any way more specific than natural language and that cannot be made sense of without knowing said rules.</rdfs:comment>
  <rdfs:isDefinedBy rdf:resource="http://www.ease-crc.org/ont/SOMA-IO.owl"/>
  <rdfs:label xml:lang="en">Structured text</rdfs:label>
  <owl:equivalentClass>
    <owl:Class>
      <owl:intersectionOf rdf:parseType="Collection">
        <rdf:Description rdf:about="&soma;Text"/>
        <owl:Restriction>
          <owl:onProperty rdf:resource="&soma;isGivenMeaningBy"/>
          <owl:someValuesFrom rdf:resource="&soma;FormalLanguage"/>
        </owl:Restriction>
      </owl:intersectionOf>
    </owl:Class>
  </owl:equivalentClass>
</owl:Class>

<owl:ObjectProperty rdf:about="&soma;hasProcessType"
    rdfs:label="has process type">
  <rdfs:comment>A relation between roles and process types, e.g. a catalysator is needed to trigger some chemical reaction.</rdfs:comment>
  <rdfs:domain rdf:resource="&dul;Role"/>
  <rdfs:isDefinedBy rdf:resource="http://www.ease-crc.org/ont/SOMA-PROC.owl"/>
  <rdfs:range rdf:resource="&soma;ProcessType"/>
  <rdfs:subPropertyOf rdf:resource="&dul;isRelatedToConcept"/>
  <owl:inverseOf rdf:resource="&soma;isProcessTypeOf"/>
</owl:ObjectProperty>

<owl:ObjectProperty rdf:about="&soma;hasExecutionState"
    rdfs:comment="A relation from an Action to its execution state."
    rdfs:label="has execution state">
  <rdfs:domain rdf:resource="&dul;Action"/>
  <rdfs:isDefinedBy rdf:resource="http://www.ease-crc.org/ont/SOMA-ACT.owl"/>
  <rdfs:range rdf:resource="&soma;ExecutionStateRegion"/>
  <rdfs:subPropertyOf rdf:resource="&dul;hasRegion"/>
</owl:ObjectProperty>

<owl:ObjectProperty rdf:about="&dul;associatedWith">
  <rdfs:isDefinedBy rdf:resource="http://www.ease-crc.org/ont/SOMA-PROC.owl"/>
  <rdfs:isDefinedBy rdf:resource="http://www.ease-crc.org/ont/SOMA.owl"/>
</owl:ObjectProperty>

<owl:Class rdf:about="&soma;FaultySoftware"
    rdfs:comment="A description of a situation where some software has a bug.">
  <rdfs:isDefinedBy rdf:resource="http://www.ease-crc.org/ont/SOMA-IO.owl"/>
  <rdfs:label xml:lang="en">Faulty software</rdfs:label>
  <rdfs:subClassOf rdf:resource="&soma;SoftwareDiagnosis"/>
</owl:Class>

<owl:Class rdf:about="&soma;Computer_Language">
  <rdfs:comment xml:lang="en">A computer language is a formal language used in communication with a computer.

From Wikipedia: https://en.wikipedia.org/wiki/Computer_language</rdfs:comment>
  <rdfs:isDefinedBy rdf:resource="http://www.ease-crc.org/ont/SOMA-IO.owl"/>
  <rdfs:label xml:lang="en">Computer Language</rdfs:label>
  <rdfs:subClassOf rdf:resource="&soma;FormalLanguage"/>
</owl:Class>

<owl:Class rdf:about="&soma;Dicing">
  <rdfs:comment>A particular kind of cutting where the goal is to produce small pieces out of some object or material. Unlike slices, the pieces to be obtained do not have one or two dimensions being more prominent than others. "Dice", the pieces dicing results in, are approximately cubic.</rdfs:comment>
  <rdfs:isDefinedBy rdf:resource="http://www.ease-crc.org/ont/SOMA-ACT.owl"/>
  <rdfs:subClassOf rdf:resource="&soma;Cutting"/>
</owl:Class>

<owl:DatatypeProperty rdf:about="&soma;hasLength"
    rdfs:comment="The length of a shape."
    rdfs:label="has length">
  <rdfs:domain rdf:resource="&soma;ShapeRegion"/>
  <rdfs:isDefinedBy rdf:resource="http://www.ease-crc.org/ont/SOMA-OBJ.owl"/>
  <rdfs:range rdf:resource="&xsd;float"/>
  <rdfs:subPropertyOf rdf:resource="&soma;hasShapeParameter"/>
</owl:DatatypeProperty>

<owl:Class rdf:about="&soma;IllocutionaryTask">
  <rdfs:comment xml:lang="en">A task which is executed by a Locution action: A Locution is what was said and meant, Illocution is what was done.

When somebody says "Is there any salt?" at the dinner table, the illocutionary act is a request: "please give me some salt" even though the locutionary act (the literal sentence) was to ask a question about the presence of salt.

Source: https://en.wikipedia.org/wiki/Illocutionary_act</rdfs:comment>
  <rdfs:isDefinedBy rdf:resource="http://www.ease-crc.org/ont/SOMA-ACT.owl"/>
  <rdfs:label xml:lang="en">Illocutionary act</rdfs:label>
  <rdfs:subClassOf>
    <owl:Class>
      <owl:intersectionOf rdf:parseType="Collection">
        <rdf:Description rdf:about="&soma;CommunicationTask"/>
        <owl:Restriction>
          <owl:allValuesFrom>
            <owl:Restriction>
              <owl:allValuesFrom>
                <owl:Class>
                  <owl:unionOf rdf:parseType="Collection">
                    <rdf:Description rdf:about="&dul;Agent"/>
                    <rdf:Description rdf:about="&dul;SocialObject"/>
                  </owl:unionOf>
                </owl:Class>
              </owl:allValuesFrom>
              <owl:onProperty rdf:resource="&dul;hasParticipant"/>
            </owl:Restriction>
          </owl:allValuesFrom>
          <owl:onProperty rdf:resource="&dul;classifies"/>
        </owl:Restriction>
      </owl:intersectionOf>
    </owl:Class>
  </rdfs:subClassOf>
</owl:Class>

<owl:Class rdf:about="&soma;CounterfactualBinding">
  <rdfs:comment>CounterfactualBindings are used to express conditions:

-- that two roles share a filler (RoleRoleBindings);
-- that the filler of a role is a particular entity (RoleFillerBindings). This is typically the case when the filler of the role may be one of a few constants, as is the case with the execution status of a robot task.

TODO: for the robot workflows we are likely to need at the start, testing equality of fillers is enough. In the future, we may want to replace that with unifiability of fillers.</rdfs:comment>
  <rdfs:isDefinedBy rdf:resource="http://www.ease-crc.org/ont/SOMA-WF.owl"/>
  <rdfs:label xml:lang="en">Counterfactual binding</rdfs:label>
  <rdfs:subClassOf rdf:resource="&soma;Binding"/>
  <owl:disjointWith rdf:resource="&soma;FactualBinding"/>
</owl:Class>

<owl:Class rdf:about="&soma;DeclarativeClause"
    rdfs:comment="A clause which makes an assertion or declaration."
    rdfs:label="Declarative clause">
  <rdfs:isDefinedBy rdf:resource="http://www.ease-crc.org/ont/SOMA-SAY.owl"/>
  <rdfs:subClassOf rdf:resource="&soma;ClausalObject"/>
</owl:Class>

<owl:Class rdf:about="&soma;Cutter">
  <rdfs:comment>A role to classify an object used to cut other objects. Usually should poses sharpness as a quality. Execptions are not considered in this context. Such as a wind, water, or other natural agents cutting(eroding) the rocks.</rdfs:comment>
  <rdfs:isDefinedBy rdf:resource="http://www.ease-crc.org/ont/SOMA-OBJ.owl"/>
  <rdfs:subClassOf rdf:resource="&soma;Tool"/>
</owl:Class>

<owl:ObjectProperty rdf:about="&soma;coOccurs"
    rdfs:label="co occurs">
  <rdf:type rdf:resource="&owl;SymmetricProperty"/>
  <rdfs:comment>A schematic relation between any events that also implies that one event is temporally contained in the other.

Sub-properties are used to distinct between different cases of event endpoint relations that hold for different types of co-occurance.</rdfs:comment>
  <rdfs:domain rdf:resource="&dul;Event"/>
  <rdfs:isDefinedBy rdf:resource="http://www.ease-crc.org/ont/SOMA.owl"/>
  <rdfs:range rdf:resource="&dul;Event"/>
  <rdfs:subPropertyOf rdf:resource="&dul;overlaps"/>
</owl:ObjectProperty>

<owl:Class rdf:about="&soma;StatusFailure">
  <rdfs:comment>A status indicating the failure during some workflow execution.</rdfs:comment>
  <rdfs:isDefinedBy rdf:resource="http://www.ease-crc.org/ont/SOMA-WF.owl"/>
  <rdfs:subClassOf rdf:resource="&dul;Region"/>
</owl:Class>

<owl:Class rdf:about="&soma;EventAdjacentRole">
  <rdfs:label xml:lang="en">Event adjacent role</rdfs:label>
  <rdfs:label xml:lang="en">Thematic role</rdfs:label>
  <rdfs:comment>A role classifying a participant in an event.

In linguistics, this is also known as a thematic role.</rdfs:comment>
  <rdfs:isDefinedBy rdf:resource="http://www.ease-crc.org/ont/SOMA-OBJ.owl"/>
  <rdfs:subClassOf rdf:resource="&dul;Role"/>
</owl:Class>

<owl:Class rdf:about="&dul;EventType">
  <rdfs:isDefinedBy rdf:resource="http://www.ease-crc.org/ont/SOMA-PROC.owl"/>
  <rdfs:isDefinedBy rdf:resource="http://www.ease-crc.org/ont/SOMA-STATE.owl"/>
</owl:Class>

<owl:DatatypeProperty rdf:about="&soma;hasNameString"
    rdfs:label="has name string">
  <rdfs:comment>A relation recording some identifier associated to an Entity.</rdfs:comment>
  <rdfs:domain rdf:resource="&dul;Entity"/>
  <rdfs:isDefinedBy rdf:resource="http://www.ease-crc.org/ont/SOMA.owl"/>
  <rdfs:range rdf:resource="&xsd;string"/>
  <rdfs:subPropertyOf rdf:resource="&dul;hasDataValue"/>
</owl:DatatypeProperty>

<owl:Class rdf:about="&soma;GoalRole">
  <rdfs:comment>A role classifying objects that constitute the goal of an action.</rdfs:comment>
  <rdfs:isDefinedBy rdf:resource="http://www.ease-crc.org/ont/SOMA-OBJ.owl"/>
  <rdfs:label xml:lang="en">Goal role</rdfs:label>
  <rdfs:subClassOf rdf:resource="&soma;EventAdjacentRole"/>
</owl:Class>

<owl:Class rdf:about="http://www.ease-crc.org/ont/SOMA.owl/NonmanifestedSituation">
  <rdfs:comment>A Situation which does not manifest in any event.

The main use case for this is to represent expectations that are not met, e.g. unfulfilled post-conditions of an action. An action with unmet postconditions is then a failure.

Because of open world semantics of DL, the default assumption for a Situation individual with no "manifests in" relations is simply that we don't know yet whether that Situation is manifested and if so by what Event.

As such, an explicit assertion is needed to make a Situation a nonmanifested one: either declare that individual's type NonmanifestedSituation, or assert that it has 0 manifestsIn relations.</rdfs:comment>
  <rdfs:isDefinedBy rdf:resource="http://www.ease-crc.org/ont/SOMA-ACT.owl"/>
  <rdfs:label xml:lang="en">Nonmanifested situation</rdfs:label>
  <rdfs:subClassOf rdf:resource="&dul;Situation"/>
  <owl:equivalentClass>
    <owl:Class>
      <owl:intersectionOf rdf:parseType="Collection">
        <rdf:Description rdf:about="&dul;Situation"/>
        <owl:Restriction>
          <owl:onClass rdf:resource="&dul;Event"/>
          <owl:onProperty rdf:resource="http://www.ease-crc.org/ont/SOMA.owl/manifestsIn"/>
          <owl:qualifiedCardinality rdf:datatype="&xsd;nonNegativeInteger">0</owl:qualifiedCardinality>
        </owl:Restriction>
      </owl:intersectionOf>
    </owl:Class>
  </owl:equivalentClass>
</owl:Class>

<owl:Class rdf:about="&soma;Temperature"
    rdfs:comment="The heat present in an object.">
  <rdfs:subClassOf>
    <owl:Restriction>
      <owl:onProperty rdf:resource="&dul;hasRegion"/>
      <owl:someValuesFrom rdf:resource="&soma;TemperatureRegion"/>
    </owl:Restriction>
  </rdfs:subClassOf>
  <rdfs:subClassOf>
    <owl:Restriction>
      <owl:allValuesFrom rdf:resource="&soma;TemperatureRegion"/>
      <owl:onProperty rdf:resource="&dul;hasRegion"/>
    </owl:Restriction>
  </rdfs:subClassOf>
  <rdfs:subClassOf rdf:resource="&soma;Intrinsic"/>
  <rdfs:isDefinedBy rdf:resource="http://www.ease-crc.org/ont/SOMA-OBJ.owl"/>
</owl:Class>

<owl:Class rdf:about="&soma;SchematicTheory">
  <rdfs:comment>A theory used to describe, analyze, and reason with the meaning of a linguistic message.

Note that such theories are useful both when analyzing an actual linguistic production, and when creating a linguistic production to describe some observed experience.</rdfs:comment>
  <rdfs:isDefinedBy rdf:resource="http://www.ease-crc.org/ont/SOMA-SAY.owl"/>
  <rdfs:label xml:lang="en">Schematic theory</rdfs:label>
  <rdfs:subClassOf rdf:resource="&dul;Theory"/>
</owl:Class>

<owl:Axiom>
  <rdfs:comment xml:lang="en">The path of the file on a computer system.</rdfs:comment>
  <owl:annotatedProperty rdf:resource="&rdfs;subClassOf"/>
  <owl:annotatedSource rdf:resource="&soma;Digital_File"/>
  <owl:annotatedTarget rdf:nodeID="bn5"/>
</owl:Axiom>

<owl:Class rdf:about="&soma;RelatumRole">
  <rdfs:subClassOf>
    <owl:Restriction>
      <owl:allValuesFrom rdf:resource="&dul;PhysicalObject"/>
      <owl:onProperty rdf:resource="&dul;classifies"/>
    </owl:Restriction>
  </rdfs:subClassOf>
  <rdfs:subClassOf rdf:resource="&soma;SpatialRelationRole"/>
  <rdfs:comment>Denotes the reference object in a spatial or spatio-temporal schema, i.e. the object with secondary focal prominence. Terminological variants: Ground (Talmy 1983), Landmark (Langacker 1986).</rdfs:comment>
  <rdfs:isDefinedBy rdf:resource="http://www.ease-crc.org/ont/SOMA-OBJ.owl"/>
  <rdfs:label xml:lang="en">Relatum role</rdfs:label>
</owl:Class>

<owl:ObjectProperty rdf:about="http://www.ease-crc.org/ont/SOMA.owl/hasExpectedTerminalSituation">
  <rdfs:subPropertyOf rdf:resource="&soma;hasTerminalSituation"/>
  <rdfs:subPropertyOf rdf:resource="&dul;hasPostcondition"/>
  <rdfs:comment>A relation between a Transition and the Situation it is expected to, and does actually, end at. You can assert this relationship when the observed outcome of a transition matches expectations.</rdfs:comment>
  <rdfs:domain rdf:resource="&soma;SituationTransition"/>
  <rdfs:isDefinedBy rdf:resource="http://www.ease-crc.org/ont/SOMA-ACT.owl"/>
  <rdfs:label xml:lang="en">has expected terminal situation</rdfs:label>
  <rdfs:range rdf:resource="&dul;Situation"/>
</owl:ObjectProperty>

<owl:Class rdf:about="&soma;ActionExecutionPlan">
  <rdfs:comment>idea: steps in workflows assert that they are defined by action execution plans.</rdfs:comment>
  <rdfs:comment>links role and parameter fillers to e.g. slots in a data structure</rdfs:comment>
  <rdfs:subClassOf>
    <owl:Restriction>
      <owl:allValuesFrom>
        <owl:Restriction>
          <owl:onProperty rdf:resource="&dul;hasParameter"/>
          <owl:someValuesFrom rdf:resource="&soma;Status"/>
        </owl:Restriction>
      </owl:allValuesFrom>
      <owl:onProperty rdf:resource="&dul;definesTask"/>
    </owl:Restriction>
  </rdfs:subClassOf>
  <rdfs:subClassOf rdf:resource="&dul;Plan"/>
  <rdfs:isDefinedBy rdf:resource="http://www.ease-crc.org/ont/SOMA.owl"/>
  <rdfs:label xml:lang="en">Action execution plan</rdfs:label>
</owl:Class>

<owl:Class rdf:about="&dul;Parameter">
  <rdfs:isDefinedBy rdf:resource="http://www.ease-crc.org/ont/SOMA-WF.owl"/>
</owl:Class>

<owl:ObjectProperty rdf:about="&dul;executesTask">
  <rdfs:subPropertyOf rdf:resource="&soma;isOccurrenceOf"/>
</owl:ObjectProperty>

<owl:Class rdf:about="&soma;Computer_Program">
  <owl:equivalentClass>
    <owl:Class>
      <owl:intersectionOf rdf:parseType="Collection">
        <rdf:Description rdf:about="&soma;Structured_Text"/>
        <owl:Restriction>
          <owl:onProperty rdf:resource="&soma;isGivenMeaningBy"/>
          <owl:someValuesFrom rdf:resource="&soma;Programming_Language"/>
        </owl:Restriction>
      </owl:intersectionOf>
    </owl:Class>
  </owl:equivalentClass>
  <owl:equivalentClass>
    <owl:Class>
      <owl:intersectionOf rdf:parseType="Collection">
        <rdf:Description rdf:about="&soma;Structured_Text"/>
        <owl:Restriction>
          <owl:onProperty rdf:resource="&dul;expresses"/>
          <owl:someValuesFrom rdf:resource="&soma;Algorithm"/>
        </owl:Restriction>
      </owl:intersectionOf>
    </owl:Class>
  </owl:equivalentClass>
  <rdfs:comment xml:lang="en">The Program itself (the specific set of instruction in a Programming Language), not the file that it is contained in nor the implemented algorithm!</rdfs:comment>
  <rdfs:isDefinedBy rdf:resource="http://www.ease-crc.org/ont/SOMA-IO.owl"/>
  <rdfs:label xml:lang="en">Computer program</rdfs:label>
</owl:Class>

<owl:AsymmetricProperty rdf:about="&soma;overlappedBy"
    soma:symbol="oi"
    rdfs:label="overlapped by">
  <rdf:type rdf:resource="&owl;IrreflexiveProperty"/>
  <rdf:type rdf:resource="&owl;ObjectProperty"/>
  <rdfs:comment>A schematic relation between any entities that also implies ordering, e.g. "she has worked into the night".</rdfs:comment>
  <rdfs:domain rdf:resource="&dul;Entity"/>
  <rdfs:isDefinedBy rdf:resource="http://www.ease-crc.org/ont/SOMA.owl"/>
  <rdfs:range rdf:resource="&dul;Entity"/>
  <rdfs:subPropertyOf rdf:resource="&dul;overlaps"/>
  <owl:inverseOf rdf:resource="&soma;overlappedOn"/>
</owl:AsymmetricProperty>

<owl:Class rdf:about="&soma;Cleaning">
  <rdfs:subClassOf>
    <owl:Restriction>
      <owl:onProperty rdf:resource="&soma;isTaskAffordedBy"/>
      <owl:someValuesFrom rdf:resource="&soma;Purification"/>
    </owl:Restriction>
  </rdfs:subClassOf>
  <rdfs:subClassOf rdf:resource="&soma;ModifyingPhysicalObject"/>
  <rdfs:comment>This task in which an agent restores all the objects to their destined locations, wiping a specific object</rdfs:comment>
  <rdfs:isDefinedBy rdf:resource="http://www.ease-crc.org/ont/SOMA-ACT.owl"/>
</owl:Class>

<owl:Class rdf:about="&dul;Plan">
  <rdfs:subClassOf>
    <owl:Restriction>
      <owl:onProperty rdf:resource="&soma;isPlanFor"/>
      <owl:someValuesFrom rdf:resource="&dul;Task"/>
    </owl:Restriction>
  </rdfs:subClassOf>
</owl:Class>

<soma:StatusFailure rdf:about="&soma;FailWFNondeterministicContinuation">
  <rdf:type rdf:resource="&owl;NamedIndividual"/>
  <rdfs:comment>A particular kind of failure: it is not clear how to continue a workflow because several possibilities exist.</rdfs:comment>
  <rdfs:isDefinedBy rdf:resource="http://www.ease-crc.org/ont/SOMA-WF.owl"/>
</soma:StatusFailure>

<owl:Class rdf:about="&soma;DesignedContainer"
    rdfs:label="Designed container">
  <rdfs:subClassOf>
    <owl:Restriction>
      <owl:onProperty rdf:resource="&soma;hasDisposition"/>
      <owl:someValuesFrom rdf:resource="&soma;Containment"/>
    </owl:Restriction>
  </rdfs:subClassOf>
  <rdfs:subClassOf rdf:resource="&dul;DesignedArtifact"/>
  <rdfs:comment>An item designed to be able to hold some other items, preventing their free movement and/or protecting them from outside influence. Containers may be used for storage, or to obtain control over items that are otherwise hard to manipulate directly (e.g. liquids).</rdfs:comment>
  <rdfs:isDefinedBy rdf:resource="http://www.ease-crc.org/ont/SOMA-OBJ.owl"/>
</owl:Class>

<owl:ObjectProperty rdf:about="&soma;isEndLinkOf"
    rdfs:label="is end link of">
  <rdfs:comment>Relates an object to kinematic components at the end of the kinematic chain.</rdfs:comment>
  <rdfs:domain rdf:resource="&dul;PhysicalObject"/>
  <rdfs:isDefinedBy rdf:resource="http://www.ease-crc.org/ont/SOMA-OBJ.owl"/>
  <rdfs:range rdf:resource="&dul;PhysicalObject"/>
  <rdfs:subPropertyOf rdf:resource="&soma;isLinkOf"/>
</owl:ObjectProperty>

<owl:Class rdf:about="&soma;DeductiveReasoning">
  <rdfs:comment>A task in which the Agent, using general logical principles that it considers logically valid, applied to premises that it considers logically true, arrives at conclusions that it considers logically certain.

Deduction is often explained as starting from the "general" (some property X is known about all members of a set S), applying it to the "specific" (some Entity Y is known to belong to set S), to arrive at a specialization of the general property (X applies to Y).</rdfs:comment>
  <rdfs:isDefinedBy rdf:resource="http://www.ease-crc.org/ont/SOMA-ACT.owl"/>
  <rdfs:label xml:lang="en">Deductive reasoning</rdfs:label>
  <rdfs:subClassOf rdf:resource="&soma;Reasoning"/>
</owl:Class>

<owl:Class rdf:about="&soma;MetacognitiveMonitoring"
    rdfs:label="Metacognitive monitoring">
  <rdfs:comment>The task to label the processes and states of the own mind, e.g., to interprete the feeling of knowing an information but not being able to retrieve it at the moment as a tip-of-the-tongue event.</rdfs:comment>
  <rdfs:isDefinedBy rdf:resource="http://www.ease-crc.org/ont/SOMA-ACT.owl"/>
  <rdfs:subClassOf rdf:resource="&soma;Introspecting"/>
</owl:Class>

<owl:Class rdf:about="&soma;MassAttribute"
    rdfs:label="Mass attribute">
  <rdfs:subClassOf>
    <owl:Restriction>
      <owl:onDataRange rdf:resource="&xsd;double"/>
      <owl:onProperty rdf:resource="&soma;hasMassValue"/>
      <owl:qualifiedCardinality rdf:datatype="&xsd;nonNegativeInteger">1</owl:qualifiedCardinality>
    </owl:Restriction>
  </rdfs:subClassOf>
  <rdfs:subClassOf rdf:resource="&dul;PhysicalAttribute"/>
  <rdfs:comment>The quantity of matter which a body contains, as measured by its acceleration under given force or by the force exerted on it by a gravitational field.</rdfs:comment>
  <rdfs:isDefinedBy rdf:resource="http://www.ease-crc.org/ont/SOMA-OBJ.owl"/>
</owl:Class>

<owl:AsymmetricProperty rdf:about="&soma;metBy"
    soma:symbol="mi">
  <rdf:type rdf:resource="&owl;IrreflexiveProperty"/>
  <rdf:type rdf:resource="&owl;ObjectProperty"/>
  <rdfs:comment>A relation between entities, expressing a 'sequence' schema where one of the entities exactly ends where the other entity starts.</rdfs:comment>
  <rdfs:domain rdf:resource="&dul;Entity"/>
  <rdfs:isDefinedBy rdf:resource="http://www.ease-crc.org/ont/SOMA.owl"/>
  <rdfs:label xml:lang="en">met by</rdfs:label>
  <rdfs:range rdf:resource="&dul;Entity"/>
  <rdfs:subPropertyOf rdf:resource="&dul;directlyFollows"/>
</owl:AsymmetricProperty>

<owl:ObjectProperty rdf:about="&soma;isParentLinkOf"
    rdfs:label="is parent link of">
  <rdfs:comment>Relates a joint to the link it connects which is closer to the root of the kinematic chain.</rdfs:comment>
  <rdfs:domain rdf:resource="&dul;PhysicalObject"/>
  <rdfs:isDefinedBy rdf:resource="http://www.ease-crc.org/ont/SOMA-OBJ.owl"/>
  <rdfs:range rdf:resource="&soma;Joint"/>
  <rdfs:subPropertyOf rdf:resource="&dul;isConstituentOf"/>
</owl:ObjectProperty>

<owl:Class rdf:about="&soma;ForgettingIrrelevantInformation">
  <rdfs:comment xml:lang="en">A mental task in which the executing agent aims to clean up its present information by deleting an irrelevant information.</rdfs:comment>
  <rdfs:isDefinedBy rdf:resource="http://www.ease-crc.org/ont/SOMA-ACT.owl"/>
  <rdfs:label xml:lang="en">Forgetting irrelevant information</rdfs:label>
  <rdfs:subClassOf rdf:resource="&soma;InformationDismissal"/>
</owl:Class>

<owl:Class rdf:about="&soma;Accessor">
  <rdfs:comment>A role classifying an object used to gain access to some other entity.</rdfs:comment>
  <rdfs:isDefinedBy rdf:resource="http://www.ease-crc.org/ont/SOMA-OBJ.owl"/>
  <rdfs:subClassOf rdf:resource="&soma;Instrument"/>
</owl:Class>

<owl:ObjectProperty rdf:about="&soma;isJointStateOf"
    rdfs:comment="Relates a joint to its state."
    rdfs:label="is joint state of">
  <rdfs:domain rdf:resource="&soma;JointState"/>
  <rdfs:isDefinedBy rdf:resource="http://www.ease-crc.org/ont/SOMA-OBJ.owl"/>
  <rdfs:range rdf:resource="&soma;Joint"/>
  <rdfs:subPropertyOf rdf:resource="&dul;isRegionFor"/>
</owl:ObjectProperty>

<owl:Class rdf:about="&soma;CoverageTheory">
  <rdfs:comment>A schematic theory of a functional relation between two objects such that one of them, the locatum, blocks access to the interior of the relatum.

Let xL, xR be objects filling the locatum, relatum roles of this schema. Then one can infer that xL coversObject xR.</rdfs:comment>
  <rdfs:isDefinedBy rdf:resource="http://www.ease-crc.org/ont/SOMA-SAY.owl"/>
  <rdfs:subClassOf rdf:resource="&soma;FunctionalSpatialSchemaTheory"/>
</owl:Class>

<owl:ObjectProperty rdf:about="&soma;causesTransition"
    rdfs:label="causes transition">
  <rdfs:comment>A Transition between two Situations is always the result of some Event, and the causesTransition relation should be used to record the causal relation from the Event to the Transition.</rdfs:comment>
  <rdfs:domain rdf:resource="&dul;Event"/>
  <rdfs:isDefinedBy rdf:resource="http://www.ease-crc.org/ont/SOMA.owl"/>
  <rdfs:range rdf:resource="&dul;Transition"/>
  <rdfs:subPropertyOf rdf:resource="&dul;isEventIncludedIn"/>
  <owl:inverseOf rdf:resource="&soma;isCausedByEvent"/>
</owl:ObjectProperty>

<owl:Class rdf:about="&soma;Natural_Language_Text">
  <rdfs:comment xml:lang="en">A Text in a Natural Language.</rdfs:comment>
  <rdfs:isDefinedBy rdf:resource="http://www.ease-crc.org/ont/SOMA-IO.owl"/>
  <rdfs:label xml:lang="en">Natural language text</rdfs:label>
  <owl:equivalentClass>
    <owl:Class>
      <owl:intersectionOf rdf:parseType="Collection">
        <rdf:Description rdf:about="&soma;Text"/>
        <owl:Restriction>
          <owl:onProperty rdf:resource="&soma;isGivenMeaningBy"/>
          <owl:someValuesFrom rdf:resource="&soma;Natural_Language"/>
        </owl:Restriction>
      </owl:intersectionOf>
    </owl:Class>
  </owl:equivalentClass>
</owl:Class>

<owl:ObjectProperty rdf:about="&soma;isInsideOf"
    rdfs:label="is inside of">
  <rdfs:subPropertyOf rdf:resource="&soma;isContainedIn"/>
  <rdfs:subPropertyOf rdf:resource="&dul;hasLocation"/>
  <rdf:type rdf:resource="&owl;TransitiveProperty"/>
  <rdfs:comment>A spatial relation holding between an object (the container), and objects it contains.</rdfs:comment>
  <rdfs:domain rdf:resource="&dul;PhysicalObject"/>
  <rdfs:isDefinedBy rdf:resource="http://www.ease-crc.org/ont/SOMA-OBJ.owl"/>
  <rdfs:range rdf:resource="&dul;PhysicalObject"/>
</owl:ObjectProperty>

<owl:ObjectProperty rdf:about="&soma;isTerminalSceneOf"
    rdfs:label="is terminal scene of">
  <rdfs:comment>A relation between StateTransitions and Scenes, which identifies the scene the transition is expected to end at.</rdfs:comment>
  <rdfs:domain rdf:resource="&soma;Scene"/>
  <rdfs:isDefinedBy rdf:resource="http://www.ease-crc.org/ont/SOMA.owl"/>
  <rdfs:range rdf:resource="&soma;StateTransition"/>
  <rdfs:subPropertyOf rdf:resource="&soma;isTerminalStateOf"/>
</owl:ObjectProperty>

<owl:Class rdf:about="&soma;ImperativeClause"
    rdfs:label="Imperative clause">
  <rdfs:subClassOf>
    <owl:Restriction>
      <owl:onProperty rdf:resource="&dul;expresses"/>
      <owl:someValuesFrom rdf:resource="&soma;StateTransition"/>
    </owl:Restriction>
  </rdfs:subClassOf>
  <rdfs:subClassOf>
    <owl:Restriction>
      <owl:allValuesFrom rdf:resource="&soma;StateTransition"/>
      <owl:onProperty rdf:resource="&dul;expresses"/>
    </owl:Restriction>
  </rdfs:subClassOf>
  <rdfs:subClassOf rdf:resource="&soma;ClausalObject"/>
  <rdfs:comment>A clause which commands some agent to perform a task or bring about a state of affairs.</rdfs:comment>
  <rdfs:isDefinedBy rdf:resource="http://www.ease-crc.org/ont/SOMA-SAY.owl"/>
</owl:Class>

<owl:Class rdf:about="&soma;Channel">
  <rdfs:subClassOf>
    <owl:Restriction>
      <owl:onProperty rdf:resource="&dul;hasTask"/>
      <owl:someValuesFrom rdf:resource="&soma;CommunicationTask"/>
    </owl:Restriction>
  </rdfs:subClassOf>
  <rdfs:subClassOf rdf:resource="&soma;PathRole"/>
  <rdfs:comment xml:lang="en">A Channel in a Communication Task is the path of travel by a Message, e.g., via WLAN, air (in the case of a Message classifying soundwaves) or a telephone cable.</rdfs:comment>
  <rdfs:isDefinedBy rdf:resource="http://www.ease-crc.org/ont/SOMA-ACT.owl"/>
  <rdfs:label xml:lang="en">Channel</rdfs:label>
</owl:Class>

<owl:Class rdf:about="&soma;Composing">
  <rdfs:subClassOf>
    <owl:Restriction>
      <owl:allValuesFrom rdf:resource="&soma;ConnectedObject"/>
      <owl:onProperty rdf:resource="&soma;affordsTrigger"/>
    </owl:Restriction>
  </rdfs:subClassOf>
  <rdfs:subClassOf rdf:resource="&soma;Variability"/>
  <rdfs:comment>The disposition of an object (the tool) to change the compositional structure of others.</rdfs:comment>
  <rdfs:isDefinedBy rdf:resource="http://www.ease-crc.org/ont/SOMA-OBJ.owl"/>
</owl:Class>

<owl:Class rdf:about="&soma;StoredObject">
  <rdfs:comment>An object being stored into some other object, usually inside a container.</rdfs:comment>
  <rdfs:isDefinedBy rdf:resource="http://www.ease-crc.org/ont/SOMA-OBJ.owl"/>
  <rdfs:subClassOf rdf:resource="&soma;EnclosedObject"/>
</owl:Class>

<owl:Class rdf:about="&soma;Barrier">
  <rdfs:comment>A role classifying an object used to prevent others from entering or leaving a restricted space or group.</rdfs:comment>
  <rdfs:isDefinedBy rdf:resource="http://www.ease-crc.org/ont/SOMA-OBJ.owl"/>
  <rdfs:subClassOf rdf:resource="&soma;Restrictor"/>
</owl:Class>

<owl:Class rdf:about="&soma;Retracting">
  <rdfs:comment>A task in which an Agent moves its arms away from a location.</rdfs:comment>
  <rdfs:isDefinedBy rdf:resource="http://www.ease-crc.org/ont/SOMA-ACT.owl"/>
  <rdfs:subClassOf rdf:resource="&soma;EndEffectorPositioning"/>
</owl:Class>

<owl:Class rdf:about="&dul;Transition"/>

<owl:Class rdf:about="&soma;CausativeRole">
  <rdfs:comment>A role classifying objects that are responsible in bringing about an event.

The paradigmatic example is the Agent performing an Action -- the Agent is the effective cause of the Action it performs. However, not all objects causing events are agents.</rdfs:comment>
  <rdfs:isDefinedBy rdf:resource="http://www.ease-crc.org/ont/SOMA-OBJ.owl"/>
  <rdfs:label xml:lang="en">Causative role</rdfs:label>
  <rdfs:subClassOf rdf:resource="&soma;EventAdjacentRole"/>
</owl:Class>

<owl:ObjectProperty rdf:about="&soma;isChildLinkOf"
    rdfs:label="is child link of">
  <rdfs:comment>Relates a joint to the link it connects which is closer to the end of the kinematic chain.</rdfs:comment>
  <rdfs:domain rdf:resource="&dul;PhysicalObject"/>
  <rdfs:isDefinedBy rdf:resource="http://www.ease-crc.org/ont/SOMA-OBJ.owl"/>
  <rdfs:range rdf:resource="&soma;Joint"/>
  <rdfs:subPropertyOf rdf:resource="&dul;isConstituentOf"/>
</owl:ObjectProperty>

<owl:Class rdf:about="&soma;Approaching">
  <rdfs:comment>A process type to classify motions by which a body approaches some object or location.</rdfs:comment>
  <rdfs:isDefinedBy rdf:resource="http://www.ease-crc.org/ont/SOMA-PROC.owl"/>
  <rdfs:subClassOf rdf:resource="&soma;Locomotion"/>
</owl:Class>

<owl:Class rdf:about="&soma;FrictionAttribute"
    rdfs:label="Friction attribute">
  <rdfs:subClassOf>
    <owl:Restriction>
      <owl:onDataRange rdf:resource="&xsd;double"/>
      <owl:onProperty rdf:resource="&soma;hasFrictionValue"/>
      <owl:qualifiedCardinality rdf:datatype="&xsd;nonNegativeInteger">1</owl:qualifiedCardinality>
    </owl:Restriction>
  </rdfs:subClassOf>
  <rdfs:subClassOf rdf:resource="&dul;PhysicalAttribute"/>
  <rdfs:comment>The resistance that one surface or object encounters when moving over another.</rdfs:comment>
  <rdfs:isDefinedBy rdf:resource="http://www.ease-crc.org/ont/SOMA-OBJ.owl"/>
</owl:Class>

<owl:ObjectProperty rdf:about="&soma;isInputParameterFor"
    rdfs:label="is input parameter for">
  <rdfs:comment>A relation between a Task and one of its input parameters.</rdfs:comment>
  <rdfs:comment>A relation from a Parameter to an EventType (typically, a Task). The parameter describes some state of affairs that precedes and will contribute to the event classified by the EventType.</rdfs:comment>
  <rdfs:domain rdf:resource="&dul;Parameter"/>
  <rdfs:isDefinedBy rdf:resource="http://www.ease-crc.org/ont/SOMA.owl"/>
  <rdfs:range rdf:resource="&dul;EventType"/>
  <rdfs:subPropertyOf rdf:resource="&dul;isParameterFor"/>
</owl:ObjectProperty>

<owl:ObjectProperty rdf:about="&soma;hasRootLink"
    rdfs:label="has root link">
  <rdfs:comment>Relates an object to kinematic components at the root of the kinematic chain.</rdfs:comment>
  <rdfs:domain rdf:resource="&dul;PhysicalObject"/>
  <rdfs:isDefinedBy rdf:resource="http://www.ease-crc.org/ont/SOMA-OBJ.owl"/>
  <rdfs:range rdf:resource="&dul;PhysicalObject"/>
  <rdfs:subPropertyOf rdf:resource="&soma;hasLink"/>
  <owl:inverseOf rdf:resource="&soma;isRootLinkOf"/>
</owl:ObjectProperty>

<owl:ObjectProperty rdf:about="&dul;involvesAgent">
  <rdfs:isDefinedBy rdf:resource="http://www.ease-crc.org/ont/SOMA.owl"/>
</owl:ObjectProperty>

<owl:ObjectProperty rdf:about="&soma;definesEventType">
  <rdfs:isDefinedBy rdf:resource="http://www.ease-crc.org/ont/SOMA-ACT.owl"/>
  <rdfs:isDefinedBy rdf:resource="http://www.ease-crc.org/ont/SOMA-OBJ.owl"/>
  <rdfs:label xml:lang="en">A relation between a description and an event type, e.g. an Affordance of an object to be cut with a knife describes that event.

The distinction to defines task is necessary to let Dispositions and Affordances not only describe which tasks might be afforded by objects, but also whihc processes (where there is no agent). For example, the fall of a knife from a shelf slicing a loaf of bread on impact is , in the absence of an executing agent, not a task but merely a process, the possibility of which is nevertheless described by the dispositions of the knife and the loaf.</rdfs:label>
  <rdfs:label xml:lang="en">defines event type</rdfs:label>
  <rdfs:domain rdf:resource="&dul;Description"/>
  <rdfs:range rdf:resource="&dul;EventType"/>
  <rdfs:subPropertyOf rdf:resource="&dul;defines"/>
  <owl:inverseOf rdf:resource="&soma;isEventTypeDefinedIn"/>
</owl:ObjectProperty>

<owl:Class rdf:about="&soma;GraphQueryLanguage">
  <rdfs:comment xml:lang="en">A Query Language that is designed for communication with some Graph Database.</rdfs:comment>
  <rdfs:isDefinedBy rdf:resource="http://www.ease-crc.org/ont/SOMA-IO.owl"/>
  <rdfs:label xml:lang="en">Graph query language</rdfs:label>
  <rdfs:subClassOf rdf:resource="&soma;QueryLanguage"/>
</owl:Class>

<owl:Class rdf:about="&soma;Human-readable_Programming_Language">
  <rdfs:subClassOf>
    <owl:Restriction>
      <owl:allValuesFrom rdf:resource="&soma;Source_Code"/>
      <owl:onProperty rdf:resource="&soma;givesMeaningTo"/>
    </owl:Restriction>
  </rdfs:subClassOf>
  <rdfs:subClassOf rdf:resource="&soma;Programming_Language"/>
  <rdfs:comment xml:lang="en">A Programming language like Java, Python etc. but not binary machine code.</rdfs:comment>
  <rdfs:isDefinedBy rdf:resource="http://www.ease-crc.org/ont/SOMA-IO.owl"/>
  <rdfs:label xml:lang="en">Human-readable Programming Language</rdfs:label>
</owl:Class>

<owl:ObjectProperty rdf:about="&soma;isContainedIn"
    rdfs:label="is contained in">
  <rdfs:comment>The inverse of the contains relation. See the contains relation for details.</rdfs:comment>
  <rdfs:domain rdf:resource="&dul;Entity"/>
  <rdfs:isDefinedBy rdf:resource="http://www.ease-crc.org/ont/SOMA.owl"/>
  <rdfs:range rdf:resource="&dul;Entity"/>
  <rdfs:subPropertyOf rdf:resource="&dul;overlaps"/>
</owl:ObjectProperty>

<owl:Class rdf:about="&soma;PhysicalAccessibility">
  <rdfs:subClassOf>
    <owl:Restriction>
      <owl:onProperty rdf:resource="&soma;isStateTypeOf"/>
      <owl:someValuesFrom rdf:resource="&soma;Item"/>
    </owl:Restriction>
  </rdfs:subClassOf>
  <rdfs:subClassOf>
    <owl:Restriction>
      <owl:onProperty rdf:resource="&soma;isStateTypeOf"/>
      <owl:someValuesFrom rdf:resource="&soma;Restrictor"/>
    </owl:Restriction>
  </rdfs:subClassOf>
  <rdfs:subClassOf rdf:resource="&soma;StateType"/>
  <rdfs:comment>Classifies States in which an item is placed in a container or protected by a protector, but the placement of the item and container is such that a, usually agentive, accessor may nevertheless reach the item in order to perform a task.</rdfs:comment>
  <rdfs:isDefinedBy rdf:resource="http://www.ease-crc.org/ont/SOMA-STATE.owl"/>
  <rdfs:label xml:lang="en">Physical accessibility</rdfs:label>
</owl:Class>

<owl:Class rdf:about="&soma;ContactState"
    rdfs:comment="Classifies States in which some objects are in contact.">
  <rdfs:subClassOf>
    <owl:Restriction>
      <owl:allValuesFrom>
        <owl:Restriction>
          <owl:minQualifiedCardinality rdf:datatype="&xsd;nonNegativeInteger">2</owl:minQualifiedCardinality>
          <owl:onClass rdf:resource="&dul;PhysicalObject"/>
          <owl:onProperty rdf:resource="&dul;hasParticipant"/>
        </owl:Restriction>
      </owl:allValuesFrom>
      <owl:onProperty rdf:resource="&dul;classifies"/>
    </owl:Restriction>
  </rdfs:subClassOf>
  <rdfs:subClassOf rdf:resource="&soma;StateType"/>
  <rdfs:isDefinedBy rdf:resource="http://www.ease-crc.org/ont/SOMA-STATE.owl"/>
  <rdfs:label xml:lang="en">Contact state</rdfs:label>
</owl:Class>

<owl:Class rdf:about="&soma;Episode"
    rdfs:comment="">
  <rdfs:isDefinedBy rdf:resource="http://www.ease-crc.org/ont/SOMA.owl"/>
  <rdfs:subClassOf rdf:resource="&dul;Situation"/>
</owl:Class>

<owl:Class rdf:about="&soma;AssumingArmPose">
  <rdfs:comment>A task by which an Agent arranges one/some/all of its arms according to some configuration.</rdfs:comment>
  <rdfs:isDefinedBy rdf:resource="http://www.ease-crc.org/ont/SOMA-ACT.owl"/>
  <rdfs:label xml:lang="en">Assuming arm pose</rdfs:label>
  <rdfs:subClassOf rdf:resource="&soma;AssumingPose"/>
</owl:Class>

<owl:Class rdf:about="&soma;Lowering">
  <rdfs:comment>A task in which an Agent reduces the elevation at which they hold an item.</rdfs:comment>
  <rdfs:isDefinedBy rdf:resource="http://www.ease-crc.org/ont/SOMA-ACT.owl"/>
  <rdfs:subClassOf rdf:resource="&soma;Actuating"/>
</owl:Class>

<owl:Class rdf:about="&soma;CausedMotionTheory">
  <rdfs:subClassOf>
    <owl:Restriction>
      <owl:onProperty rdf:resource="&dul;defines"/>
      <owl:someValuesFrom rdf:resource="&soma;CausalEventRole"/>
    </owl:Restriction>
  </rdfs:subClassOf>
  <rdfs:subClassOf>
    <owl:Restriction>
      <owl:onProperty rdf:resource="&dul;defines"/>
      <owl:someValuesFrom rdf:resource="&soma;Instrument"/>
    </owl:Restriction>
  </rdfs:subClassOf>
  <rdfs:subClassOf>
    <owl:Restriction>
      <owl:onProperty rdf:resource="&dul;defines"/>
      <owl:someValuesFrom rdf:resource="&soma;Patient"/>
    </owl:Restriction>
  </rdfs:subClassOf>
  <rdfs:subClassOf>
    <owl:Restriction>
      <owl:onProperty rdf:resource="&dul;defines"/>
      <owl:someValuesFrom rdf:resource="&soma;PerformerRole"/>
    </owl:Restriction>
  </rdfs:subClassOf>
  <rdfs:subClassOf>
    <owl:Restriction>
      <owl:onProperty rdf:resource="&dul;hasPart"/>
      <owl:someValuesFrom rdf:resource="&soma;SourcePathGoalTheory"/>
    </owl:Restriction>
  </rdfs:subClassOf>
  <rdfs:subClassOf rdf:resource="&soma;ImageSchemaTheory"/>
  <rdfs:comment>A schematic theory describing a situation in which an agent performs an action which causes an object to move along a certain path. A popular example being "He sneezed the napkin off the table." (Goldberg 1995)

Let xA, xP be objects filling the agent, patient roles of this schema. Then one can infer that xA movesObject xP.</rdfs:comment>
  <rdfs:isDefinedBy rdf:resource="http://www.ease-crc.org/ont/SOMA-SAY.owl"/>
  <rdfs:label xml:lang="en">Caused motion theory</rdfs:label>
</owl:Class>

<owl:Class rdf:about="&soma;Natural_Language">
  <rdfs:subClassOf>
    <owl:Restriction>
      <owl:allValuesFrom rdf:resource="&soma;Natural_Language_Text"/>
      <owl:onProperty rdf:resource="&soma;givesMeaningTo"/>
    </owl:Restriction>
  </rdfs:subClassOf>
  <rdfs:subClassOf rdf:resource="&soma;Language"/>
  <rdfs:comment xml:lang="en">A Natural Language is any language that has evolved naturally in humans through use and repetition without conscious planning or premeditation.

From Wikipedia: https://en.wikipedia.org/wiki/Natural_language</rdfs:comment>
  <rdfs:isDefinedBy rdf:resource="http://www.ease-crc.org/ont/SOMA-IO.owl"/>
  <rdfs:label xml:lang="en">Natural Language</rdfs:label>
</owl:Class>

<owl:ObjectProperty rdf:about="&soma;isAlterationResultOf"
    rdfs:label="is alteration result of">
  <rdfs:comment>Relates an action that alters an object to the region that the alteration reached during the action.</rdfs:comment>
  <rdfs:domain rdf:resource="&dul;Region"/>
  <rdfs:isDefinedBy rdf:resource="http://www.ease-crc.org/ont/SOMA-OBJ.owl"/>
  <rdfs:range rdf:resource="&dul;Action"/>
  <rdfs:subPropertyOf rdf:resource="&dul;isRegionFor"/>
</owl:ObjectProperty>

<owl:ObjectProperty rdf:about="&soma;firstMember">
  <rdfs:comment>A relation between a collection and a member of it that is least according to some ordering. This ordering can be arbitrary, i.e. the order in which Entities are recorded in the Collection.</rdfs:comment>
  <rdfs:domain rdf:resource="&dul;Collection"/>
  <rdfs:isDefinedBy rdf:resource="http://www.ease-crc.org/ont/SOMA.owl"/>
  <rdfs:label xml:lang="en">first member</rdfs:label>
  <rdfs:range rdf:resource="&dul;Entity"/>
  <rdfs:subPropertyOf rdf:resource="&dul;hasMember"/>
</owl:ObjectProperty>

<owl:Class rdf:about="&soma;SoftwareRole">
  <rdfs:subClassOf>
    <owl:Restriction>
      <owl:allValuesFrom rdf:resource="&soma;Software"/>
      <owl:onProperty rdf:resource="&dul;classifies"/>
    </owl:Restriction>
  </rdfs:subClassOf>
  <rdfs:subClassOf rdf:resource="&dul;Role"/>
  <rdfs:comment xml:lang="en">A Software Role is a Role applying to only Software and encoding the purpose of the Software: Its Role within Interface Patterns (e.g. Client vs. Server), its functionality (e.g. Database vs. Comnputer Game), and so on.</rdfs:comment>
  <rdfs:isDefinedBy rdf:resource="http://www.ease-crc.org/ont/SOMA-IO.owl"/>
  <rdfs:label xml:lang="en">Software role</rdfs:label>
</owl:Class>

<owl:Class rdf:about="&soma;Room"
    rdfs:comment="Space that can be occupied or where something can be done.">
  <rdfs:isDefinedBy rdf:resource="http://www.ease-crc.org/ont/SOMA-OBJ.owl"/>
  <rdfs:subClassOf rdf:resource="&dul;PhysicalPlace"/>
</owl:Class>

<owl:ObjectProperty rdf:about="&dul;definesRole">
  <rdfs:isDefinedBy rdf:resource="http://www.ease-crc.org/ont/SOMA-STATE.owl"/>
</owl:ObjectProperty>

<owl:Class rdf:about="&soma;PhysicalBlockage">
  <rdfs:subClassOf>
    <owl:Restriction>
      <owl:onProperty rdf:resource="&soma;isStateTypeOf"/>
      <owl:someValuesFrom rdf:resource="&soma;Item"/>
    </owl:Restriction>
  </rdfs:subClassOf>
  <rdfs:subClassOf>
    <owl:Restriction>
      <owl:onProperty rdf:resource="&soma;isStateTypeOf"/>
      <owl:someValuesFrom rdf:resource="&soma;Restrictor"/>
    </owl:Restriction>
  </rdfs:subClassOf>
  <rdfs:subClassOf rdf:resource="&soma;StateType"/>
  <rdfs:comment>Classifies States in which an object, in general called restrictor, blocks access to an item. A usually agentive accessor, whose access is blocked, may be specified.</rdfs:comment>
  <rdfs:isDefinedBy rdf:resource="http://www.ease-crc.org/ont/SOMA-STATE.owl"/>
  <rdfs:label xml:lang="en">Physical blockage</rdfs:label>
</owl:Class>

<owl:ObjectProperty rdf:about="&dul;directlyPrecedes"/>

<owl:Class rdf:about="&dul;Description">
  <rdfs:isDefinedBy rdf:resource="http://www.ease-crc.org/ont/SOMA-PROC.owl"/>
  <rdfs:isDefinedBy rdf:resource="http://www.ease-crc.org/ont/SOMA-STATE.owl"/>
  <rdfs:isDefinedBy rdf:resource="http://www.ease-crc.org/ont/SOMA-WF.owl"/>
</owl:Class>

<owl:Class rdf:about="&soma;Proprioceiving">
  <rdfs:comment>A task in which the Agent gathers and interprets sensor information about itself.</rdfs:comment>
  <rdfs:isDefinedBy rdf:resource="http://www.ease-crc.org/ont/SOMA-ACT.owl"/>
  <rdfs:subClassOf rdf:resource="&soma;PhysicalTask"/>
</owl:Class>

<owl:ObjectProperty rdf:about="&soma;definesTrigger"
    rdfs:label="defines trigger">
  <rdfs:comment>Relates an affordance which is a relation between a bearer and a trigger, to the role of the trigger when the affordance is manifested.</rdfs:comment>
  <rdfs:domain rdf:resource="&soma;Affordance"/>
  <rdfs:isDefinedBy rdf:resource="http://www.ease-crc.org/ont/SOMA-OBJ.owl"/>
  <rdfs:range rdf:resource="&dul;Role"/>
  <rdfs:subPropertyOf rdf:resource="&dul;definesRole"/>
  <owl:inverseOf rdf:resource="&soma;isTriggerDefinedIn"/>
</owl:ObjectProperty>

<owl:Class rdf:about="&soma;ThinkAloud">
  <rdfs:comment>A task in which an Agent, while in the course of performing some other task(s), reports on their own decision processes that guide this other task(s) for the benefit of an outside observer.</rdfs:comment>
  <rdfs:isDefinedBy rdf:resource="http://www.ease-crc.org/ont/SOMA-ACT.owl"/>
  <rdfs:label xml:lang="en">Think-aloud</rdfs:label>
  <rdfs:subClassOf rdf:resource="&soma;CommunicationReport"/>
</owl:Class>

<owl:Class rdf:about="&soma;QualityTransition">
  <rdfs:comment>todo(DB): added for NEEMs (quale change), but not sure yet about it...</rdfs:comment>
  <rdfs:isDefinedBy rdf:resource="http://www.ease-crc.org/ont/SOMA-OBJ.owl"/>
  <rdfs:label xml:lang="en">Quality transition</rdfs:label>
  <rdfs:subClassOf rdf:resource="&dul;Transition"/>
</owl:Class>

<owl:Class rdf:about="&soma;CausalEventRole">
  <rdfs:comment>A role filled by a description of some action or process that brings about a motion.

As an example, consider the utterance "the tennisman served the ball by hitting it with the racket." In this utterance, the filler of the CausalEventRole is expressed by the "by hitting it with the racket" constituent.</rdfs:comment>
  <rdfs:isDefinedBy rdf:resource="http://www.ease-crc.org/ont/SOMA-OBJ.owl"/>
  <rdfs:label xml:lang="en">Causal event role</rdfs:label>
  <rdfs:subClassOf rdf:resource="&soma;CausativeRole"/>
</owl:Class>

<owl:Class rdf:about="&soma;TimeRole">
  <rdfs:comment>A role filled by a description of the location in time and/or duration of an event or object.</rdfs:comment>
  <rdfs:isDefinedBy rdf:resource="http://www.ease-crc.org/ont/SOMA-OBJ.owl"/>
  <rdfs:label xml:lang="en">Time role</rdfs:label>
  <rdfs:subClassOf rdf:resource="&soma;SpatioTemporalRole"/>
</owl:Class>

<owl:Class rdf:about="&dul;Theory"/>

<owl:ObjectProperty rdf:about="&soma;hasJointLimit"
    rdfs:comment="Relates a joint to its physical limits."
    rdfs:label="has joint limit">
  <rdfs:domain rdf:resource="&soma;Joint"/>
  <rdfs:isDefinedBy rdf:resource="http://www.ease-crc.org/ont/SOMA-OBJ.owl"/>
  <rdfs:range rdf:resource="&soma;JointLimit"/>
  <rdfs:subPropertyOf rdf:resource="&dul;hasRegion"/>
  <owl:inverseOf rdf:resource="&soma;isJointLimitOf"/>
</owl:ObjectProperty>

<owl:Class rdf:about="&soma;Locomotion">
  <rdfs:comment>Conceptually related to Navigation, but distinguishable from it because of the profile, ie. the focus of the task.

Navigation is about reaching some goal.

Locomotion is concerned more with the actual motion.</rdfs:comment>
  <rdfs:comment>The Agent repositions their body in the environment.</rdfs:comment>
  <rdfs:subClassOf rdf:resource="&soma;BodyMovement"/>
  <rdfs:subClassOf rdf:resource="&soma;DirectedMotion"/>
  <rdfs:isDefinedBy rdf:resource="http://www.ease-crc.org/ont/SOMA-PROC.owl"/>
  <owl:disjointWith rdf:resource="&soma;PrehensileMotion"/>
</owl:Class>

<owl:DatatypeProperty rdf:about="&soma;hasJointParameter"
    rdfs:comment="Assigns a value for an attribute of a joint."
    rdfs:label="has joint parameter">
  <rdfs:domain rdf:resource="&dul;PhysicalAttribute"/>
  <rdfs:isDefinedBy rdf:resource="http://www.ease-crc.org/ont/SOMA-OBJ.owl"/>
  <rdfs:range rdf:resource="&xsd;double"/>
  <rdfs:subPropertyOf rdf:resource="&dul;hasRegionDataValue"/>
</owl:DatatypeProperty>

<owl:ObjectProperty rdf:about="&soma;affordanceDefinesTask"
    rdfs:comment="A relation between an Affordance and a Task"
    rdfs:label="affordance defines task">
  <rdfs:subPropertyOf rdf:resource="&soma;affordanceDefines"/>
  <rdfs:subPropertyOf rdf:resource="&dul;definesTask"/>
  <rdfs:domain rdf:resource="&soma;Affordance"/>
  <rdfs:isDefinedBy rdf:resource="http://www.ease-crc.org/ont/SOMA-OBJ.owl"/>
  <rdfs:range rdf:resource="&dul;Task"/>
  <owl:inverseOf rdf:resource="&soma;isTaskDefinedInAffordance"/>
</owl:ObjectProperty>

<owl:Class rdf:about="&soma;MonitoringJointState">
  <rdfs:comment>A task in which the Agent keeps track of the physical state of its joints, e.g. their positions, velocities, efforts.</rdfs:comment>
  <rdfs:isDefinedBy rdf:resource="http://www.ease-crc.org/ont/SOMA-ACT.owl"/>
  <rdfs:label xml:lang="en">Monitoring joint state</rdfs:label>
  <rdfs:subClassOf rdf:resource="&soma;Proprioceiving"/>
</owl:Class>

<owl:Class rdf:about="&soma;Dreaming">
  <rdfs:comment>Any form of re-processing episodic memories for long-term memory by natural or aritifical agents.</rdfs:comment>
  <rdfs:isDefinedBy rdf:resource="http://www.ease-crc.org/ont/SOMA-ACT.owl"/>
  <rdfs:subClassOf rdf:resource="&soma;DerivingInformation"/>
</owl:Class>

<owl:Class rdf:about="&soma;Destination">
  <rdfs:comment>A role classifying the location where an event or object is directed towards.</rdfs:comment>
  <rdfs:isDefinedBy rdf:resource="http://www.ease-crc.org/ont/SOMA-OBJ.owl"/>
  <rdfs:subClassOf rdf:resource="&soma;Location"/>
</owl:Class>

<owl:ObjectProperty rdf:about="&soma;isQualeOf"
    rdfs:label="is quale of">
  <rdfs:comment>Relates a quality to its "value", called quale, which is an atomic quality region.</rdfs:comment>
  <rdfs:domain rdf:resource="&dul;Region"/>
  <rdfs:isDefinedBy rdf:resource="http://www.ease-crc.org/ont/SOMA-OBJ.owl"/>
  <rdfs:range rdf:resource="&dul;Quality"/>
  <rdfs:subPropertyOf rdf:resource="&dul;isRegionFor"/>
</owl:ObjectProperty>

<owl:ObjectProperty rdf:about="&soma;hasAction"
    rdfs:comment="A relation from an Action to a component Action."
    rdfs:label="has action">
  <rdfs:domain rdf:resource="&dul;Action"/>
  <rdfs:isDefinedBy rdf:resource="http://www.ease-crc.org/ont/SOMA-ACT.owl"/>
  <rdfs:range rdf:resource="&dul;Action"/>
  <rdfs:subPropertyOf rdf:resource="&dul;hasConstituent"/>
</owl:ObjectProperty>

</rdf:RDF>
